<?xml version="1.0"?>
<rdf:RDF xmlns="http://openenergy-platform.org/ontology/oeo/oeo-physical/"
     xml:base="http://openenergy-platform.org/ontology/oeo/oeo-physical/"
     xmlns:dc="http://purl.org/dc/elements/1.1/"
     xmlns:uo="http://purl.obolibrary.org/obo/uo#"
     xmlns:obo="http://purl.obolibrary.org/obo/"
     xmlns:oeo="http://openenergy-platform.org/ontology/oeo/"
     xmlns:owl="http://www.w3.org/2002/07/owl#"
     xmlns:rdf="http://www.w3.org/1999/02/22-rdf-syntax-ns#"
     xmlns:xml="http://www.w3.org/XML/1998/namespace"
     xmlns:xsd="http://www.w3.org/2001/XMLSchema#"
     xmlns:foaf="http://xmlns.com/foaf/0.1/"
     xmlns:rdfs="http://www.w3.org/2000/01/rdf-schema#"
     xmlns:terms="http://purl.org/dc/terms/"
     xmlns:protege="http://protege.stanford.edu/plugins/owl/protege#"
     xmlns:oboInOwl="http://www.geneontology.org/formats/oboInOwl#">
    <owl:Ontology rdf:about="http://openenergy-platform.org/ontology/oeo/oeo-physical/">
        <owl:versionIRI rdf:resource="http://openenergy-platform.org/ontology/oeo/releases/1.5.0/oeo-physical.omn"/>
        <owl:imports rdf:resource="http://openenergy-platform.org/ontology/oeo/releases/1.5.0/oeo-shared.omn"/>
        <dc:description>The Open Energy Ontology is an ontology for all aspects of the energy modelling domain. The &apos;Physical&apos; module covers all those aspects of the world that are relevant for the energy systems domain, including physical entities such as generators, power lines, technologies, hardware, portions of matter; attributes of those, such as the energy they carry or release, whether they can be a pollutant, or their origins; representational transformations into maps and measures, such as coordinates, units, quantities; and the processes that modify the physical entities, such as energy production.</dc:description>
        <dc:license>http://creativecommons.org/publicdomain/zero/1.0/</dc:license>
        <terms:title>Open Energy Ontology (Physical module)</terms:title>
    </owl:Ontology>
    


    <!-- 
    ///////////////////////////////////////////////////////////////////////////////////////
    //
    // Annotation properties
    //
    ///////////////////////////////////////////////////////////////////////////////////////
     -->

    


    <!-- http://purl.obolibrary.org/obo/IAO_0000112 -->

    <owl:AnnotationProperty rdf:about="http://purl.obolibrary.org/obo/IAO_0000112"/>
    


    <!-- http://purl.obolibrary.org/obo/IAO_0000115 -->

    <owl:AnnotationProperty rdf:about="http://purl.obolibrary.org/obo/IAO_0000115"/>
    


    <!-- http://purl.obolibrary.org/obo/IAO_0000116 -->

    <owl:AnnotationProperty rdf:about="http://purl.obolibrary.org/obo/IAO_0000116"/>
    


    <!-- http://purl.obolibrary.org/obo/IAO_0000118 -->

    <owl:AnnotationProperty rdf:about="http://purl.obolibrary.org/obo/IAO_0000118"/>
    


    <!-- http://purl.obolibrary.org/obo/IAO_0000119 -->

    <owl:AnnotationProperty rdf:about="http://purl.obolibrary.org/obo/IAO_0000119"/>
    


    <!-- http://purl.obolibrary.org/obo/IAO_0000233 -->

    <owl:AnnotationProperty rdf:about="http://purl.obolibrary.org/obo/IAO_0000233"/>
    


    <!-- http://purl.org/dc/elements/1.1/contributor -->

    <owl:AnnotationProperty rdf:about="http://purl.org/dc/elements/1.1/contributor"/>
    


    <!-- http://purl.org/dc/elements/1.1/description -->

    <owl:AnnotationProperty rdf:about="http://purl.org/dc/elements/1.1/description"/>
    


    <!-- http://purl.org/dc/elements/1.1/license -->

    <owl:AnnotationProperty rdf:about="http://purl.org/dc/elements/1.1/license"/>
    


    <!-- http://purl.org/dc/terms/title -->

    <owl:AnnotationProperty rdf:about="http://purl.org/dc/terms/title"/>
    


    <!-- http://www.geneontology.org/formats/oboInOwl#hasExactSynonym -->

    <owl:AnnotationProperty rdf:about="http://www.geneontology.org/formats/oboInOwl#hasExactSynonym"/>
    


    <!-- http://www.w3.org/2000/01/rdf-schema#comment -->

    <owl:AnnotationProperty rdf:about="http://www.w3.org/2000/01/rdf-schema#comment"/>
    


    <!-- http://www.w3.org/2000/01/rdf-schema#isDefinedBy -->

    <owl:AnnotationProperty rdf:about="http://www.w3.org/2000/01/rdf-schema#isDefinedBy"/>
    


    <!-- http://www.w3.org/2000/01/rdf-schema#label -->

    <owl:AnnotationProperty rdf:about="http://www.w3.org/2000/01/rdf-schema#label"/>
    


    <!-- 
    ///////////////////////////////////////////////////////////////////////////////////////
    //
    // Datatypes
    //
    ///////////////////////////////////////////////////////////////////////////////////////
     -->

    


    <!-- http://www.w3.org/1999/02/22-rdf-syntax-ns#PlainLiteral -->

    <rdfs:Datatype rdf:about="http://www.w3.org/1999/02/22-rdf-syntax-ns#PlainLiteral"/>
    


    <!-- 
    ///////////////////////////////////////////////////////////////////////////////////////
    //
    // Object Properties
    //
    ///////////////////////////////////////////////////////////////////////////////////////
     -->

    


    <!-- http://openenergy-platform.org/ontology/oeo/OEO_00000500 -->

    <owl:ObjectProperty rdf:about="http://openenergy-platform.org/ontology/oeo/OEO_00000500"/>
    


    <!-- http://openenergy-platform.org/ontology/oeo/OEO_00000501 -->

    <owl:ObjectProperty rdf:about="http://openenergy-platform.org/ontology/oeo/OEO_00000501"/>
    


    <!-- http://openenergy-platform.org/ontology/oeo/OEO_00000502 -->

    <owl:ObjectProperty rdf:about="http://openenergy-platform.org/ontology/oeo/OEO_00000502"/>
    


    <!-- http://openenergy-platform.org/ontology/oeo/OEO_00000503 -->

    <owl:ObjectProperty rdf:about="http://openenergy-platform.org/ontology/oeo/OEO_00000503"/>
    


    <!-- http://openenergy-platform.org/ontology/oeo/OEO_00000521 -->

    <owl:ObjectProperty rdf:about="http://openenergy-platform.org/ontology/oeo/OEO_00000521">
        <owl:inverseOf rdf:resource="http://openenergy-platform.org/ontology/oeo/OEO_00000525"/>
        <rdfs:domain rdf:resource="http://openenergy-platform.org/ontology/oeo/OEO_00000061"/>
        <rdfs:range rdf:resource="http://openenergy-platform.org/ontology/oeo/OEO_00000407"/>
        <obo:IAO_0000115>the property of an artificial object to apply to a technology.</obo:IAO_0000115>
        <rdfs:label>applies technology</rdfs:label>
    </owl:ObjectProperty>
    


    <!-- http://openenergy-platform.org/ontology/oeo/OEO_00000522 -->

    <owl:ObjectProperty rdf:about="http://openenergy-platform.org/ontology/oeo/OEO_00000522"/>
    


    <!-- http://openenergy-platform.org/ontology/oeo/OEO_00000523 -->

    <owl:ObjectProperty rdf:about="http://openenergy-platform.org/ontology/oeo/OEO_00000523">
        <rdfs:subPropertyOf rdf:resource="http://openenergy-platform.org/ontology/oeo/OEO_00000522"/>
        <rdfs:range rdf:resource="http://openenergy-platform.org/ontology/oeo/OEO_00020039"/>
        <obo:IAO_0000233>change range
issue: https://github.com/OpenEnergyPlatform/ontology/pull/721
pull request: https://github.com/OpenEnergyPlatform/ontology/pull/722</obo:IAO_0000233>
        <rdfs:comment>A relation that holds between a publication/model calculation/model and the energy carrier it covers.</rdfs:comment>
        <rdfs:label>covers energy carrier</rdfs:label>
    </owl:ObjectProperty>
    


    <!-- http://openenergy-platform.org/ontology/oeo/OEO_00000524 -->

    <owl:ObjectProperty rdf:about="http://openenergy-platform.org/ontology/oeo/OEO_00000524">
        <rdfs:subPropertyOf rdf:resource="http://www.w3.org/2002/07/owl#topObjectProperty"/>
        <rdfs:domain rdf:resource="http://openenergy-platform.org/ontology/oeo/OEO_00000020"/>
        <rdfs:range rdf:resource="http://openenergy-platform.org/ontology/oeo/OEO_00010078"/>
        <obo:IAO_0000115>A relation between a greenhouse gas and the global warming potential it has.</obo:IAO_0000115>
        <obo:IAO_0000233>issue: https://github.com/OpenEnergyPlatform/ontology/issues/66
pull request: https://github.com/OpenEnergyPlatform/ontology/pull/478
issue: https://github.com/OpenEnergyPlatform/ontology/issues/420
pull request: https://github.com/OpenEnergyPlatform/ontology/pull/651
issue: https://github.com/OpenEnergyPlatform/ontology/issues/420
pull request: https://github.com/OpenEnergyPlatform/ontology/pull/683</obo:IAO_0000233>
        <rdfs:label>has global warming potential</rdfs:label>
    </owl:ObjectProperty>
    


    <!-- http://openenergy-platform.org/ontology/oeo/OEO_00000525 -->

    <owl:ObjectProperty rdf:about="http://openenergy-platform.org/ontology/oeo/OEO_00000525">
        <rdfs:domain rdf:resource="http://openenergy-platform.org/ontology/oeo/OEO_00000407"/>
        <rdfs:range rdf:resource="http://openenergy-platform.org/ontology/oeo/OEO_00000061"/>
        <obo:IAO_0000115>The property of a technology to be applied to an artificial object.</obo:IAO_0000115>
        <rdfs:label>is applied to object</rdfs:label>
    </owl:ObjectProperty>
    


    <!-- http://openenergy-platform.org/ontology/oeo/OEO_00000526 -->

    <owl:ObjectProperty rdf:about="http://openenergy-platform.org/ontology/oeo/OEO_00000526">
        <rdfs:subPropertyOf rdf:resource="http://www.w3.org/2002/07/owl#topObjectProperty"/>
        <rdf:type rdf:resource="http://www.w3.org/2002/07/owl#SymmetricProperty"/>
        <obo:IAO_0000115>A relation that holds between two nodes in a graph that are connected to each other through an edge.</obo:IAO_0000115>
        <obo:IAO_0000233>issue: https://github.com/OpenEnergyPlatform/ontology/issues/66
pull requests: https://github.com/OpenEnergyPlatform/ontology/pull/478</obo:IAO_0000233>
        <rdfs:label>is connected to</rdfs:label>
    </owl:ObjectProperty>
    


    <!-- http://openenergy-platform.org/ontology/oeo/OEO_00000527 -->

    <owl:ObjectProperty rdf:about="http://openenergy-platform.org/ontology/oeo/OEO_00000527">
        <rdfs:subPropertyOf rdf:resource="http://openenergy-platform.org/ontology/oeo/OEO_00000526"/>
        <owl:propertyDisjointWith rdf:resource="http://openenergy-platform.org/ontology/oeo/OEO_00000528"/>
        <obo:IAO_0000115>A relation that holds between a directed graph and a node in that graph that has edges ending but not starting there.</obo:IAO_0000115>
        <obo:IAO_0000233>issue: https://github.com/OpenEnergyPlatform/ontology/issues/66
pull requests: https://github.com/OpenEnergyPlatform/ontology/pull/478</obo:IAO_0000233>
        <rdfs:label>has sink</rdfs:label>
    </owl:ObjectProperty>
    


    <!-- http://openenergy-platform.org/ontology/oeo/OEO_00000528 -->

    <owl:ObjectProperty rdf:about="http://openenergy-platform.org/ontology/oeo/OEO_00000528">
        <rdfs:subPropertyOf rdf:resource="http://openenergy-platform.org/ontology/oeo/OEO_00000526"/>
        <obo:IAO_0000115>A relation that holds between a directed graph and a node in that graph that has edges starting but not ending there.</obo:IAO_0000115>
        <obo:IAO_0000233>issue: https://github.com/OpenEnergyPlatform/ontology/issues/66
pull requests: https://github.com/OpenEnergyPlatform/ontology/pull/478</obo:IAO_0000233>
        <rdfs:label>has source</rdfs:label>
    </owl:ObjectProperty>
    


    <!-- http://openenergy-platform.org/ontology/oeo/OEO_00000529 -->

    <owl:ObjectProperty rdf:about="http://openenergy-platform.org/ontology/oeo/OEO_00000529">
        <rdfs:subPropertyOf rdf:resource="http://purl.obolibrary.org/obo/RO_0000086"/>
        <rdfs:domain rdf:resource="http://openenergy-platform.org/ontology/oeo/OEO_00000331"/>
        <rdfs:range rdf:resource="http://openenergy-platform.org/ontology/oeo/OEO_00000395"/>
        <obo:IAO_0000115>x has normal state of matter y if and only if a portion of x occurs in state y under normal pressure (1 bar) and normal temperature (0°C)</obo:IAO_0000115>
        <rdfs:label>has normal state of matter</rdfs:label>
    </owl:ObjectProperty>
    


    <!-- http://openenergy-platform.org/ontology/oeo/OEO_00000530 -->

    <owl:ObjectProperty rdf:about="http://openenergy-platform.org/ontology/oeo/OEO_00000530">
        <rdfs:subPropertyOf rdf:resource="http://purl.obolibrary.org/obo/RO_0000086"/>
        <rdfs:domain>
            <owl:Class>
                <owl:unionOf rdf:parseType="Collection">
                    <rdf:Description rdf:about="http://openenergy-platform.org/ontology/oeo/OEO_00000150"/>
                    <rdf:Description rdf:about="http://openenergy-platform.org/ontology/oeo/OEO_00000331"/>
                </owl:unionOf>
            </owl:Class>
        </rdfs:domain>
        <rdfs:range rdf:resource="http://openenergy-platform.org/ontology/oeo/OEO_00000316"/>
        <obo:IAO_0000115>x has the origin of y</obo:IAO_0000115>
        <rdfs:label>has origin</rdfs:label>
    </owl:ObjectProperty>
    <owl:Axiom>
        <owl:annotatedSource rdf:resource="http://openenergy-platform.org/ontology/oeo/OEO_00000530"/>
        <owl:annotatedProperty rdf:resource="http://www.w3.org/2000/01/rdf-schema#domain"/>
        <owl:annotatedTarget>
            <owl:Class>
                <owl:unionOf rdf:parseType="Collection">
                    <rdf:Description rdf:about="http://openenergy-platform.org/ontology/oeo/OEO_00000150"/>
                    <rdf:Description rdf:about="http://openenergy-platform.org/ontology/oeo/OEO_00000331"/>
                </owl:unionOf>
            </owl:Class>
        </owl:annotatedTarget>
        <obo:IAO_0000233>add energy
issue: https://github.com/OpenEnergyPlatform/ontology/issues/728
pull request: https://github.com/OpenEnergyPlatform/ontology/pull/742</obo:IAO_0000233>
    </owl:Axiom>
    


    <!-- http://openenergy-platform.org/ontology/oeo/OEO_00000531 -->

    <owl:ObjectProperty rdf:about="http://openenergy-platform.org/ontology/oeo/OEO_00000531">
        <rdfs:subPropertyOf rdf:resource="http://purl.obolibrary.org/obo/RO_0000086"/>
        <rdfs:domain rdf:resource="http://openenergy-platform.org/ontology/oeo/OEO_00000331"/>
        <rdfs:range rdf:resource="http://openenergy-platform.org/ontology/oeo/OEO_00000395"/>
        <rdfs:label>has state of matter</rdfs:label>
    </owl:ObjectProperty>
    


    <!-- http://openenergy-platform.org/ontology/oeo/OEO_00000532 -->

    <owl:ObjectProperty rdf:about="http://openenergy-platform.org/ontology/oeo/OEO_00000532">
        <rdfs:subPropertyOf rdf:resource="http://purl.obolibrary.org/obo/RO_0002233"/>
        <rdf:type rdf:resource="http://www.w3.org/2002/07/owl#AsymmetricProperty"/>
        <rdf:type rdf:resource="http://www.w3.org/2002/07/owl#IrreflexiveProperty"/>
        <rdfs:domain rdf:resource="http://purl.obolibrary.org/obo/BFO_0000015"/>
        <rdfs:range>
            <owl:Class>
                <owl:unionOf rdf:parseType="Collection">
                    <rdf:Description rdf:about="http://openenergy-platform.org/ontology/oeo/OEO_00000150"/>
                    <rdf:Description rdf:about="http://purl.obolibrary.org/obo/BFO_0000040"/>
                </owl:unionOf>
            </owl:Class>
        </rdfs:range>
        <obo:IAO_0000115 xml:lang="en">p has physical input c iff: p has input c, and c is a material entity or energy</obo:IAO_0000115>
        <obo:IAO_0000233>issue: https://github.com/OpenEnergyPlatform/ontology/issues/664
pull request: https://github.com/OpenEnergyPlatform/ontology/pull/702</obo:IAO_0000233>
        <rdfs:label>has physical input</rdfs:label>
    </owl:ObjectProperty>
    


    <!-- http://openenergy-platform.org/ontology/oeo/OEO_00000533 -->

    <owl:ObjectProperty rdf:about="http://openenergy-platform.org/ontology/oeo/OEO_00000533">
        <rdfs:subPropertyOf rdf:resource="http://purl.obolibrary.org/obo/RO_0002234"/>
        <obo:IAO_0000115 xml:lang="en">p has physical output c iff: p has output c, and c is a material entity or energy</obo:IAO_0000115>
        <obo:IAO_0000233>issue: https://github.com/OpenEnergyPlatform/ontology/issues/618
pull request:: https://github.com/OpenEnergyPlatform/ontology/pull/716</obo:IAO_0000233>
        <rdfs:label>has physical output</rdfs:label>
    </owl:ObjectProperty>
    


    <!-- http://openenergy-platform.org/ontology/oeo/OEO_00020056 -->

    <owl:ObjectProperty rdf:about="http://openenergy-platform.org/ontology/oeo/OEO_00020056"/>
    


    <!-- http://openenergy-platform.org/ontology/oeo/OEO_00040010 -->

    <owl:ObjectProperty rdf:about="http://openenergy-platform.org/ontology/oeo/OEO_00040010"/>
    


    <!-- http://openenergy-platform.org/ontology/oeo/OEO_00140002 -->

    <owl:ObjectProperty rdf:about="http://openenergy-platform.org/ontology/oeo/OEO_00140002"/>
    


    <!-- http://purl.obolibrary.org/obo/BFO_0000050 -->

    <owl:ObjectProperty rdf:about="http://purl.obolibrary.org/obo/BFO_0000050"/>
    


    <!-- http://purl.obolibrary.org/obo/BFO_0000051 -->

    <owl:ObjectProperty rdf:about="http://purl.obolibrary.org/obo/BFO_0000051"/>
    


    <!-- http://purl.obolibrary.org/obo/RO_0000053 -->

    <owl:ObjectProperty rdf:about="http://purl.obolibrary.org/obo/RO_0000053"/>
    


    <!-- http://purl.obolibrary.org/obo/RO_0000056 -->

    <owl:ObjectProperty rdf:about="http://purl.obolibrary.org/obo/RO_0000056"/>
    


    <!-- http://purl.obolibrary.org/obo/RO_0000057 -->

    <owl:ObjectProperty rdf:about="http://purl.obolibrary.org/obo/RO_0000057"/>
    


    <!-- http://purl.obolibrary.org/obo/RO_0000085 -->

    <owl:ObjectProperty rdf:about="http://purl.obolibrary.org/obo/RO_0000085"/>
    


    <!-- http://purl.obolibrary.org/obo/RO_0000086 -->

    <owl:ObjectProperty rdf:about="http://purl.obolibrary.org/obo/RO_0000086"/>
    


    <!-- http://purl.obolibrary.org/obo/RO_0000087 -->

    <owl:ObjectProperty rdf:about="http://purl.obolibrary.org/obo/RO_0000087"/>
    


    <!-- http://purl.obolibrary.org/obo/RO_0000091 -->

    <owl:ObjectProperty rdf:about="http://purl.obolibrary.org/obo/RO_0000091"/>
    


    <!-- http://purl.obolibrary.org/obo/RO_0002233 -->

    <owl:ObjectProperty rdf:about="http://purl.obolibrary.org/obo/RO_0002233">
        <obo:IAO_0000233>issue: https://github.com/OpenEnergyPlatform/ontology/issues/664
pull request: https://github.com/OpenEnergyPlatform/ontology/pull/702</obo:IAO_0000233>
        <rdfs:comment>OEO adjustment: The range of this property has been changed from material entity to continuant. A subclass &quot;has physical input&quot; has been added for material entities and energies.</rdfs:comment>
    </owl:ObjectProperty>
    


    <!-- http://purl.obolibrary.org/obo/RO_0002234 -->

    <owl:ObjectProperty rdf:about="http://purl.obolibrary.org/obo/RO_0002234"/>
    


    <!-- http://purl.obolibrary.org/obo/uo#is_unit_of -->

    <owl:ObjectProperty rdf:about="http://purl.obolibrary.org/obo/uo#is_unit_of"/>
    


    <!-- http://www.w3.org/2002/07/owl#topObjectProperty -->

    <owl:ObjectProperty rdf:about="http://www.w3.org/2002/07/owl#topObjectProperty"/>
    


    <!-- 
    ///////////////////////////////////////////////////////////////////////////////////////
    //
    // Classes
    //
    ///////////////////////////////////////////////////////////////////////////////////////
     -->

    


    <!-- http://openenergy-platform.org/ontology/oeo/OEO_00000001 -->

    <owl:Class rdf:about="http://openenergy-platform.org/ontology/oeo/OEO_00000001">
        <rdfs:subClassOf rdf:resource="http://purl.obolibrary.org/obo/BFO_0000023"/>
        <obo:IAO_0000115>A fuel role is a role of a portion of matter that has the disposition to be an energy carrier and is used in a process that releases the carried energy by transforming the portion of matter into a different kind of portion of matter in a way that releases heat or does work.</obo:IAO_0000115>
        <obo:IAO_0000233>issue: https://github.com/OpenEnergyPlatform/ontology/issues/227
pull request: https://github.com/OpenEnergyPlatform/ontology/pull/279</obo:IAO_0000233>
        <rdfs:label>fuel role</rdfs:label>
    </owl:Class>
    


    <!-- http://openenergy-platform.org/ontology/oeo/OEO_00000003 -->

    <owl:Class rdf:about="http://openenergy-platform.org/ontology/oeo/OEO_00000003">
        <rdfs:subClassOf rdf:resource="http://openenergy-platform.org/ontology/oeo/OEO_00000334"/>
        <rdfs:subClassOf>
            <owl:Restriction>
                <owl:onProperty rdf:resource="http://openenergy-platform.org/ontology/oeo/OEO_00000503"/>
                <owl:someValuesFrom rdf:resource="http://openenergy-platform.org/ontology/oeo/OEO_00000072"/>
            </owl:Restriction>
        </rdfs:subClassOf>
        <obo:IAO_0000115>A biofuel power unit is a power generating unit using biofuel.</obo:IAO_0000115>
        <rdfs:label>biofuel power unit</rdfs:label>
    </owl:Class>
    


    <!-- http://openenergy-platform.org/ontology/oeo/OEO_00000004 -->

    <owl:Class rdf:about="http://openenergy-platform.org/ontology/oeo/OEO_00000004">
        <rdfs:subClassOf rdf:resource="http://openenergy-platform.org/ontology/oeo/OEO_00000073"/>
        <obo:IAO_0000115>A biogas powerplant is a biofuel powerplant having an aggregate of biogas powerunits as its power generating units.</obo:IAO_0000115>
        <rdfs:label>biogas powerplant</rdfs:label>
    </owl:Class>
    


    <!-- http://openenergy-platform.org/ontology/oeo/OEO_00000005 -->

    <owl:Class rdf:about="http://openenergy-platform.org/ontology/oeo/OEO_00000005">
        <rdfs:subClassOf rdf:resource="http://openenergy-platform.org/ontology/oeo/OEO_00000003"/>
        <rdfs:subClassOf>
            <owl:Restriction>
                <owl:onProperty rdf:resource="http://openenergy-platform.org/ontology/oeo/OEO_00000503"/>
                <owl:someValuesFrom rdf:resource="http://openenergy-platform.org/ontology/oeo/OEO_00000074"/>
            </owl:Restriction>
        </rdfs:subClassOf>
        <obo:IAO_0000115>A biogas power unit is a biofuel power unit using biogas as fuel.</obo:IAO_0000115>
        <rdfs:label>biogas power unit</rdfs:label>
    </owl:Class>
    


    <!-- http://openenergy-platform.org/ontology/oeo/OEO_00000006 -->

    <owl:Class rdf:about="http://openenergy-platform.org/ontology/oeo/OEO_00000006">
        <rdfs:subClassOf rdf:resource="http://openenergy-platform.org/ontology/oeo/OEO_00000331"/>
        <rdfs:subClassOf>
            <owl:Restriction>
                <owl:onProperty rdf:resource="http://purl.obolibrary.org/obo/RO_0000091"/>
                <owl:someValuesFrom rdf:resource="http://openenergy-platform.org/ontology/oeo/OEO_00000198"/>
            </owl:Restriction>
        </rdfs:subClassOf>
        <rdfs:subClassOf>
            <owl:Restriction>
                <owl:onProperty rdf:resource="http://openenergy-platform.org/ontology/oeo/OEO_00000529"/>
                <owl:hasValue rdf:resource="http://openenergy-platform.org/ontology/oeo/OEO_00000182"/>
            </owl:Restriction>
        </rdfs:subClassOf>
        <obo:IAO_0000115>Carbon dioxide is a portion of matter with the chemical formula CO2. It has a gaseous normal state of matter. It occurs naturally in the atmosphere as a trace gas and can work as a greenhouse gas.</obo:IAO_0000115>
        <obo:IAO_0000118>CO2</obo:IAO_0000118>
        <rdfs:label>carbon dioxide</rdfs:label>
    </owl:Class>
    


    <!-- http://openenergy-platform.org/ontology/oeo/OEO_00000007 -->

    <owl:Class rdf:about="http://openenergy-platform.org/ontology/oeo/OEO_00000007">
        <rdfs:subClassOf rdf:resource="http://openenergy-platform.org/ontology/oeo/OEO_00000150"/>
        <obo:IAO_0000115>Chemical energy is energy that is stored in the chemical bonds of a substance, which can be released by a chemical reaction.</obo:IAO_0000115>
        <obo:IAO_0000233>issue: https://github.com/OpenEnergyPlatform/ontology/issues/174
pull request: https://github.com/OpenEnergyPlatform/ontology/pull/214</obo:IAO_0000233>
        <rdfs:label>chemical energy</rdfs:label>
    </owl:Class>
    


    <!-- http://openenergy-platform.org/ontology/oeo/OEO_00000008 -->

    <owl:Class rdf:about="http://openenergy-platform.org/ontology/oeo/OEO_00000008">
        <rdfs:subClassOf rdf:resource="http://openenergy-platform.org/ontology/oeo/OEO_00000334"/>
        <rdfs:subClassOf>
            <owl:Restriction>
                <owl:onProperty rdf:resource="http://openenergy-platform.org/ontology/oeo/OEO_00000503"/>
                <owl:someValuesFrom rdf:resource="http://openenergy-platform.org/ontology/oeo/OEO_00000088"/>
            </owl:Restriction>
        </rdfs:subClassOf>
        <obo:IAO_0000115>A coal power unit is a power generating unit using coal as fuel.</obo:IAO_0000115>
        <rdfs:label>coal power unit</rdfs:label>
    </owl:Class>
    


    <!-- http://openenergy-platform.org/ontology/oeo/OEO_00000009 -->

    <owl:Class rdf:about="http://openenergy-platform.org/ontology/oeo/OEO_00000009">
        <rdfs:subClassOf rdf:resource="http://openenergy-platform.org/ontology/oeo/OEO_00000212"/>
        <rdfs:comment>An electric heat pump is a heat pump that uses electric energy as drive energy.</rdfs:comment>
        <rdfs:label>electric heat pump</rdfs:label>
    </owl:Class>
    


    <!-- http://openenergy-platform.org/ontology/oeo/OEO_00000010 -->

    <owl:Class rdf:about="http://openenergy-platform.org/ontology/oeo/OEO_00000010">
        <rdfs:subClassOf rdf:resource="http://openenergy-platform.org/ontology/oeo/OEO_00000188"/>
        <obo:IAO_0000115>An electro motive generator is a generator that converts kinetic energy into electric energy.</obo:IAO_0000115>
        <rdfs:label>electro motive generator</rdfs:label>
    </owl:Class>
    


    <!-- http://openenergy-platform.org/ontology/oeo/OEO_00000011 -->

    <owl:Class rdf:about="http://openenergy-platform.org/ontology/oeo/OEO_00000011">
        <rdfs:subClassOf rdf:resource="http://openenergy-platform.org/ontology/oeo/OEO_00000061"/>
        <rdfs:subClassOf>
            <owl:Restriction>
                <owl:onProperty rdf:resource="http://purl.obolibrary.org/obo/RO_0000056"/>
                <owl:someValuesFrom rdf:resource="http://openenergy-platform.org/ontology/oeo/OEO_00020003"/>
            </owl:Restriction>
        </rdfs:subClassOf>
        <obo:IAO_0000115>An energy converting device is an artificial object that transforms or changes a certain type of energy.</obo:IAO_0000115>
        <obo:IAO_0000233>issue: https://github.com/OpenEnergyPlatform/ontology/issues/173
pull request: https://github.com/OpenEnergyPlatform/ontology/pull/273

issue: https://github.com/OpenEnergyPlatform/ontology/issues/372
pull request: https://github.com/OpenEnergyPlatform/ontology/pull/646</obo:IAO_0000233>
        <rdfs:comment>formerly called energy transformer</rdfs:comment>
        <rdfs:label>energy converting device</rdfs:label>
    </owl:Class>
    


    <!-- http://openenergy-platform.org/ontology/oeo/OEO_00000012 -->

    <owl:Class rdf:about="http://openenergy-platform.org/ontology/oeo/OEO_00000012">
        <rdfs:subClassOf rdf:resource="http://openenergy-platform.org/ontology/oeo/OEO_00000151"/>
        <rdfs:subClassOf rdf:resource="http://purl.obolibrary.org/obo/BFO_0000034"/>
        <obo:IAO_0000115>Energy storage is a function of an artificial object that has been engineered to contain energy for conversion as usable energy later.</obo:IAO_0000115>
        <obo:IAO_0000233>issue: https://github.com/OpenEnergyPlatform/ontology/issues/209
pull request: https://github.com/OpenEnergyPlatform/ontology/pull/276</obo:IAO_0000233>
        <rdfs:label>energy storage</rdfs:label>
    </owl:Class>
    


    <!-- http://openenergy-platform.org/ontology/oeo/OEO_00000013 -->

    <owl:Class rdf:about="http://openenergy-platform.org/ontology/oeo/OEO_00000013">
        <owl:equivalentClass>
            <owl:Class>
                <owl:unionOf rdf:parseType="Collection">
                    <rdf:Description rdf:about="http://openenergy-platform.org/ontology/oeo/OEO_00000026"/>
                    <rdf:Description rdf:about="http://openenergy-platform.org/ontology/oeo/OEO_00000038"/>
                    <rdf:Description rdf:about="http://openenergy-platform.org/ontology/oeo/OEO_00000219"/>
                    <rdf:Description rdf:about="http://openenergy-platform.org/ontology/oeo/OEO_00000322"/>
                </owl:unionOf>
            </owl:Class>
        </owl:equivalentClass>
        <rdfs:subClassOf rdf:resource="http://openenergy-platform.org/ontology/oeo/OEO_00000020"/>
        <obo:IAO_0000115>A fluorinated greenhouse gas is a greenhouse gas that is produced by fluorination. Hence it contains Fluor (F) atoms and is of anthropogenic origin.</obo:IAO_0000115>
        <rdfs:label>fluorinated greenhouse gas</rdfs:label>
    </owl:Class>
    


    <!-- http://openenergy-platform.org/ontology/oeo/OEO_00000014 -->

    <owl:Class rdf:about="http://openenergy-platform.org/ontology/oeo/OEO_00000014">
        <owl:equivalentClass>
            <owl:Class>
                <owl:intersectionOf rdf:parseType="Collection">
                    <rdf:Description rdf:about="http://openenergy-platform.org/ontology/oeo/OEO_00000099"/>
                    <owl:Restriction>
                        <owl:onProperty rdf:resource="http://openenergy-platform.org/ontology/oeo/OEO_00000530"/>
                        <owl:someValuesFrom rdf:resource="http://openenergy-platform.org/ontology/oeo/OEO_00030002"/>
                    </owl:Restriction>
                </owl:intersectionOf>
            </owl:Class>
        </owl:equivalentClass>
        <rdfs:subClassOf>
            <owl:Restriction>
                <owl:onProperty rdf:resource="http://openenergy-platform.org/ontology/oeo/OEO_00000530"/>
                <owl:someValuesFrom rdf:resource="http://openenergy-platform.org/ontology/oeo/OEO_00030003"/>
            </owl:Restriction>
        </rdfs:subClassOf>
        <obo:IAO_0000115>A fossil combustion fuel is a combustion fuel with the origin fossil.</obo:IAO_0000115>
        <rdfs:comment>This class is used to implement the subset relationship between origins fossil and geogenic: Every object with the origin fossil also has the origin geogenic.</rdfs:comment>
        <rdfs:label>fossil combustion fuel</rdfs:label>
    </owl:Class>
    


    <!-- http://openenergy-platform.org/ontology/oeo/OEO_00000016 -->

    <owl:Class rdf:about="http://openenergy-platform.org/ontology/oeo/OEO_00000016">
        <rdfs:subClassOf rdf:resource="http://openenergy-platform.org/ontology/oeo/OEO_00000188"/>
        <rdfs:subClassOf>
            <owl:Restriction>
                <owl:onProperty rdf:resource="http://openenergy-platform.org/ontology/oeo/OEO_00000503"/>
                <owl:someValuesFrom rdf:resource="http://openenergy-platform.org/ontology/oeo/OEO_00000220"/>
            </owl:Restriction>
        </rdfs:subClassOf>
        <obo:IAO_0000115>A fuel cell is a generator that converts chemical energy into electricity using redox reactions.</obo:IAO_0000115>
        <rdfs:label>fuel cell</rdfs:label>
    </owl:Class>
    


    <!-- http://openenergy-platform.org/ontology/oeo/OEO_00000017 -->

    <owl:Class rdf:about="http://openenergy-platform.org/ontology/oeo/OEO_00000017">
        <rdfs:subClassOf rdf:resource="http://openenergy-platform.org/ontology/oeo/OEO_00000334"/>
        <rdfs:subClassOf>
            <owl:Restriction>
                <owl:onProperty rdf:resource="http://openenergy-platform.org/ontology/oeo/OEO_00000503"/>
                <owl:someValuesFrom>
                    <owl:Class>
                        <owl:intersectionOf rdf:parseType="Collection">
                            <rdf:Description rdf:about="http://openenergy-platform.org/ontology/oeo/OEO_00000173"/>
                            <owl:Restriction>
                                <owl:onProperty rdf:resource="http://openenergy-platform.org/ontology/oeo/OEO_00000529"/>
                                <owl:hasValue rdf:resource="http://openenergy-platform.org/ontology/oeo/OEO_00000182"/>
                            </owl:Restriction>
                        </owl:intersectionOf>
                    </owl:Class>
                </owl:someValuesFrom>
            </owl:Restriction>
        </rdfs:subClassOf>
        <obo:IAO_0000115>A gas fired power unit is a power generating unit using gas as fuel.</obo:IAO_0000115>
        <rdfs:label>gas fired power unit</rdfs:label>
    </owl:Class>
    


    <!-- http://openenergy-platform.org/ontology/oeo/OEO_00000019 -->

    <owl:Class rdf:about="http://openenergy-platform.org/ontology/oeo/OEO_00000019">
        <rdfs:subClassOf rdf:resource="http://openenergy-platform.org/ontology/oeo/OEO_00000334"/>
        <obo:IAO_0000115>A geothermal power unit is a power unit using geothermal heat.</obo:IAO_0000115>
        <rdfs:label>geothermal power unit</rdfs:label>
    </owl:Class>
    


    <!-- http://openenergy-platform.org/ontology/oeo/OEO_00000020 -->

    <owl:Class rdf:about="http://openenergy-platform.org/ontology/oeo/OEO_00000020">
        <owl:equivalentClass>
            <owl:Class>
                <owl:intersectionOf rdf:parseType="Collection">
                    <rdf:Description rdf:about="http://openenergy-platform.org/ontology/oeo/OEO_00000331"/>
                    <owl:Restriction>
                        <owl:onProperty rdf:resource="http://purl.obolibrary.org/obo/RO_0000091"/>
                        <owl:someValuesFrom rdf:resource="http://openenergy-platform.org/ontology/oeo/OEO_00000198"/>
                    </owl:Restriction>
                </owl:intersectionOf>
            </owl:Class>
        </owl:equivalentClass>
        <rdfs:subClassOf rdf:resource="http://openenergy-platform.org/ontology/oeo/OEO_00000331"/>
        <rdfs:subClassOf>
            <owl:Restriction>
                <owl:onProperty rdf:resource="http://openenergy-platform.org/ontology/oeo/OEO_00000529"/>
                <owl:hasValue rdf:resource="http://openenergy-platform.org/ontology/oeo/OEO_00000182"/>
            </owl:Restriction>
        </rdfs:subClassOf>
        <obo:IAO_0000115>A greenhouse gas is a portion of matter that has the disposition to contribute to the greenhouse effect.</obo:IAO_0000115>
        <obo:IAO_0000233>issue: https://github.com/OpenEnergyPlatform/ontology/issues/56
pull request: https://github.com/OpenEnergyPlatform/ontology/pull/234</obo:IAO_0000233>
        <rdfs:label>greenhouse gas</rdfs:label>
    </owl:Class>
    


    <!-- http://openenergy-platform.org/ontology/oeo/OEO_00000021 -->

    <owl:Class rdf:about="http://openenergy-platform.org/ontology/oeo/OEO_00000021">
        <rdfs:subClassOf rdf:resource="http://openenergy-platform.org/ontology/oeo/OEO_00000008"/>
        <rdfs:subClassOf>
            <owl:Restriction>
                <owl:onProperty rdf:resource="http://openenergy-platform.org/ontology/oeo/OEO_00000503"/>
                <owl:someValuesFrom rdf:resource="http://openenergy-platform.org/ontology/oeo/OEO_00000204"/>
            </owl:Restriction>
        </rdfs:subClassOf>
        <obo:IAO_0000115>A hard coal power unit is a coal power unit using hard coal as fuel.</obo:IAO_0000115>
        <rdfs:label>hard coal power unit</rdfs:label>
    </owl:Class>
    


    <!-- http://openenergy-platform.org/ontology/oeo/OEO_00000022 -->

    <owl:Class rdf:about="http://openenergy-platform.org/ontology/oeo/OEO_00000022">
        <rdfs:subClassOf rdf:resource="http://openenergy-platform.org/ontology/oeo/OEO_00000334"/>
        <rdfs:subClassOf>
            <owl:Restriction>
                <owl:onProperty rdf:resource="http://openenergy-platform.org/ontology/oeo/OEO_00000503"/>
                <owl:someValuesFrom rdf:resource="http://openenergy-platform.org/ontology/oeo/OEO_00000220"/>
            </owl:Restriction>
        </rdfs:subClassOf>
        <obo:IAO_0000115>A hydrogen power unit is a power generating unit using hydrogen as fuel.</obo:IAO_0000115>
        <rdfs:label>hydrogen power unit</rdfs:label>
    </owl:Class>
    


    <!-- http://openenergy-platform.org/ontology/oeo/OEO_00000024 -->

    <owl:Class rdf:about="http://openenergy-platform.org/ontology/oeo/OEO_00000024">
        <owl:equivalentClass>
            <owl:Restriction>
                <owl:onProperty rdf:resource="http://openenergy-platform.org/ontology/oeo/OEO_00000503"/>
                <owl:someValuesFrom rdf:resource="http://openenergy-platform.org/ontology/oeo/OEO_00000251"/>
            </owl:Restriction>
        </owl:equivalentClass>
        <rdfs:subClassOf rdf:resource="http://openenergy-platform.org/ontology/oeo/OEO_00000008"/>
        <obo:IAO_0000115>A lignite power unit is a coal power unit using lignite as fuel.</obo:IAO_0000115>
        <rdfs:label>lignite power unit</rdfs:label>
    </owl:Class>
    


    <!-- http://openenergy-platform.org/ontology/oeo/OEO_00000025 -->

    <owl:Class rdf:about="http://openenergy-platform.org/ontology/oeo/OEO_00000025">
        <rdfs:subClassOf rdf:resource="http://openenergy-platform.org/ontology/oeo/OEO_00000331"/>
        <rdfs:subClassOf>
            <owl:Restriction>
                <owl:onProperty rdf:resource="http://purl.obolibrary.org/obo/RO_0000087"/>
                <owl:someValuesFrom rdf:resource="http://openenergy-platform.org/ontology/oeo/OEO_00000001"/>
            </owl:Restriction>
        </rdfs:subClassOf>
        <rdfs:subClassOf>
            <owl:Restriction>
                <owl:onProperty rdf:resource="http://purl.obolibrary.org/obo/RO_0000091"/>
                <owl:someValuesFrom rdf:resource="http://openenergy-platform.org/ontology/oeo/OEO_00000097"/>
            </owl:Restriction>
        </rdfs:subClassOf>
        <rdfs:subClassOf>
            <owl:Restriction>
                <owl:onProperty rdf:resource="http://purl.obolibrary.org/obo/RO_0000091"/>
                <owl:someValuesFrom rdf:resource="http://openenergy-platform.org/ontology/oeo/OEO_00000198"/>
            </owl:Restriction>
        </rdfs:subClassOf>
        <rdfs:subClassOf>
            <owl:Restriction>
                <owl:onProperty rdf:resource="http://purl.obolibrary.org/obo/RO_0000091"/>
                <owl:someValuesFrom rdf:resource="http://openenergy-platform.org/ontology/oeo/OEO_00010011"/>
            </owl:Restriction>
        </rdfs:subClassOf>
        <rdfs:subClassOf>
            <owl:Restriction>
                <owl:onProperty rdf:resource="http://openenergy-platform.org/ontology/oeo/OEO_00000529"/>
                <owl:hasValue rdf:resource="http://openenergy-platform.org/ontology/oeo/OEO_00000182"/>
            </owl:Restriction>
        </rdfs:subClassOf>
        <obo:IAO_0000115>Methane is a portion of matter with the chemical formular CH4. It has a gaseous normal state of matter. It occurs naturally in the atmosphere as a trace gas and can work as a greenhouse gas. As it can be oxidised it can be used as a fuel.</obo:IAO_0000115>
        <obo:IAO_0000118>CH4</obo:IAO_0000118>
        <rdfs:label>methane</rdfs:label>
    </owl:Class>
    


    <!-- http://openenergy-platform.org/ontology/oeo/OEO_00000026 -->

    <owl:Class rdf:about="http://openenergy-platform.org/ontology/oeo/OEO_00000026">
        <rdfs:subClassOf rdf:resource="http://openenergy-platform.org/ontology/oeo/OEO_00000331"/>
        <rdfs:subClassOf>
            <owl:Restriction>
                <owl:onProperty rdf:resource="http://openenergy-platform.org/ontology/oeo/OEO_00000530"/>
                <owl:someValuesFrom rdf:resource="http://openenergy-platform.org/ontology/oeo/OEO_00030000"/>
            </owl:Restriction>
        </rdfs:subClassOf>
        <rdfs:subClassOf>
            <owl:Restriction>
                <owl:onProperty rdf:resource="http://openenergy-platform.org/ontology/oeo/OEO_00000529"/>
                <owl:hasValue rdf:resource="http://openenergy-platform.org/ontology/oeo/OEO_00000182"/>
            </owl:Restriction>
        </rdfs:subClassOf>
        <obo:IAO_0000115>Nitrogen trifluoride is a portion of matter with the chemical formula NF3. It has a gaseous normal state of matter. It can work as a potent greenhouse gas and has an anthropogenic origin.</obo:IAO_0000115>
        <obo:IAO_0000118>NF3</obo:IAO_0000118>
        <rdfs:label>nitrogen trifluoride</rdfs:label>
    </owl:Class>
    


    <!-- http://openenergy-platform.org/ontology/oeo/OEO_00000027 -->

    <owl:Class rdf:about="http://openenergy-platform.org/ontology/oeo/OEO_00000027">
        <rdfs:subClassOf rdf:resource="http://openenergy-platform.org/ontology/oeo/OEO_00000331"/>
        <rdfs:subClassOf>
            <owl:Restriction>
                <owl:onProperty rdf:resource="http://purl.obolibrary.org/obo/RO_0000091"/>
                <owl:someValuesFrom rdf:resource="http://openenergy-platform.org/ontology/oeo/OEO_00000198"/>
            </owl:Restriction>
        </rdfs:subClassOf>
        <rdfs:subClassOf>
            <owl:Restriction>
                <owl:onProperty rdf:resource="http://openenergy-platform.org/ontology/oeo/OEO_00000529"/>
                <owl:hasValue rdf:resource="http://openenergy-platform.org/ontology/oeo/OEO_00000182"/>
            </owl:Restriction>
        </rdfs:subClassOf>
        <obo:IAO_0000115>Nitrous oxide is a portion of matter with the chemical formula N2O. It has a gaseous normal state of matter. It occurs naturally in the atmosphere as a trace gas and it can work as a greenhouse gas.</obo:IAO_0000115>
        <obo:IAO_0000118>N2O</obo:IAO_0000118>
        <rdfs:label>nitrous oxide</rdfs:label>
    </owl:Class>
    


    <!-- http://openenergy-platform.org/ontology/oeo/OEO_00000028 -->

    <owl:Class rdf:about="http://openenergy-platform.org/ontology/oeo/OEO_00000028">
        <rdfs:subClassOf rdf:resource="http://openenergy-platform.org/ontology/oeo/OEO_00000151"/>
        <obo:IAO_0000115>A nuclear energy carrier is an energy carrier used in nuclear power stations to produce heat for steam turbines. Heat is created when the nuclear fuel undergoes nuclear fission.</obo:IAO_0000115>
        <obo:IAO_0000233>issue: https://github.com/OpenEnergyPlatform/ontology/issues/182
pull request: https://github.com/OpenEnergyPlatform/ontology/pull/237</obo:IAO_0000233>
        <rdfs:label>nuclear energy carrier disposition</rdfs:label>
    </owl:Class>
    


    <!-- http://openenergy-platform.org/ontology/oeo/OEO_00000029 -->

    <owl:Class rdf:about="http://openenergy-platform.org/ontology/oeo/OEO_00000029">
        <rdfs:subClassOf rdf:resource="http://openenergy-platform.org/ontology/oeo/OEO_00000334"/>
        <rdfs:subClassOf>
            <owl:Restriction>
                <owl:onProperty rdf:resource="http://openenergy-platform.org/ontology/oeo/OEO_00000503"/>
                <owl:someValuesFrom rdf:resource="http://openenergy-platform.org/ontology/oeo/OEO_00000302"/>
            </owl:Restriction>
        </rdfs:subClassOf>
        <obo:IAO_0000115>A nuclear power unit is a power generating unit using nuclear fuel.</obo:IAO_0000115>
        <rdfs:label>nuclear power unit</rdfs:label>
    </owl:Class>
    


    <!-- http://openenergy-platform.org/ontology/oeo/OEO_00000030 -->

    <owl:Class rdf:about="http://openenergy-platform.org/ontology/oeo/OEO_00000030">
        <rdfs:subClassOf rdf:resource="http://openenergy-platform.org/ontology/oeo/OEO_00000334"/>
        <rdfs:subClassOf>
            <owl:Restriction>
                <owl:onProperty rdf:resource="http://openenergy-platform.org/ontology/oeo/OEO_00000503"/>
                <owl:someValuesFrom rdf:resource="http://openenergy-platform.org/ontology/oeo/OEO_00000309"/>
            </owl:Restriction>
        </rdfs:subClassOf>
        <obo:IAO_0000115>An oil power unit is a power generating unit using oil as fuel.</obo:IAO_0000115>
        <rdfs:label>oil power unit</rdfs:label>
    </owl:Class>
    


    <!-- http://openenergy-platform.org/ontology/oeo/OEO_00000031 -->

    <owl:Class rdf:about="http://openenergy-platform.org/ontology/oeo/OEO_00000031">
        <rdfs:subClassOf rdf:resource="http://openenergy-platform.org/ontology/oeo/OEO_00000061"/>
        <rdfs:subClassOf>
            <owl:Restriction>
                <owl:onProperty rdf:resource="http://purl.obolibrary.org/obo/BFO_0000051"/>
                <owl:someValuesFrom rdf:resource="http://openenergy-platform.org/ontology/oeo/OEO_00000334"/>
            </owl:Restriction>
        </rdfs:subClassOf>
        <rdfs:subClassOf>
            <owl:Restriction>
                <owl:onProperty rdf:resource="http://purl.obolibrary.org/obo/BFO_0000051"/>
                <owl:someValuesFrom rdf:resource="http://openenergy-platform.org/ontology/oeo/OEO_00020006"/>
            </owl:Restriction>
        </rdfs:subClassOf>
        <rdfs:subClassOf>
            <owl:Restriction>
                <owl:onProperty rdf:resource="http://purl.obolibrary.org/obo/RO_0000056"/>
                <owl:someValuesFrom rdf:resource="http://openenergy-platform.org/ontology/oeo/OEO_00020003"/>
            </owl:Restriction>
        </rdfs:subClassOf>
        <obo:IAO_0000115>A powerplant is an artificial object consisting of power generating units and a grid component that feeds electric energy into an electric grid.</obo:IAO_0000115>
        <obo:IAO_0000233>issue: https://github.com/OpenEnergyPlatform/ontology/issues/588
pull request: https://github.com/OpenEnergyPlatform/ontology/pull/594

issue: https://github.com/OpenEnergyPlatform/ontology/issues/173
pull request: https://github.com/OpenEnergyPlatform/ontology/pull/273

issue: https://github.com/OpenEnergyPlatform/ontology/issues/372
pull request: https://github.com/OpenEnergyPlatform/ontology/pull/646</obo:IAO_0000233>
        <rdfs:label>powerplant</rdfs:label>
    </owl:Class>
    


    <!-- http://openenergy-platform.org/ontology/oeo/OEO_00000032 -->

    <owl:Class rdf:about="http://openenergy-platform.org/ontology/oeo/OEO_00000032">
        <rdfs:subClassOf rdf:resource="http://openenergy-platform.org/ontology/oeo/OEO_00000188"/>
        <obo:IAO_0000115>A PV cell is a generator that converts light into electrical energy.</obo:IAO_0000115>
        <rdfs:label>PV cell</rdfs:label>
    </owl:Class>
    


    <!-- http://openenergy-platform.org/ontology/oeo/OEO_00000033 -->

    <owl:Class rdf:about="http://openenergy-platform.org/ontology/oeo/OEO_00000033">
        <owl:equivalentClass>
            <owl:Class>
                <owl:intersectionOf rdf:parseType="Collection">
                    <rdf:Description rdf:about="http://openenergy-platform.org/ontology/oeo/OEO_00000173"/>
                    <owl:Restriction>
                        <owl:onProperty rdf:resource="http://openenergy-platform.org/ontology/oeo/OEO_00000530"/>
                        <owl:someValuesFrom rdf:resource="http://openenergy-platform.org/ontology/oeo/OEO_00030004"/>
                    </owl:Restriction>
                </owl:intersectionOf>
            </owl:Class>
        </owl:equivalentClass>
        <rdfs:subClassOf>
            <owl:Restriction>
                <owl:onProperty rdf:resource="http://purl.obolibrary.org/obo/RO_0000091"/>
                <owl:someValuesFrom rdf:resource="http://openenergy-platform.org/ontology/oeo/OEO_00000097"/>
            </owl:Restriction>
        </rdfs:subClassOf>
        <obo:IAO_0000115>A renewable fuel is a fuel that has a renewable origin and an energy carrier disposition that is used as a fuel.</obo:IAO_0000115>
        <rdfs:label>renewable fuel</rdfs:label>
    </owl:Class>
    


    <!-- http://openenergy-platform.org/ontology/oeo/OEO_00000034 -->

    <owl:Class rdf:about="http://openenergy-platform.org/ontology/oeo/OEO_00000034">
        <rdfs:subClassOf rdf:resource="http://openenergy-platform.org/ontology/oeo/OEO_00000334"/>
        <obo:IAO_0000115>A solar power unit is a power generating unit using solar power.</obo:IAO_0000115>
        <rdfs:label>solar power unit</rdfs:label>
    </owl:Class>
    


    <!-- http://openenergy-platform.org/ontology/oeo/OEO_00000035 -->

    <owl:Class rdf:about="http://openenergy-platform.org/ontology/oeo/OEO_00000035">
        <rdfs:subClassOf rdf:resource="http://openenergy-platform.org/ontology/oeo/OEO_00000034"/>
        <rdfs:subClassOf>
            <owl:Restriction>
                <owl:onProperty rdf:resource="http://purl.obolibrary.org/obo/BFO_0000051"/>
                <owl:someValuesFrom rdf:resource="http://openenergy-platform.org/ontology/oeo/OEO_00000387"/>
            </owl:Restriction>
        </rdfs:subClassOf>
        <obo:IAO_0000115>A solar thermal power unit is a solar power unit that has solar thermal collectors as parts.</obo:IAO_0000115>
        <rdfs:label>solar thermal power unit</rdfs:label>
    </owl:Class>
    


    <!-- http://openenergy-platform.org/ontology/oeo/OEO_00000036 -->

    <owl:Class rdf:about="http://openenergy-platform.org/ontology/oeo/OEO_00000036">
        <rdfs:subClassOf rdf:resource="http://openenergy-platform.org/ontology/oeo/OEO_00000073"/>
        <obo:IAO_0000115>A solid biomass powerplant is a biomass powerplant having an aggregate of solid biomass power units as its power generating units.</obo:IAO_0000115>
        <rdfs:label>solid biomass powerplant</rdfs:label>
    </owl:Class>
    


    <!-- http://openenergy-platform.org/ontology/oeo/OEO_00000037 -->

    <owl:Class rdf:about="http://openenergy-platform.org/ontology/oeo/OEO_00000037">
        <rdfs:subClassOf rdf:resource="http://openenergy-platform.org/ontology/oeo/OEO_00000003"/>
        <rdfs:subClassOf>
            <owl:Restriction>
                <owl:onProperty rdf:resource="http://openenergy-platform.org/ontology/oeo/OEO_00000503"/>
                <owl:someValuesFrom rdf:resource="http://openenergy-platform.org/ontology/oeo/OEO_00000332"/>
            </owl:Restriction>
        </rdfs:subClassOf>
        <obo:IAO_0000115>A solid biomass power unit is a biomass power unit using solid biomass as fuel.</obo:IAO_0000115>
        <rdfs:label>solid biomass power unit</rdfs:label>
    </owl:Class>
    


    <!-- http://openenergy-platform.org/ontology/oeo/OEO_00000038 -->

    <owl:Class rdf:about="http://openenergy-platform.org/ontology/oeo/OEO_00000038">
        <rdfs:subClassOf rdf:resource="http://openenergy-platform.org/ontology/oeo/OEO_00000331"/>
        <rdfs:subClassOf>
            <owl:Restriction>
                <owl:onProperty rdf:resource="http://openenergy-platform.org/ontology/oeo/OEO_00000530"/>
                <owl:someValuesFrom rdf:resource="http://openenergy-platform.org/ontology/oeo/OEO_00030000"/>
            </owl:Restriction>
        </rdfs:subClassOf>
        <rdfs:subClassOf>
            <owl:Restriction>
                <owl:onProperty rdf:resource="http://openenergy-platform.org/ontology/oeo/OEO_00000529"/>
                <owl:hasValue rdf:resource="http://openenergy-platform.org/ontology/oeo/OEO_00000182"/>
            </owl:Restriction>
        </rdfs:subClassOf>
        <obo:IAO_0000115>Sulphur hexafluoride is a portion of matter with the chemical formula SF6. It has a gaseous normal state of matter. It can work as a potent greenhouse gas and has an anthropogenic origin.</obo:IAO_0000115>
        <obo:IAO_0000118>SF6</obo:IAO_0000118>
        <rdfs:label>sulphur hexafluoride</rdfs:label>
    </owl:Class>
    


    <!-- http://openenergy-platform.org/ontology/oeo/OEO_00000039 -->

    <owl:Class rdf:about="http://openenergy-platform.org/ontology/oeo/OEO_00000039">
        <rdfs:subClassOf rdf:resource="http://openenergy-platform.org/ontology/oeo/OEO_00000012"/>
        <obo:IAO_0000115>A thermal energy storage is an energy storage that stores thermal energy for later use.</obo:IAO_0000115>
        <rdfs:label>thermal energy storage</rdfs:label>
    </owl:Class>
    


    <!-- http://openenergy-platform.org/ontology/oeo/OEO_00000040 -->

    <owl:Class rdf:about="http://openenergy-platform.org/ontology/oeo/OEO_00000040">
        <rdfs:subClassOf rdf:resource="http://openenergy-platform.org/ontology/oeo/OEO_00000331"/>
        <rdfs:subClassOf>
            <owl:Restriction>
                <owl:onProperty rdf:resource="http://openenergy-platform.org/ontology/oeo/OEO_00000530"/>
                <owl:someValuesFrom rdf:resource="http://openenergy-platform.org/ontology/oeo/OEO_00030003"/>
            </owl:Restriction>
        </rdfs:subClassOf>
        <rdfs:subClassOf>
            <owl:Restriction>
                <owl:onProperty rdf:resource="http://purl.obolibrary.org/obo/RO_0000087"/>
                <owl:someValuesFrom rdf:resource="http://openenergy-platform.org/ontology/oeo/OEO_00000001"/>
            </owl:Restriction>
        </rdfs:subClassOf>
        <rdfs:subClassOf>
            <owl:Restriction>
                <owl:onProperty rdf:resource="http://purl.obolibrary.org/obo/RO_0000091"/>
                <owl:someValuesFrom rdf:resource="http://openenergy-platform.org/ontology/oeo/OEO_00000028"/>
            </owl:Restriction>
        </rdfs:subClassOf>
        <rdfs:subClassOf>
            <owl:Restriction>
                <owl:onProperty rdf:resource="http://openenergy-platform.org/ontology/oeo/OEO_00000529"/>
                <owl:hasValue rdf:resource="http://openenergy-platform.org/ontology/oeo/OEO_00000390"/>
            </owl:Restriction>
        </rdfs:subClassOf>
        <obo:IAO_0000115>Uranium is a portion of matter that has the atomic number 92. It is a silver-grey metal.</obo:IAO_0000115>
        <obo:IAO_0000233>issue: https://github.com/OpenEnergyPlatform/ontology/issues/182
pull request: https://github.com/OpenEnergyPlatform/ontology/pull/237</obo:IAO_0000233>
        <rdfs:label>uranium</rdfs:label>
    </owl:Class>
    


    <!-- http://openenergy-platform.org/ontology/oeo/OEO_00000041 -->

    <owl:Class rdf:about="http://openenergy-platform.org/ontology/oeo/OEO_00000041">
        <rdfs:subClassOf rdf:resource="http://openenergy-platform.org/ontology/oeo/OEO_00000334"/>
        <rdfs:subClassOf>
            <owl:Restriction>
                <owl:onProperty rdf:resource="http://openenergy-platform.org/ontology/oeo/OEO_00000503"/>
                <owl:someValuesFrom rdf:resource="http://openenergy-platform.org/ontology/oeo/OEO_00000439"/>
            </owl:Restriction>
        </rdfs:subClassOf>
        <obo:IAO_0000115>A waste power unit is a power generating unit using waste as fuel.</obo:IAO_0000115>
        <rdfs:label>waste power unit</rdfs:label>
    </owl:Class>
    


    <!-- http://openenergy-platform.org/ontology/oeo/OEO_00000042 -->

    <owl:Class rdf:about="http://openenergy-platform.org/ontology/oeo/OEO_00000042">
        <rdfs:subClassOf rdf:resource="http://purl.obolibrary.org/obo/BFO_0000023"/>
        <obo:IAO_0000115>A waste role is a role of an object aggregate that has been discarded after primary use.</obo:IAO_0000115>
        <obo:IAO_0000233>issue: https://github.com/OpenEnergyPlatform/ontology/issues/132
pull request: https://github.com/OpenEnergyPlatform/ontology/pull/207</obo:IAO_0000233>
        <rdfs:label>waste role</rdfs:label>
    </owl:Class>
    


    <!-- http://openenergy-platform.org/ontology/oeo/OEO_00000043 -->

    <owl:Class rdf:about="http://openenergy-platform.org/ontology/oeo/OEO_00000043">
        <rdfs:subClassOf rdf:resource="http://purl.obolibrary.org/obo/BFO_0000015"/>
        <rdfs:subClassOf>
            <owl:Restriction>
                <owl:onProperty rdf:resource="http://purl.obolibrary.org/obo/RO_0000057"/>
                <owl:someValuesFrom rdf:resource="http://openenergy-platform.org/ontology/oeo/OEO_00000054"/>
            </owl:Restriction>
        </rdfs:subClassOf>
        <obo:IAO_0000115>Wind is a process of air naturally moving.</obo:IAO_0000115>
        <obo:IAO_0000233>issue: https://github.com/OpenEnergyPlatform/ontology/issues/211
pull request: https://github.com/OpenEnergyPlatform/ontology/pull/225</obo:IAO_0000233>
        <rdfs:label>wind</rdfs:label>
    </owl:Class>
    


    <!-- http://openenergy-platform.org/ontology/oeo/OEO_00000044 -->

    <owl:Class rdf:about="http://openenergy-platform.org/ontology/oeo/OEO_00000044">
        <rdfs:subClassOf rdf:resource="http://openenergy-platform.org/ontology/oeo/OEO_00000334"/>
        <rdfs:subClassOf>
            <owl:Restriction>
                <owl:onProperty rdf:resource="http://purl.obolibrary.org/obo/BFO_0000051"/>
                <owl:someValuesFrom rdf:resource="http://openenergy-platform.org/ontology/oeo/OEO_00000425"/>
            </owl:Restriction>
        </rdfs:subClassOf>
        <rdfs:subClassOf>
            <owl:Restriction>
                <owl:onProperty rdf:resource="http://purl.obolibrary.org/obo/RO_0000086"/>
                <owl:someValuesFrom rdf:resource="http://openenergy-platform.org/ontology/oeo/OEO_00140000"/>
            </owl:Restriction>
        </rdfs:subClassOf>
        <obo:IAO_0000115>A wind energy converting unit is a power generating unit that uses wind energy.</obo:IAO_0000115>
        <obo:IAO_0000118>wind turbine</obo:IAO_0000118>
        <rdfs:label>wind energy converting unit</rdfs:label>
    </owl:Class>
    


    <!-- http://openenergy-platform.org/ontology/oeo/OEO_00000047 -->

    <owl:Class rdf:about="http://openenergy-platform.org/ontology/oeo/OEO_00000047">
        <rdfs:subClassOf rdf:resource="http://openenergy-platform.org/ontology/oeo/OEO_00000253"/>
        <owl:disjointWith rdf:resource="http://openenergy-platform.org/ontology/oeo/OEO_00000126"/>
        <obo:IAO_0000115 xml:lang="en">An AC-line is a powerline for transferring high voltage alternating current.</obo:IAO_0000115>
        <obo:IAO_0000233>issue: https://github.com/OpenEnergyPlatform/ontology/issues/231
pull request: https://github.com/OpenEnergyPlatform/ontology/pull/385</obo:IAO_0000233>
        <rdfs:comment>undirected</rdfs:comment>
        <rdfs:label xml:lang="en">AC-line</rdfs:label>
    </owl:Class>
    


    <!-- http://openenergy-platform.org/ontology/oeo/OEO_00000054 -->

    <owl:Class rdf:about="http://openenergy-platform.org/ontology/oeo/OEO_00000054">
        <rdfs:subClassOf rdf:resource="http://openenergy-platform.org/ontology/oeo/OEO_00000331"/>
        <rdfs:subClassOf>
            <owl:Restriction>
                <owl:onProperty rdf:resource="http://openenergy-platform.org/ontology/oeo/OEO_00000501"/>
                <owl:someValuesFrom rdf:resource="http://openenergy-platform.org/ontology/oeo/OEO_00000399"/>
            </owl:Restriction>
        </rdfs:subClassOf>
        <rdfs:subClassOf>
            <owl:Restriction>
                <owl:onProperty rdf:resource="http://openenergy-platform.org/ontology/oeo/OEO_00000530"/>
                <owl:someValuesFrom rdf:resource="http://openenergy-platform.org/ontology/oeo/OEO_00030004"/>
            </owl:Restriction>
        </rdfs:subClassOf>
        <rdfs:subClassOf>
            <owl:Restriction>
                <owl:onProperty rdf:resource="http://purl.obolibrary.org/obo/RO_0000086"/>
                <owl:someValuesFrom rdf:resource="http://openenergy-platform.org/ontology/oeo/OEO_00000446"/>
            </owl:Restriction>
        </rdfs:subClassOf>
        <rdfs:subClassOf>
            <owl:Restriction>
                <owl:onProperty rdf:resource="http://purl.obolibrary.org/obo/RO_0000091"/>
                <owl:someValuesFrom rdf:resource="http://openenergy-platform.org/ontology/oeo/OEO_00000151"/>
            </owl:Restriction>
        </rdfs:subClassOf>
        <rdfs:subClassOf>
            <owl:Restriction>
                <owl:onProperty rdf:resource="http://openenergy-platform.org/ontology/oeo/OEO_00000529"/>
                <owl:hasValue rdf:resource="http://openenergy-platform.org/ontology/oeo/OEO_00000182"/>
            </owl:Restriction>
        </rdfs:subClassOf>
        <obo:IAO_0000115 xml:lang="en">Air is a portion of matter that consists of a composition of gases that forms the Earth&apos;s atmosphere.</obo:IAO_0000115>
        <obo:IAO_0000119>https://en.wikipedia.org/wiki/Air_(disambiguation)</obo:IAO_0000119>
        <obo:IAO_0000233>add origin
issue: https://github.com/OpenEnergyPlatform/ontology/issues/515
pull request: https://github.com/OpenEnergyPlatform/ontology/pull/684</obo:IAO_0000233>
        <rdfs:label>air</rdfs:label>
    </owl:Class>
    


    <!-- http://openenergy-platform.org/ontology/oeo/OEO_00000055 -->

    <owl:Class rdf:about="http://openenergy-platform.org/ontology/oeo/OEO_00000055">
        <rdfs:subClassOf rdf:resource="http://openenergy-platform.org/ontology/oeo/OEO_00000330"/>
        <rdfs:subClassOf>
            <owl:Restriction>
                <owl:onProperty rdf:resource="http://purl.obolibrary.org/obo/RO_0000057"/>
                <owl:someValuesFrom rdf:resource="http://openenergy-platform.org/ontology/oeo/OEO_00010012"/>
            </owl:Restriction>
        </rdfs:subClassOf>
        <obo:IAO_0000115 xml:lang="en">Air pollution occurs when harmful or excessive quantities of substances including gases, particles, and biological molecules are introduced into Earth&apos;s atmosphere.</obo:IAO_0000115>
        <obo:IAO_0000119 xml:lang="en">https://en.wikipedia.org/w/index.php?title=Air_pollution&amp;oldid=877082014</obo:IAO_0000119>
        <obo:IAO_0000233>issue: https://github.com/OpenEnergyPlatform/ontology/issues/406
pull request: https://github.com/OpenEnergyPlatform/ontology/pull/410</obo:IAO_0000233>
        <rdfs:label>air pollution</rdfs:label>
    </owl:Class>
    


    <!-- http://openenergy-platform.org/ontology/oeo/OEO_00000056 -->

    <owl:Class rdf:about="http://openenergy-platform.org/ontology/oeo/OEO_00000056">
        <rdfs:subClassOf rdf:resource="http://openenergy-platform.org/ontology/oeo/OEO_00000207"/>
        <obo:IAO_0000115 xml:lang="en">Ambient thermal energy is thermal energy that is stored in the ambient air, beneath the surface of solid earth or in surface water. It is captured by heat pumps.</obo:IAO_0000115>
        <obo:IAO_0000233>issue: https://github.com/OpenEnergyPlatform/ontology/issues/728
pull request: https://github.com/OpenEnergyPlatform/ontology/pull/742</obo:IAO_0000233>
        <rdfs:label>ambient thermal energy</rdfs:label>
    </owl:Class>
    


    <!-- http://openenergy-platform.org/ontology/oeo/OEO_00000058 -->

    <owl:Class rdf:about="http://openenergy-platform.org/ontology/oeo/OEO_00000058">
        <rdfs:subClassOf rdf:resource="http://openenergy-platform.org/ontology/oeo/OEO_00000204"/>
        <obo:IAO_0000115>Anthracite is a hard coal with a high caloric value due to its high carbon content (about 90 % fixed carbon).</obo:IAO_0000115>
        <obo:IAO_0000119 xml:lang="en">REGULATION (EC) No 1099/2008 OF THE EUROPEAN PARLIAMENT AND OF THE COUNCIL of 22 October 2008 on energy statistics https://eur-lex.europa.eu/legal-content/EN/TXT/HTML/?uri=CELEX:32008R1099&amp;from=EN</obo:IAO_0000119>
        <rdfs:comment xml:lang="en">Its gross calorific value is greater than 23 865 kJ/kg (5 700 kcal/kg) on an ash-free but moist basis.</rdfs:comment>
        <rdfs:label>anthracite</rdfs:label>
    </owl:Class>
    


    <!-- http://openenergy-platform.org/ontology/oeo/OEO_00000061 -->

    <owl:Class rdf:about="http://openenergy-platform.org/ontology/oeo/OEO_00000061">
        <rdfs:subClassOf rdf:resource="http://purl.obolibrary.org/obo/BFO_0000030"/>
        <obo:IAO_0000115>An artificial object is an object that was deliberately manufactured by humans to address a particular purpose.</obo:IAO_0000115>
        <obo:IAO_0000233>issue: https://github.com/OpenEnergyPlatform/ontology/issues/86
pull requests: https://github.com/OpenEnergyPlatform/ontology/pull/121 (artificial object definition),
 https://github.com/OpenEnergyPlatform/ontology/pull/128 (subclasses)</obo:IAO_0000233>
        <rdfs:label>artificial object</rdfs:label>
    </owl:Class>
    


    <!-- http://openenergy-platform.org/ontology/oeo/OEO_00000062 -->

    <owl:Class rdf:about="http://openenergy-platform.org/ontology/oeo/OEO_00000062">
        <rdfs:subClassOf rdf:resource="http://openenergy-platform.org/ontology/oeo/OEO_00000292"/>
        <obo:IAO_0000115 xml:lang="en">Associated gas is a natural gas that is a byproduct from crude oil exploitation.</obo:IAO_0000115>
        <obo:IAO_0000119 xml:lang="en">REGULATION (EC) No 1099/2008 OF THE EUROPEAN PARLIAMENT AND OF THE COUNCIL of 22 October 2008 on energy statistics https://eur-lex.europa.eu/legal-content/EN/TXT/HTML/?uri=CELEX:32008R1099&amp;from=EN</obo:IAO_0000119>
        <rdfs:label>associated gas</rdfs:label>
    </owl:Class>
    


    <!-- http://openenergy-platform.org/ontology/oeo/OEO_00000066 -->

    <owl:Class rdf:about="http://openenergy-platform.org/ontology/oeo/OEO_00000066">
        <rdfs:subClassOf rdf:resource="http://openenergy-platform.org/ontology/oeo/OEO_00000183"/>
        <obo:IAO_0000115 xml:lang="en">Aviation gasoline is gasoline used as motor spirit and prepared especially for aviation piston engines, with an octane number suited to the engine, a freezing point of -60 °C and a distillation range usually within the limits of 30 °C and 180 °C.</obo:IAO_0000115>
        <obo:IAO_0000119 xml:lang="en">REGULATION (EC) No 1099/2008 OF THE EUROPEAN PARLIAMENT AND OF THE COUNCIL of 22 October 2008 on energy statistics https://eur-lex.europa.eu/legal-content/EN/TXT/HTML/?uri=CELEX:32008R1099&amp;from=EN</obo:IAO_0000119>
        <rdfs:label>aviation gasoline</rdfs:label>
    </owl:Class>
    


    <!-- http://openenergy-platform.org/ontology/oeo/OEO_00000068 -->

    <owl:Class rdf:about="http://openenergy-platform.org/ontology/oeo/OEO_00000068">
        <rdfs:subClassOf rdf:resource="http://openenergy-platform.org/ontology/oeo/OEO_00000159"/>
        <rdfs:subClassOf>
            <owl:Restriction>
                <owl:onProperty rdf:resource="http://purl.obolibrary.org/obo/RO_0000085"/>
                <owl:someValuesFrom rdf:resource="http://openenergy-platform.org/ontology/oeo/OEO_00000070"/>
            </owl:Restriction>
        </rdfs:subClassOf>
        <obo:IAO_0000115 xml:lang="en">A battery is a device using different chemical or physical reactions to store energy.</obo:IAO_0000115>
        <rdfs:label>battery</rdfs:label>
    </owl:Class>
    


    <!-- http://openenergy-platform.org/ontology/oeo/OEO_00000070 -->

    <owl:Class rdf:about="http://openenergy-platform.org/ontology/oeo/OEO_00000070">
        <rdfs:subClassOf rdf:resource="http://openenergy-platform.org/ontology/oeo/OEO_00000012"/>
        <owl:disjointWith rdf:resource="http://openenergy-platform.org/ontology/oeo/OEO_00000269"/>
        <obo:IAO_0000115 xml:lang="en">A battery storage is a energy storage that uses batteries to store energy.</obo:IAO_0000115>
        <rdfs:label>battery storage</rdfs:label>
    </owl:Class>
    


    <!-- http://openenergy-platform.org/ontology/oeo/OEO_00000071 -->

    <owl:Class rdf:about="http://openenergy-platform.org/ontology/oeo/OEO_00000071">
        <rdfs:subClassOf rdf:resource="http://openenergy-platform.org/ontology/oeo/OEO_00000331"/>
        <rdfs:subClassOf>
            <owl:Restriction>
                <owl:onProperty rdf:resource="http://openenergy-platform.org/ontology/oeo/OEO_00000530"/>
                <owl:someValuesFrom rdf:resource="http://openenergy-platform.org/ontology/oeo/OEO_00030001"/>
            </owl:Restriction>
        </rdfs:subClassOf>
        <rdfs:subClassOf>
            <owl:Restriction>
                <owl:onProperty rdf:resource="http://purl.obolibrary.org/obo/RO_0000087"/>
                <owl:someValuesFrom rdf:resource="http://openenergy-platform.org/ontology/oeo/OEO_00000001"/>
            </owl:Restriction>
        </rdfs:subClassOf>
        <rdfs:subClassOf>
            <owl:Restriction>
                <owl:onProperty rdf:resource="http://purl.obolibrary.org/obo/RO_0000091"/>
                <owl:someValuesFrom rdf:resource="http://openenergy-platform.org/ontology/oeo/OEO_00000097"/>
            </owl:Restriction>
        </rdfs:subClassOf>
        <rdfs:subClassOf>
            <owl:Restriction>
                <owl:onProperty rdf:resource="http://openenergy-platform.org/ontology/oeo/OEO_00000529"/>
                <owl:hasValue rdf:resource="http://openenergy-platform.org/ontology/oeo/OEO_00000256"/>
            </owl:Restriction>
        </rdfs:subClassOf>
        <obo:IAO_0000115>Biodiesel is a portion of matter that includes bio-diesel (a methyl-ester produced from vegetable or animal oil, of diesel quality), biodimethylether (dimethylether produced from biomass), Fischer-Tropsch (Fischer-Tropsch produced from biomass), cold extracted bio-oil (oil produced from oil seed through mechanical processing only) and all other liquid biofuels which are added to, blended with or used straight as transport diesel.</obo:IAO_0000115>
        <obo:IAO_0000119>REGULATION (EC) No 1099/2008 OF THE EUROPEAN PARLIAMENT AND OF THE COUNCIL of 22 October 2008 on energy statistics https://eur-lex.europa.eu/legal-content/EN/TXT/HTML/?uri=CELEX:32008R1099&amp;from=EN</obo:IAO_0000119>
        <rdfs:label>biodiesel</rdfs:label>
    </owl:Class>
    


    <!-- http://openenergy-platform.org/ontology/oeo/OEO_00000072 -->

    <owl:Class rdf:about="http://openenergy-platform.org/ontology/oeo/OEO_00000072">
        <owl:equivalentClass>
            <owl:Class>
                <owl:intersectionOf rdf:parseType="Collection">
                    <rdf:Description rdf:about="http://openenergy-platform.org/ontology/oeo/OEO_00000173"/>
                    <owl:Restriction>
                        <owl:onProperty rdf:resource="http://openenergy-platform.org/ontology/oeo/OEO_00000530"/>
                        <owl:someValuesFrom rdf:resource="http://openenergy-platform.org/ontology/oeo/OEO_00030001"/>
                    </owl:Restriction>
                </owl:intersectionOf>
            </owl:Class>
        </owl:equivalentClass>
        <rdfs:subClassOf rdf:resource="http://openenergy-platform.org/ontology/oeo/OEO_00000173"/>
        <rdfs:subClassOf>
            <owl:Restriction>
                <owl:onProperty rdf:resource="http://openenergy-platform.org/ontology/oeo/OEO_00000530"/>
                <owl:someValuesFrom rdf:resource="http://openenergy-platform.org/ontology/oeo/OEO_00030001"/>
            </owl:Restriction>
        </rdfs:subClassOf>
        <rdfs:subClassOf>
            <owl:Restriction>
                <owl:onProperty rdf:resource="http://openenergy-platform.org/ontology/oeo/OEO_00000530"/>
                <owl:someValuesFrom rdf:resource="http://openenergy-platform.org/ontology/oeo/OEO_00030004"/>
            </owl:Restriction>
        </rdfs:subClassOf>
        <rdfs:subClassOf>
            <owl:Restriction>
                <owl:onProperty rdf:resource="http://purl.obolibrary.org/obo/RO_0000091"/>
                <owl:someValuesFrom rdf:resource="http://openenergy-platform.org/ontology/oeo/OEO_00000097"/>
            </owl:Restriction>
        </rdfs:subClassOf>
        <obo:IAO_0000115>A biofuel is a fuel that is produced through contemporary biological processes, such as agriculture and anaerobic digestion, rather than a fuel produced by geological processes such as those involved in the formation of fossil fuels, such as coal and petroleum, from prehistoric biological matter.

Biofuels can be derived directly from plants (i.e. energy crops), or indirectly from agricultural, commercial, domestic, and/or industrial wastes.[1] Renewable biofuels generally involve contemporary carbon fixation, such as those that occur in plants or microalgae through the process of photosynthesis. Other renewable biofuels are made through the use or conversion of biomass (referring to recently living organisms, most often referring to plants or plant-derived materials). This biomass can be converted to convenient energy-containing substances in three different ways: thermal conversion, chemical conversion, and biochemical conversion. This biomass conversion can result in fuel in solid, liquid, or gas form. This new biomass can also be used directly for biofuels.</obo:IAO_0000115>
        <obo:IAO_0000119>https://en.wikipedia.org/w/index.php?title=Biofuel&amp;oldid=866432109</obo:IAO_0000119>
        <obo:IAO_0000233>issue: https://github.com/OpenEnergyPlatform/ontology/issues/396
pull request: https://github.com/OpenEnergyPlatform/ontology/pull/400</obo:IAO_0000233>
        <rdfs:label>biofuel</rdfs:label>
    </owl:Class>
    


    <!-- http://openenergy-platform.org/ontology/oeo/OEO_00000073 -->

    <owl:Class rdf:about="http://openenergy-platform.org/ontology/oeo/OEO_00000073">
        <rdfs:subClassOf rdf:resource="http://openenergy-platform.org/ontology/oeo/OEO_00000031"/>
        <rdfs:subClassOf>
            <owl:Restriction>
                <owl:onProperty rdf:resource="http://purl.obolibrary.org/obo/BFO_0000051"/>
                <owl:someValuesFrom rdf:resource="http://openenergy-platform.org/ontology/oeo/OEO_00000003"/>
            </owl:Restriction>
        </rdfs:subClassOf>
        <obo:IAO_0000115>A biofuel powerplant is a powerplant having an aggregate of biofuel power units as its power generating units.</obo:IAO_0000115>
        <rdfs:label>biofuel powerplant</rdfs:label>
    </owl:Class>
    


    <!-- http://openenergy-platform.org/ontology/oeo/OEO_00000074 -->

    <owl:Class rdf:about="http://openenergy-platform.org/ontology/oeo/OEO_00000074">
        <rdfs:subClassOf rdf:resource="http://openenergy-platform.org/ontology/oeo/OEO_00000072"/>
        <rdfs:subClassOf>
            <owl:Restriction>
                <owl:onProperty rdf:resource="http://openenergy-platform.org/ontology/oeo/OEO_00000530"/>
                <owl:someValuesFrom rdf:resource="http://openenergy-platform.org/ontology/oeo/OEO_00030001"/>
            </owl:Restriction>
        </rdfs:subClassOf>
        <rdfs:subClassOf>
            <owl:Restriction>
                <owl:onProperty rdf:resource="http://purl.obolibrary.org/obo/RO_0000091"/>
                <owl:someValuesFrom rdf:resource="http://openenergy-platform.org/ontology/oeo/OEO_00000097"/>
            </owl:Restriction>
        </rdfs:subClassOf>
        <rdfs:subClassOf>
            <owl:Restriction>
                <owl:onProperty rdf:resource="http://openenergy-platform.org/ontology/oeo/OEO_00000529"/>
                <owl:hasValue rdf:resource="http://openenergy-platform.org/ontology/oeo/OEO_00000182"/>
            </owl:Restriction>
        </rdfs:subClassOf>
        <obo:IAO_0000115>A biogas is a biofuel which has a gaseous state and is composed principally of methane and carbon dioxide produced by anaerobic digestion of biomass. It is used as a biofuel.</obo:IAO_0000115>
        <rdfs:label>biogas</rdfs:label>
    </owl:Class>
    


    <!-- http://openenergy-platform.org/ontology/oeo/OEO_00000075 -->

    <owl:Class rdf:about="http://openenergy-platform.org/ontology/oeo/OEO_00000075">
        <rdfs:subClassOf rdf:resource="http://openenergy-platform.org/ontology/oeo/OEO_00000331"/>
        <rdfs:subClassOf>
            <owl:Restriction>
                <owl:onProperty rdf:resource="http://openenergy-platform.org/ontology/oeo/OEO_00000530"/>
                <owl:someValuesFrom rdf:resource="http://openenergy-platform.org/ontology/oeo/OEO_00030001"/>
            </owl:Restriction>
        </rdfs:subClassOf>
        <rdfs:subClassOf>
            <owl:Restriction>
                <owl:onProperty rdf:resource="http://purl.obolibrary.org/obo/BFO_0000051"/>
                <owl:someValuesFrom rdf:resource="http://openenergy-platform.org/ontology/oeo/OEO_00020001"/>
            </owl:Restriction>
        </rdfs:subClassOf>
        <rdfs:subClassOf>
            <owl:Restriction>
                <owl:onProperty rdf:resource="http://purl.obolibrary.org/obo/RO_0000087"/>
                <owl:someValuesFrom rdf:resource="http://openenergy-platform.org/ontology/oeo/OEO_00000001"/>
            </owl:Restriction>
        </rdfs:subClassOf>
        <rdfs:subClassOf>
            <owl:Restriction>
                <owl:onProperty rdf:resource="http://purl.obolibrary.org/obo/RO_0000091"/>
                <owl:someValuesFrom rdf:resource="http://openenergy-platform.org/ontology/oeo/OEO_00000097"/>
            </owl:Restriction>
        </rdfs:subClassOf>
        <rdfs:subClassOf>
            <owl:Restriction>
                <owl:onProperty rdf:resource="http://openenergy-platform.org/ontology/oeo/OEO_00000529"/>
                <owl:hasValue rdf:resource="http://openenergy-platform.org/ontology/oeo/OEO_00000256"/>
            </owl:Restriction>
        </rdfs:subClassOf>
        <obo:IAO_0000115>Biogasoline is a portion of matter that includes bioethanol (ethanol produced from biomass and/or the biodegradable fraction of waste), biomethanol (methanol produced from biomass and/or the biodegradable fraction of waste), bioETBE (ethyl-tertio-butyl-ether produced on the basis of bioethanol; the percentage by volume of bioETBE that is calculated as biofuel is 47 %) and bioMTBE (methyl-tertio-butyl-ether produced on the basis of biomethanol: the percentage by volume of bioMTBE that is calculated as biofuel is 36 %)</obo:IAO_0000115>
        <obo:IAO_0000118 xml:lang="en">Bioethanol</obo:IAO_0000118>
        <obo:IAO_0000119>REGULATION (EC) No 1099/2008 OF THE EUROPEAN PARLIAMENT AND OF THE COUNCIL of 22 October 2008 on energy statistics https://eur-lex.europa.eu/legal-content/EN/TXT/HTML/?uri=CELEX:32008R1099&amp;from=EN</obo:IAO_0000119>
        <obo:IAO_0000233>issue: https://github.com/OpenEnergyPlatform/ontology/issues/439
pull request: https://github.com/OpenEnergyPlatform/ontology/pull/445</obo:IAO_0000233>
        <rdfs:label>biogasoline</rdfs:label>
        <rdfs:label xml:lang="en">biogasoline</rdfs:label>
    </owl:Class>
    


    <!-- http://openenergy-platform.org/ontology/oeo/OEO_00000077 -->

    <owl:Class rdf:about="http://openenergy-platform.org/ontology/oeo/OEO_00000077">
        <rdfs:subClassOf rdf:resource="http://openenergy-platform.org/ontology/oeo/OEO_00000263"/>
        <obo:IAO_0000115 xml:lang="en">Blast furnace gas is manufactured coal based gas produced during the combustion of coke in blast furnaces in the iron and steel industry. It is recovered and used as a fuel partly within the plant and partly in other steel industry processes or in power stations equipped to burn it. The quantity of fuel should be reported on a gross calorific value basis.</obo:IAO_0000115>
        <obo:IAO_0000119 xml:lang="en">REGULATION (EC) No 1099/2008 OF THE EUROPEAN PARLIAMENT AND OF THE COUNCIL of 22 October 2008 on energy statistics https://eur-lex.europa.eu/legal-content/EN/TXT/HTML/?uri=CELEX:32008R1099&amp;from=EN</obo:IAO_0000119>
        <rdfs:label>blast furnace gas</rdfs:label>
    </owl:Class>
    


    <!-- http://openenergy-platform.org/ontology/oeo/OEO_00000084 -->

    <owl:Class rdf:about="http://openenergy-platform.org/ontology/oeo/OEO_00000084">
        <rdfs:subClassOf rdf:resource="http://openenergy-platform.org/ontology/oeo/OEO_00000331"/>
        <rdfs:subClassOf>
            <owl:Restriction>
                <owl:onProperty rdf:resource="http://openenergy-platform.org/ontology/oeo/OEO_00000530"/>
                <owl:someValuesFrom rdf:resource="http://openenergy-platform.org/ontology/oeo/OEO_00030001"/>
            </owl:Restriction>
        </rdfs:subClassOf>
        <rdfs:subClassOf>
            <owl:Restriction>
                <owl:onProperty rdf:resource="http://purl.obolibrary.org/obo/RO_0000087"/>
                <owl:someValuesFrom rdf:resource="http://openenergy-platform.org/ontology/oeo/OEO_00000001"/>
            </owl:Restriction>
        </rdfs:subClassOf>
        <rdfs:subClassOf>
            <owl:Restriction>
                <owl:onProperty rdf:resource="http://purl.obolibrary.org/obo/RO_0000091"/>
                <owl:someValuesFrom rdf:resource="http://openenergy-platform.org/ontology/oeo/OEO_00000097"/>
            </owl:Restriction>
        </rdfs:subClassOf>
        <rdfs:subClassOf>
            <owl:Restriction>
                <owl:onProperty rdf:resource="http://openenergy-platform.org/ontology/oeo/OEO_00000529"/>
                <owl:hasValue rdf:resource="http://openenergy-platform.org/ontology/oeo/OEO_00000390"/>
            </owl:Restriction>
        </rdfs:subClassOf>
        <obo:IAO_0000115 xml:lang="en">Charcoal is a portion of matter consisting of the solid residue of the destructive distillation and pyrolysis of wood and other vegetal material.It is used as a fuel.</obo:IAO_0000115>
        <obo:IAO_0000119 xml:lang="en">REGULATION (EC) No 1099/2008 OF THE EUROPEAN PARLIAMENT AND OF THE COUNCIL of 22 October 2008 on energy statistics https://eur-lex.europa.eu/legal-content/EN/TXT/HTML/?uri=CELEX:32008R1099&amp;from=EN</obo:IAO_0000119>
        <rdfs:label>charcoal</rdfs:label>
    </owl:Class>
    


    <!-- http://openenergy-platform.org/ontology/oeo/OEO_00000088 -->

    <owl:Class rdf:about="http://openenergy-platform.org/ontology/oeo/OEO_00000088">
        <rdfs:subClassOf rdf:resource="http://openenergy-platform.org/ontology/oeo/OEO_00000331"/>
        <rdfs:subClassOf>
            <owl:Restriction>
                <owl:onProperty rdf:resource="http://openenergy-platform.org/ontology/oeo/OEO_00000530"/>
                <owl:someValuesFrom rdf:resource="http://openenergy-platform.org/ontology/oeo/OEO_00030002"/>
            </owl:Restriction>
        </rdfs:subClassOf>
        <rdfs:subClassOf>
            <owl:Restriction>
                <owl:onProperty rdf:resource="http://purl.obolibrary.org/obo/RO_0000087"/>
                <owl:someValuesFrom rdf:resource="http://openenergy-platform.org/ontology/oeo/OEO_00000001"/>
            </owl:Restriction>
        </rdfs:subClassOf>
        <rdfs:subClassOf>
            <owl:Restriction>
                <owl:onProperty rdf:resource="http://purl.obolibrary.org/obo/RO_0000091"/>
                <owl:someValuesFrom rdf:resource="http://openenergy-platform.org/ontology/oeo/OEO_00000097"/>
            </owl:Restriction>
        </rdfs:subClassOf>
        <rdfs:subClassOf>
            <owl:Restriction>
                <owl:onProperty rdf:resource="http://openenergy-platform.org/ontology/oeo/OEO_00000529"/>
                <owl:hasValue rdf:resource="http://openenergy-platform.org/ontology/oeo/OEO_00000390"/>
            </owl:Restriction>
        </rdfs:subClassOf>
        <obo:IAO_0000115 xml:lang="en">Coal is a portion of matter consisting of combustible black or brownish-black sedimentary rock, formed as rock strata called coal seams. Coal is mostly carbon with variable amounts of other elements; chiefly hydrogen, sulfur, oxygen, and nitrogen.coal is formed if dead plant matter decays into peat and over millions of years the heat and pressure of deep burial converts the peat into coal.</obo:IAO_0000115>
        <obo:IAO_0000119>https://en.wikipedia.org/w/index.php?title=Coal&amp;oldid=907331967</obo:IAO_0000119>
        <rdfs:label>coal</rdfs:label>
    </owl:Class>
    


    <!-- http://openenergy-platform.org/ontology/oeo/OEO_00000089 -->

    <owl:Class rdf:about="http://openenergy-platform.org/ontology/oeo/OEO_00000089">
        <rdfs:subClassOf rdf:resource="http://openenergy-platform.org/ontology/oeo/OEO_00000031"/>
        <rdfs:subClassOf>
            <owl:Restriction>
                <owl:onProperty rdf:resource="http://purl.obolibrary.org/obo/BFO_0000051"/>
                <owl:someValuesFrom rdf:resource="http://openenergy-platform.org/ontology/oeo/OEO_00000008"/>
            </owl:Restriction>
        </rdfs:subClassOf>
        <rdfs:subClassOf>
            <owl:Restriction>
                <owl:onProperty rdf:resource="http://purl.obolibrary.org/obo/BFO_0000051"/>
                <owl:someValuesFrom rdf:resource="http://openenergy-platform.org/ontology/oeo/OEO_00000396"/>
            </owl:Restriction>
        </rdfs:subClassOf>
        <obo:IAO_0000115 xml:lang="en">A coal powerplant is a powerplant having an aggregate of coal power units as its power generating units.</obo:IAO_0000115>
        <rdfs:label>coal powerplant</rdfs:label>
    </owl:Class>
    


    <!-- http://openenergy-platform.org/ontology/oeo/OEO_00000093 -->

    <owl:Class rdf:about="http://openenergy-platform.org/ontology/oeo/OEO_00000093">
        <rdfs:subClassOf rdf:resource="http://openenergy-platform.org/ontology/oeo/OEO_00000263"/>
        <obo:IAO_0000115 xml:lang="en">Coke oven gas is manufactured coal based gas obtained as a by-product of the manufacture of coke oven coke for the production of iron and steel.</obo:IAO_0000115>
        <obo:IAO_0000119 xml:lang="en">REGULATION (EC) No 1099/2008 OF THE EUROPEAN PARLIAMENT AND OF THE COUNCIL of 22 October 2008 on energy statistics https://eur-lex.europa.eu/legal-content/EN/TXT/HTML/?uri=CELEX:32008R1099&amp;from=EN</obo:IAO_0000119>
        <rdfs:label>coke oven gas</rdfs:label>
    </owl:Class>
    


    <!-- http://openenergy-platform.org/ontology/oeo/OEO_00000094 -->

    <owl:Class rdf:about="http://openenergy-platform.org/ontology/oeo/OEO_00000094">
        <rdfs:subClassOf rdf:resource="http://openenergy-platform.org/ontology/oeo/OEO_00000204"/>
        <obo:IAO_0000115 xml:lang="en">Coking coal is hard coal that is bituminous with a quality that allows the production of a coke suitable to support a blast furnace charge. Its gross calorific value is greater than 23 865 kJ/kg (5 700 kcal/kg) on an ash-free but moist basis.</obo:IAO_0000115>
        <obo:IAO_0000119 xml:lang="en">REGULATION (EC) No 1099/2008 OF THE EUROPEAN PARLIAMENT AND OF THE COUNCIL of 22 October 2008 on energy statistics https://eur-lex.europa.eu/legal-content/EN/TXT/HTML/?uri=CELEX:32008R1099&amp;from=EN</obo:IAO_0000119>
        <rdfs:label>coking coal</rdfs:label>
    </owl:Class>
    


    <!-- http://openenergy-platform.org/ontology/oeo/OEO_00000096 -->

    <owl:Class rdf:about="http://openenergy-platform.org/ontology/oeo/OEO_00000096">
        <rdfs:subClassOf rdf:resource="http://openenergy-platform.org/ontology/oeo/OEO_00000292"/>
        <obo:IAO_0000115 xml:lang="en">Colliery gas is natural gas found in coal mines (British English: colliery). The main component is methane. Synonyms are firedamp, mine gas. It is used as a fossil fuel.</obo:IAO_0000115>
        <rdfs:label>colliery gas</rdfs:label>
    </owl:Class>
    


    <!-- http://openenergy-platform.org/ontology/oeo/OEO_00000097 -->

    <owl:Class rdf:about="http://openenergy-platform.org/ontology/oeo/OEO_00000097">
        <rdfs:subClassOf rdf:resource="http://openenergy-platform.org/ontology/oeo/OEO_00000151"/>
        <obo:IAO_0000115>A combustible energy carrier is an energy carrier that releases energy from a material entity in form of heat or work, by chemical reaction with other substances.</obo:IAO_0000115>
        <rdfs:label>combustible energy carrier disposition</rdfs:label>
    </owl:Class>
    


    <!-- http://openenergy-platform.org/ontology/oeo/OEO_00000099 -->

    <owl:Class rdf:about="http://openenergy-platform.org/ontology/oeo/OEO_00000099">
        <owl:equivalentClass>
            <owl:Class>
                <owl:intersectionOf rdf:parseType="Collection">
                    <rdf:Description rdf:about="http://openenergy-platform.org/ontology/oeo/OEO_00000173"/>
                    <owl:Restriction>
                        <owl:onProperty rdf:resource="http://purl.obolibrary.org/obo/RO_0000091"/>
                        <owl:someValuesFrom rdf:resource="http://openenergy-platform.org/ontology/oeo/OEO_00000097"/>
                    </owl:Restriction>
                </owl:intersectionOf>
            </owl:Class>
        </owl:equivalentClass>
        <rdfs:subClassOf rdf:resource="http://openenergy-platform.org/ontology/oeo/OEO_00000173"/>
        <obo:IAO_0000115>A combustible fuel is a fuel that realizes its fuel role in processes that release energy in the form of heat or work by chemical reaction with other substances.</obo:IAO_0000115>
        <obo:IAO_0000233>issue: https://github.com/OpenEnergyPlatform/ontology/issues/182
pull request: https://github.com/OpenEnergyPlatform/ontology/pull/237</obo:IAO_0000233>
        <rdfs:label>combustion fuel</rdfs:label>
    </owl:Class>
    


    <!-- http://openenergy-platform.org/ontology/oeo/OEO_00000102 -->

    <owl:Class rdf:about="http://openenergy-platform.org/ontology/oeo/OEO_00000102">
        <rdfs:subClassOf rdf:resource="http://openenergy-platform.org/ontology/oeo/OEO_00000054"/>
        <obo:IAO_0000115 xml:lang="en">Compressed air is air that has been compressed to store energy. To discharge energy, the air is expanded.</obo:IAO_0000115>
        <rdfs:label>compressed air</rdfs:label>
    </owl:Class>
    


    <!-- http://openenergy-platform.org/ontology/oeo/OEO_00000115 -->

    <owl:Class rdf:about="http://openenergy-platform.org/ontology/oeo/OEO_00000115">
        <rdfs:subClassOf rdf:resource="http://openenergy-platform.org/ontology/oeo/OEO_00000309"/>
        <rdfs:subClassOf>
            <owl:Restriction>
                <owl:onProperty rdf:resource="http://openenergy-platform.org/ontology/oeo/OEO_00000529"/>
                <owl:hasValue rdf:resource="http://openenergy-platform.org/ontology/oeo/OEO_00000256"/>
            </owl:Restriction>
        </rdfs:subClassOf>
        <obo:IAO_0000115 xml:lang="en">Crude oil is an oil and petroleum product of natural origin comprising a mixture of hydrocarbons and associated impurities, such as sulphur. It exists in the liquid phase under normal surface temperature and pressure and its physical characteristics (density, viscosity, etc.) are highly variable. This category includes field or lease condensate recovered from associated and non-associated gas where it is commingled with the commercial crude oil stream.</obo:IAO_0000115>
        <obo:IAO_0000119 xml:lang="en">REGULATION (EC) No 1099/2008 OF THE EUROPEAN PARLIAMENT AND OF THE COUNCIL of 22 October 2008 on energy statistics https://eur-lex.europa.eu/legal-content/EN/TXT/HTML/?uri=CELEX:32008R1099&amp;from=EN</obo:IAO_0000119>
        <rdfs:label>crude oil</rdfs:label>
    </owl:Class>
    


    <!-- http://openenergy-platform.org/ontology/oeo/OEO_00000117 -->

    <owl:Class rdf:about="http://openenergy-platform.org/ontology/oeo/OEO_00000117">
        <rdfs:subClassOf rdf:resource="http://openenergy-platform.org/ontology/oeo/OEO_00000441"/>
        <rdfs:subClassOf>
            <owl:Restriction>
                <owl:onProperty rdf:resource="http://openenergy-platform.org/ontology/oeo/OEO_00000501"/>
                <owl:someValuesFrom rdf:resource="http://openenergy-platform.org/ontology/oeo/OEO_00000399"/>
            </owl:Restriction>
        </rdfs:subClassOf>
        <obo:IAO_0000115 xml:lang="en">A dam is a barrier that stops or restricts the flow of water or underground streams. Reservoirs created by dams not only suppress floods but also provide water for activities such as irrigation, human consumption, industrial use, aquaculture, and navigability. Hydropower is often used in conjunction with dams to generate electricity.</obo:IAO_0000115>
        <obo:IAO_0000119 xml:lang="en">https://en.wikipedia.org/w/index.php?title=Dam&amp;oldid=906014627</obo:IAO_0000119>
        <rdfs:label>dammed water</rdfs:label>
    </owl:Class>
    


    <!-- http://openenergy-platform.org/ontology/oeo/OEO_00000126 -->

    <owl:Class rdf:about="http://openenergy-platform.org/ontology/oeo/OEO_00000126">
        <rdfs:subClassOf rdf:resource="http://openenergy-platform.org/ontology/oeo/OEO_00000253"/>
        <obo:IAO_0000115 xml:lang="en">An HVDC-line is a powerline for transferring high voltage direct current.</obo:IAO_0000115>
        <obo:IAO_0000233>issue: https://github.com/OpenEnergyPlatform/ontology/issues/231
pull request: https://github.com/OpenEnergyPlatform/ontology/pull/385</obo:IAO_0000233>
        <rdfs:comment>directed</rdfs:comment>
        <rdfs:label xml:lang="en">HVDC-line</rdfs:label>
    </owl:Class>
    


    <!-- http://openenergy-platform.org/ontology/oeo/OEO_00000129 -->

    <owl:Class rdf:about="http://openenergy-platform.org/ontology/oeo/OEO_00000129">
        <owl:equivalentClass rdf:resource="http://openenergy-platform.org/ontology/oeo/OEO_00000132"/>
        <rdfs:subClassOf rdf:resource="http://openenergy-platform.org/ontology/oeo/OEO_00000207"/>
        <obo:IAO_0000115 xml:lang="en">Derived heat covers the total heat production in heating plants and in combined heat and power plants. It includes the heat used by the auxiliaries of the installation which use hot fluid (space heating, liquid fuel heating, etc.) And losses in the installation/network heat exchanges. For autoproducing entities (= entities generating electricity and/or heat wholly or partially for their own use as an activity which supports their primary activity) the heat used by the undertaking for its own processes is not included.</obo:IAO_0000115>
        <obo:IAO_0000119 xml:lang="en">https://ec.europa.eu/eurostat/ramon/nomenclatures/index.cfm?TargetUrl=DSP_GLOSSARY_NOM_DTL_VIEW&amp;StrNom=CODED2&amp;StrLanguageCode=EN&amp;IntKey=16452285&amp;RdoSearch=&amp;TxtSearch=&amp;CboTheme=&amp;IntCurrentPage=1</obo:IAO_0000119>
        <rdfs:label>derived heat</rdfs:label>
    </owl:Class>
    


    <!-- http://openenergy-platform.org/ontology/oeo/OEO_00000131 -->

    <owl:Class rdf:about="http://openenergy-platform.org/ontology/oeo/OEO_00000131">
        <rdfs:subClassOf rdf:resource="http://openenergy-platform.org/ontology/oeo/OEO_00000181"/>
        <obo:IAO_0000115 xml:lang="en">Diesel fuel is gas diesel oil used on-road for diesel compression ignition (cars, trucks, etc.), usually of low sulphur content.</obo:IAO_0000115>
        <obo:IAO_0000118 xml:lang="en">TransportDiesel</obo:IAO_0000118>
        <obo:IAO_0000119 xml:lang="en">REGULATION (EC) No 1099/2008 OF THE EUROPEAN PARLIAMENT AND OF THE COUNCIL of 22 October 2008 on energy statistics https://eur-lex.europa.eu/legal-content/EN/TXT/HTML/?uri=CELEX:32008R1099&amp;from=EN</obo:IAO_0000119>
        <rdfs:label>diesel fuel</rdfs:label>
        <rdfs:label xml:lang="en">diesel fuel</rdfs:label>
    </owl:Class>
    


    <!-- http://openenergy-platform.org/ontology/oeo/OEO_00000132 -->

    <owl:Class rdf:about="http://openenergy-platform.org/ontology/oeo/OEO_00000132">
        <rdfs:subClassOf rdf:resource="http://openenergy-platform.org/ontology/oeo/OEO_00000207"/>
        <obo:IAO_0000115 xml:lang="en">District heating (also known as heat networks or teleheating) is a system for distributing heat generated in a centralized location through a system of insulated pipes for residential and commercial heating requirements such as space heating and water heating. The heat is often obtained from a cogeneration plant burning fossil fuels or biomass, but heat-only boiler stations, geothermal heating, heat pumps and central solar heating are also used, as well as heat waste from nuclear power electricity generation. </obo:IAO_0000115>
        <obo:IAO_0000119 xml:lang="en">https://en.wikipedia.org/w/index.php?title=District_heating&amp;oldid=906646999</obo:IAO_0000119>
        <rdfs:label>district heat</rdfs:label>
    </owl:Class>
    


    <!-- http://openenergy-platform.org/ontology/oeo/OEO_00000139 -->

    <owl:Class rdf:about="http://openenergy-platform.org/ontology/oeo/OEO_00000139">
        <rdfs:subClassOf rdf:resource="http://openenergy-platform.org/ontology/oeo/OEO_00000150"/>
        <obo:IAO_0000115 xml:lang="en">Electrical energy is a form of energy derived from the potential or kinetic energy of charged particles.</obo:IAO_0000115>
        <obo:IAO_0000118>electricity</obo:IAO_0000118>
        <obo:IAO_0000119 xml:lang="en">https://en.wikipedia.org/wiki/Electrical_energy</obo:IAO_0000119>
        <obo:IAO_0000233>definition of electrical energy:
issue: https://github.com/OpenEnergyPlatform/ontology/issues/224
pull request:  https://github.com/OpenEnergyPlatform/ontology/pull/524

alternative term electricity:
issue: https://github.com/OpenEnergyPlatform/ontology/issues/381
pull request: https://github.com/OpenEnergyPlatform/ontology/pull/621</obo:IAO_0000233>
        <rdfs:label>electrical energy</rdfs:label>
    </owl:Class>
    


    <!-- http://openenergy-platform.org/ontology/oeo/OEO_00000143 -->

    <owl:Class rdf:about="http://openenergy-platform.org/ontology/oeo/OEO_00000143">
        <rdfs:subClassOf rdf:resource="http://openenergy-platform.org/ontology/oeo/OEO_00000200"/>
        <rdfs:subClassOf>
            <owl:Restriction>
                <owl:onProperty rdf:resource="http://purl.obolibrary.org/obo/BFO_0000051"/>
                <owl:someValuesFrom rdf:resource="http://openenergy-platform.org/ontology/oeo/OEO_00000144"/>
            </owl:Restriction>
        </rdfs:subClassOf>
        <rdfs:subClassOf>
            <owl:Restriction>
                <owl:onProperty rdf:resource="http://purl.obolibrary.org/obo/BFO_0000051"/>
                <owl:minQualifiedCardinality rdf:datatype="http://www.w3.org/2001/XMLSchema#nonNegativeInteger">1</owl:minQualifiedCardinality>
                <owl:onClass rdf:resource="http://openenergy-platform.org/ontology/oeo/OEO_00000253"/>
            </owl:Restriction>
        </rdfs:subClassOf>
        <obo:IAO_0000115 xml:lang="en">An electricity grid is a supply grid that distributes electrical energy / electricity.</obo:IAO_0000115>
        <obo:IAO_0000233>issue: https://github.com/OpenEnergyPlatform/ontology/issues/138
pull request: https://github.com/OpenEnergyPlatform/ontology/pull/165</obo:IAO_0000233>
        <rdfs:label>electricity grid</rdfs:label>
    </owl:Class>
    


    <!-- http://openenergy-platform.org/ontology/oeo/OEO_00000144 -->

    <owl:Class rdf:about="http://openenergy-platform.org/ontology/oeo/OEO_00000144">
        <owl:equivalentClass>
            <owl:Class>
                <owl:intersectionOf rdf:parseType="Collection">
                    <rdf:Description rdf:about="http://openenergy-platform.org/ontology/oeo/OEO_00020006"/>
                    <owl:Restriction>
                        <owl:onProperty rdf:resource="http://purl.obolibrary.org/obo/BFO_0000050"/>
                        <owl:someValuesFrom rdf:resource="http://openenergy-platform.org/ontology/oeo/OEO_00000143"/>
                    </owl:Restriction>
                </owl:intersectionOf>
            </owl:Class>
        </owl:equivalentClass>
        <rdfs:subClassOf rdf:resource="http://openenergy-platform.org/ontology/oeo/OEO_00020006"/>
        <obo:IAO_0000115 xml:lang="en">An electricity grid component is a grid component that is part of an electricity grid.</obo:IAO_0000115>
        <obo:IAO_0000233>issue: https://github.com/OpenEnergyPlatform/ontology/issues/36
pull request: https://github.com/OpenEnergyPlatform/ontology/pull/385</obo:IAO_0000233>
        <rdfs:label>electricity grid component</rdfs:label>
    </owl:Class>
    


    <!-- http://openenergy-platform.org/ontology/oeo/OEO_00000146 -->

    <owl:Class rdf:about="http://openenergy-platform.org/ontology/oeo/OEO_00000146">
        <rdfs:subClassOf rdf:resource="http://openenergy-platform.org/ontology/oeo/OEO_00010023"/>
        <rdfs:subClassOf>
            <owl:Restriction>
                <owl:onProperty rdf:resource="http://openenergy-platform.org/ontology/oeo/OEO_00000503"/>
                <owl:someValuesFrom rdf:resource="http://openenergy-platform.org/ontology/oeo/OEO_00000139"/>
            </owl:Restriction>
        </rdfs:subClassOf>
        <rdfs:subClassOf>
            <owl:Restriction>
                <owl:onProperty rdf:resource="http://purl.obolibrary.org/obo/BFO_0000051"/>
                <owl:someValuesFrom rdf:resource="http://openenergy-platform.org/ontology/oeo/OEO_00010028"/>
            </owl:Restriction>
        </rdfs:subClassOf>
        <obo:IAO_0000115 xml:lang="en">An electric vehicle (abbreviated as EV) is a vehicle that uses one or more electric motors for propulsion.</obo:IAO_0000115>
        <obo:IAO_0000118>EV</obo:IAO_0000118>
        <obo:IAO_0000233>https://github.com/OpenEnergyPlatform/ontology/issues/425
pull request: https://github.com/OpenEnergyPlatform/ontology/pull/431</obo:IAO_0000233>
        <rdfs:label>electric vehicle</rdfs:label>
    </owl:Class>
    


    <!-- http://openenergy-platform.org/ontology/oeo/OEO_00000147 -->

    <owl:Class rdf:about="http://openenergy-platform.org/ontology/oeo/OEO_00000147">
        <rdfs:subClassOf rdf:resource="http://purl.obolibrary.org/obo/BFO_0000015"/>
        <rdfs:subClassOf>
            <owl:Restriction>
                <owl:onProperty rdf:resource="http://openenergy-platform.org/ontology/oeo/OEO_00000500"/>
                <owl:someValuesFrom rdf:resource="http://openenergy-platform.org/ontology/oeo/OEO_00000148"/>
            </owl:Restriction>
        </rdfs:subClassOf>
        <obo:IAO_0000115 xml:lang="en">emission is a process releasing byproducts from human activity (e.g. production, distribution or consumption) into the environment.</obo:IAO_0000115>
        <obo:IAO_0000233>issue: https://github.com/OpenEnergyPlatform/ontology/issues/56
pull request: https://github.com/OpenEnergyPlatform/ontology/pull/234</obo:IAO_0000233>
        <rdfs:label>emission</rdfs:label>
    </owl:Class>
    


    <!-- http://openenergy-platform.org/ontology/oeo/OEO_00000148 -->

    <owl:Class rdf:about="http://openenergy-platform.org/ontology/oeo/OEO_00000148">
        <rdfs:subClassOf rdf:resource="http://openenergy-platform.org/ontology/oeo/OEO_00030019"/>
        <rdfs:subClassOf>
            <owl:Restriction>
                <owl:onProperty rdf:resource="http://openenergy-platform.org/ontology/oeo/OEO_00000502"/>
                <owl:someValuesFrom rdf:resource="http://openenergy-platform.org/ontology/oeo/OEO_00000147"/>
            </owl:Restriction>
        </rdfs:subClassOf>
        <rdfs:subClassOf>
            <owl:Restriction>
                <owl:onProperty rdf:resource="http://openenergy-platform.org/ontology/oeo/OEO_00000502"/>
                <owl:someValuesFrom rdf:resource="http://purl.obolibrary.org/obo/BFO_0000015"/>
            </owl:Restriction>
        </rdfs:subClassOf>
        <obo:IAO_0000115>An emission factor is a process attribute that quantifies the emissions or removals of a gas per unit activity.</obo:IAO_0000115>
        <obo:IAO_0000233>issue: https://github.com/OpenEnergyPlatform/ontology/issues/243
pull request: https://github.com/OpenEnergyPlatform/ontology/pull/581</obo:IAO_0000233>
        <rdfs:label>emission factor</rdfs:label>
    </owl:Class>
    


    <!-- http://openenergy-platform.org/ontology/oeo/OEO_00000150 -->

    <owl:Class rdf:about="http://openenergy-platform.org/ontology/oeo/OEO_00000150">
        <rdfs:subClassOf rdf:resource="http://purl.obolibrary.org/obo/BFO_0000019"/>
        <obo:IAO_0000115>Energy is a quality of matter which manifests as a capacity to perform work (such as causing motion or the interaction of molecules)</obo:IAO_0000115>
        <obo:IAO_0000119>Derived from https://www.lexico.com/en/definition/energy</obo:IAO_0000119>
        <obo:IAO_0000233>issue: https://github.com/OpenEnergyPlatform/ontology/issues/224
pull request: https://github.com/OpenEnergyPlatform/ontology/pull/364
fix grammar error:
pull request: https://github.com/OpenEnergyPlatform/ontology/pull/657
update definition
issue: https://github.com/OpenEnergyPlatform/ontology/issues/660
pull request: https://github.com/OpenEnergyPlatform/ontology/pull/665</obo:IAO_0000233>
        <rdfs:comment>Energy is power integrated over time.</rdfs:comment>
        <rdfs:label>energy</rdfs:label>
    </owl:Class>
    


    <!-- http://openenergy-platform.org/ontology/oeo/OEO_00000151 -->

    <owl:Class rdf:about="http://openenergy-platform.org/ontology/oeo/OEO_00000151">
        <rdfs:subClassOf rdf:resource="http://purl.obolibrary.org/obo/BFO_0000016"/>
        <obo:IAO_0000115 xml:lang="en">An energy carrier disposition is a disposition of an material entity that contains energy for conversion as usable energy.</obo:IAO_0000115>
        <obo:IAO_0000233>issue: https://github.com/OpenEnergyPlatform/ontology/issues/209
pull request: https://github.com/OpenEnergyPlatform/ontology/pull/276
issue: https://github.com/OpenEnergyPlatform/ontology/issues/407
pull request: https://github.com/OpenEnergyPlatform/ontology/pull/627</obo:IAO_0000233>
        <rdfs:label>energy carrier disposition</rdfs:label>
    </owl:Class>
    


    <!-- http://openenergy-platform.org/ontology/oeo/OEO_00000159 -->

    <owl:Class rdf:about="http://openenergy-platform.org/ontology/oeo/OEO_00000159">
        <rdfs:subClassOf rdf:resource="http://openenergy-platform.org/ontology/oeo/OEO_00000061"/>
        <obo:IAO_0000115>An energy storage object is an artificial object that has the function energy storage.</obo:IAO_0000115>
        <obo:IAO_0000233>issue: https://github.com/OpenEnergyPlatform/ontology/issues/209
pull request: https://github.com/OpenEnergyPlatform/ontology/pull/276</obo:IAO_0000233>
        <rdfs:label>energy storage object</rdfs:label>
    </owl:Class>
    


    <!-- http://openenergy-platform.org/ontology/oeo/OEO_00000165 -->

    <owl:Class rdf:about="http://openenergy-platform.org/ontology/oeo/OEO_00000165">
        <rdfs:subClassOf rdf:resource="http://openenergy-platform.org/ontology/oeo/OEO_00000324"/>
        <owl:disjointWith rdf:resource="http://openenergy-platform.org/ontology/oeo/OEO_00000361"/>
        <obo:IAO_0000115 xml:lang="en">A field photovoltaic powerplant (also: solar farm, solar park) is a photovoltaic powerplant that is installed out in the open on the ground.</obo:IAO_0000115>
        <obo:IAO_0000118>Solar park</obo:IAO_0000118>
        <rdfs:label>field photovoltaic powerplant</rdfs:label>
    </owl:Class>
    


    <!-- http://openenergy-platform.org/ontology/oeo/OEO_00000169 -->

    <owl:Class rdf:about="http://openenergy-platform.org/ontology/oeo/OEO_00000169">
        <rdfs:subClassOf rdf:resource="http://openenergy-platform.org/ontology/oeo/OEO_00000068"/>
        <obo:IAO_0000115 xml:lang="en">A flow battery, or redox flow battery (after reduction–oxidation), is a type of electrochemical cell where chemical energy is provided by two chemical components dissolved in liquids contained within the system and separated by a membrane. Ion exchange (accompanied by flow of electric current) occurs through the membrane while both liquids circulate in their own respective space.</obo:IAO_0000115>
        <obo:IAO_0000119 xml:lang="en">https://en.wikipedia.org/w/index.php?title=Flow_battery&amp;oldid=907053515</obo:IAO_0000119>
        <rdfs:label>flow battery</rdfs:label>
    </owl:Class>
    


    <!-- http://openenergy-platform.org/ontology/oeo/OEO_00000173 -->

    <owl:Class rdf:about="http://openenergy-platform.org/ontology/oeo/OEO_00000173">
        <owl:equivalentClass>
            <owl:Class>
                <owl:intersectionOf rdf:parseType="Collection">
                    <owl:Restriction>
                        <owl:onProperty rdf:resource="http://purl.obolibrary.org/obo/RO_0000087"/>
                        <owl:someValuesFrom rdf:resource="http://openenergy-platform.org/ontology/oeo/OEO_00000001"/>
                    </owl:Restriction>
                    <owl:Restriction>
                        <owl:onProperty rdf:resource="http://purl.obolibrary.org/obo/RO_0000091"/>
                        <owl:someValuesFrom rdf:resource="http://openenergy-platform.org/ontology/oeo/OEO_00000151"/>
                    </owl:Restriction>
                </owl:intersectionOf>
            </owl:Class>
        </owl:equivalentClass>
        <rdfs:subClassOf rdf:resource="http://openenergy-platform.org/ontology/oeo/OEO_00000331"/>
        <obo:IAO_0000115>A fuel is a portion of matter that has the disposition to be an energy carrier and which has a fuel role that is realised in processes that release the carried energy by transforming the portion of matter into a different kind of portion of matter in a way that releases heat or does work.</obo:IAO_0000115>
        <obo:IAO_0000233>issue: https://github.com/OpenEnergyPlatform/ontology/issues/227
pull request: https://github.com/OpenEnergyPlatform/ontology/pull/279</obo:IAO_0000233>
        <rdfs:label>fuel</rdfs:label>
    </owl:Class>
    


    <!-- http://openenergy-platform.org/ontology/oeo/OEO_00000174 -->

    <owl:Class rdf:about="http://openenergy-platform.org/ontology/oeo/OEO_00000174">
        <owl:equivalentClass>
            <owl:Restriction>
                <owl:onProperty rdf:resource="http://purl.obolibrary.org/obo/BFO_0000051"/>
                <owl:someValuesFrom rdf:resource="http://openenergy-platform.org/ontology/oeo/OEO_00000175"/>
            </owl:Restriction>
        </owl:equivalentClass>
        <rdfs:subClassOf rdf:resource="http://openenergy-platform.org/ontology/oeo/OEO_00000031"/>
        <rdfs:subClassOf>
            <owl:Restriction>
                <owl:onProperty rdf:resource="http://purl.obolibrary.org/obo/RO_0000056"/>
                <owl:someValuesFrom rdf:resource="http://openenergy-platform.org/ontology/oeo/OEO_00050001"/>
            </owl:Restriction>
        </rdfs:subClassOf>
        <obo:IAO_0000115>A fueled powerplant is a powerplant that has fueled power units as parts.</obo:IAO_0000115>
        <obo:IAO_0000233>issue: https://github.com/OpenEnergyPlatform/ontology/issues/292
pull request: https://github.com/OpenEnergyPlatform/ontology/pull/306</obo:IAO_0000233>
        <rdfs:label>fueled powerplant</rdfs:label>
    </owl:Class>
    


    <!-- http://openenergy-platform.org/ontology/oeo/OEO_00000175 -->

    <owl:Class rdf:about="http://openenergy-platform.org/ontology/oeo/OEO_00000175">
        <owl:equivalentClass>
            <owl:Class>
                <owl:intersectionOf rdf:parseType="Collection">
                    <rdf:Description rdf:about="http://openenergy-platform.org/ontology/oeo/OEO_00000334"/>
                    <owl:Restriction>
                        <owl:onProperty rdf:resource="http://openenergy-platform.org/ontology/oeo/OEO_00000503"/>
                        <owl:someValuesFrom rdf:resource="http://openenergy-platform.org/ontology/oeo/OEO_00000173"/>
                    </owl:Restriction>
                </owl:intersectionOf>
            </owl:Class>
        </owl:equivalentClass>
        <rdfs:subClassOf rdf:resource="http://openenergy-platform.org/ontology/oeo/OEO_00000334"/>
        <rdfs:subClassOf>
            <owl:Restriction>
                <owl:onProperty rdf:resource="http://purl.obolibrary.org/obo/RO_0000056"/>
                <owl:someValuesFrom rdf:resource="http://openenergy-platform.org/ontology/oeo/OEO_00050001"/>
            </owl:Restriction>
        </rdfs:subClassOf>
        <obo:IAO_0000115>A fueled power unit is a power generating unit that uses fuel.</obo:IAO_0000115>
        <obo:IAO_0000233>issue: https://github.com/OpenEnergyPlatform/ontology/issues/292
pull request: https://github.com/OpenEnergyPlatform/ontology/pull/306</obo:IAO_0000233>
        <rdfs:label>fueled power unit</rdfs:label>
    </owl:Class>
    


    <!-- http://openenergy-platform.org/ontology/oeo/OEO_00000181 -->

    <owl:Class rdf:about="http://openenergy-platform.org/ontology/oeo/OEO_00000181">
        <rdfs:subClassOf rdf:resource="http://openenergy-platform.org/ontology/oeo/OEO_00000309"/>
        <rdfs:subClassOf>
            <owl:Restriction>
                <owl:onProperty rdf:resource="http://openenergy-platform.org/ontology/oeo/OEO_00000529"/>
                <owl:hasValue rdf:resource="http://openenergy-platform.org/ontology/oeo/OEO_00000256"/>
            </owl:Restriction>
        </rdfs:subClassOf>
        <obo:IAO_0000115 xml:lang="en">Gas/diesel oil is an oil and petroleum product that is primarily a medium distillate distilling between 180 °C and 380 °C. Includes blending components. Several grades are available depending on uses.</obo:IAO_0000115>
        <obo:IAO_0000119 xml:lang="en">REGULATION (EC) No 1099/2008 OF THE EUROPEAN PARLIAMENT AND OF THE COUNCIL of 22 October 2008 on energy statistics https://eur-lex.europa.eu/legal-content/EN/TXT/HTML/?uri=CELEX:32008R1099&amp;from=EN</obo:IAO_0000119>
        <rdfs:label>gas diesel oil</rdfs:label>
    </owl:Class>
    


    <!-- http://openenergy-platform.org/ontology/oeo/OEO_00000183 -->

    <owl:Class rdf:about="http://openenergy-platform.org/ontology/oeo/OEO_00000183">
        <rdfs:subClassOf rdf:resource="http://openenergy-platform.org/ontology/oeo/OEO_00000309"/>
        <rdfs:subClassOf>
            <owl:Restriction>
                <owl:onProperty rdf:resource="http://openenergy-platform.org/ontology/oeo/OEO_00000529"/>
                <owl:hasValue rdf:resource="http://openenergy-platform.org/ontology/oeo/OEO_00000256"/>
            </owl:Restriction>
        </rdfs:subClassOf>
        <obo:IAO_0000115>Gasoline (American English) or petrol (British English) is an oil and petroleum product in the form of a transparent petroleum-derived liquid that is used primarily as a fuel in spark-ignited internal combustion engines. It consists mostly of organic compounds obtained by the fractional distillation of petroleum, enhanced with a variety of additives.</obo:IAO_0000115>
        <obo:IAO_0000115>https://en.wikipedia.org/w/index.php?title=Gasoline&amp;oldid=867948640</obo:IAO_0000115>
        <obo:IAO_0000118>petrol</obo:IAO_0000118>
        <rdfs:label>gasoline</rdfs:label>
    </owl:Class>
    


    <!-- http://openenergy-platform.org/ontology/oeo/OEO_00000184 -->

    <owl:Class rdf:about="http://openenergy-platform.org/ontology/oeo/OEO_00000184">
        <rdfs:subClassOf rdf:resource="http://openenergy-platform.org/ontology/oeo/OEO_00000031"/>
        <rdfs:subClassOf>
            <owl:Restriction>
                <owl:onProperty rdf:resource="http://purl.obolibrary.org/obo/BFO_0000051"/>
                <owl:someValuesFrom rdf:resource="http://openenergy-platform.org/ontology/oeo/OEO_00000017"/>
            </owl:Restriction>
        </rdfs:subClassOf>
        <obo:IAO_0000115 xml:lang="en">A gas powerplant is a powerplant having an aggregate of gas fired power units as its power generating units.</obo:IAO_0000115>
        <rdfs:label>gas powerplant</rdfs:label>
    </owl:Class>
    


    <!-- http://openenergy-platform.org/ontology/oeo/OEO_00000185 -->

    <owl:Class rdf:about="http://openenergy-platform.org/ontology/oeo/OEO_00000185">
        <rdfs:subClassOf rdf:resource="http://openenergy-platform.org/ontology/oeo/OEO_00000425"/>
        <rdfs:subClassOf>
            <owl:Restriction>
                <owl:onProperty rdf:resource="http://openenergy-platform.org/ontology/oeo/OEO_00000533"/>
                <owl:someValuesFrom rdf:resource="http://openenergy-platform.org/ontology/oeo/OEO_00000333"/>
            </owl:Restriction>
        </rdfs:subClassOf>
        <rdfs:subClassOf>
            <owl:Restriction>
                <owl:onProperty rdf:resource="http://openenergy-platform.org/ontology/oeo/OEO_00000532"/>
                <owl:allValuesFrom rdf:resource="http://openenergy-platform.org/ontology/oeo/OEO_00000292"/>
            </owl:Restriction>
        </rdfs:subClassOf>
        <obo:IAO_0000115 xml:lang="en">A gas turbine is a turbine that converts chemical energy into rotational energy using a continous internal combustion process. Hence it is also called combustion turbine.</obo:IAO_0000115>
        <obo:IAO_0000118>Combustion turbine</obo:IAO_0000118>
        <obo:IAO_0000233>issue: https://github.com/OpenEnergyPlatform/ontology/issues/299
pull request: https://github.com/OpenEnergyPlatform/ontology/pull/300</obo:IAO_0000233>
        <rdfs:label>gas turbine</rdfs:label>
    </owl:Class>
    


    <!-- http://openenergy-platform.org/ontology/oeo/OEO_00000186 -->

    <owl:Class rdf:about="http://openenergy-platform.org/ontology/oeo/OEO_00000186">
        <rdfs:subClassOf rdf:resource="http://openenergy-platform.org/ontology/oeo/OEO_00000263"/>
        <obo:IAO_0000115 xml:lang="en">Gasworks gas is manufactured coal based gas that covers all types of gases produced in public utility or private plants, whose main purpose is manufacture, transport and distribution of gas. It includes gas produced by carbonisation (including gas produced by coke ovens and transferred to gasworks gas), by total gasification with or without enrichment with oil products (LPG, residual fuel oil, etc.), and by reforming and simple mixing of gases and/or air, reported under the rows ‘from other sources’. Under the transformation sector identify amounts of gasworks gas transferred to blended natural gas which will be distributed and consumed through the natural gas grid.

The production of other coal gases (i.e. coke oven gas, blast furnace gas and oxygen steel furnace gas) should be reported in the columns concerning such gases, and not as production of gasworks gas. The coal gases transferred to gasworks plants should then be reported (in their own column) in the transformation sector in the gasworks plants row. The total amount of gasworks gas resulting from transfers of other coal gases should appear in the production line for gasworks gas.</obo:IAO_0000115>
        <obo:IAO_0000119 xml:lang="en">REGULATION (EC) No 1099/2008 OF THE EUROPEAN PARLIAMENT AND OF THE COUNCIL of 22 October 2008 on energy statistics https://eur-lex.europa.eu/legal-content/EN/TXT/HTML/?uri=CELEX:32008R1099&amp;from=EN</obo:IAO_0000119>
        <rdfs:label>gasworks gas</rdfs:label>
    </owl:Class>
    


    <!-- http://openenergy-platform.org/ontology/oeo/OEO_00000188 -->

    <owl:Class rdf:about="http://openenergy-platform.org/ontology/oeo/OEO_00000188">
        <rdfs:subClassOf rdf:resource="http://openenergy-platform.org/ontology/oeo/OEO_00000011"/>
        <rdfs:subClassOf>
            <owl:Restriction>
                <owl:onProperty rdf:resource="http://openenergy-platform.org/ontology/oeo/OEO_00000533"/>
                <owl:someValuesFrom rdf:resource="http://openenergy-platform.org/ontology/oeo/OEO_00000139"/>
            </owl:Restriction>
        </rdfs:subClassOf>
        <obo:IAO_0000115 xml:lang="en">A generator is an energy converting device that converts other forms of energy into electrical energy.</obo:IAO_0000115>
        <obo:IAO_0000233>issue: https://github.com/OpenEnergyPlatform/ontology/issues/173
pull request: https://github.com/OpenEnergyPlatform/ontology/pull/273</obo:IAO_0000233>
        <rdfs:label>generator</rdfs:label>
    </owl:Class>
    


    <!-- http://openenergy-platform.org/ontology/oeo/OEO_00000189 -->

    <owl:Class rdf:about="http://openenergy-platform.org/ontology/oeo/OEO_00000189">
        <rdfs:subClassOf rdf:resource="http://purl.obolibrary.org/obo/BFO_0000141"/>
        <rdfs:label>geographic coordinate</rdfs:label>
    </owl:Class>
    


    <!-- http://openenergy-platform.org/ontology/oeo/OEO_00000191 -->

    <owl:Class rdf:about="http://openenergy-platform.org/ontology/oeo/OEO_00000191">
        <rdfs:subClassOf rdf:resource="http://openenergy-platform.org/ontology/oeo/OEO_00000207"/>
        <rdfs:subClassOf>
            <owl:Restriction>
                <owl:onProperty rdf:resource="http://purl.obolibrary.org/obo/RO_0000091"/>
                <owl:someValuesFrom rdf:resource="http://openenergy-platform.org/ontology/oeo/OEO_00000033"/>
            </owl:Restriction>
        </rdfs:subClassOf>
        <obo:IAO_0000115>Geothermal energy is thermal energy that is released from within the earth&apos;s crust.</obo:IAO_0000115>
        <obo:IAO_0000233>issue: https://github.com/OpenEnergyPlatform/ontology/issues/727
pull request: https://github.com/OpenEnergyPlatform/ontology/pull/739</obo:IAO_0000233>
        <rdfs:label>geothermal energy</rdfs:label>
    </owl:Class>
    


    <!-- http://openenergy-platform.org/ontology/oeo/OEO_00000192 -->

    <owl:Class rdf:about="http://openenergy-platform.org/ontology/oeo/OEO_00000192">
        <rdfs:subClassOf rdf:resource="http://openenergy-platform.org/ontology/oeo/OEO_00000031"/>
        <rdfs:subClassOf>
            <owl:Restriction>
                <owl:onProperty rdf:resource="http://purl.obolibrary.org/obo/BFO_0000051"/>
                <owl:someValuesFrom rdf:resource="http://openenergy-platform.org/ontology/oeo/OEO_00000019"/>
            </owl:Restriction>
        </rdfs:subClassOf>
        <rdfs:subClassOf>
            <owl:Restriction>
                <owl:onProperty rdf:resource="http://purl.obolibrary.org/obo/BFO_0000051"/>
                <owl:someValuesFrom rdf:resource="http://openenergy-platform.org/ontology/oeo/OEO_00000396"/>
            </owl:Restriction>
        </rdfs:subClassOf>
        <obo:IAO_0000115 xml:lang="en">A geothermal powerplant is a powerplant having an aggregate of geothermal power units as its power generating units.</obo:IAO_0000115>
        <rdfs:label>geothermal powerplant</rdfs:label>
    </owl:Class>
    


    <!-- http://openenergy-platform.org/ontology/oeo/OEO_00000198 -->

    <owl:Class rdf:about="http://openenergy-platform.org/ontology/oeo/OEO_00000198">
        <rdfs:subClassOf rdf:resource="http://purl.obolibrary.org/obo/BFO_0000016"/>
        <obo:IAO_0000115>The greenhouse effect disposition is the disposition of a gas to contribute to the greenhouse effect, when it is emitted into the atmosphere.</obo:IAO_0000115>
        <obo:IAO_0000233>issue: https://github.com/OpenEnergyPlatform/ontology/issues/56
pull request: https://github.com/OpenEnergyPlatform/ontology/pull/234</obo:IAO_0000233>
        <rdfs:label>greenhouse effect disposition</rdfs:label>
    </owl:Class>
    


    <!-- http://openenergy-platform.org/ontology/oeo/OEO_00000199 -->

    <owl:Class rdf:about="http://openenergy-platform.org/ontology/oeo/OEO_00000199">
        <rdfs:subClassOf rdf:resource="http://openenergy-platform.org/ontology/oeo/OEO_00000147"/>
        <rdfs:subClassOf>
            <owl:Restriction>
                <owl:onProperty rdf:resource="http://purl.obolibrary.org/obo/RO_0000057"/>
                <owl:someValuesFrom rdf:resource="http://openenergy-platform.org/ontology/oeo/OEO_00000020"/>
            </owl:Restriction>
        </rdfs:subClassOf>
        <obo:IAO_0000115>A greenhouse gas emission is an emission that releases a greenhouse gas.</obo:IAO_0000115>
        <obo:IAO_0000233>issue: https://github.com/OpenEnergyPlatform/ontology/issues/406
pull request: https://github.com/OpenEnergyPlatform/ontology/pull/410
issue: https://github.com/OpenEnergyPlatform/ontology/issues/56
pull request: https://github.com/OpenEnergyPlatform/ontology/pull/234</obo:IAO_0000233>
        <rdfs:label>greenhouse gas emission</rdfs:label>
    </owl:Class>
    


    <!-- http://openenergy-platform.org/ontology/oeo/OEO_00000200 -->

    <owl:Class rdf:about="http://openenergy-platform.org/ontology/oeo/OEO_00000200">
        <rdfs:subClassOf rdf:resource="http://purl.obolibrary.org/obo/BFO_0000027"/>
        <obo:IAO_0000115>A supply grid is an object aggregate of systematically connected artificial objects that can work as a supply system.</obo:IAO_0000115>
        <obo:IAO_0000118>grid</obo:IAO_0000118>
        <obo:IAO_0000118>network</obo:IAO_0000118>
        <obo:IAO_0000233>issue: https://github.com/OpenEnergyPlatform/ontology/issues/36
pull request: https://github.com/OpenEnergyPlatform/ontology/pull/385

issue: https://github.com/OpenEnergyPlatform/ontology/issues/114
pull request: https://github.com/OpenEnergyPlatform/ontology/pull/137</obo:IAO_0000233>
        <rdfs:label>supply grid</rdfs:label>
    </owl:Class>
    


    <!-- http://openenergy-platform.org/ontology/oeo/OEO_00000204 -->

    <owl:Class rdf:about="http://openenergy-platform.org/ontology/oeo/OEO_00000204">
        <rdfs:subClassOf rdf:resource="http://openenergy-platform.org/ontology/oeo/OEO_00000088"/>
        <owl:disjointWith rdf:resource="http://openenergy-platform.org/ontology/oeo/OEO_00000251"/>
        <obo:IAO_0000115 xml:lang="en">Hard coal is coal with a gross calorific value greater than 23 865 kJ/kg (5 700 kcal/kg) on an ashfree but moist basis and with a mean random reflectance of vitrinite of at least 0,6.</obo:IAO_0000115>
        <obo:IAO_0000119 xml:lang="en">REGULATION (EC) No 1099/2008 OF THE EUROPEAN PARLIAMENT AND OF THE COUNCIL of 22 October 2008 on energy statistics https://eur-lex.europa.eu/legal-content/EN/TXT/HTML/?uri=CELEX:32008R1099&amp;from=EN</obo:IAO_0000119>
        <rdfs:label>hard coal</rdfs:label>
    </owl:Class>
    


    <!-- http://openenergy-platform.org/ontology/oeo/OEO_00000205 -->

    <owl:Class rdf:about="http://openenergy-platform.org/ontology/oeo/OEO_00000205">
        <rdfs:subClassOf rdf:resource="http://openenergy-platform.org/ontology/oeo/OEO_00000089"/>
        <rdfs:subClassOf>
            <owl:Restriction>
                <owl:onProperty rdf:resource="http://purl.obolibrary.org/obo/BFO_0000051"/>
                <owl:someValuesFrom rdf:resource="http://openenergy-platform.org/ontology/oeo/OEO_00000021"/>
            </owl:Restriction>
        </rdfs:subClassOf>
        <obo:IAO_0000115 xml:lang="en">A hard coal powerplant is a coal powerplant having an aggregate of hard coal power units as its power generating units.</obo:IAO_0000115>
        <rdfs:label>hard coal powerplant</rdfs:label>
    </owl:Class>
    


    <!-- http://openenergy-platform.org/ontology/oeo/OEO_00000206 -->

    <owl:Class rdf:about="http://openenergy-platform.org/ontology/oeo/OEO_00000206">
        <rdfs:subClassOf rdf:resource="http://openenergy-platform.org/ontology/oeo/OEO_00000061"/>
        <obo:IAO_0000115>Hardware is an artificial object that is part of an electronic system.</obo:IAO_0000115>
        <obo:IAO_0000233>issue: https://github.com/OpenEnergyPlatform/ontology/issues/319
pull request: https://github.com/OpenEnergyPlatform/ontology/pull/350</obo:IAO_0000233>
        <rdfs:label>hardware</rdfs:label>
    </owl:Class>
    


    <!-- http://openenergy-platform.org/ontology/oeo/OEO_00000207 -->

    <owl:Class rdf:about="http://openenergy-platform.org/ontology/oeo/OEO_00000207">
        <rdfs:subClassOf rdf:resource="http://openenergy-platform.org/ontology/oeo/OEO_00000150"/>
        <obo:IAO_0000115 xml:lang="en">Thermal energy is the energy that a material entity contains in the undirected motion of its constituent parts (e.g. molecules and atoms).</obo:IAO_0000115>
        <obo:IAO_0000233 xml:lang="en">issue: https://github.com/OpenEnergyPlatform/ontology/issues/522
pull request: https://github.com/OpenEnergyPlatform/ontology/pull/609</obo:IAO_0000233>
        <rdfs:label xml:lang="en">thermal energy</rdfs:label>
    </owl:Class>
    


    <!-- http://openenergy-platform.org/ontology/oeo/OEO_00000210 -->

    <owl:Class rdf:about="http://openenergy-platform.org/ontology/oeo/OEO_00000210">
        <rdfs:subClassOf rdf:resource="http://openenergy-platform.org/ontology/oeo/OEO_00000011"/>
        <rdfs:subClassOf>
            <owl:Restriction>
                <owl:onProperty rdf:resource="http://openenergy-platform.org/ontology/oeo/OEO_00000533"/>
                <owl:someValuesFrom rdf:resource="http://openenergy-platform.org/ontology/oeo/OEO_00000207"/>
            </owl:Restriction>
        </rdfs:subClassOf>
        <obo:IAO_0000115>A heater is an energy converting device that converts other forms of energy into useful heat.</obo:IAO_0000115>
        <obo:IAO_0000233>issue: https://github.com/OpenEnergyPlatform/ontology/issues/173
pull request: https://github.com/OpenEnergyPlatform/ontology/pull/273</obo:IAO_0000233>
        <rdfs:label>heater</rdfs:label>
    </owl:Class>
    


    <!-- http://openenergy-platform.org/ontology/oeo/OEO_00000211 -->

    <owl:Class rdf:about="http://openenergy-platform.org/ontology/oeo/OEO_00000211">
        <rdfs:subClassOf rdf:resource="http://openenergy-platform.org/ontology/oeo/OEO_00000181"/>
        <obo:IAO_0000115 xml:lang="en">Heating oil is gas diesel oil for industrial and commercial uses, marine diesel and diesel used in rail traffic, other gas oil, including heavy gas oils which distil between 380 °C and 540 °C and which are used as petrochemical feedstocks.</obo:IAO_0000115>
        <obo:IAO_0000118 xml:lang="en">OtherGasOil</obo:IAO_0000118>
        <obo:IAO_0000119 xml:lang="en">REGULATION (EC) No 1099/2008 OF THE EUROPEAN PARLIAMENT AND OF THE COUNCIL of 22 October 2008 on energy statistics https://eur-lex.europa.eu/legal-content/EN/TXT/HTML/?uri=CELEX:32008R1099&amp;from=EN</obo:IAO_0000119>
        <rdfs:label>heating oil</rdfs:label>
        <rdfs:label xml:lang="en">heating oil</rdfs:label>
    </owl:Class>
    


    <!-- http://openenergy-platform.org/ontology/oeo/OEO_00000212 -->

    <owl:Class rdf:about="http://openenergy-platform.org/ontology/oeo/OEO_00000212">
        <rdfs:subClassOf rdf:resource="http://openenergy-platform.org/ontology/oeo/OEO_00000210"/>
        <obo:IAO_0000115 xml:lang="en">A heat pump is a heater that transforms low temperature heat to high temperature heat using external energy.</obo:IAO_0000115>
        <rdfs:label>heat pump</rdfs:label>
    </owl:Class>
    


    <!-- http://openenergy-platform.org/ontology/oeo/OEO_00000218 -->

    <owl:Class rdf:about="http://openenergy-platform.org/ontology/oeo/OEO_00000218">
        <rdfs:subClassOf rdf:resource="http://openenergy-platform.org/ontology/oeo/OEO_00230020"/>
        <obo:IAO_0000115 xml:lang="en">Hydro energy is kinetic energy of moving liquid water which can result directly from its potential energy.</obo:IAO_0000115>
        <obo:IAO_0000233>issue: https://github.com/OpenEnergyPlatform/ontology/issues/679
pull request: https://github.com/OpenEnergyPlatform/ontology/pull/681</obo:IAO_0000233>
        <rdfs:label>hydro energy</rdfs:label>
    </owl:Class>
    


    <!-- http://openenergy-platform.org/ontology/oeo/OEO_00000219 -->

    <owl:Class rdf:about="http://openenergy-platform.org/ontology/oeo/OEO_00000219">
        <rdfs:subClassOf rdf:resource="http://openenergy-platform.org/ontology/oeo/OEO_00000331"/>
        <rdfs:subClassOf>
            <owl:Restriction>
                <owl:onProperty rdf:resource="http://openenergy-platform.org/ontology/oeo/OEO_00000530"/>
                <owl:someValuesFrom rdf:resource="http://openenergy-platform.org/ontology/oeo/OEO_00030000"/>
            </owl:Restriction>
        </rdfs:subClassOf>
        <obo:IAO_0000115 xml:lang="en">Hydrofluorocarbons (HFCs) are portions of matter consisting of organic compounds that contain fluorine and hydrogen atoms, and are the most common type of organofluorine compounds. They are frequently used in air conditioning and as refrigerants in place of the older chlorofluorocarbons such as R-12 and hydrochlorofluorocarbons such as R-21.</obo:IAO_0000115>
        <obo:IAO_0000118>HFC</obo:IAO_0000118>
        <obo:IAO_0000119 xml:lang="en">https://en.wikipedia.org/w/index.php?title=Hydrofluorocarbon&amp;oldid=904556263</obo:IAO_0000119>
        <rdfs:label>hydrofluorocarbon</rdfs:label>
    </owl:Class>
    


    <!-- http://openenergy-platform.org/ontology/oeo/OEO_00000220 -->

    <owl:Class rdf:about="http://openenergy-platform.org/ontology/oeo/OEO_00000220">
        <rdfs:subClassOf rdf:resource="http://openenergy-platform.org/ontology/oeo/OEO_00000331"/>
        <rdfs:subClassOf>
            <owl:Restriction>
                <owl:onProperty rdf:resource="http://purl.obolibrary.org/obo/RO_0000087"/>
                <owl:someValuesFrom rdf:resource="http://openenergy-platform.org/ontology/oeo/OEO_00000001"/>
            </owl:Restriction>
        </rdfs:subClassOf>
        <rdfs:subClassOf>
            <owl:Restriction>
                <owl:onProperty rdf:resource="http://purl.obolibrary.org/obo/RO_0000091"/>
                <owl:someValuesFrom rdf:resource="http://openenergy-platform.org/ontology/oeo/OEO_00000097"/>
            </owl:Restriction>
        </rdfs:subClassOf>
        <rdfs:subClassOf>
            <owl:Restriction>
                <owl:onProperty rdf:resource="http://openenergy-platform.org/ontology/oeo/OEO_00000529"/>
                <owl:hasValue rdf:resource="http://openenergy-platform.org/ontology/oeo/OEO_00000182"/>
            </owl:Restriction>
        </rdfs:subClassOf>
        <obo:IAO_0000115 xml:lang="en">Hydrogen is a portion of matter with the chemical formular H2. It has a gaseous normal state of matter. As it can be oxidised it can be used as a fuel.</obo:IAO_0000115>
        <obo:IAO_0000118>H2</obo:IAO_0000118>
        <obo:IAO_0000233>issue: https://github.com/OpenEnergyPlatform/ontology/issues/134</obo:IAO_0000233>
        <rdfs:label>hydrogen</rdfs:label>
    </owl:Class>
    


    <!-- http://openenergy-platform.org/ontology/oeo/OEO_00000221 -->

    <owl:Class rdf:about="http://openenergy-platform.org/ontology/oeo/OEO_00000221">
        <rdfs:subClassOf rdf:resource="http://openenergy-platform.org/ontology/oeo/OEO_00000031"/>
        <rdfs:subClassOf>
            <owl:Restriction>
                <owl:onProperty rdf:resource="http://purl.obolibrary.org/obo/BFO_0000051"/>
                <owl:someValuesFrom rdf:resource="http://openenergy-platform.org/ontology/oeo/OEO_00000022"/>
            </owl:Restriction>
        </rdfs:subClassOf>
        <rdfs:subClassOf>
            <owl:Restriction>
                <owl:onProperty rdf:resource="http://purl.obolibrary.org/obo/BFO_0000051"/>
                <owl:someValuesFrom rdf:resource="http://openenergy-platform.org/ontology/oeo/OEO_00000222"/>
            </owl:Restriction>
        </rdfs:subClassOf>
        <obo:IAO_0000115 xml:lang="en">A hydrogen powerplant is a powerplant having an aggregate of hydrogen power units as its power generating units.</obo:IAO_0000115>
        <rdfs:label>hydrogen powerplant</rdfs:label>
    </owl:Class>
    


    <!-- http://openenergy-platform.org/ontology/oeo/OEO_00000222 -->

    <owl:Class rdf:about="http://openenergy-platform.org/ontology/oeo/OEO_00000222">
        <rdfs:subClassOf rdf:resource="http://openenergy-platform.org/ontology/oeo/OEO_00000185"/>
        <rdfs:subClassOf>
            <owl:Restriction>
                <owl:onProperty rdf:resource="http://openenergy-platform.org/ontology/oeo/OEO_00000533"/>
                <owl:someValuesFrom rdf:resource="http://openenergy-platform.org/ontology/oeo/OEO_00000333"/>
            </owl:Restriction>
        </rdfs:subClassOf>
        <rdfs:subClassOf>
            <owl:Restriction>
                <owl:onProperty rdf:resource="http://openenergy-platform.org/ontology/oeo/OEO_00000532"/>
                <owl:allValuesFrom rdf:resource="http://openenergy-platform.org/ontology/oeo/OEO_00000220"/>
            </owl:Restriction>
        </rdfs:subClassOf>
        <obo:IAO_0000115 xml:lang="en">A hydrogen turbine is a gas turbine fueled with hydrogen.</obo:IAO_0000115>
        <obo:IAO_0000233>issue: https://github.com/OpenEnergyPlatform/ontology/issues/299
pull request: https://github.com/OpenEnergyPlatform/ontology/pull/300</obo:IAO_0000233>
        <rdfs:label>hydrogen turbine</rdfs:label>
    </owl:Class>
    


    <!-- http://openenergy-platform.org/ontology/oeo/OEO_00000226 -->

    <owl:Class rdf:about="http://openenergy-platform.org/ontology/oeo/OEO_00000226">
        <rdfs:subClassOf rdf:resource="http://openenergy-platform.org/ontology/oeo/OEO_00000439"/>
        <obo:IAO_0000115 xml:lang="en">Industrial waste fuel is waste fuel of industrial non-renewable origin (solids or liquids) combusted directly for the production of electricity and/or heat. The quantity of fuel used should be reported on a net calorific value basis. Renewable industrial waste should be reported in the solid biomass, biogas and/or liquid biofuels categories.</obo:IAO_0000115>
        <obo:IAO_0000119 xml:lang="en">REGULATION (EC) No 1099/2008 OF THE EUROPEAN PARLIAMENT AND OF THE COUNCIL of 22 October 2008 on energy statistics https://eur-lex.europa.eu/legal-content/EN/TXT/HTML/?uri=CELEX:32008R1099&amp;from=EN</obo:IAO_0000119>
        <rdfs:label>industrial waste fuel</rdfs:label>
    </owl:Class>
    


    <!-- http://openenergy-platform.org/ontology/oeo/OEO_00000240 -->

    <owl:Class rdf:about="http://openenergy-platform.org/ontology/oeo/OEO_00000240">
        <rdfs:subClassOf rdf:resource="http://openenergy-platform.org/ontology/oeo/OEO_00010023"/>
        <rdfs:subClassOf>
            <owl:Restriction>
                <owl:onProperty rdf:resource="http://openenergy-platform.org/ontology/oeo/OEO_00000503"/>
                <owl:someValuesFrom rdf:resource="http://openenergy-platform.org/ontology/oeo/OEO_00000099"/>
            </owl:Restriction>
        </rdfs:subClassOf>
        <rdfs:subClassOf>
            <owl:Restriction>
                <owl:onProperty rdf:resource="http://purl.obolibrary.org/obo/BFO_0000051"/>
                <owl:someValuesFrom rdf:resource="http://openenergy-platform.org/ontology/oeo/OEO_00010029"/>
            </owl:Restriction>
        </rdfs:subClassOf>
        <obo:IAO_0000115>An internal combustion vehicle is a vehicle powered by an internal combustion engine.</obo:IAO_0000115>
        <obo:IAO_0000233>issue: https://github.com/OpenEnergyPlatform/ontology/issues/425
pull request: https://github.com/OpenEnergyPlatform/ontology/pull/431</obo:IAO_0000233>
        <rdfs:label>internal combustion vehicle</rdfs:label>
    </owl:Class>
    


    <!-- http://openenergy-platform.org/ontology/oeo/OEO_00000245 -->

    <owl:Class rdf:about="http://openenergy-platform.org/ontology/oeo/OEO_00000245">
        <rdfs:subClassOf rdf:resource="http://openenergy-platform.org/ontology/oeo/OEO_00000246"/>
        <obo:IAO_0000115 xml:lang="en">Jet fuel is kerosene used for aviation turbine power units. It has the same distillation characteristics between 150 °C and 300 °C (generally not above 250 °C) and flash point as kerosene. In addition, it has particular specifications (such as freezing point) which are established by the International air Transport Association (IATA).</obo:IAO_0000115>
        <obo:IAO_0000119 xml:lang="en">REGULATION (EC) No 1099/2008 OF THE EUROPEAN PARLIAMENT AND OF THE COUNCIL of 22 October 2008 on energy statistics https://eur-lex.europa.eu/legal-content/EN/TXT/HTML/?uri=CELEX:32008R1099&amp;from=EN</obo:IAO_0000119>
        <rdfs:label xml:lang="en">KeroseneTypeJetFuel</rdfs:label>
        <rdfs:label>jet fuel</rdfs:label>
    </owl:Class>
    


    <!-- http://openenergy-platform.org/ontology/oeo/OEO_00000246 -->

    <owl:Class rdf:about="http://openenergy-platform.org/ontology/oeo/OEO_00000246">
        <rdfs:subClassOf rdf:resource="http://openenergy-platform.org/ontology/oeo/OEO_00000309"/>
        <rdfs:subClassOf>
            <owl:Restriction>
                <owl:onProperty rdf:resource="http://openenergy-platform.org/ontology/oeo/OEO_00000529"/>
                <owl:hasValue rdf:resource="http://openenergy-platform.org/ontology/oeo/OEO_00000256"/>
            </owl:Restriction>
        </rdfs:subClassOf>
        <obo:IAO_0000115>Kerosene, also known as paraffin, lamp oil, and coal oil (an obsolete term), is an oil and petroleum product consisting of combustible hydrocarbon liquid which is derived from petroleum. It is widely used as a fuel in industry as well as households. It is sometimes spelled kerosine in scientific and industrial usage.
[...]

Kerosene is widely used to power jet engines of aircraft (jet fuel) and some rocket engines and is also commonly used as a cooking and lighting fuel and for fire toys such as poi. In parts of Asia, kerosene is sometimes used as fuel for small outboard motors or even motorcycles.</obo:IAO_0000115>
        <obo:IAO_0000119>https://en.wikipedia.org/w/index.php?title=Kerosene&amp;oldid=867958484</obo:IAO_0000119>
        <rdfs:label>kerosene</rdfs:label>
    </owl:Class>
    


    <!-- http://openenergy-platform.org/ontology/oeo/OEO_00000248 -->

    <owl:Class rdf:about="http://openenergy-platform.org/ontology/oeo/OEO_00000248">
        <rdfs:subClassOf rdf:resource="http://openenergy-platform.org/ontology/oeo/OEO_00000068"/>
        <obo:IAO_0000115 xml:lang="en">A lithium-ion battery or Li-ion battery (abbreviated as LIB) is a type of rechargeable battery [...] In the batteries lithium ions move from the negative electrode to the positive electrode during discharge and back when charging. Li-ion batteries use an intercalated lithium compound as one electrode material, compared to the metallic lithium used in a non-rechargeable lithium battery. </obo:IAO_0000115>
        <obo:IAO_0000119 xml:lang="en">https://en.wikipedia.org/w/index.php?title=Lithium-ion_battery&amp;oldid=906786251</obo:IAO_0000119>
        <rdfs:label>lithium-ion battery</rdfs:label>
    </owl:Class>
    


    <!-- http://openenergy-platform.org/ontology/oeo/OEO_00000251 -->

    <owl:Class rdf:about="http://openenergy-platform.org/ontology/oeo/OEO_00000251">
        <rdfs:subClassOf rdf:resource="http://openenergy-platform.org/ontology/oeo/OEO_00000088"/>
        <rdfs:subClassOf>
            <owl:Restriction>
                <owl:onProperty rdf:resource="http://openenergy-platform.org/ontology/oeo/OEO_00000530"/>
                <owl:someValuesFrom rdf:resource="http://openenergy-platform.org/ontology/oeo/OEO_00030002"/>
            </owl:Restriction>
        </rdfs:subClassOf>
        <rdfs:subClassOf>
            <owl:Restriction>
                <owl:onProperty rdf:resource="http://openenergy-platform.org/ontology/oeo/OEO_00000529"/>
                <owl:hasValue rdf:resource="http://openenergy-platform.org/ontology/oeo/OEO_00000390"/>
            </owl:Restriction>
        </rdfs:subClassOf>
        <obo:IAO_0000115 xml:lang="en">Lignite is coal that is non-agglomerating with a gross calorific value less than 17 435 kJ/kg (4 165 kcal/kg) and greater than 31 % volatile matter on a dry mineral matter free basis.	

Oil shale and tar sands produced and combusted directly should be reported in this category. Oil shale and tar sands used as inputs for other transformation processes should also be reported in this category.	

This includes the portion of the oil shale or tar sands consumed in the transformation process.</obo:IAO_0000115>
        <obo:IAO_0000119 xml:lang="en">REGULATION (EC) No 1099/2008 OF THE EUROPEAN PARLIAMENT AND OF THE COUNCIL of 22 October 2008 on energy statistics https://eur-lex.europa.eu/legal-content/EN/TXT/HTML/?uri=CELEX:32008R1099&amp;from=EN</obo:IAO_0000119>
        <rdfs:label>lignite</rdfs:label>
    </owl:Class>
    


    <!-- http://openenergy-platform.org/ontology/oeo/OEO_00000252 -->

    <owl:Class rdf:about="http://openenergy-platform.org/ontology/oeo/OEO_00000252">
        <rdfs:subClassOf rdf:resource="http://openenergy-platform.org/ontology/oeo/OEO_00000089"/>
        <rdfs:subClassOf>
            <owl:Restriction>
                <owl:onProperty rdf:resource="http://purl.obolibrary.org/obo/BFO_0000051"/>
                <owl:someValuesFrom rdf:resource="http://openenergy-platform.org/ontology/oeo/OEO_00000024"/>
            </owl:Restriction>
        </rdfs:subClassOf>
        <obo:IAO_0000115 xml:lang="en">A lignite powerplant is a coal powerplant having an aggregate of lignite power units as its power generating units.</obo:IAO_0000115>
        <rdfs:label>lignite powerplant</rdfs:label>
    </owl:Class>
    


    <!-- http://openenergy-platform.org/ontology/oeo/OEO_00000253 -->

    <owl:Class rdf:about="http://openenergy-platform.org/ontology/oeo/OEO_00000253">
        <rdfs:subClassOf rdf:resource="http://openenergy-platform.org/ontology/oeo/OEO_00000255"/>
        <rdfs:subClassOf>
            <owl:Restriction>
                <owl:onProperty rdf:resource="http://purl.obolibrary.org/obo/BFO_0000050"/>
                <owl:someValuesFrom rdf:resource="http://openenergy-platform.org/ontology/oeo/OEO_00000143"/>
            </owl:Restriction>
        </rdfs:subClassOf>
        <obo:IAO_0000115 xml:lang="en">A powerline is a grid component that is an uninterrupted transmission system between two nodes in an electricity grid.</obo:IAO_0000115>
        <obo:IAO_0000233>issue: https://github.com/OpenEnergyPlatform/ontology/issues/231
pull request: https://github.com/OpenEnergyPlatform/ontology/pull/385</obo:IAO_0000233>
        <rdfs:label xml:lang="en">power line</rdfs:label>
    </owl:Class>
    


    <!-- http://openenergy-platform.org/ontology/oeo/OEO_00000255 -->

    <owl:Class rdf:about="http://openenergy-platform.org/ontology/oeo/OEO_00000255">
        <rdfs:subClassOf rdf:resource="http://openenergy-platform.org/ontology/oeo/OEO_00020006"/>
        <owl:disjointWith rdf:resource="http://openenergy-platform.org/ontology/oeo/OEO_00000296"/>
        <obo:IAO_0000115 xml:lang="en">A grid component link is a grid component that serves as a connection between two other grid components.</obo:IAO_0000115>
        <obo:IAO_0000233 xml:lang="en">issue: https://github.com/OpenEnergyPlatform/ontology/issues/36
pull request: https://github.com/OpenEnergyPlatform/ontology/pull/385</obo:IAO_0000233>
        <rdfs:label>grid component link</rdfs:label>
    </owl:Class>
    


    <!-- http://openenergy-platform.org/ontology/oeo/OEO_00000257 -->

    <owl:Class rdf:about="http://openenergy-platform.org/ontology/oeo/OEO_00000257">
        <rdfs:subClassOf rdf:resource="http://openenergy-platform.org/ontology/oeo/OEO_00000054"/>
        <obo:IAO_0000115 xml:lang="en">Liquid air is air that has been compressed and cooled to store energy until it condenses as a liquid. To discharge energy, the air is expanded.</obo:IAO_0000115>
        <rdfs:label>liquid air</rdfs:label>
    </owl:Class>
    


    <!-- http://openenergy-platform.org/ontology/oeo/OEO_00000258 -->

    <owl:Class rdf:about="http://openenergy-platform.org/ontology/oeo/OEO_00000258">
        <owl:equivalentClass>
            <owl:Class>
                <owl:intersectionOf rdf:parseType="Collection">
                    <rdf:Description rdf:about="http://openenergy-platform.org/ontology/oeo/OEO_00000072"/>
                    <owl:Restriction>
                        <owl:onProperty rdf:resource="http://openenergy-platform.org/ontology/oeo/OEO_00000529"/>
                        <owl:hasValue rdf:resource="http://openenergy-platform.org/ontology/oeo/OEO_00000256"/>
                    </owl:Restriction>
                </owl:intersectionOf>
            </owl:Class>
        </owl:equivalentClass>
        <rdfs:subClassOf>
            <owl:Restriction>
                <owl:onProperty rdf:resource="http://openenergy-platform.org/ontology/oeo/OEO_00000530"/>
                <owl:someValuesFrom rdf:resource="http://openenergy-platform.org/ontology/oeo/OEO_00030001"/>
            </owl:Restriction>
        </rdfs:subClassOf>
        <rdfs:subClassOf>
            <owl:Restriction>
                <owl:onProperty rdf:resource="http://openenergy-platform.org/ontology/oeo/OEO_00000530"/>
                <owl:someValuesFrom rdf:resource="http://openenergy-platform.org/ontology/oeo/OEO_00030004"/>
            </owl:Restriction>
        </rdfs:subClassOf>
        <rdfs:subClassOf>
            <owl:Restriction>
                <owl:onProperty rdf:resource="http://openenergy-platform.org/ontology/oeo/OEO_00000529"/>
                <owl:hasValue rdf:resource="http://openenergy-platform.org/ontology/oeo/OEO_00000256"/>
            </owl:Restriction>
        </rdfs:subClassOf>
        <obo:IAO_0000115>A liquid biofuel is a biofuel that has liquid as its normal state of matter.</obo:IAO_0000115>
        <rdfs:label>liquid biofuel</rdfs:label>
    </owl:Class>
    


    <!-- http://openenergy-platform.org/ontology/oeo/OEO_00000259 -->

    <owl:Class rdf:about="http://openenergy-platform.org/ontology/oeo/OEO_00000259">
        <rdfs:subClassOf rdf:resource="http://openenergy-platform.org/ontology/oeo/OEO_00000283"/>
        <obo:IAO_0000115 xml:lang="en">Rechargeable liquid-metal batteries are used for electric vehicles and potentially also for grid energy storage, to balance out intermittent renewable power sources such as solar panels and wind turbines.</obo:IAO_0000115>
        <obo:IAO_0000119 xml:lang="en">https://en.wikipedia.org/w/index.php?title=Molten-salt_battery&amp;oldid=900557096</obo:IAO_0000119>
        <rdfs:label>liquid-metal battery</rdfs:label>
    </owl:Class>
    


    <!-- http://openenergy-platform.org/ontology/oeo/OEO_00000263 -->

    <owl:Class rdf:about="http://openenergy-platform.org/ontology/oeo/OEO_00000263">
        <rdfs:subClassOf rdf:resource="http://openenergy-platform.org/ontology/oeo/OEO_00000331"/>
        <rdfs:subClassOf>
            <owl:Restriction>
                <owl:onProperty rdf:resource="http://openenergy-platform.org/ontology/oeo/OEO_00000530"/>
                <owl:someValuesFrom rdf:resource="http://openenergy-platform.org/ontology/oeo/OEO_00030002"/>
            </owl:Restriction>
        </rdfs:subClassOf>
        <rdfs:subClassOf>
            <owl:Restriction>
                <owl:onProperty rdf:resource="http://purl.obolibrary.org/obo/RO_0000087"/>
                <owl:someValuesFrom rdf:resource="http://openenergy-platform.org/ontology/oeo/OEO_00000001"/>
            </owl:Restriction>
        </rdfs:subClassOf>
        <rdfs:subClassOf>
            <owl:Restriction>
                <owl:onProperty rdf:resource="http://purl.obolibrary.org/obo/RO_0000091"/>
                <owl:someValuesFrom rdf:resource="http://openenergy-platform.org/ontology/oeo/OEO_00000097"/>
            </owl:Restriction>
        </rdfs:subClassOf>
        <rdfs:subClassOf>
            <owl:Restriction>
                <owl:onProperty rdf:resource="http://openenergy-platform.org/ontology/oeo/OEO_00000529"/>
                <owl:hasValue rdf:resource="http://openenergy-platform.org/ontology/oeo/OEO_00000182"/>
            </owl:Restriction>
        </rdfs:subClassOf>
        <obo:IAO_0000115 xml:lang="en">A manufactured coal based gas is a portion of matter that is gaseous and manufactured from coal. It is used as fossil fuel.</obo:IAO_0000115>
        <rdfs:label>manufactured coal based gas</rdfs:label>
    </owl:Class>
    


    <!-- http://openenergy-platform.org/ontology/oeo/OEO_00000269 -->

    <owl:Class rdf:about="http://openenergy-platform.org/ontology/oeo/OEO_00000269">
        <rdfs:subClassOf rdf:resource="http://openenergy-platform.org/ontology/oeo/OEO_00000012"/>
        <obo:IAO_0000115 xml:lang="en">A methanation gas storage is a energy storage that uses carbon dioxide and hydrogen from electrolysis to produce methan and store this. The methan can then be used to produce electricity or heat in a gas generator.</obo:IAO_0000115>
        <rdfs:label>methanation gas storage</rdfs:label>
    </owl:Class>
    


    <!-- http://openenergy-platform.org/ontology/oeo/OEO_00000282 -->

    <owl:Class rdf:about="http://openenergy-platform.org/ontology/oeo/OEO_00000282">
        <rdfs:subClassOf rdf:resource="http://openenergy-platform.org/ontology/oeo/OEO_00000283"/>
        <obo:IAO_0000115 xml:lang="en">Molten-salt batteries are a class of battery that uses molten salts as an electrolyte and offers both a high energy density and a high power density.</obo:IAO_0000115>
        <obo:IAO_0000119 xml:lang="en">https://en.wikipedia.org/w/index.php?title=Molten-salt_battery&amp;oldid=900557096</obo:IAO_0000119>
        <rdfs:label>molten-salt battery</rdfs:label>
    </owl:Class>
    


    <!-- http://openenergy-platform.org/ontology/oeo/OEO_00000283 -->

    <owl:Class rdf:about="http://openenergy-platform.org/ontology/oeo/OEO_00000283">
        <rdfs:subClassOf rdf:resource="http://openenergy-platform.org/ontology/oeo/OEO_00000068"/>
        <obo:IAO_0000115 xml:lang="en">Molten-state batteries consist of two molten metal alloys separated by an electrolyte.</obo:IAO_0000115>
        <obo:IAO_0000115 xml:lang="en">Wastes produced by households, hospitals and the tertiary sector incinerated at specific installations, on a net calorific value basis.</obo:IAO_0000115>
        <obo:IAO_0000119 xml:lang="en">REGULATION (EC) No 1099/2008 OF THE EUROPEAN PARLIAMENT AND OF THE COUNCIL of 22 October 2008 on energy statistics https://eur-lex.europa.eu/legal-content/EN/TXT/HTML/?uri=CELEX:32008R1099&amp;from=EN</obo:IAO_0000119>
        <rdfs:label>molten state battery</rdfs:label>
    </owl:Class>
    


    <!-- http://openenergy-platform.org/ontology/oeo/OEO_00000286 -->

    <owl:Class rdf:about="http://openenergy-platform.org/ontology/oeo/OEO_00000286">
        <rdfs:subClassOf rdf:resource="http://openenergy-platform.org/ontology/oeo/OEO_00000183"/>
        <obo:IAO_0000115 xml:lang="en">Motor gasoline is gasoline consisting of a mixture of light hydrocarbons distilling between 35 oC and 215 oC. It is used as a fuel for land based spark ignition engines. Motor gasoline may include additives, oxygenates and octane enhancers, including lead compounds such as TEL and TML.

Includes motor gasoline blending components (excluding additives/oxygenates), e.g. alkylates, isomerate, reformate, cracked gasoline destined for use as finished motor gasoline.</obo:IAO_0000115>
        <obo:IAO_0000119 xml:lang="en">REGULATION (EC) No 1099/2008 OF THE EUROPEAN PARLIAMENT AND OF THE COUNCIL of 22 October 2008 on energy statistics https://eur-lex.europa.eu/legal-content/EN/TXT/HTML/?uri=CELEX:32008R1099&amp;from=EN</obo:IAO_0000119>
        <rdfs:label>motor gasoline</rdfs:label>
    </owl:Class>
    


    <!-- http://openenergy-platform.org/ontology/oeo/OEO_00000290 -->

    <owl:Class rdf:about="http://openenergy-platform.org/ontology/oeo/OEO_00000290">
        <rdfs:subClassOf rdf:resource="http://openenergy-platform.org/ontology/oeo/OEO_00000439"/>
        <obo:IAO_0000115 xml:lang="en">Municipal waste fuel is waste fuel of waste produced by households, hospitals and the tertiary sector incinerated at specific installations, on a net calorific value basis.</obo:IAO_0000115>
        <obo:IAO_0000119 xml:lang="en">REGULATION (EC) No 1099/2008 OF THE EUROPEAN PARLIAMENT AND OF THE COUNCIL of 22 October 2008 on energy statistics https://eur-lex.europa.eu/legal-content/EN/TXT/HTML/?uri=CELEX:32008R1099&amp;from=EN</obo:IAO_0000119>
        <rdfs:label>municipal waste fuel</rdfs:label>
    </owl:Class>
    


    <!-- http://openenergy-platform.org/ontology/oeo/OEO_00000292 -->

    <owl:Class rdf:about="http://openenergy-platform.org/ontology/oeo/OEO_00000292">
        <rdfs:subClassOf rdf:resource="http://openenergy-platform.org/ontology/oeo/OEO_00000331"/>
        <rdfs:subClassOf>
            <owl:Restriction>
                <owl:onProperty rdf:resource="http://openenergy-platform.org/ontology/oeo/OEO_00000530"/>
                <owl:someValuesFrom rdf:resource="http://openenergy-platform.org/ontology/oeo/OEO_00030002"/>
            </owl:Restriction>
        </rdfs:subClassOf>
        <rdfs:subClassOf>
            <owl:Restriction>
                <owl:onProperty rdf:resource="http://purl.obolibrary.org/obo/BFO_0000051"/>
                <owl:someValuesFrom rdf:resource="http://openenergy-platform.org/ontology/oeo/OEO_00000025"/>
            </owl:Restriction>
        </rdfs:subClassOf>
        <rdfs:subClassOf>
            <owl:Restriction>
                <owl:onProperty rdf:resource="http://purl.obolibrary.org/obo/RO_0000087"/>
                <owl:someValuesFrom rdf:resource="http://openenergy-platform.org/ontology/oeo/OEO_00000001"/>
            </owl:Restriction>
        </rdfs:subClassOf>
        <rdfs:subClassOf>
            <owl:Restriction>
                <owl:onProperty rdf:resource="http://purl.obolibrary.org/obo/RO_0000091"/>
                <owl:someValuesFrom rdf:resource="http://openenergy-platform.org/ontology/oeo/OEO_00000097"/>
            </owl:Restriction>
        </rdfs:subClassOf>
        <rdfs:subClassOf>
            <owl:Restriction>
                <owl:onProperty rdf:resource="http://openenergy-platform.org/ontology/oeo/OEO_00000529"/>
                <owl:hasValue rdf:resource="http://openenergy-platform.org/ontology/oeo/OEO_00000182"/>
            </owl:Restriction>
        </rdfs:subClassOf>
        <obo:IAO_0000115 xml:lang="en">Natural gas is a portion of matter which comprises gases occurring in underground deposits, whether liquefied or gaseous, consisting mainly of methane.

It includes both ‘non-associated’ gas originating from fields producing hydrocarbons only in gaseous form, and ‘associated’ gas produced in association with crude oil as well as methane recovered from coal mines (colliery gas) or from coal seams (coal seam gas).

It does not include gases created by anaerobic digestion of biomass (e.g. municipal or sewage gas) nor gasworks gas.</obo:IAO_0000115>
        <obo:IAO_0000119 xml:lang="en">REGULATION (EC) No 1099/2008 OF THE EUROPEAN PARLIAMENT AND OF THE COUNCIL of 22 October 2008 on energy statistics https://eur-lex.europa.eu/legal-content/EN/TXT/HTML/?uri=CELEX:32008R1099&amp;from=EN</obo:IAO_0000119>
        <obo:IAO_0000233>issue: https://github.com/OpenEnergyPlatform/ontology/issues/430
pull request: https://github.com/OpenEnergyPlatform/ontology/pull/431</obo:IAO_0000233>
        <rdfs:label>natural gas</rdfs:label>
    </owl:Class>
    


    <!-- http://openenergy-platform.org/ontology/oeo/OEO_00000293 -->

    <owl:Class rdf:about="http://openenergy-platform.org/ontology/oeo/OEO_00000293">
        <rdfs:subClassOf rdf:resource="http://purl.obolibrary.org/obo/BFO_0000015"/>
        <obo:IAO_0000115>Negative emission is the process of absorbing a substance, usually a pollutant that was emitted before.</obo:IAO_0000115>
        <obo:IAO_0000233>issue: https://github.com/OpenEnergyPlatform/ontology/issues/56
pull request: https://github.com/OpenEnergyPlatform/ontology/pull/234</obo:IAO_0000233>
        <rdfs:label>negative emission</rdfs:label>
    </owl:Class>
    


    <!-- http://openenergy-platform.org/ontology/oeo/OEO_00000296 -->

    <owl:Class rdf:about="http://openenergy-platform.org/ontology/oeo/OEO_00000296">
        <rdfs:subClassOf rdf:resource="http://openenergy-platform.org/ontology/oeo/OEO_00020006"/>
        <obo:IAO_0000115 xml:lang="en">A grid node is a grid component of a supply grid where two or more links meet.</obo:IAO_0000115>
        <obo:IAO_0000233 xml:lang="en">issue: https://github.com/OpenEnergyPlatform/ontology/issues/36
pull request: https://github.com/OpenEnergyPlatform/ontology/pull/385</obo:IAO_0000233>
        <rdfs:label>grid node</rdfs:label>
    </owl:Class>
    


    <!-- http://openenergy-platform.org/ontology/oeo/OEO_00000297 -->

    <owl:Class rdf:about="http://openenergy-platform.org/ontology/oeo/OEO_00000297">
        <rdfs:subClassOf rdf:resource="http://openenergy-platform.org/ontology/oeo/OEO_00000292"/>
        <obo:IAO_0000115>Non associated gas is natural gas originating from fields producing hydrocarbons only in gaseous form.</obo:IAO_0000115>
        <obo:IAO_0000119>REGULATION (EC) No 1099/2008 OF THE EUROPEAN PARLIAMENT AND OF THE COUNCIL of 22 October 2008 on energy statistics https://eur-lex.europa.eu/legal-content/EN/TXT/HTML/?uri=CELEX:32008R1099&amp;from=EN</obo:IAO_0000119>
        <rdfs:label>non associated gas</rdfs:label>
    </owl:Class>
    


    <!-- http://openenergy-platform.org/ontology/oeo/OEO_00000298 -->

    <owl:Class rdf:about="http://openenergy-platform.org/ontology/oeo/OEO_00000298">
        <rdfs:subClassOf rdf:resource="http://openenergy-platform.org/ontology/oeo/OEO_00000437"/>
        <obo:IAO_0000115 xml:lang="en">A non-methane volatile organic compound (NMVOC) is a volatile organic compound other than methane.</obo:IAO_0000115>
        <obo:IAO_0000118>NMVOC</obo:IAO_0000118>
        <obo:IAO_0000119>This definition is partly based on Article 2 of the European Air Quality Directive (2008/50/EC): https://eur-lex.europa.eu/legal-content/EN/TXT/?uri=CELEX:32008L0050</obo:IAO_0000119>
        <obo:IAO_0000233>issue: https://github.com/OpenEnergyPlatform/ontology/issues/263
pull request: https://github.com/OpenEnergyPlatform/ontology/pull/356</obo:IAO_0000233>
        <rdfs:label>non-methane volatile organic compound</rdfs:label>
    </owl:Class>
    


    <!-- http://openenergy-platform.org/ontology/oeo/OEO_00000299 -->

    <owl:Class rdf:about="http://openenergy-platform.org/ontology/oeo/OEO_00000299">
        <rdfs:subClassOf rdf:resource="http://openenergy-platform.org/ontology/oeo/OEO_00000290"/>
        <rdfs:subClassOf>
            <owl:Restriction>
                <owl:onProperty rdf:resource="http://openenergy-platform.org/ontology/oeo/OEO_00000530"/>
                <owl:someValuesFrom rdf:resource="http://openenergy-platform.org/ontology/oeo/OEO_00030002"/>
            </owl:Restriction>
        </rdfs:subClassOf>
        <obo:IAO_0000115 xml:lang="en">Non renewable municipal waste fuel is municipal waste fuel of non-biological origin.</obo:IAO_0000115>
        <obo:IAO_0000119 xml:lang="en">REGULATION (EC) No 1099/2008 OF THE EUROPEAN PARLIAMENT AND OF THE COUNCIL of 22 October 2008 on energy statistics https://eur-lex.europa.eu/legal-content/EN/TXT/HTML/?uri=CELEX:32008R1099&amp;from=EN</obo:IAO_0000119>
        <rdfs:label>non renewable municipal waste fuel</rdfs:label>
    </owl:Class>
    


    <!-- http://openenergy-platform.org/ontology/oeo/OEO_00000300 -->

    <owl:Class rdf:about="http://openenergy-platform.org/ontology/oeo/OEO_00000300">
        <rdfs:subClassOf rdf:resource="http://openenergy-platform.org/ontology/oeo/OEO_00000150"/>
        <obo:IAO_0000115 xml:lang="en">Nuclear binding energy is the energy that is required to disassemble the nucleus of an atom into its component parts.</obo:IAO_0000115>
        <obo:IAO_0000119 xml:lang="en">Derived from https://en.wikipedia.org/w/index.php?title=Nuclear_binding_energy&amp;oldid=1007327561</obo:IAO_0000119>
        <obo:IAO_0000233>issue: https://github.com/OpenEnergyPlatform/ontology/issues/211
pull request: https://github.com/OpenEnergyPlatform/ontology/pull/225
convertion to nuclear binding energy
issue: https://github.com/OpenEnergyPlatform/ontology/issues/522
pull request: https://github.com/OpenEnergyPlatform/ontology/pull/698</obo:IAO_0000233>
        <rdfs:label>nuclear binding energy</rdfs:label>
    </owl:Class>
    


    <!-- http://openenergy-platform.org/ontology/oeo/OEO_00000302 -->

    <owl:Class rdf:about="http://openenergy-platform.org/ontology/oeo/OEO_00000302">
        <owl:equivalentClass>
            <owl:Class>
                <owl:intersectionOf rdf:parseType="Collection">
                    <rdf:Description rdf:about="http://openenergy-platform.org/ontology/oeo/OEO_00000173"/>
                    <owl:Restriction>
                        <owl:onProperty rdf:resource="http://purl.obolibrary.org/obo/RO_0000091"/>
                        <owl:someValuesFrom rdf:resource="http://openenergy-platform.org/ontology/oeo/OEO_00000028"/>
                    </owl:Restriction>
                </owl:intersectionOf>
            </owl:Class>
        </owl:equivalentClass>
        <rdfs:subClassOf rdf:resource="http://openenergy-platform.org/ontology/oeo/OEO_00000173"/>
        <rdfs:subClassOf>
            <owl:Restriction>
                <owl:onProperty rdf:resource="http://purl.obolibrary.org/obo/RO_0000086"/>
                <owl:someValuesFrom rdf:resource="http://openenergy-platform.org/ontology/oeo/OEO_00000300"/>
            </owl:Restriction>
        </rdfs:subClassOf>
        <obo:IAO_0000115>A nuclear fuel is a fuel that realizes its fuel role in processes that release energy in the form of heat or work by undergoing nuclear fission.</obo:IAO_0000115>
        <obo:IAO_0000233>issue: https://github.com/OpenEnergyPlatform/ontology/issues/182
pull request: https://github.com/OpenEnergyPlatform/ontology/pull/237</obo:IAO_0000233>
        <rdfs:label>nuclear fuel</rdfs:label>
    </owl:Class>
    


    <!-- http://openenergy-platform.org/ontology/oeo/OEO_00000303 -->

    <owl:Class rdf:about="http://openenergy-platform.org/ontology/oeo/OEO_00000303">
        <rdfs:subClassOf rdf:resource="http://openenergy-platform.org/ontology/oeo/OEO_00000031"/>
        <rdfs:subClassOf>
            <owl:Restriction>
                <owl:onProperty rdf:resource="http://purl.obolibrary.org/obo/BFO_0000051"/>
                <owl:someValuesFrom rdf:resource="http://openenergy-platform.org/ontology/oeo/OEO_00000029"/>
            </owl:Restriction>
        </rdfs:subClassOf>
        <rdfs:subClassOf>
            <owl:Restriction>
                <owl:onProperty rdf:resource="http://purl.obolibrary.org/obo/BFO_0000051"/>
                <owl:someValuesFrom rdf:resource="http://openenergy-platform.org/ontology/oeo/OEO_00000396"/>
            </owl:Restriction>
        </rdfs:subClassOf>
        <obo:IAO_0000115>A nuclear powerplant is a powerplant having an aggregate of nuclear power units as its power generating units.</obo:IAO_0000115>
        <rdfs:label>nuclear powerplant</rdfs:label>
    </owl:Class>
    


    <!-- http://openenergy-platform.org/ontology/oeo/OEO_00000308 -->

    <owl:Class rdf:about="http://openenergy-platform.org/ontology/oeo/OEO_00000308">
        <rdfs:subClassOf rdf:resource="http://openenergy-platform.org/ontology/oeo/OEO_00000447"/>
        <owl:disjointWith rdf:resource="http://openenergy-platform.org/ontology/oeo/OEO_00000311"/>
        <obo:IAO_0000115 xml:lang="en">An offshore wind farm is a wind farm that is build in a body of water, usually the ocean.</obo:IAO_0000115>
        <rdfs:label>offshore wind farm</rdfs:label>
    </owl:Class>
    


    <!-- http://openenergy-platform.org/ontology/oeo/OEO_00000309 -->

    <owl:Class rdf:about="http://openenergy-platform.org/ontology/oeo/OEO_00000309">
        <rdfs:subClassOf rdf:resource="http://openenergy-platform.org/ontology/oeo/OEO_00000331"/>
        <rdfs:subClassOf>
            <owl:Restriction>
                <owl:onProperty rdf:resource="http://openenergy-platform.org/ontology/oeo/OEO_00000530"/>
                <owl:someValuesFrom rdf:resource="http://openenergy-platform.org/ontology/oeo/OEO_00030002"/>
            </owl:Restriction>
        </rdfs:subClassOf>
        <rdfs:subClassOf>
            <owl:Restriction>
                <owl:onProperty rdf:resource="http://purl.obolibrary.org/obo/RO_0000087"/>
                <owl:someValuesFrom rdf:resource="http://openenergy-platform.org/ontology/oeo/OEO_00000001"/>
            </owl:Restriction>
        </rdfs:subClassOf>
        <rdfs:subClassOf>
            <owl:Restriction>
                <owl:onProperty rdf:resource="http://purl.obolibrary.org/obo/RO_0000091"/>
                <owl:someValuesFrom rdf:resource="http://openenergy-platform.org/ontology/oeo/OEO_00000097"/>
            </owl:Restriction>
        </rdfs:subClassOf>
        <obo:IAO_0000115 xml:lang="en">Petroleum (/pəˈtroʊliəm/) is a naturally occurring, yellowish-black liquid found in geological formations beneath the Earth&apos;s surface. It is commonly refined into various types of fuels. Components of petroleum are separated using a technique called fractional distillation, i.e. separation of a liquid mixture into fractions differing in boiling point by means of distillation, typically using a fractionating column.

It consists of hydrocarbons of various molecular weights and other organic compounds. The name petroleum covers both naturally occurring unprocessed crude oil and petroleum products that are made up of refined crude oil. A fossil fuel, petroleum is formed when large quantities of dead organisms, mostly zooplankton and algae, are buried underneath sedimentary rock and subjected to both intense heat and pressure.</obo:IAO_0000115>
        <obo:IAO_0000119 xml:lang="en">https://en.wikipedia.org/w/index.php?title=Petroleum&amp;oldid=868006507</obo:IAO_0000119>
        <rdfs:label>oil and petroleum products</rdfs:label>
    </owl:Class>
    


    <!-- http://openenergy-platform.org/ontology/oeo/OEO_00000310 -->

    <owl:Class rdf:about="http://openenergy-platform.org/ontology/oeo/OEO_00000310">
        <rdfs:subClassOf rdf:resource="http://openenergy-platform.org/ontology/oeo/OEO_00000031"/>
        <rdfs:subClassOf>
            <owl:Restriction>
                <owl:onProperty rdf:resource="http://purl.obolibrary.org/obo/BFO_0000051"/>
                <owl:someValuesFrom rdf:resource="http://openenergy-platform.org/ontology/oeo/OEO_00000030"/>
            </owl:Restriction>
        </rdfs:subClassOf>
        <rdfs:subClassOf>
            <owl:Restriction>
                <owl:onProperty rdf:resource="http://purl.obolibrary.org/obo/BFO_0000051"/>
                <owl:someValuesFrom rdf:resource="http://openenergy-platform.org/ontology/oeo/OEO_00000396"/>
            </owl:Restriction>
        </rdfs:subClassOf>
        <obo:IAO_0000115>An oil powerplant is a powerplant having an aggregate of oil power units as its power generating units.</obo:IAO_0000115>
        <rdfs:label>oil powerplant</rdfs:label>
    </owl:Class>
    


    <!-- http://openenergy-platform.org/ontology/oeo/OEO_00000311 -->

    <owl:Class rdf:about="http://openenergy-platform.org/ontology/oeo/OEO_00000311">
        <rdfs:subClassOf rdf:resource="http://openenergy-platform.org/ontology/oeo/OEO_00000447"/>
        <obo:IAO_0000115 xml:lang="en">An onshore wind farm is a wind farm that is build on land.</obo:IAO_0000115>
        <rdfs:label>onshore wind farm</rdfs:label>
    </owl:Class>
    


    <!-- http://openenergy-platform.org/ontology/oeo/OEO_00000316 -->

    <owl:Class rdf:about="http://openenergy-platform.org/ontology/oeo/OEO_00000316">
        <rdfs:subClassOf rdf:resource="http://purl.obolibrary.org/obo/BFO_0000019"/>
        <obo:IAO_0000115>The origin is a quality that indicates where something comes from (its source).</obo:IAO_0000115>
        <obo:IAO_0000233>issue: https://github.com/OpenEnergyPlatform/ontology/issues/108
pull request: https://github.com/OpenEnergyPlatform/ontology/pull/130</obo:IAO_0000233>
        <rdfs:label>origin</rdfs:label>
    </owl:Class>
    


    <!-- http://openenergy-platform.org/ontology/oeo/OEO_00000318 -->

    <owl:Class rdf:about="http://openenergy-platform.org/ontology/oeo/OEO_00000318">
        <rdfs:subClassOf rdf:resource="http://openenergy-platform.org/ontology/oeo/OEO_00000331"/>
        <rdfs:subClassOf>
            <owl:Class>
                <owl:unionOf rdf:parseType="Collection">
                    <owl:Restriction>
                        <owl:onProperty rdf:resource="http://openenergy-platform.org/ontology/oeo/OEO_00000529"/>
                        <owl:hasValue rdf:resource="http://openenergy-platform.org/ontology/oeo/OEO_00000256"/>
                    </owl:Restriction>
                    <owl:Restriction>
                        <owl:onProperty rdf:resource="http://openenergy-platform.org/ontology/oeo/OEO_00000529"/>
                        <owl:hasValue rdf:resource="http://openenergy-platform.org/ontology/oeo/OEO_00000390"/>
                    </owl:Restriction>
                </owl:unionOf>
            </owl:Class>
        </rdfs:subClassOf>
        <rdfs:subClassOf>
            <owl:Restriction>
                <owl:onProperty rdf:resource="http://purl.obolibrary.org/obo/RO_0000056"/>
                <owl:someValuesFrom rdf:resource="http://openenergy-platform.org/ontology/oeo/OEO_00000055"/>
            </owl:Restriction>
        </rdfs:subClassOf>
        <obo:IAO_0000115 xml:lang="en">Particulate matter is a portion of matter consisting of small particles. It can act as an air pollutant.</obo:IAO_0000115>
        <obo:IAO_0000118>PM</obo:IAO_0000118>
        <obo:IAO_0000233>issue: https://github.com/OpenEnergyPlatform/ontology/issues/263
pull request: https://github.com/OpenEnergyPlatform/ontology/pull/356</obo:IAO_0000233>
        <rdfs:label>particulate matter</rdfs:label>
    </owl:Class>
    


    <!-- http://openenergy-platform.org/ontology/oeo/OEO_00000320 -->

    <owl:Class rdf:about="http://openenergy-platform.org/ontology/oeo/OEO_00000320">
        <rdfs:subClassOf rdf:resource="http://openenergy-platform.org/ontology/oeo/OEO_00000331"/>
        <rdfs:subClassOf>
            <owl:Restriction>
                <owl:onProperty rdf:resource="http://openenergy-platform.org/ontology/oeo/OEO_00000530"/>
                <owl:someValuesFrom rdf:resource="http://openenergy-platform.org/ontology/oeo/OEO_00030002"/>
            </owl:Restriction>
        </rdfs:subClassOf>
        <rdfs:subClassOf>
            <owl:Restriction>
                <owl:onProperty rdf:resource="http://purl.obolibrary.org/obo/RO_0000087"/>
                <owl:someValuesFrom rdf:resource="http://openenergy-platform.org/ontology/oeo/OEO_00000001"/>
            </owl:Restriction>
        </rdfs:subClassOf>
        <rdfs:subClassOf>
            <owl:Restriction>
                <owl:onProperty rdf:resource="http://purl.obolibrary.org/obo/RO_0000091"/>
                <owl:someValuesFrom rdf:resource="http://openenergy-platform.org/ontology/oeo/OEO_00000097"/>
            </owl:Restriction>
        </rdfs:subClassOf>
        <rdfs:subClassOf>
            <owl:Restriction>
                <owl:onProperty rdf:resource="http://openenergy-platform.org/ontology/oeo/OEO_00000529"/>
                <owl:hasValue rdf:resource="http://openenergy-platform.org/ontology/oeo/OEO_00000390"/>
            </owl:Restriction>
        </rdfs:subClassOf>
        <obo:IAO_0000115 xml:lang="en">Peat is a portion of matter consisting of combustible soft, porous or compressed, sedimentary deposit of plant origin with high water content (up to 90 % in the raw state), easily cut, of light to dark brown colour. Peat used for non-energy purposes is not included.

This definition is without prejudice to the definition of renewable energy sources in Directive 2001/77/EC and to the 2006 IPCC Guidelines for National Greenhouse Gas Inventories.</obo:IAO_0000115>
        <obo:IAO_0000119 xml:lang="en">REGULATION (EC) No 1099/2008 OF THE EUROPEAN PARLIAMENT AND OF THE COUNCIL of 22 October 2008 on energy statistics https://eur-lex.europa.eu/legal-content/EN/TXT/HTML/?uri=CELEX:32008R1099&amp;from=EN</obo:IAO_0000119>
        <rdfs:label>peat</rdfs:label>
    </owl:Class>
    


    <!-- http://openenergy-platform.org/ontology/oeo/OEO_00000322 -->

    <owl:Class rdf:about="http://openenergy-platform.org/ontology/oeo/OEO_00000322">
        <rdfs:subClassOf rdf:resource="http://openenergy-platform.org/ontology/oeo/OEO_00000331"/>
        <rdfs:subClassOf>
            <owl:Restriction>
                <owl:onProperty rdf:resource="http://openenergy-platform.org/ontology/oeo/OEO_00000530"/>
                <owl:someValuesFrom rdf:resource="http://openenergy-platform.org/ontology/oeo/OEO_00030000"/>
            </owl:Restriction>
        </rdfs:subClassOf>
        <obo:IAO_0000115>Perfluorocarbons (PFCs) are portions of matter consisting of organic compounds that contain fluorine atoms but no hydrogen atoms.</obo:IAO_0000115>
        <obo:IAO_0000118>PFC</obo:IAO_0000118>
        <rdfs:label>perfluorocarbon</rdfs:label>
    </owl:Class>
    


    <!-- http://openenergy-platform.org/ontology/oeo/OEO_00000324 -->

    <owl:Class rdf:about="http://openenergy-platform.org/ontology/oeo/OEO_00000324">
        <rdfs:subClassOf rdf:resource="http://openenergy-platform.org/ontology/oeo/OEO_00000386"/>
        <rdfs:subClassOf>
            <owl:Restriction>
                <owl:onProperty rdf:resource="http://purl.obolibrary.org/obo/BFO_0000051"/>
                <owl:someValuesFrom rdf:resource="http://openenergy-platform.org/ontology/oeo/OEO_00000348"/>
            </owl:Restriction>
        </rdfs:subClassOf>
        <obo:IAO_0000115 xml:lang="en">A photovoltaic powerplant is a powerplant having an aggregate of PV panels as its power generating units.</obo:IAO_0000115>
        <rdfs:label>photovoltaic powerplant</rdfs:label>
    </owl:Class>
    


    <!-- http://openenergy-platform.org/ontology/oeo/OEO_00000330 -->

    <owl:Class rdf:about="http://openenergy-platform.org/ontology/oeo/OEO_00000330">
        <rdfs:subClassOf rdf:resource="http://openenergy-platform.org/ontology/oeo/OEO_00000147"/>
        <obo:IAO_0000115 xml:lang="en">Pollution is an emission with a negative effect on the environment or organisms.</obo:IAO_0000115>
        <obo:IAO_0000233>issue: https://github.com/OpenEnergyPlatform/ontology/issues/56
pull request: https://github.com/OpenEnergyPlatform/ontology/pull/234</obo:IAO_0000233>
        <rdfs:label>pollution</rdfs:label>
    </owl:Class>
    


    <!-- http://openenergy-platform.org/ontology/oeo/OEO_00000331 -->

    <owl:Class rdf:about="http://openenergy-platform.org/ontology/oeo/OEO_00000331">
        <rdfs:subClassOf rdf:resource="http://purl.obolibrary.org/obo/BFO_0000027"/>
        <obo:IAO_0000115 xml:lang="en">A portion of matter is a part of a material entity that has a state_of_matter property.</obo:IAO_0000115>
        <obo:IAO_0000233>issue: https://github.com/OpenEnergyPlatform/ontology/issues/227
pull request: https://github.com/OpenEnergyPlatform/ontology/pull/279</obo:IAO_0000233>
        <rdfs:comment>wiki page: https://github.com/OpenEnergyPlatform/ontology/wiki/Explanation-on-mass-nouns</rdfs:comment>
        <rdfs:label>portion of matter</rdfs:label>
    </owl:Class>
    


    <!-- http://openenergy-platform.org/ontology/oeo/OEO_00000332 -->

    <owl:Class rdf:about="http://openenergy-platform.org/ontology/oeo/OEO_00000332">
        <owl:equivalentClass>
            <owl:Class>
                <owl:intersectionOf rdf:parseType="Collection">
                    <rdf:Description rdf:about="http://openenergy-platform.org/ontology/oeo/OEO_00000072"/>
                    <owl:Restriction>
                        <owl:onProperty rdf:resource="http://openenergy-platform.org/ontology/oeo/OEO_00000529"/>
                        <owl:hasValue rdf:resource="http://openenergy-platform.org/ontology/oeo/OEO_00000390"/>
                    </owl:Restriction>
                </owl:intersectionOf>
            </owl:Class>
        </owl:equivalentClass>
        <rdfs:subClassOf>
            <owl:Restriction>
                <owl:onProperty rdf:resource="http://openenergy-platform.org/ontology/oeo/OEO_00000530"/>
                <owl:someValuesFrom rdf:resource="http://openenergy-platform.org/ontology/oeo/OEO_00030001"/>
            </owl:Restriction>
        </rdfs:subClassOf>
        <rdfs:subClassOf>
            <owl:Restriction>
                <owl:onProperty rdf:resource="http://openenergy-platform.org/ontology/oeo/OEO_00000530"/>
                <owl:someValuesFrom rdf:resource="http://openenergy-platform.org/ontology/oeo/OEO_00030004"/>
            </owl:Restriction>
        </rdfs:subClassOf>
        <rdfs:subClassOf>
            <owl:Restriction>
                <owl:onProperty rdf:resource="http://purl.obolibrary.org/obo/RO_0000087"/>
                <owl:someValuesFrom rdf:resource="http://openenergy-platform.org/ontology/oeo/OEO_00000001"/>
            </owl:Restriction>
        </rdfs:subClassOf>
        <rdfs:subClassOf>
            <owl:Restriction>
                <owl:onProperty rdf:resource="http://purl.obolibrary.org/obo/RO_0000091"/>
                <owl:someValuesFrom rdf:resource="http://openenergy-platform.org/ontology/oeo/OEO_00000097"/>
            </owl:Restriction>
        </rdfs:subClassOf>
        <rdfs:subClassOf>
            <owl:Restriction>
                <owl:onProperty rdf:resource="http://openenergy-platform.org/ontology/oeo/OEO_00000529"/>
                <owl:hasValue rdf:resource="http://openenergy-platform.org/ontology/oeo/OEO_00000390"/>
            </owl:Restriction>
        </rdfs:subClassOf>
        <obo:IAO_0000115>Solid biomass is a portion of matter consisting of organic, non-fossil material of biological origin which may be used as fuel for heat production or electricity generation.</obo:IAO_0000115>
        <obo:IAO_0000118>portion of solid biomass</obo:IAO_0000118>
        <obo:IAO_0000118 xml:lang="en">solid biomass</obo:IAO_0000118>
        <obo:IAO_0000119>https://eur-lex.europa.eu/legal-content/EN/TXT/HTML/?uri=CELEX:32008R1099&amp;from=EN</obo:IAO_0000119>
        <rdfs:label xml:lang="en">solid biofuel</rdfs:label>
    </owl:Class>
    


    <!-- http://openenergy-platform.org/ontology/oeo/OEO_00000333 -->

    <owl:Class rdf:about="http://openenergy-platform.org/ontology/oeo/OEO_00000333">
        <rdfs:subClassOf rdf:resource="http://openenergy-platform.org/ontology/oeo/OEO_00030019"/>
        <rdfs:subClassOf>
            <owl:Restriction>
                <owl:onProperty rdf:resource="http://openenergy-platform.org/ontology/oeo/OEO_00000502"/>
                <owl:someValuesFrom rdf:resource="http://openenergy-platform.org/ontology/oeo/OEO_00020003"/>
            </owl:Restriction>
        </rdfs:subClassOf>
        <obo:IAO_0000115 xml:lang="en">Power is the process attribute that is the amount of energy transformed or transferred per time unit.</obo:IAO_0000115>
        <obo:IAO_0000233>classification:
issue: https://github.com/OpenEnergyPlatform/ontology/issues/205
pull request: https://github.com/OpenEnergyPlatform/ontology/pull/386

definition:
issue: https://github.com/OpenEnergyPlatform/ontology/issues/79
pull request: https://github.com/OpenEnergyPlatform/ontology/pull/369</obo:IAO_0000233>
        <rdfs:comment>Power is the derivative of energy transformation over time</rdfs:comment>
        <rdfs:label>power</rdfs:label>
    </owl:Class>
    


    <!-- http://openenergy-platform.org/ontology/oeo/OEO_00000334 -->

    <owl:Class rdf:about="http://openenergy-platform.org/ontology/oeo/OEO_00000334">
        <rdfs:subClassOf rdf:resource="http://openenergy-platform.org/ontology/oeo/OEO_00000061"/>
        <rdfs:subClassOf>
            <owl:Restriction>
                <owl:onProperty rdf:resource="http://purl.obolibrary.org/obo/BFO_0000051"/>
                <owl:someValuesFrom rdf:resource="http://openenergy-platform.org/ontology/oeo/OEO_00000188"/>
            </owl:Restriction>
        </rdfs:subClassOf>
        <rdfs:subClassOf>
            <owl:Restriction>
                <owl:onProperty rdf:resource="http://purl.obolibrary.org/obo/RO_0000056"/>
                <owl:someValuesFrom rdf:resource="http://openenergy-platform.org/ontology/oeo/OEO_00020003"/>
            </owl:Restriction>
        </rdfs:subClassOf>
        <obo:IAO_0000115>A power generating unit is an artificial object that contains a generator, among other parts.</obo:IAO_0000115>
        <obo:IAO_0000233>issue: https://github.com/OpenEnergyPlatform/ontology/issues/173
pull request: https://github.com/OpenEnergyPlatform/ontology/pull/273

issue: https://github.com/OpenEnergyPlatform/ontology/issues/372
pull request: https://github.com/OpenEnergyPlatform/ontology/pull/646</obo:IAO_0000233>
        <rdfs:label>power generating unit</rdfs:label>
    </owl:Class>
    


    <!-- http://openenergy-platform.org/ontology/oeo/OEO_00000335 -->

    <owl:Class rdf:about="http://openenergy-platform.org/ontology/oeo/OEO_00000335">
        <rdfs:subClassOf rdf:resource="http://openenergy-platform.org/ontology/oeo/OEO_00000159"/>
        <obo:IAO_0000115 xml:lang="en">a power-to-gas (often abbreviated P2G) system is an energy storage object that converts electrical power to a gas fuel. When using surplus power from wind generation, the concept is sometimes called windgas. There are currently three methods in use; all use electricity to split water into hydrogen and oxygen by means of electrolysis.</obo:IAO_0000115>
        <obo:IAO_0000118>P2G</obo:IAO_0000118>
        <obo:IAO_0000118>PtG</obo:IAO_0000118>
        <obo:IAO_0000119 xml:lang="en">https://en.wikipedia.org/w/index.php?title=Power-to-gas&amp;oldid=907220452</obo:IAO_0000119>
        <rdfs:label>power-to-gas system</rdfs:label>
    </owl:Class>
    


    <!-- http://openenergy-platform.org/ontology/oeo/OEO_00000343 -->

    <owl:Class rdf:about="http://openenergy-platform.org/ontology/oeo/OEO_00000343">
        <rdfs:subClassOf rdf:resource="http://openenergy-platform.org/ontology/oeo/OEO_00000012"/>
        <obo:IAO_0000115 xml:lang="en">A pumped storage (pumped-storage hdyroelectricity) is an energy storage that uses water from a higher reservoir to generate energy.</obo:IAO_0000115>
        <rdfs:label>pumped storage</rdfs:label>
    </owl:Class>
    


    <!-- http://openenergy-platform.org/ontology/oeo/OEO_00000345 -->

    <owl:Class rdf:about="http://openenergy-platform.org/ontology/oeo/OEO_00000345">
        <rdfs:subClassOf rdf:resource="http://openenergy-platform.org/ontology/oeo/OEO_00000441"/>
        <rdfs:subClassOf>
            <owl:Restriction>
                <owl:onProperty rdf:resource="http://openenergy-platform.org/ontology/oeo/OEO_00000501"/>
                <owl:someValuesFrom rdf:resource="http://openenergy-platform.org/ontology/oeo/OEO_00000399"/>
            </owl:Restriction>
        </rdfs:subClassOf>
        <obo:IAO_0000115 xml:lang="en">Pumped water is water which was pumped into an upper reservoir and thus contains potential energy.</obo:IAO_0000115>
        <rdfs:label>pumped water</rdfs:label>
    </owl:Class>
    


    <!-- http://openenergy-platform.org/ontology/oeo/OEO_00000348 -->

    <owl:Class rdf:about="http://openenergy-platform.org/ontology/oeo/OEO_00000348">
        <rdfs:subClassOf rdf:resource="http://openenergy-platform.org/ontology/oeo/OEO_00000034"/>
        <rdfs:subClassOf>
            <owl:Restriction>
                <owl:onProperty rdf:resource="http://openenergy-platform.org/ontology/oeo/OEO_00000533"/>
                <owl:someValuesFrom rdf:resource="http://openenergy-platform.org/ontology/oeo/OEO_00000333"/>
            </owl:Restriction>
        </rdfs:subClassOf>
        <rdfs:subClassOf>
            <owl:Restriction>
                <owl:onProperty rdf:resource="http://purl.obolibrary.org/obo/BFO_0000051"/>
                <owl:someValuesFrom rdf:resource="http://openenergy-platform.org/ontology/oeo/OEO_00000032"/>
            </owl:Restriction>
        </rdfs:subClassOf>
        <obo:IAO_0000115 xml:lang="en">A PV panel (photovoltaic panel) is a solar power unit absorbing sunlight as a source of energy to generate electricity.</obo:IAO_0000115>
        <rdfs:comment>A photovoltaic (PV) module is a packaged, connected assembly of typically 6x10 photovoltaic solar cells. Photovoltaic modules constitute the photovoltaic array of a photovoltaic system that generates and supplies solar electricity in commercial and residential applications.</rdfs:comment>
        <rdfs:label>PV panel</rdfs:label>
    </owl:Class>
    


    <!-- http://openenergy-platform.org/ontology/oeo/OEO_00000350 -->

    <owl:Class rdf:about="http://openenergy-platform.org/ontology/oeo/OEO_00000350"/>
    


    <!-- http://openenergy-platform.org/ontology/oeo/OEO_00000356 -->

    <owl:Class rdf:about="http://openenergy-platform.org/ontology/oeo/OEO_00000356">
        <rdfs:subClassOf rdf:resource="http://openenergy-platform.org/ontology/oeo/OEO_00000290"/>
        <rdfs:subClassOf>
            <owl:Restriction>
                <owl:onProperty rdf:resource="http://openenergy-platform.org/ontology/oeo/OEO_00000530"/>
                <owl:someValuesFrom rdf:resource="http://openenergy-platform.org/ontology/oeo/OEO_00030001"/>
            </owl:Restriction>
        </rdfs:subClassOf>
        <rdfs:subClassOf>
            <owl:Restriction>
                <owl:onProperty rdf:resource="http://openenergy-platform.org/ontology/oeo/OEO_00000530"/>
                <owl:someValuesFrom rdf:resource="http://openenergy-platform.org/ontology/oeo/OEO_00030004"/>
            </owl:Restriction>
        </rdfs:subClassOf>
        <obo:IAO_0000115 xml:lang="en">Renewable municipal waste fuel is municipal waste fuel of biological origin.</obo:IAO_0000115>
        <obo:IAO_0000119 xml:lang="en">REGULATION (EC) No 1099/2008 OF THE EUROPEAN PARLIAMENT AND OF THE COUNCIL of 22 October 2008 on energy statistics https://eur-lex.europa.eu/legal-content/EN/TXT/HTML/?uri=CELEX:32008R1099&amp;from=EN</obo:IAO_0000119>
        <rdfs:label>renewable municipal waste fuel</rdfs:label>
    </owl:Class>
    


    <!-- http://openenergy-platform.org/ontology/oeo/OEO_00000361 -->

    <owl:Class rdf:about="http://openenergy-platform.org/ontology/oeo/OEO_00000361">
        <rdfs:subClassOf rdf:resource="http://openenergy-platform.org/ontology/oeo/OEO_00000324"/>
        <obo:IAO_0000115 xml:lang="en">A rooftop photovoltaic powerplant is a photovoltaic powerplant that is installed on top of the roof of a building.</obo:IAO_0000115>
        <rdfs:label>rooftop photovoltaic powerplant</rdfs:label>
    </owl:Class>
    


    <!-- http://openenergy-platform.org/ontology/oeo/OEO_00000374 -->

    <owl:Class rdf:about="http://openenergy-platform.org/ontology/oeo/OEO_00000374">
        <rdfs:subClassOf rdf:resource="http://openenergy-platform.org/ontology/oeo/OEO_00000159"/>
        <obo:IAO_0000115 xml:lang="en">Superconducting magnetic energy storage (SMES) systems store energy in the magnetic field created by the flow of direct current in a superconducting coil which has been cryogenically cooled to a temperature below its superconducting critical temperature.
          A typical smes system includes three parts: superconducting coil, power conditioning system and cryogenically cooled refrigerator. Once the superconducting coil is charged, the current will not decay and the magnetic energy can be stored indefinitely.</obo:IAO_0000115>
        <obo:IAO_0000119>https://en.wikipedia.org/w/index.php?title=Superconducting_magnetic_energy_storage&amp;oldid=902190687</obo:IAO_0000119>
        <rdfs:label>SMES</rdfs:label>
    </owl:Class>
    


    <!-- http://openenergy-platform.org/ontology/oeo/OEO_00000376 -->

    <owl:Class rdf:about="http://openenergy-platform.org/ontology/oeo/OEO_00000376">
        <rdfs:subClassOf rdf:resource="http://openenergy-platform.org/ontology/oeo/OEO_00000068"/>
        <obo:IAO_0000115 xml:lang="en">Sodium-ion batteries (SIB) are a type of rechargeable metal-ion battery that uses sodium ions as charge carriers.</obo:IAO_0000115>
        <obo:IAO_0000119 xml:lang="en">https://en.wikipedia.org/w/index.php?title=Sodium-ion_battery&amp;oldid=906459441</obo:IAO_0000119>
        <rdfs:label>sodium-ion battery</rdfs:label>
    </owl:Class>
    


    <!-- http://openenergy-platform.org/ontology/oeo/OEO_00000377 -->

    <owl:Class rdf:about="http://openenergy-platform.org/ontology/oeo/OEO_00000377">
        <rdfs:subClassOf rdf:resource="http://openenergy-platform.org/ontology/oeo/OEO_00000283"/>
        <obo:IAO_0000115 xml:lang="en">A sodium–sulfur battery is a type of molten-salt battery constructed from liquid sodium (Na) and sulfur (S).This type of battery has a high energy density, high efficiency of charge/discharge and long cycle life, and is fabricated from inexpensive materials. The operating temperatures of 300 to 350 °C and the highly corrosive nature of the sodium polysulfides, primarily make them suitable for stationary energy storage applications. The cell becomes more economical with increasing size.</obo:IAO_0000115>
        <obo:IAO_0000119 xml:lang="en">https://en.wikipedia.org/w/index.php?title=Sodium%E2%80%93sulfur_battery&amp;oldid=900392594</obo:IAO_0000119>
        <rdfs:label>sodium-sulfur battery</rdfs:label>
    </owl:Class>
    


    <!-- http://openenergy-platform.org/ontology/oeo/OEO_00000384 -->

    <owl:Class rdf:about="http://openenergy-platform.org/ontology/oeo/OEO_00000384">
        <rdfs:subClassOf rdf:resource="http://openenergy-platform.org/ontology/oeo/OEO_00020040"/>
        <obo:IAO_0000115 xml:lang="en">Solar energy is radiative energy of the sun.</obo:IAO_0000115>
        <obo:IAO_0000233>issue: https://github.com/OpenEnergyPlatform/ontology/issues/211
pull request: https://github.com/OpenEnergyPlatform/ontology/pull/225
restructure solar energy
issue: https://github.com/OpenEnergyPlatform/ontology/issues/663
pull request: https://github.com/OpenEnergyPlatform/ontology/pull/672
remove disposition renewable fuel
issue: https://github.com/OpenEnergyPlatform/ontology/issues/726
pull request: https://github.com/OpenEnergyPlatform/ontology/pull/732</obo:IAO_0000233>
        <rdfs:label>solar energy</rdfs:label>
    </owl:Class>
    


    <!-- http://openenergy-platform.org/ontology/oeo/OEO_00000386 -->

    <owl:Class rdf:about="http://openenergy-platform.org/ontology/oeo/OEO_00000386">
        <rdfs:subClassOf rdf:resource="http://openenergy-platform.org/ontology/oeo/OEO_00000031"/>
        <rdfs:subClassOf>
            <owl:Restriction>
                <owl:onProperty rdf:resource="http://purl.obolibrary.org/obo/BFO_0000051"/>
                <owl:someValuesFrom rdf:resource="http://openenergy-platform.org/ontology/oeo/OEO_00000348"/>
            </owl:Restriction>
        </rdfs:subClassOf>
        <obo:IAO_0000115 xml:lang="en">A solar powerplant is a powerplant having an aggregate of solar power units as its power generating units.</obo:IAO_0000115>
        <rdfs:label>solar power plant</rdfs:label>
    </owl:Class>
    


    <!-- http://openenergy-platform.org/ontology/oeo/OEO_00000387 -->

    <owl:Class rdf:about="http://openenergy-platform.org/ontology/oeo/OEO_00000387">
        <rdfs:subClassOf rdf:resource="http://openenergy-platform.org/ontology/oeo/OEO_00000210"/>
        <rdfs:subClassOf>
            <owl:Restriction>
                <owl:onProperty rdf:resource="http://openenergy-platform.org/ontology/oeo/OEO_00000532"/>
                <owl:allValuesFrom rdf:resource="http://openenergy-platform.org/ontology/oeo/OEO_00000388"/>
            </owl:Restriction>
        </rdfs:subClassOf>
        <obo:IAO_0000115 xml:lang="en">A solar thermal collector is a heater that absorbs solar radiation to convert it into heat.</obo:IAO_0000115>
        <obo:IAO_0000119 xml:lang="en">https://en.wikipedia.org/w/index.php?title=Solar_thermal_collector&amp;oldid=903948846</obo:IAO_0000119>
        <rdfs:label>solar thermal collector</rdfs:label>
    </owl:Class>
    


    <!-- http://openenergy-platform.org/ontology/oeo/OEO_00000388 -->

    <owl:Class rdf:about="http://openenergy-platform.org/ontology/oeo/OEO_00000388">
        <rdfs:subClassOf rdf:resource="http://openenergy-platform.org/ontology/oeo/OEO_00000207"/>
        <obo:IAO_0000115 xml:lang="en">Heat from solar radiation; can consist of:
(a) solar thermal-electric plants; or
(b) equipment for the production of domestic hot water or for the seasonal heating of swimming pools (e.g. flat plate collectors, mainly of the thermosyphon type).</obo:IAO_0000115>
        <obo:IAO_0000119 xml:lang="en">REGULATION (EC) No 1099/2008 OF THE EUROPEAN PARLIAMENT AND OF THE COUNCIL of 22 October 2008 on energy statistics https://eur-lex.europa.eu/legal-content/EN/TXT/HTML/?uri=CELEX:32008R1099&amp;from=EN</obo:IAO_0000119>
        <rdfs:label>solar thermal heat</rdfs:label>
    </owl:Class>
    


    <!-- http://openenergy-platform.org/ontology/oeo/OEO_00000389 -->

    <owl:Class rdf:about="http://openenergy-platform.org/ontology/oeo/OEO_00000389">
        <rdfs:subClassOf rdf:resource="http://openenergy-platform.org/ontology/oeo/OEO_00000386"/>
        <rdfs:subClassOf>
            <owl:Restriction>
                <owl:onProperty rdf:resource="http://purl.obolibrary.org/obo/BFO_0000051"/>
                <owl:someValuesFrom rdf:resource="http://openenergy-platform.org/ontology/oeo/OEO_00000035"/>
            </owl:Restriction>
        </rdfs:subClassOf>
        <rdfs:subClassOf>
            <owl:Restriction>
                <owl:onProperty rdf:resource="http://purl.obolibrary.org/obo/BFO_0000051"/>
                <owl:someValuesFrom rdf:resource="http://openenergy-platform.org/ontology/oeo/OEO_00000396"/>
            </owl:Restriction>
        </rdfs:subClassOf>
        <obo:IAO_0000115 xml:lang="en">A solar thermal powerplant is a powerplant consisting of solar thermal power units.</obo:IAO_0000115>
        <rdfs:label>solar thermal powerplant</rdfs:label>
    </owl:Class>
    


    <!-- http://openenergy-platform.org/ontology/oeo/OEO_00000391 -->

    <owl:Class rdf:about="http://openenergy-platform.org/ontology/oeo/OEO_00000391">
        <owl:equivalentClass>
            <owl:Class>
                <owl:intersectionOf rdf:parseType="Collection">
                    <owl:Restriction>
                        <owl:onProperty rdf:resource="http://openenergy-platform.org/ontology/oeo/OEO_00000530"/>
                        <owl:someValuesFrom rdf:resource="http://openenergy-platform.org/ontology/oeo/OEO_00030002"/>
                    </owl:Restriction>
                    <owl:Restriction>
                        <owl:onProperty rdf:resource="http://purl.obolibrary.org/obo/RO_0000091"/>
                        <owl:someValuesFrom rdf:resource="http://openenergy-platform.org/ontology/oeo/OEO_00000097"/>
                    </owl:Restriction>
                    <owl:Restriction>
                        <owl:onProperty rdf:resource="http://openenergy-platform.org/ontology/oeo/OEO_00000529"/>
                        <owl:hasValue rdf:resource="http://openenergy-platform.org/ontology/oeo/OEO_00000390"/>
                    </owl:Restriction>
                </owl:intersectionOf>
            </owl:Class>
        </owl:equivalentClass>
        <rdfs:subClassOf rdf:resource="http://openenergy-platform.org/ontology/oeo/OEO_00000173"/>
        <rdfs:subClassOf>
            <owl:Restriction>
                <owl:onProperty rdf:resource="http://openenergy-platform.org/ontology/oeo/OEO_00000530"/>
                <owl:someValuesFrom rdf:resource="http://openenergy-platform.org/ontology/oeo/OEO_00030002"/>
            </owl:Restriction>
        </rdfs:subClassOf>
        <rdfs:subClassOf>
            <owl:Restriction>
                <owl:onProperty rdf:resource="http://openenergy-platform.org/ontology/oeo/OEO_00000529"/>
                <owl:hasValue rdf:resource="http://openenergy-platform.org/ontology/oeo/OEO_00000390"/>
            </owl:Restriction>
        </rdfs:subClassOf>
        <obo:IAO_0000115>Solid fossil fuels are fuels of fossil origin and that have a solid state of matter under normal conditions.</obo:IAO_0000115>
        <obo:IAO_0000233>issue: https://github.com/OpenEnergyPlatform/ontology/issues/106
pull request: https://github.com/OpenEnergyPlatform/ontology/pull/164</obo:IAO_0000233>
        <rdfs:label>solid fossil fuel</rdfs:label>
    </owl:Class>
    


    <!-- http://openenergy-platform.org/ontology/oeo/OEO_00000395 -->

    <owl:Class rdf:about="http://openenergy-platform.org/ontology/oeo/OEO_00000395">
        <rdfs:subClassOf rdf:resource="http://purl.obolibrary.org/obo/BFO_0000019"/>
        <obo:IAO_0000115>In physics, a state of matter is one of the distinct forms in which matter can exist. Four states of matter are observable in everyday life: solid, liquid, gas, and plasma. Many intermediate states are known to exist, such as liquid crystal, and some states only exist under extreme conditions</obo:IAO_0000115>
        <obo:IAO_0000119>https://en.wikipedia.org/w/index.php?title=State_of_matter&amp;oldid=903680856</obo:IAO_0000119>
        <obo:IAO_0000233>issue: https://github.com/OpenEnergyPlatform/ontology/issues/38
pull request: https://github.com/OpenEnergyPlatform/ontology/pull/39</obo:IAO_0000233>
        <rdfs:label>state of matter</rdfs:label>
    </owl:Class>
    


    <!-- http://openenergy-platform.org/ontology/oeo/OEO_00000396 -->

    <owl:Class rdf:about="http://openenergy-platform.org/ontology/oeo/OEO_00000396">
        <rdfs:subClassOf rdf:resource="http://openenergy-platform.org/ontology/oeo/OEO_00000425"/>
        <rdfs:subClassOf>
            <owl:Restriction>
                <owl:onProperty rdf:resource="http://openenergy-platform.org/ontology/oeo/OEO_00000533"/>
                <owl:someValuesFrom rdf:resource="http://openenergy-platform.org/ontology/oeo/OEO_00000333"/>
            </owl:Restriction>
        </rdfs:subClassOf>
        <obo:IAO_0000115>A steam turbine is a turbine that converts heat from pressurized steam into rotational energy.</obo:IAO_0000115>
        <rdfs:label>steam turbine</rdfs:label>
    </owl:Class>
    


    <!-- http://openenergy-platform.org/ontology/oeo/OEO_00000399 -->

    <owl:Class rdf:about="http://openenergy-platform.org/ontology/oeo/OEO_00000399">
        <rdfs:subClassOf rdf:resource="http://openenergy-platform.org/ontology/oeo/OEO_00020006"/>
        <rdfs:subClassOf>
            <owl:Restriction>
                <owl:onProperty rdf:resource="http://purl.obolibrary.org/obo/BFO_0000050"/>
                <owl:someValuesFrom rdf:resource="http://openenergy-platform.org/ontology/oeo/OEO_00000200"/>
            </owl:Restriction>
        </rdfs:subClassOf>
        <obo:IAO_0000115 xml:lang="en">A storage unit is a grid component that stores energy.</obo:IAO_0000115>
        <rdfs:label>storage unit</rdfs:label>
    </owl:Class>
    


    <!-- http://openenergy-platform.org/ontology/oeo/OEO_00000401 -->

    <owl:Class rdf:about="http://openenergy-platform.org/ontology/oeo/OEO_00000401">
        <rdfs:subClassOf rdf:resource="http://openenergy-platform.org/ontology/oeo/OEO_00000088"/>
        <obo:IAO_0000115 xml:lang="en">Sub bituminous coal is coal that is non-agglomerating with a gross calorific value between 17 435 kJ/kg (4 165 kcal/kg) and 23 865 kJ/kg (5 700 kcal/kg) containing more than 31 % volatile matter on a dry mineral matter free basis.</obo:IAO_0000115>
        <obo:IAO_0000119 xml:lang="en">REGULATION (EC) No 1099/2008 OF THE EUROPEAN PARLIAMENT AND OF THE COUNCIL of 22 October 2008 on energy statistics https://eur-lex.europa.eu/legal-content/EN/TXT/HTML/?uri=CELEX:32008R1099&amp;from=EN</obo:IAO_0000119>
        <rdfs:label>sub bituminous coal</rdfs:label>
    </owl:Class>
    


    <!-- http://openenergy-platform.org/ontology/oeo/OEO_00000407 -->

    <owl:Class rdf:about="http://openenergy-platform.org/ontology/oeo/OEO_00000407">
        <rdfs:subClassOf rdf:resource="http://purl.obolibrary.org/obo/IAO_0000030"/>
        <obo:IAO_0000115 xml:lang="en">A Technology is an information content entity that specifies how to create an artificial object.</obo:IAO_0000115>
        <obo:IAO_0000233>issue: https://github.com/OpenEnergyPlatform/ontology/issues/136
pull request: https://github.com/OpenEnergyPlatform/ontology/pull/334</obo:IAO_0000233>
        <rdfs:label>technology</rdfs:label>
    </owl:Class>
    


    <!-- http://openenergy-platform.org/ontology/oeo/OEO_00000419 -->

    <owl:Class rdf:about="http://openenergy-platform.org/ontology/oeo/OEO_00000419"/>
    


    <!-- http://openenergy-platform.org/ontology/oeo/OEO_00000420 -->

    <owl:Class rdf:about="http://openenergy-platform.org/ontology/oeo/OEO_00000420">
        <rdfs:subClassOf rdf:resource="http://openenergy-platform.org/ontology/oeo/OEO_00020006"/>
        <rdfs:subClassOf>
            <owl:Restriction>
                <owl:onProperty rdf:resource="http://purl.obolibrary.org/obo/BFO_0000050"/>
                <owl:someValuesFrom rdf:resource="http://openenergy-platform.org/ontology/oeo/OEO_00000143"/>
            </owl:Restriction>
        </rdfs:subClassOf>
        <obo:IAO_0000115 xml:lang="en">A transformer is an electricity grid component that passively transfers electrical energy from one electrical circuit to another.</obo:IAO_0000115>
        <obo:IAO_0000233 xml:lang="en">issue: https://github.com/OpenEnergyPlatform/ontology/issues/231
pull request: https://github.com/OpenEnergyPlatform/ontology/pull/385</obo:IAO_0000233>
        <rdfs:comment xml:lang="en">Source: https://en.wikipedia.org/wiki/Transformer</rdfs:comment>
        <rdfs:label>transformer</rdfs:label>
    </owl:Class>
    


    <!-- http://openenergy-platform.org/ontology/oeo/OEO_00000425 -->

    <owl:Class rdf:about="http://openenergy-platform.org/ontology/oeo/OEO_00000425">
        <rdfs:subClassOf rdf:resource="http://openenergy-platform.org/ontology/oeo/OEO_00000011"/>
        <obo:IAO_0000115 xml:lang="en">A turbine is an energy converting device that converts energy from a moving fluid flow into rotational energy.</obo:IAO_0000115>
        <rdfs:label>turbine</rdfs:label>
    </owl:Class>
    


    <!-- http://openenergy-platform.org/ontology/oeo/OEO_00000429 -->

    <owl:Class rdf:about="http://openenergy-platform.org/ontology/oeo/OEO_00000429">
        <rdfs:subClassOf rdf:resource="http://openenergy-platform.org/ontology/oeo/OEO_00000159"/>
        <rdfs:subClassOf>
            <owl:Restriction>
                <owl:onProperty rdf:resource="http://openenergy-platform.org/ontology/oeo/OEO_00000503"/>
                <owl:someValuesFrom rdf:resource="http://openenergy-platform.org/ontology/oeo/OEO_00000220"/>
            </owl:Restriction>
        </rdfs:subClassOf>
        <obo:IAO_0000115 xml:lang="en">An underground hydrogen storage is an energy storage object that stores hydrogen underground. Examples are underground caverns, salt domes and depleted oil/gas fields.</obo:IAO_0000115>
        <obo:IAO_0000119>https://en.wikipedia.org/w/index.php?title=Underground_hydrogen_storage&amp;oldid=895350780</obo:IAO_0000119>
        <obo:IAO_0000233>Issue:https://github.com/OpenEnergyPlatform/ontology/issues/448
Pull request: https://github.com/OpenEnergyPlatform/ontology/pull/462</obo:IAO_0000233>
        <rdfs:label>underground hydrogen storage</rdfs:label>
    </owl:Class>
    


    <!-- http://openenergy-platform.org/ontology/oeo/OEO_00000437 -->

    <owl:Class rdf:about="http://openenergy-platform.org/ontology/oeo/OEO_00000437">
        <owl:equivalentClass>
            <owl:Class>
                <owl:unionOf rdf:parseType="Collection">
                    <rdf:Description rdf:about="http://openenergy-platform.org/ontology/oeo/OEO_00000025"/>
                    <rdf:Description rdf:about="http://openenergy-platform.org/ontology/oeo/OEO_00000298"/>
                </owl:unionOf>
            </owl:Class>
        </owl:equivalentClass>
        <rdfs:subClassOf>
            <owl:Class>
                <owl:intersectionOf rdf:parseType="Collection">
                    <rdf:Description rdf:about="http://openenergy-platform.org/ontology/oeo/OEO_00000331"/>
                    <owl:Restriction>
                        <owl:onProperty rdf:resource="http://purl.obolibrary.org/obo/RO_0000091"/>
                        <owl:someValuesFrom rdf:resource="http://openenergy-platform.org/ontology/oeo/OEO_00010011"/>
                    </owl:Restriction>
                </owl:intersectionOf>
            </owl:Class>
        </rdfs:subClassOf>
        <rdfs:subClassOf>
            <owl:Restriction>
                <owl:onProperty rdf:resource="http://purl.obolibrary.org/obo/RO_0000056"/>
                <owl:someValuesFrom rdf:resource="http://openenergy-platform.org/ontology/oeo/OEO_00000055"/>
            </owl:Restriction>
        </rdfs:subClassOf>
        <obo:IAO_0000115 xml:lang="en">A volatile organic compound (VOC) is a portion of matter consisting of organic compounds that is capable of producing photochemical oxidants by reactions with nitrogen oxides in the presence of sunlight. Hence it can act as an air pollutant.</obo:IAO_0000115>
        <obo:IAO_0000118>VOC</obo:IAO_0000118>
        <obo:IAO_0000119>This definition is partly based on Article 2 of the European Air Quality Directive (2008/50/EC): https://eur-lex.europa.eu/legal-content/EN/TXT/?uri=CELEX:32008L0050</obo:IAO_0000119>
        <obo:IAO_0000233>issue: https://github.com/OpenEnergyPlatform/ontology/issues/263
pull request: https://github.com/OpenEnergyPlatform/ontology/pull/356</obo:IAO_0000233>
        <rdfs:label>volatile organic compound</rdfs:label>
    </owl:Class>
    


    <!-- http://openenergy-platform.org/ontology/oeo/OEO_00000439 -->

    <owl:Class rdf:about="http://openenergy-platform.org/ontology/oeo/OEO_00000439">
        <owl:equivalentClass>
            <owl:Class>
                <owl:intersectionOf rdf:parseType="Collection">
                    <rdf:Description rdf:about="http://openenergy-platform.org/ontology/oeo/OEO_00000173"/>
                    <owl:Restriction>
                        <owl:onProperty rdf:resource="http://purl.obolibrary.org/obo/RO_0000087"/>
                        <owl:someValuesFrom rdf:resource="http://openenergy-platform.org/ontology/oeo/OEO_00000042"/>
                    </owl:Restriction>
                </owl:intersectionOf>
            </owl:Class>
        </owl:equivalentClass>
        <rdfs:subClassOf>
            <owl:Restriction>
                <owl:onProperty rdf:resource="http://purl.obolibrary.org/obo/RO_0000091"/>
                <owl:someValuesFrom rdf:resource="http://openenergy-platform.org/ontology/oeo/OEO_00000097"/>
            </owl:Restriction>
        </rdfs:subClassOf>
        <obo:IAO_0000115 xml:lang="en">A waste fuel is a fuel in which the material entity is waste.</obo:IAO_0000115>
        <obo:IAO_0000233>label and definition:
issue: https://github.com/OpenEnergyPlatform/ontology/issues/132
pull request: https://github.com/OpenEnergyPlatform/ontology/pull/207

comment:
issue: https://github.com/OpenEnergyPlatform/ontology/issues/629
pull request: https://github.com/OpenEnergyPlatform/ontology/pull/631</obo:IAO_0000233>
        <rdfs:comment>The energy content of waste fuel is typically released by incineration or gasification. The energy content of nuclear waste is not considered as a waste fuel.</rdfs:comment>
        <rdfs:label>waste fuel</rdfs:label>
    </owl:Class>
    


    <!-- http://openenergy-platform.org/ontology/oeo/OEO_00000440 -->

    <owl:Class rdf:about="http://openenergy-platform.org/ontology/oeo/OEO_00000440">
        <rdfs:subClassOf rdf:resource="http://openenergy-platform.org/ontology/oeo/OEO_00000031"/>
        <rdfs:subClassOf>
            <owl:Restriction>
                <owl:onProperty rdf:resource="http://purl.obolibrary.org/obo/BFO_0000051"/>
                <owl:someValuesFrom rdf:resource="http://openenergy-platform.org/ontology/oeo/OEO_00000041"/>
            </owl:Restriction>
        </rdfs:subClassOf>
        <rdfs:subClassOf>
            <owl:Restriction>
                <owl:onProperty rdf:resource="http://purl.obolibrary.org/obo/BFO_0000051"/>
                <owl:someValuesFrom rdf:resource="http://openenergy-platform.org/ontology/oeo/OEO_00000396"/>
            </owl:Restriction>
        </rdfs:subClassOf>
        <obo:IAO_0000115 xml:lang="en">A waste powerplant is a powerplant having an aggregate of waste power units as its power generating units.</obo:IAO_0000115>
        <rdfs:label>waste powerplant</rdfs:label>
    </owl:Class>
    


    <!-- http://openenergy-platform.org/ontology/oeo/OEO_00000441 -->

    <owl:Class rdf:about="http://openenergy-platform.org/ontology/oeo/OEO_00000441">
        <rdfs:subClassOf rdf:resource="http://openenergy-platform.org/ontology/oeo/OEO_00000331"/>
        <rdfs:subClassOf>
            <owl:Restriction>
                <owl:onProperty rdf:resource="http://openenergy-platform.org/ontology/oeo/OEO_00000530"/>
                <owl:someValuesFrom rdf:resource="http://openenergy-platform.org/ontology/oeo/OEO_00030004"/>
            </owl:Restriction>
        </rdfs:subClassOf>
        <rdfs:subClassOf>
            <owl:Restriction>
                <owl:onProperty rdf:resource="http://purl.obolibrary.org/obo/RO_0000091"/>
                <owl:someValuesFrom rdf:resource="http://openenergy-platform.org/ontology/oeo/OEO_00000151"/>
            </owl:Restriction>
        </rdfs:subClassOf>
        <rdfs:subClassOf>
            <owl:Restriction>
                <owl:onProperty rdf:resource="http://openenergy-platform.org/ontology/oeo/OEO_00000529"/>
                <owl:hasValue rdf:resource="http://openenergy-platform.org/ontology/oeo/OEO_00000256"/>
            </owl:Restriction>
        </rdfs:subClassOf>
        <obo:IAO_0000115>Water is a portion of matter with the chemical formula H2O. It has a liquid normal state of matter.</obo:IAO_0000115>
        <obo:IAO_0000233>definition:
issue: https://github.com/OpenEnergyPlatform/ontology/issues/685
pull request: https://github.com/OpenEnergyPlatform/ontology/pull/689
add origin
issue: https://github.com/OpenEnergyPlatform/ontology/issues/515
pull request: https://github.com/OpenEnergyPlatform/ontology/pull/684</obo:IAO_0000233>
        <rdfs:label>water</rdfs:label>
    </owl:Class>
    


    <!-- http://openenergy-platform.org/ontology/oeo/OEO_00000442 -->

    <owl:Class rdf:about="http://openenergy-platform.org/ontology/oeo/OEO_00000442">
        <rdfs:subClassOf rdf:resource="http://openenergy-platform.org/ontology/oeo/OEO_00000425"/>
        <rdfs:subClassOf>
            <owl:Restriction>
                <owl:onProperty rdf:resource="http://openenergy-platform.org/ontology/oeo/OEO_00000533"/>
                <owl:someValuesFrom rdf:resource="http://openenergy-platform.org/ontology/oeo/OEO_00000333"/>
            </owl:Restriction>
        </rdfs:subClassOf>
        <rdfs:subClassOf>
            <owl:Restriction>
                <owl:onProperty rdf:resource="http://openenergy-platform.org/ontology/oeo/OEO_00000532"/>
                <owl:allValuesFrom rdf:resource="http://openenergy-platform.org/ontology/oeo/OEO_00000218"/>
            </owl:Restriction>
        </rdfs:subClassOf>
        <obo:IAO_0000115 xml:lang="en">A water turbine is a turbine converting kinetic energy and potential energy of water into rotational energy.</obo:IAO_0000115>
        <obo:IAO_0000233>issue: https://github.com/OpenEnergyPlatform/ontology/issues/299
pull request: https://github.com/OpenEnergyPlatform/ontology/pull/300</obo:IAO_0000233>
        <rdfs:label>water turbine</rdfs:label>
    </owl:Class>
    


    <!-- http://openenergy-platform.org/ontology/oeo/OEO_00000446 -->

    <owl:Class rdf:about="http://openenergy-platform.org/ontology/oeo/OEO_00000446">
        <rdfs:subClassOf rdf:resource="http://openenergy-platform.org/ontology/oeo/OEO_00230020"/>
        <rdfs:subClassOf>
            <owl:Restriction>
                <owl:onProperty rdf:resource="http://openenergy-platform.org/ontology/oeo/OEO_00000503"/>
                <owl:someValuesFrom rdf:resource="http://openenergy-platform.org/ontology/oeo/OEO_00000043"/>
            </owl:Restriction>
        </rdfs:subClassOf>
        <obo:IAO_0000115 xml:lang="en">Wind energy is the kinetic energy of moving air.</obo:IAO_0000115>
        <obo:IAO_0000233>issue: https://github.com/OpenEnergyPlatform/ontology/issues/211
pull request: https://github.com/OpenEnergyPlatform/ontology/pull/225
reclassify and change def
issue: https://github.com/OpenEnergyPlatform/ontology/issues/662
pull request: https://github.com/OpenEnergyPlatform/ontology/pull/666
remove disposition renewable fuel
issue: https://github.com/OpenEnergyPlatform/ontology/issues/726
pull request: https://github.com/OpenEnergyPlatform/ontology/pull/732</obo:IAO_0000233>
        <rdfs:label>wind energy</rdfs:label>
    </owl:Class>
    


    <!-- http://openenergy-platform.org/ontology/oeo/OEO_00000447 -->

    <owl:Class rdf:about="http://openenergy-platform.org/ontology/oeo/OEO_00000447">
        <rdfs:subClassOf rdf:resource="http://openenergy-platform.org/ontology/oeo/OEO_00000031"/>
        <rdfs:subClassOf>
            <owl:Restriction>
                <owl:onProperty rdf:resource="http://purl.obolibrary.org/obo/BFO_0000051"/>
                <owl:someValuesFrom rdf:resource="http://openenergy-platform.org/ontology/oeo/OEO_00000044"/>
            </owl:Restriction>
        </rdfs:subClassOf>
        <obo:IAO_0000115 xml:lang="en">A wind farm is a powerplant having an aggregate of wind energy converters as its power generating units.</obo:IAO_0000115>
        <rdfs:label>wind farm</rdfs:label>
    </owl:Class>
    


    <!-- http://openenergy-platform.org/ontology/oeo/OEO_00000448 -->

    <owl:Class rdf:about="http://openenergy-platform.org/ontology/oeo/OEO_00000448">
        <rdfs:subClassOf rdf:resource="http://openenergy-platform.org/ontology/oeo/OEO_00000425"/>
        <rdfs:subClassOf>
            <owl:Restriction>
                <owl:onProperty rdf:resource="http://openenergy-platform.org/ontology/oeo/OEO_00000533"/>
                <owl:someValuesFrom rdf:resource="http://openenergy-platform.org/ontology/oeo/OEO_00000333"/>
            </owl:Restriction>
        </rdfs:subClassOf>
        <obo:IAO_0000115 xml:lang="en">A wind rotor (or wind turbine) is a turbine that converts the wind&apos;s kinetic energy into rotational energy.</obo:IAO_0000115>
        <obo:IAO_0000118>wind turbine</obo:IAO_0000118>
        <obo:IAO_0000233>issue: https://github.com/OpenEnergyPlatform/ontology/issues/299
pull request: https://github.com/OpenEnergyPlatform/ontology/pull/300</obo:IAO_0000233>
        <rdfs:label>wind rotor</rdfs:label>
    </owl:Class>
    


    <!-- http://openenergy-platform.org/ontology/oeo/OEO_00000449 -->

    <owl:Class rdf:about="http://openenergy-platform.org/ontology/oeo/OEO_00000449">
        <rdfs:subClassOf rdf:resource="http://openenergy-platform.org/ontology/oeo/OEO_00000332"/>
        <rdfs:subClassOf>
            <owl:Restriction>
                <owl:onProperty rdf:resource="http://purl.obolibrary.org/obo/RO_0000087"/>
                <owl:someValuesFrom rdf:resource="http://openenergy-platform.org/ontology/oeo/OEO_00000001"/>
            </owl:Restriction>
        </rdfs:subClassOf>
        <obo:IAO_0000115 xml:lang="en">Wood and other is solid biomass of purpose-grown energy crops (poplar, willow etc.), a multitude of woody materials generated by an industrial process (wood/paper industry in particular) or provided directly by forestry and agriculture (firewood, wood chips, wood pellets, bark, sawdust, shavings, chips, black liquor etc.) as well as wastes such as straw, rice husks, nut shells, poultry litter, crushed grape dregs etc. Combustion is the preferred technology for these solid wastes. The quantity of fuel used should be reported on a net calorific value basis.</obo:IAO_0000115>
        <obo:IAO_0000119 xml:lang="en">REGULATION (EC) No 1099/2008 OF THE EUROPEAN PARLIAMENT AND OF THE COUNCIL of 22 October 2008 on energy statistics https://eur-lex.europa.eu/legal-content/EN/TXT/HTML/?uri=CELEX:32008R1099&amp;from=EN</obo:IAO_0000119>
        <rdfs:label>wood and other</rdfs:label>
    </owl:Class>
    


    <!-- http://openenergy-platform.org/ontology/oeo/OEO_00010000 -->

    <owl:Class rdf:about="http://openenergy-platform.org/ontology/oeo/OEO_00010000">
        <rdfs:subClassOf rdf:resource="http://openenergy-platform.org/ontology/oeo/OEO_00000331"/>
        <rdfs:subClassOf>
            <owl:Restriction>
                <owl:onProperty rdf:resource="http://purl.obolibrary.org/obo/RO_0000056"/>
                <owl:someValuesFrom rdf:resource="http://openenergy-platform.org/ontology/oeo/OEO_00000055"/>
            </owl:Restriction>
        </rdfs:subClassOf>
        <rdfs:subClassOf>
            <owl:Restriction>
                <owl:onProperty rdf:resource="http://openenergy-platform.org/ontology/oeo/OEO_00000529"/>
                <owl:hasValue rdf:resource="http://openenergy-platform.org/ontology/oeo/OEO_00000182"/>
            </owl:Restriction>
        </rdfs:subClassOf>
        <obo:IAO_0000115>Ammonia is a portion of matter with the chemical formula NH3. It has a gaseous normal state of matter and can act as an air pollutant. Synonyms are trihydridonitrogen and nitrogen trihydride.</obo:IAO_0000115>
        <obo:IAO_0000118>NH3</obo:IAO_0000118>
        <obo:IAO_0000233>issue: https://github.com/OpenEnergyPlatform/ontology/issues/263
pull request: https://github.com/OpenEnergyPlatform/ontology/pull/356</obo:IAO_0000233>
        <rdfs:label xml:lang="en">ammonia</rdfs:label>
    </owl:Class>
    


    <!-- http://openenergy-platform.org/ontology/oeo/OEO_00010001 -->

    <owl:Class rdf:about="http://openenergy-platform.org/ontology/oeo/OEO_00010001">
        <rdfs:subClassOf rdf:resource="http://openenergy-platform.org/ontology/oeo/OEO_00000331"/>
        <rdfs:subClassOf>
            <owl:Restriction>
                <owl:onProperty rdf:resource="http://purl.obolibrary.org/obo/RO_0000056"/>
                <owl:someValuesFrom rdf:resource="http://openenergy-platform.org/ontology/oeo/OEO_00000055"/>
            </owl:Restriction>
        </rdfs:subClassOf>
        <rdfs:subClassOf>
            <owl:Restriction>
                <owl:onProperty rdf:resource="http://openenergy-platform.org/ontology/oeo/OEO_00000529"/>
                <owl:hasValue rdf:resource="http://openenergy-platform.org/ontology/oeo/OEO_00000182"/>
            </owl:Restriction>
        </rdfs:subClassOf>
        <obo:IAO_0000115>Carbon monoxide is a portion of matter with the chemical formula CO. It has a gaseous normal state of matter and can act as an air pollutant.</obo:IAO_0000115>
        <obo:IAO_0000118>CO</obo:IAO_0000118>
        <obo:IAO_0000233>issue: https://github.com/OpenEnergyPlatform/ontology/issues/263
pull request: https://github.com/OpenEnergyPlatform/ontology/pull/356</obo:IAO_0000233>
        <rdfs:label xml:lang="en">carbon monoxide</rdfs:label>
    </owl:Class>
    


    <!-- http://openenergy-platform.org/ontology/oeo/OEO_00010002 -->

    <owl:Class rdf:about="http://openenergy-platform.org/ontology/oeo/OEO_00010002">
        <rdfs:subClassOf rdf:resource="http://openenergy-platform.org/ontology/oeo/OEO_00000331"/>
        <rdfs:subClassOf>
            <owl:Restriction>
                <owl:onProperty rdf:resource="http://purl.obolibrary.org/obo/RO_0000056"/>
                <owl:someValuesFrom rdf:resource="http://openenergy-platform.org/ontology/oeo/OEO_00000055"/>
            </owl:Restriction>
        </rdfs:subClassOf>
        <rdfs:subClassOf>
            <owl:Restriction>
                <owl:onProperty rdf:resource="http://openenergy-platform.org/ontology/oeo/OEO_00000529"/>
                <owl:hasValue rdf:resource="http://openenergy-platform.org/ontology/oeo/OEO_00000182"/>
            </owl:Restriction>
        </rdfs:subClassOf>
        <obo:IAO_0000115>Nitrogen oxides are a portion of matter consisting of compounds of nitrogen and oxygen. It is a collective term for numerous oxides of nitrogen with a gaseous normal state of matter. They can act as air pollutants.</obo:IAO_0000115>
        <obo:IAO_0000118>NOx</obo:IAO_0000118>
        <obo:IAO_0000233>issue: https://github.com/OpenEnergyPlatform/ontology/issues/263
pull request: https://github.com/OpenEnergyPlatform/ontology/pull/356</obo:IAO_0000233>
        <rdfs:label xml:lang="en">nitrogen oxides</rdfs:label>
    </owl:Class>
    


    <!-- http://openenergy-platform.org/ontology/oeo/OEO_00010003 -->

    <owl:Class rdf:about="http://openenergy-platform.org/ontology/oeo/OEO_00010003">
        <rdfs:subClassOf rdf:resource="http://openenergy-platform.org/ontology/oeo/OEO_00010002"/>
        <obo:IAO_0000115>Nitric oxide is a portion of matter with the chemical formula NO. It is a gas and can act as an air pollutant. Synonyms are nitrogen oxide or nitrogen monoxide.</obo:IAO_0000115>
        <obo:IAO_0000118>NO</obo:IAO_0000118>
        <obo:IAO_0000118>nitrogen monoxide</obo:IAO_0000118>
        <obo:IAO_0000118>nitrogen oxide</obo:IAO_0000118>
        <obo:IAO_0000233>issue: https://github.com/OpenEnergyPlatform/ontology/issues/263
pull request: https://github.com/OpenEnergyPlatform/ontology/pull/356</obo:IAO_0000233>
        <rdfs:label xml:lang="en">nitric oxide</rdfs:label>
    </owl:Class>
    


    <!-- http://openenergy-platform.org/ontology/oeo/OEO_00010004 -->

    <owl:Class rdf:about="http://openenergy-platform.org/ontology/oeo/OEO_00010004">
        <rdfs:subClassOf rdf:resource="http://openenergy-platform.org/ontology/oeo/OEO_00010002"/>
        <obo:IAO_0000115>Nitrogen dioxide is a portion of matter with the chemical formula NO2. It is a gas and can act as an air pollutant.</obo:IAO_0000115>
        <obo:IAO_0000118>NO2</obo:IAO_0000118>
        <obo:IAO_0000233>issue: https://github.com/OpenEnergyPlatform/ontology/issues/263
pull request: https://github.com/OpenEnergyPlatform/ontology/pull/356</obo:IAO_0000233>
        <rdfs:label xml:lang="en">nitrogen dioxide</rdfs:label>
    </owl:Class>
    


    <!-- http://openenergy-platform.org/ontology/oeo/OEO_00010007 -->

    <owl:Class rdf:about="http://openenergy-platform.org/ontology/oeo/OEO_00010007">
        <rdfs:subClassOf rdf:resource="http://openenergy-platform.org/ontology/oeo/OEO_00000331"/>
        <rdfs:subClassOf>
            <owl:Restriction>
                <owl:onProperty rdf:resource="http://purl.obolibrary.org/obo/RO_0000056"/>
                <owl:someValuesFrom rdf:resource="http://openenergy-platform.org/ontology/oeo/OEO_00000055"/>
            </owl:Restriction>
        </rdfs:subClassOf>
        <rdfs:subClassOf>
            <owl:Restriction>
                <owl:onProperty rdf:resource="http://openenergy-platform.org/ontology/oeo/OEO_00000529"/>
                <owl:hasValue rdf:resource="http://openenergy-platform.org/ontology/oeo/OEO_00000182"/>
            </owl:Restriction>
        </rdfs:subClassOf>
        <obo:IAO_0000115>Sulphur dioxide is a portion of matter with the chemical formula SO2. It has a gaseous normal state of matter and can act as an air pollutant.</obo:IAO_0000115>
        <obo:IAO_0000118>SO2</obo:IAO_0000118>
        <obo:IAO_0000233>issue: https://github.com/OpenEnergyPlatform/ontology/issues/263
pull request: https://github.com/OpenEnergyPlatform/ontology/pull/356</obo:IAO_0000233>
        <rdfs:label xml:lang="en">sulphur dioxide</rdfs:label>
    </owl:Class>
    


    <!-- http://openenergy-platform.org/ontology/oeo/OEO_00010009 -->

    <owl:Class rdf:about="http://openenergy-platform.org/ontology/oeo/OEO_00010009">
        <rdfs:subClassOf rdf:resource="http://openenergy-platform.org/ontology/oeo/OEO_00000318"/>
        <obo:IAO_0000115>PM10 is particulate matter which passes through a size-selective inlet as defined in the reference method for the sampling and measurement of PM10, EN 12341, with a 50 % efficiency cut-off at 10 µm aerodynamic diameter.</obo:IAO_0000115>
        <obo:IAO_0000119>This definition is partly based on Article 2 of the European Air Quality Directive (2008/50/EC): https://eur-lex.europa.eu/legal-content/EN/TXT/?uri=CELEX:32008L0050</obo:IAO_0000119>
        <obo:IAO_0000233>issue: https://github.com/OpenEnergyPlatform/ontology/issues/263
pull request: https://github.com/OpenEnergyPlatform/ontology/pull/356</obo:IAO_0000233>
        <rdfs:label xml:lang="en">PM10</rdfs:label>
    </owl:Class>
    


    <!-- http://openenergy-platform.org/ontology/oeo/OEO_00010010 -->

    <owl:Class rdf:about="http://openenergy-platform.org/ontology/oeo/OEO_00010010">
        <rdfs:subClassOf rdf:resource="http://openenergy-platform.org/ontology/oeo/OEO_00000318"/>
        <obo:IAO_0000115>PM2.5 is particulate matter which passes through a size-selective inlet as defined in the reference method for the sampling and measurement of PM2,5, EN 14907, with a 50 % efficiency cut-off at 2,5 µm aerodynamic diameter.</obo:IAO_0000115>
        <obo:IAO_0000119>This definition is partly based on Article 2 of the European Air Quality Directive (2008/50/EC): https://eur-lex.europa.eu/legal-content/EN/TXT/?uri=CELEX:32008L0050</obo:IAO_0000119>
        <obo:IAO_0000233>issue: https://github.com/OpenEnergyPlatform/ontology/issues/263
pull request: https://github.com/OpenEnergyPlatform/ontology/pull/356</obo:IAO_0000233>
        <rdfs:label xml:lang="en">PM2.5</rdfs:label>
    </owl:Class>
    


    <!-- http://openenergy-platform.org/ontology/oeo/OEO_00010011 -->

    <owl:Class rdf:about="http://openenergy-platform.org/ontology/oeo/OEO_00010011">
        <rdfs:subClassOf rdf:resource="http://purl.obolibrary.org/obo/BFO_0000016"/>
        <obo:IAO_0000115>The volatility disposition is the disposition of a portion of matter to sublimate or evaporate from the solid or liquid form and enter the surrounding air.</obo:IAO_0000115>
        <obo:IAO_0000233>issue: https://github.com/OpenEnergyPlatform/ontology/issues/263
pull request: https://github.com/OpenEnergyPlatform/ontology/pull/356</obo:IAO_0000233>
        <rdfs:label xml:lang="en">volatility</rdfs:label>
    </owl:Class>
    


    <!-- http://openenergy-platform.org/ontology/oeo/OEO_00010012 -->

    <owl:Class rdf:about="http://openenergy-platform.org/ontology/oeo/OEO_00010012">
        <owl:equivalentClass>
            <owl:Class>
                <owl:intersectionOf rdf:parseType="Collection">
                    <rdf:Description rdf:about="http://openenergy-platform.org/ontology/oeo/OEO_00000331"/>
                    <owl:Restriction>
                        <owl:onProperty rdf:resource="http://purl.obolibrary.org/obo/RO_0000056"/>
                        <owl:someValuesFrom rdf:resource="http://openenergy-platform.org/ontology/oeo/OEO_00000055"/>
                    </owl:Restriction>
                </owl:intersectionOf>
            </owl:Class>
        </owl:equivalentClass>
        <rdfs:subClassOf rdf:resource="http://openenergy-platform.org/ontology/oeo/OEO_00000331"/>
        <obo:IAO_0000115>An air pollutant is a portion of matter that has the disposition to participates in air pollution.</obo:IAO_0000115>
        <obo:IAO_0000233>issue: https://github.com/OpenEnergyPlatform/ontology/issues/263
pull request: https://github.com/OpenEnergyPlatform/ontology/pull/356</obo:IAO_0000233>
        <rdfs:label xml:lang="en">air pollutant</rdfs:label>
    </owl:Class>
    


    <!-- http://openenergy-platform.org/ontology/oeo/OEO_00010015 -->

    <owl:Class rdf:about="http://openenergy-platform.org/ontology/oeo/OEO_00010015">
        <rdfs:subClassOf rdf:resource="http://openenergy-platform.org/ontology/oeo/OEO_00000220"/>
        <rdfs:subClassOf>
            <owl:Restriction>
                <owl:onProperty rdf:resource="http://openenergy-platform.org/ontology/oeo/OEO_00000530"/>
                <owl:someValuesFrom rdf:resource="http://openenergy-platform.org/ontology/oeo/OEO_00030002"/>
            </owl:Restriction>
        </rdfs:subClassOf>
        <obo:IAO_0000115>Fossil hydrogen is hydrogen with fossil origin. It is usually produced from fossil fuels applying the steam reforming process.</obo:IAO_0000115>
        <obo:IAO_0000233>issue: https://github.com/OpenEnergyPlatform/ontology/issues/134
pull request: https://github.com/OpenEnergyPlatform/ontology/pull/411</obo:IAO_0000233>
        <rdfs:label>fossil hydrogen</rdfs:label>
    </owl:Class>
    


    <!-- http://openenergy-platform.org/ontology/oeo/OEO_00010016 -->

    <owl:Class rdf:about="http://openenergy-platform.org/ontology/oeo/OEO_00010016">
        <rdfs:subClassOf rdf:resource="http://openenergy-platform.org/ontology/oeo/OEO_00000220"/>
        <rdfs:subClassOf>
            <owl:Restriction>
                <owl:onProperty rdf:resource="http://openenergy-platform.org/ontology/oeo/OEO_00000530"/>
                <owl:someValuesFrom rdf:resource="http://openenergy-platform.org/ontology/oeo/OEO_00030005"/>
            </owl:Restriction>
        </rdfs:subClassOf>
        <obo:IAO_0000115>Synthetic hydrogen is hydrogen with synthetic origin. It is usually produced from water applying the water electrolysis process.</obo:IAO_0000115>
        <obo:IAO_0000233>issue: https://github.com/OpenEnergyPlatform/ontology/issues/134
pull request: https://github.com/OpenEnergyPlatform/ontology/pull/411</obo:IAO_0000233>
        <rdfs:label>synthetic hydrogen</rdfs:label>
    </owl:Class>
    


    <!-- http://openenergy-platform.org/ontology/oeo/OEO_00010017 -->

    <owl:Class rdf:about="http://openenergy-platform.org/ontology/oeo/OEO_00010017">
        <owl:equivalentClass>
            <owl:Class>
                <owl:intersectionOf rdf:parseType="Collection">
                    <rdf:Description rdf:about="http://openenergy-platform.org/ontology/oeo/OEO_00000173"/>
                    <owl:Restriction>
                        <owl:onProperty rdf:resource="http://openenergy-platform.org/ontology/oeo/OEO_00000530"/>
                        <owl:someValuesFrom rdf:resource="http://openenergy-platform.org/ontology/oeo/OEO_00030005"/>
                    </owl:Restriction>
                </owl:intersectionOf>
            </owl:Class>
        </owl:equivalentClass>
        <rdfs:subClassOf>
            <owl:Restriction>
                <owl:onProperty rdf:resource="http://purl.obolibrary.org/obo/RO_0000091"/>
                <owl:someValuesFrom rdf:resource="http://openenergy-platform.org/ontology/oeo/OEO_00000097"/>
            </owl:Restriction>
        </rdfs:subClassOf>
        <obo:IAO_0000115>A synthetic fuel is a fuel produced from one or more portion(s) of matter using electric energy.</obo:IAO_0000115>
        <obo:IAO_0000118>e-fuel</obo:IAO_0000118>
        <obo:IAO_0000118>electric fuel</obo:IAO_0000118>
        <obo:IAO_0000233>issue: https://github.com/OpenEnergyPlatform/ontology/issues/134
pull request: https://github.com/OpenEnergyPlatform/ontology/pull/411</obo:IAO_0000233>
        <rdfs:label>synthetic fuel</rdfs:label>
    </owl:Class>
    


    <!-- http://openenergy-platform.org/ontology/oeo/OEO_00010018 -->

    <owl:Class rdf:about="http://openenergy-platform.org/ontology/oeo/OEO_00010018">
        <rdfs:subClassOf rdf:resource="http://openenergy-platform.org/ontology/oeo/OEO_00000025"/>
        <rdfs:subClassOf>
            <owl:Restriction>
                <owl:onProperty rdf:resource="http://openenergy-platform.org/ontology/oeo/OEO_00000530"/>
                <owl:someValuesFrom rdf:resource="http://openenergy-platform.org/ontology/oeo/OEO_00030005"/>
            </owl:Restriction>
        </rdfs:subClassOf>
        <obo:IAO_0000115>Synthetic methane is synthetic fuel produced in a power-to-gas system from water and carbon dioxide using electric energy.</obo:IAO_0000115>
        <obo:IAO_0000233>issue: https://github.com/OpenEnergyPlatform/ontology/issues/134
pull request: https://github.com/OpenEnergyPlatform/ontology/pull/411</obo:IAO_0000233>
        <rdfs:label>synthetic methane</rdfs:label>
    </owl:Class>
    


    <!-- http://openenergy-platform.org/ontology/oeo/OEO_00010019 -->

    <owl:Class rdf:about="http://openenergy-platform.org/ontology/oeo/OEO_00010019">
        <owl:equivalentClass>
            <owl:Class>
                <owl:intersectionOf rdf:parseType="Collection">
                    <rdf:Description rdf:about="http://openenergy-platform.org/ontology/oeo/OEO_00010017"/>
                    <owl:Restriction>
                        <owl:onProperty rdf:resource="http://openenergy-platform.org/ontology/oeo/OEO_00000529"/>
                        <owl:hasValue rdf:resource="http://openenergy-platform.org/ontology/oeo/OEO_00000256"/>
                    </owl:Restriction>
                </owl:intersectionOf>
            </owl:Class>
        </owl:equivalentClass>
        <rdfs:subClassOf rdf:resource="http://openenergy-platform.org/ontology/oeo/OEO_00010017"/>
        <obo:IAO_0000115>Synthetic liquid fuel is synthetic fuel produced in a power-to-liquid system from water and carbon dioxide using electric energy applying.</obo:IAO_0000115>
        <obo:IAO_0000233>issue: https://github.com/OpenEnergyPlatform/ontology/issues/134
pull request: https://github.com/OpenEnergyPlatform/ontology/pull/411</obo:IAO_0000233>
        <rdfs:label>synthetic liquid fuel</rdfs:label>
    </owl:Class>
    


    <!-- http://openenergy-platform.org/ontology/oeo/OEO_00010020 -->

    <owl:Class rdf:about="http://openenergy-platform.org/ontology/oeo/OEO_00010020">
        <rdfs:subClassOf rdf:resource="http://openenergy-platform.org/ontology/oeo/OEO_00000159"/>
        <obo:IAO_0000115>A power-to-liquid (often abbreviated P2L or PtL) system is an energy storage object that converts electrical power to a liquid fuel.</obo:IAO_0000115>
        <obo:IAO_0000118>P2L</obo:IAO_0000118>
        <obo:IAO_0000118>PtL</obo:IAO_0000118>
        <obo:IAO_0000233>issue: https://github.com/OpenEnergyPlatform/ontology/issues/134
pull request: https://github.com/OpenEnergyPlatform/ontology/pull/411</obo:IAO_0000233>
        <rdfs:label>power-to-liquid system</rdfs:label>
    </owl:Class>
    


    <!-- http://openenergy-platform.org/ontology/oeo/OEO_00010021 -->

    <owl:Class rdf:about="http://openenergy-platform.org/ontology/oeo/OEO_00010021">
        <rdfs:subClassOf rdf:resource="http://openenergy-platform.org/ontology/oeo/OEO_00000011"/>
        <obo:IAO_0000115>A water electrolyser is an energy converting device that uses an electric current to decompose water into hydrogen and oxygen gas. Electric energy is converted into chemical energy (and waste heat).</obo:IAO_0000115>
        <obo:IAO_0000233>issue: https://github.com/OpenEnergyPlatform/ontology/issues/134
pull request: https://github.com/OpenEnergyPlatform/ontology/pull/411</obo:IAO_0000233>
        <rdfs:label>water electrolyser</rdfs:label>
    </owl:Class>
    


    <!-- http://openenergy-platform.org/ontology/oeo/OEO_00010022 -->

    <owl:Class rdf:about="http://openenergy-platform.org/ontology/oeo/OEO_00010022">
        <rdfs:subClassOf rdf:resource="http://openenergy-platform.org/ontology/oeo/OEO_00000011"/>
        <obo:IAO_0000115>A steam reformer is an energy converting device that produces syngas from hydrocarbons such as natural gas.</obo:IAO_0000115>
        <obo:IAO_0000233>issue: https://github.com/OpenEnergyPlatform/ontology/issues/134
pull request: https://github.com/OpenEnergyPlatform/ontology/pull/411</obo:IAO_0000233>
        <rdfs:label>steam reformer</rdfs:label>
    </owl:Class>
    


    <!-- http://openenergy-platform.org/ontology/oeo/OEO_00010023 -->

    <owl:Class rdf:about="http://openenergy-platform.org/ontology/oeo/OEO_00010023">
        <rdfs:subClassOf rdf:resource="http://openenergy-platform.org/ontology/oeo/OEO_00000061"/>
        <obo:IAO_0000115>A vehicle is an artifical object that is used for transporting people or goods.</obo:IAO_0000115>
        <obo:IAO_0000233>issue: https://github.com/OpenEnergyPlatform/ontology/issues/425
pull request: https://github.com/OpenEnergyPlatform/ontology/pull/431</obo:IAO_0000233>
        <rdfs:label xml:lang="en">vehicle</rdfs:label>
    </owl:Class>
    


    <!-- http://openenergy-platform.org/ontology/oeo/OEO_00010024 -->

    <owl:Class rdf:about="http://openenergy-platform.org/ontology/oeo/OEO_00010024">
        <rdfs:subClassOf rdf:resource="http://openenergy-platform.org/ontology/oeo/OEO_00000146"/>
        <rdfs:subClassOf>
            <owl:Restriction>
                <owl:onProperty rdf:resource="http://purl.obolibrary.org/obo/BFO_0000051"/>
                <owl:someValuesFrom rdf:resource="http://openenergy-platform.org/ontology/oeo/OEO_00010026"/>
            </owl:Restriction>
        </rdfs:subClassOf>
        <obo:IAO_0000115>A battery electric vehicle (BEV) is an electric vehicle that stores energy in an on-board battery.</obo:IAO_0000115>
        <obo:IAO_0000118>BEV</obo:IAO_0000118>
        <obo:IAO_0000233>issue: https://github.com/OpenEnergyPlatform/ontology/issues/425
pull request: https://github.com/OpenEnergyPlatform/ontology/pull/453

issue: https://github.com/OpenEnergyPlatform/ontology/issues/637
pull request: https://github.com/OpenEnergyPlatform/ontology/pull/655</obo:IAO_0000233>
        <rdfs:label xml:lang="en">battery electric vehicle</rdfs:label>
    </owl:Class>
    


    <!-- http://openenergy-platform.org/ontology/oeo/OEO_00010025 -->

    <owl:Class rdf:about="http://openenergy-platform.org/ontology/oeo/OEO_00010025">
        <rdfs:subClassOf rdf:resource="http://openenergy-platform.org/ontology/oeo/OEO_00000146"/>
        <rdfs:subClassOf>
            <owl:Restriction>
                <owl:onProperty rdf:resource="http://openenergy-platform.org/ontology/oeo/OEO_00000503"/>
                <owl:someValuesFrom rdf:resource="http://openenergy-platform.org/ontology/oeo/OEO_00000220"/>
            </owl:Restriction>
        </rdfs:subClassOf>
        <rdfs:subClassOf>
            <owl:Restriction>
                <owl:onProperty rdf:resource="http://purl.obolibrary.org/obo/BFO_0000051"/>
                <owl:someValuesFrom rdf:resource="http://openenergy-platform.org/ontology/oeo/OEO_00000016"/>
            </owl:Restriction>
        </rdfs:subClassOf>
        <obo:IAO_0000115>A fuel cell electric vehicle (FCEV) is an electric vehicle that uses electrical energy from a fuel cell.</obo:IAO_0000115>
        <obo:IAO_0000118>FCEV</obo:IAO_0000118>
        <obo:IAO_0000233>issue: https://github.com/OpenEnergyPlatform/ontology/issues/425
pull request: https://github.com/OpenEnergyPlatform/ontology/pull/453

issue: https://github.com/OpenEnergyPlatform/ontology/issues/637
pull request: https://github.com/OpenEnergyPlatform/ontology/pull/655</obo:IAO_0000233>
        <rdfs:label xml:lang="en">fuel cell electric vehicle</rdfs:label>
    </owl:Class>
    


    <!-- http://openenergy-platform.org/ontology/oeo/OEO_00010026 -->

    <owl:Class rdf:about="http://openenergy-platform.org/ontology/oeo/OEO_00010026">
        <rdfs:subClassOf rdf:resource="http://openenergy-platform.org/ontology/oeo/OEO_00000068"/>
        <obo:IAO_0000233>issue: https://github.com/OpenEnergyPlatform/ontology/issues/425
pull request: https://github.com/OpenEnergyPlatform/ontology/pull/453</obo:IAO_0000233>
        <dc:description>A traction battery is a battery that is used in vehicles for propulsion.</dc:description>
        <rdfs:label xml:lang="en">traction battery</rdfs:label>
    </owl:Class>
    


    <!-- http://openenergy-platform.org/ontology/oeo/OEO_00010027 -->

    <owl:Class rdf:about="http://openenergy-platform.org/ontology/oeo/OEO_00010027">
        <rdfs:subClassOf rdf:resource="http://openenergy-platform.org/ontology/oeo/OEO_00010032"/>
        <rdfs:subClassOf>
            <owl:Restriction>
                <owl:onProperty rdf:resource="http://openenergy-platform.org/ontology/oeo/OEO_00000503"/>
                <owl:someValuesFrom rdf:resource="http://openenergy-platform.org/ontology/oeo/OEO_00000139"/>
            </owl:Restriction>
        </rdfs:subClassOf>
        <obo:IAO_0000233>issue: https://github.com/OpenEnergyPlatform/ontology/issues/425
pull request: https://github.com/OpenEnergyPlatform/ontology/pull/453</obo:IAO_0000233>
        <dc:description>An electric motor is an energy converting device that converts electrical energy into kinetic energy.</dc:description>
        <rdfs:label xml:lang="en">electric motor</rdfs:label>
    </owl:Class>
    


    <!-- http://openenergy-platform.org/ontology/oeo/OEO_00010028 -->

    <owl:Class rdf:about="http://openenergy-platform.org/ontology/oeo/OEO_00010028">
        <rdfs:subClassOf rdf:resource="http://openenergy-platform.org/ontology/oeo/OEO_00010027"/>
        <obo:IAO_0000233>issue: https://github.com/OpenEnergyPlatform/ontology/issues/425
pull request: https://github.com/OpenEnergyPlatform/ontology/pull/453</obo:IAO_0000233>
        <dc:description>A traction motor is an electric motor used for propulsion.</dc:description>
        <rdfs:label xml:lang="en">traction motor</rdfs:label>
    </owl:Class>
    


    <!-- http://openenergy-platform.org/ontology/oeo/OEO_00010029 -->

    <owl:Class rdf:about="http://openenergy-platform.org/ontology/oeo/OEO_00010029">
        <rdfs:subClassOf rdf:resource="http://openenergy-platform.org/ontology/oeo/OEO_00010032"/>
        <rdfs:subClassOf>
            <owl:Restriction>
                <owl:onProperty rdf:resource="http://openenergy-platform.org/ontology/oeo/OEO_00000503"/>
                <owl:someValuesFrom rdf:resource="http://openenergy-platform.org/ontology/oeo/OEO_00000099"/>
            </owl:Restriction>
        </rdfs:subClassOf>
        <obo:IAO_0000233>issue: https://github.com/OpenEnergyPlatform/ontology/issues/425
pull request: https://github.com/OpenEnergyPlatform/ontology/pull/453</obo:IAO_0000233>
        <dc:description>An internal combustion engine is an energy converting device that converts chemical energy into into rotational energy using a cyclic combustion process.</dc:description>
        <rdfs:label xml:lang="en">internal combustion engine</rdfs:label>
    </owl:Class>
    


    <!-- http://openenergy-platform.org/ontology/oeo/OEO_00010030 -->

    <owl:Class rdf:about="http://openenergy-platform.org/ontology/oeo/OEO_00010030">
        <rdfs:subClassOf rdf:resource="http://openenergy-platform.org/ontology/oeo/OEO_00010023"/>
        <rdfs:subClassOf>
            <owl:Restriction>
                <owl:onProperty rdf:resource="http://openenergy-platform.org/ontology/oeo/OEO_00000503"/>
                <owl:someValuesFrom rdf:resource="http://openenergy-platform.org/ontology/oeo/OEO_00000099"/>
            </owl:Restriction>
        </rdfs:subClassOf>
        <rdfs:subClassOf>
            <owl:Restriction>
                <owl:onProperty rdf:resource="http://openenergy-platform.org/ontology/oeo/OEO_00000503"/>
                <owl:someValuesFrom rdf:resource="http://openenergy-platform.org/ontology/oeo/OEO_00000139"/>
            </owl:Restriction>
        </rdfs:subClassOf>
        <rdfs:subClassOf>
            <owl:Restriction>
                <owl:onProperty rdf:resource="http://purl.obolibrary.org/obo/BFO_0000051"/>
                <owl:someValuesFrom rdf:resource="http://openenergy-platform.org/ontology/oeo/OEO_00010026"/>
            </owl:Restriction>
        </rdfs:subClassOf>
        <rdfs:subClassOf>
            <owl:Restriction>
                <owl:onProperty rdf:resource="http://purl.obolibrary.org/obo/BFO_0000051"/>
                <owl:someValuesFrom rdf:resource="http://openenergy-platform.org/ontology/oeo/OEO_00010028"/>
            </owl:Restriction>
        </rdfs:subClassOf>
        <rdfs:subClassOf>
            <owl:Restriction>
                <owl:onProperty rdf:resource="http://purl.obolibrary.org/obo/BFO_0000051"/>
                <owl:someValuesFrom rdf:resource="http://openenergy-platform.org/ontology/oeo/OEO_00010029"/>
            </owl:Restriction>
        </rdfs:subClassOf>
        <obo:IAO_0000115>A plug-in hybrid electric vehicle (PHEV) is a vehicle that contains both a traction motor and an internal combustion engine and can switch between their usage for propulsion. It contains a traction battery that can be charged with electrical energy from an external supply.</obo:IAO_0000115>
        <obo:IAO_0000118>PHEV</obo:IAO_0000118>
        <obo:IAO_0000233>issue: https://github.com/OpenEnergyPlatform/ontology/issues/425
pull request: https://github.com/OpenEnergyPlatform/ontology/pull/453</obo:IAO_0000233>
        <rdfs:label xml:lang="en">plug-in hybrid electric vehicle</rdfs:label>
    </owl:Class>
    


    <!-- http://openenergy-platform.org/ontology/oeo/OEO_00010031 -->

    <owl:Class rdf:about="http://openenergy-platform.org/ontology/oeo/OEO_00010031">
        <rdfs:subClassOf rdf:resource="http://openenergy-platform.org/ontology/oeo/OEO_00000146"/>
        <obo:IAO_0000115>A grid supplied electric vehicle is an electric vehicle that uses electrical energy via a conductor.</obo:IAO_0000115>
        <obo:IAO_0000233>issue: https://github.com/OpenEnergyPlatform/ontology/issues/425
pull request: https://github.com/OpenEnergyPlatform/ontology/pull/453</obo:IAO_0000233>
        <rdfs:label xml:lang="en">grid supplied electric vehicle</rdfs:label>
    </owl:Class>
    


    <!-- http://openenergy-platform.org/ontology/oeo/OEO_00010032 -->

    <owl:Class rdf:about="http://openenergy-platform.org/ontology/oeo/OEO_00010032">
        <rdfs:subClassOf rdf:resource="http://openenergy-platform.org/ontology/oeo/OEO_00000011"/>
        <obo:IAO_0000233>issue: https://github.com/OpenEnergyPlatform/ontology/issues/425
pull request: https://github.com/OpenEnergyPlatform/ontology/pull/453</obo:IAO_0000233>
        <dc:description>A motor is an energy converting device that converts other forms of energy into rotational kinetic energy.</dc:description>
        <rdfs:label>motor</rdfs:label>
    </owl:Class>
    


    <!-- http://openenergy-platform.org/ontology/oeo/OEO_00010072 -->

    <owl:Class rdf:about="http://openenergy-platform.org/ontology/oeo/OEO_00010072">
        <rdfs:subClassOf rdf:resource="http://purl.obolibrary.org/obo/UO_0000000"/>
        <obo:IAO_0000115>An areal power density unit is a unit which is a measure for the power per surface area.</obo:IAO_0000115>
        <obo:IAO_0000233>issue: https://github.com/OpenEnergyPlatform/ontology/issues/597
pull request: https://github.com/OpenEnergyPlatform/ontology/pull/615</obo:IAO_0000233>
        <rdfs:label>areal power density unit</rdfs:label>
    </owl:Class>
    


    <!-- http://openenergy-platform.org/ontology/oeo/OEO_00010073 -->

    <owl:Class rdf:about="http://openenergy-platform.org/ontology/oeo/OEO_00010073">
        <rdfs:subClassOf rdf:resource="http://purl.obolibrary.org/obo/UO_0000000"/>
        <obo:IAO_0000115>An areal energy density unit is a unit which is a measure for the energy per surface area.</obo:IAO_0000115>
        <obo:IAO_0000233>issue: https://github.com/OpenEnergyPlatform/ontology/issues/597
pull request: https://github.com/OpenEnergyPlatform/ontology/pull/615</obo:IAO_0000233>
        <rdfs:label>areal energy density unit</rdfs:label>
    </owl:Class>
    


    <!-- http://openenergy-platform.org/ontology/oeo/OEO_00010074 -->

    <owl:Class rdf:about="http://openenergy-platform.org/ontology/oeo/OEO_00010074">
        <rdfs:subClassOf rdf:resource="http://openenergy-platform.org/ontology/oeo/OEO_00000350"/>
        <rdfs:subClassOf>
            <owl:Restriction>
                <owl:onProperty rdf:resource="http://openenergy-platform.org/ontology/oeo/OEO_00040010"/>
                <owl:someValuesFrom rdf:resource="http://openenergy-platform.org/ontology/oeo/OEO_00010072"/>
            </owl:Restriction>
        </rdfs:subClassOf>
        <obo:IAO_0000115>An areal power density is a quantity value that indicates a certain power per area.</obo:IAO_0000115>
        <obo:IAO_0000233>issue: https://github.com/OpenEnergyPlatform/ontology/issues/597
pull request: https://github.com/OpenEnergyPlatform/ontology/pull/615</obo:IAO_0000233>
        <rdfs:label>areal power density</rdfs:label>
    </owl:Class>
    


    <!-- http://openenergy-platform.org/ontology/oeo/OEO_00010075 -->

    <owl:Class rdf:about="http://openenergy-platform.org/ontology/oeo/OEO_00010075">
        <rdfs:subClassOf rdf:resource="http://openenergy-platform.org/ontology/oeo/OEO_00000350"/>
        <rdfs:subClassOf>
            <owl:Restriction>
                <owl:onProperty rdf:resource="http://openenergy-platform.org/ontology/oeo/OEO_00040010"/>
                <owl:someValuesFrom rdf:resource="http://openenergy-platform.org/ontology/oeo/OEO_00010073"/>
            </owl:Restriction>
        </rdfs:subClassOf>
        <obo:IAO_0000115>An areal energy density is a quantity value that states a certain energy amount per area.</obo:IAO_0000115>
        <obo:IAO_0000233>issue: https://github.com/OpenEnergyPlatform/ontology/issues/597
pull request: https://github.com/OpenEnergyPlatform/ontology/pull/615</obo:IAO_0000233>
        <rdfs:label>areal energy density</rdfs:label>
    </owl:Class>
    


    <!-- http://openenergy-platform.org/ontology/oeo/OEO_00010076 -->

    <owl:Class rdf:about="http://openenergy-platform.org/ontology/oeo/OEO_00010076">
        <rdfs:subClassOf rdf:resource="http://openenergy-platform.org/ontology/oeo/OEO_00010074"/>
        <obo:IAO_0000115>An areal solar power density is an areal power density that indicates the arriving solar power per area. A synonym for areal solar power density is irradiance.</obo:IAO_0000115>
        <obo:IAO_0000118>irradiance</obo:IAO_0000118>
        <obo:IAO_0000233>issue: https://github.com/OpenEnergyPlatform/ontology/issues/597
pull request: https://github.com/OpenEnergyPlatform/ontology/pull/615</obo:IAO_0000233>
        <rdfs:label>areal solar power density</rdfs:label>
    </owl:Class>
    


    <!-- http://openenergy-platform.org/ontology/oeo/OEO_00010077 -->

    <owl:Class rdf:about="http://openenergy-platform.org/ontology/oeo/OEO_00010077">
        <rdfs:subClassOf rdf:resource="http://openenergy-platform.org/ontology/oeo/OEO_00010075"/>
        <obo:IAO_0000115>An areal solar energy density is an areal energy density that gives the arriving solar power per area. A synonym for areal solar power density is irradiation.</obo:IAO_0000115>
        <obo:IAO_0000118>irradiation</obo:IAO_0000118>
        <obo:IAO_0000233>issue: https://github.com/OpenEnergyPlatform/ontology/issues/597
pull request: https://github.com/OpenEnergyPlatform/ontology/pull/615</obo:IAO_0000233>
        <rdfs:label>areal solar energy density</rdfs:label>
    </owl:Class>
    


    <!-- http://openenergy-platform.org/ontology/oeo/OEO_00010078 -->

    <owl:Class rdf:about="http://openenergy-platform.org/ontology/oeo/OEO_00010078">
        <rdfs:subClassOf rdf:resource="http://openenergy-platform.org/ontology/oeo/OEO_00000350"/>
        <rdfs:subClassOf>
            <owl:Restriction>
                <owl:onProperty rdf:resource="http://openenergy-platform.org/ontology/oeo/OEO_00040010"/>
                <owl:someValuesFrom rdf:resource="http://purl.obolibrary.org/obo/UO_0010006"/>
            </owl:Restriction>
        </rdfs:subClassOf>
        <obo:IAO_0000115>Global warming potential (GWP) is a quantity value that measures the the time-integrated radiative forcing due to a pulse emission of a given component, relative to a pulse emission of an equal mass of carbon dioxide (CO2).</obo:IAO_0000115>
        <obo:IAO_0000118>GWP</obo:IAO_0000118>
        <obo:IAO_0000233>issue: https://github.com/OpenEnergyPlatform/ontology/issues/420
pull request: https://github.com/OpenEnergyPlatform/ontology/pull/683</obo:IAO_0000233>
        <rdfs:label xml:lang="en">global warming potential</rdfs:label>
    </owl:Class>
    


    <!-- http://openenergy-platform.org/ontology/oeo/OEO_00010079 -->

    <owl:Class rdf:about="http://openenergy-platform.org/ontology/oeo/OEO_00010079"/>
    


    <!-- http://openenergy-platform.org/ontology/oeo/OEO_00010080 -->

    <owl:Class rdf:about="http://openenergy-platform.org/ontology/oeo/OEO_00010080">
        <owl:equivalentClass>
            <owl:Class>
                <owl:intersectionOf rdf:parseType="Collection">
                    <owl:Restriction>
                        <owl:onProperty rdf:resource="http://purl.obolibrary.org/obo/BFO_0000051"/>
                        <owl:someValuesFrom rdf:resource="http://openenergy-platform.org/ontology/oeo/OEO_00020047"/>
                    </owl:Restriction>
                    <owl:Restriction>
                        <owl:onProperty rdf:resource="http://purl.obolibrary.org/obo/BFO_0000051"/>
                        <owl:someValuesFrom rdf:resource="http://openenergy-platform.org/ontology/oeo/OEO_00050020"/>
                    </owl:Restriction>
                </owl:intersectionOf>
            </owl:Class>
        </owl:equivalentClass>
        <rdfs:subClassOf rdf:resource="http://openenergy-platform.org/ontology/oeo/OEO_00020046"/>
        <obo:IAO_0000115>A solar-steam-electric process is a solar energy transformation that converts solar energy into electrical energy. It has two partical process: a solar thermal energy transformation and a steam power process.</obo:IAO_0000115>
        <obo:IAO_0000233>issue: https://github.com/OpenEnergyPlatform/ontology/issues/668
pull request: https://github.com/OpenEnergyPlatform/ontology/pull/701</obo:IAO_0000233>
        <rdfs:label xml:lang="en">solar-steam-electric process</rdfs:label>
    </owl:Class>
    


    <!-- http://openenergy-platform.org/ontology/oeo/OEO_00010081 -->

    <owl:Class rdf:about="http://openenergy-platform.org/ontology/oeo/OEO_00010081">
        <rdfs:subClassOf rdf:resource="http://openenergy-platform.org/ontology/oeo/OEO_00020046"/>
        <rdfs:subClassOf>
            <owl:Restriction>
                <owl:onProperty rdf:resource="http://openenergy-platform.org/ontology/oeo/OEO_00000533"/>
                <owl:someValuesFrom rdf:resource="http://openenergy-platform.org/ontology/oeo/OEO_00000007"/>
            </owl:Restriction>
        </rdfs:subClassOf>
        <obo:IAO_0000115 xml:lang="en">A solar chemical energy transformation is a solar energy transformation that converts solar energy into chemical energy.</obo:IAO_0000115>
        <obo:IAO_0000233>issue: https://github.com/OpenEnergyPlatform/ontology/issues/673
pull request: https://github.com/OpenEnergyPlatform/ontology/pull/735</obo:IAO_0000233>
        <rdfs:label xml:lang="en">solar chemical energy transformation</rdfs:label>
    </owl:Class>
    


    <!-- http://openenergy-platform.org/ontology/oeo/OEO_00020001 -->

    <owl:Class rdf:about="http://openenergy-platform.org/ontology/oeo/OEO_00020001">
        <rdfs:subClassOf rdf:resource="http://openenergy-platform.org/ontology/oeo/OEO_00000331"/>
        <rdfs:subClassOf>
            <owl:Restriction>
                <owl:onProperty rdf:resource="http://purl.obolibrary.org/obo/BFO_0000050"/>
                <owl:someValuesFrom rdf:resource="http://openenergy-platform.org/ontology/oeo/OEO_00000075"/>
            </owl:Restriction>
        </rdfs:subClassOf>
        <rdfs:subClassOf>
            <owl:Restriction>
                <owl:onProperty rdf:resource="http://purl.obolibrary.org/obo/RO_0000087"/>
                <owl:someValuesFrom rdf:resource="http://openenergy-platform.org/ontology/oeo/OEO_00000001"/>
            </owl:Restriction>
        </rdfs:subClassOf>
        <rdfs:subClassOf>
            <owl:Restriction>
                <owl:onProperty rdf:resource="http://purl.obolibrary.org/obo/RO_0000091"/>
                <owl:someValuesFrom rdf:resource="http://openenergy-platform.org/ontology/oeo/OEO_00000097"/>
            </owl:Restriction>
        </rdfs:subClassOf>
        <rdfs:subClassOf>
            <owl:Restriction>
                <owl:onProperty rdf:resource="http://openenergy-platform.org/ontology/oeo/OEO_00000529"/>
                <owl:hasValue rdf:resource="http://openenergy-platform.org/ontology/oeo/OEO_00000256"/>
            </owl:Restriction>
        </rdfs:subClassOf>
        <obo:IAO_0000115 xml:lang="en">Ethanol is a portion of matter with the chemical formula C2H6O. It has a liquid normal state of matter and can be used as a combustion fuel.</obo:IAO_0000115>
        <obo:IAO_0000233 xml:lang="en">class:
issue: https://github.com/OpenEnergyPlatform/ontology/issues/439
pull request: https://github.com/OpenEnergyPlatform/ontology/pull/445
axioms:
issue: https://github.com/OpenEnergyPlatform/ontology/issues/703
pull request: https://github.com/OpenEnergyPlatform/ontology/pull/704</obo:IAO_0000233>
        <rdfs:label xml:lang="en">ethanol</rdfs:label>
    </owl:Class>
    


    <!-- http://openenergy-platform.org/ontology/oeo/OEO_00020003 -->

    <owl:Class rdf:about="http://openenergy-platform.org/ontology/oeo/OEO_00020003">
        <rdfs:subClassOf rdf:resource="http://openenergy-platform.org/ontology/oeo/OEO_00000419"/>
        <rdfs:subClassOf>
            <owl:Restriction>
                <owl:onProperty rdf:resource="http://openenergy-platform.org/ontology/oeo/OEO_00000532"/>
                <owl:someValuesFrom rdf:resource="http://openenergy-platform.org/ontology/oeo/OEO_00000150"/>
            </owl:Restriction>
        </rdfs:subClassOf>
        <rdfs:subClassOf>
            <owl:Restriction>
                <owl:onProperty rdf:resource="http://purl.obolibrary.org/obo/RO_0002234"/>
                <owl:someValuesFrom rdf:resource="http://openenergy-platform.org/ontology/oeo/OEO_00000150"/>
            </owl:Restriction>
        </rdfs:subClassOf>
        <obo:IAO_0000115>Energy transformation is a process in which one ore more certain types of energy as input result in certain types of energy as output.</obo:IAO_0000115>
        <obo:IAO_0000233>class added:
issue: https://github.com/OpenEnergyPlatform/ontology/issues/77
pull request: https://github.com/OpenEnergyPlatform/ontology/pull/371

make class a subclass of transformation:
issue: https://github.com/OpenEnergyPlatform/ontology/issues/435
pull request: https://github.com/OpenEnergyPlatform/ontology/pull/450

add input and output relations:
issue: https://github.com/OpenEnergyPlatform/ontology/issues/680
pull request: https://github.com/OpenEnergyPlatform/ontology/pull/690
pull request: https://github.com/OpenEnergyPlatform/ontology/pull/702</obo:IAO_0000233>
        <rdfs:label xml:lang="en">energy transformation</rdfs:label>
    </owl:Class>
    


    <!-- http://openenergy-platform.org/ontology/oeo/OEO_00020004 -->

    <owl:Class rdf:about="http://openenergy-platform.org/ontology/oeo/OEO_00020004">
        <rdfs:subClassOf rdf:resource="http://openenergy-platform.org/ontology/oeo/OEO_00000200"/>
        <rdfs:subClassOf>
            <owl:Restriction>
                <owl:onProperty rdf:resource="http://purl.obolibrary.org/obo/BFO_0000051"/>
                <owl:someValuesFrom rdf:resource="http://openenergy-platform.org/ontology/oeo/OEO_00020007"/>
            </owl:Restriction>
        </rdfs:subClassOf>
        <obo:IAO_0000115>A gas grid is a supply grid that distributes gaseous fuel, e.g. methane.</obo:IAO_0000115>
        <obo:IAO_0000233>issue: https://github.com/OpenEnergyPlatform/ontology/issues/36
pull request: https://github.com/OpenEnergyPlatform/ontology/385</obo:IAO_0000233>
        <rdfs:label xml:lang="en">gas grid</rdfs:label>
    </owl:Class>
    


    <!-- http://openenergy-platform.org/ontology/oeo/OEO_00020005 -->

    <owl:Class rdf:about="http://openenergy-platform.org/ontology/oeo/OEO_00020005">
        <rdfs:subClassOf rdf:resource="http://openenergy-platform.org/ontology/oeo/OEO_00000200"/>
        <rdfs:subClassOf>
            <owl:Restriction>
                <owl:onProperty rdf:resource="http://purl.obolibrary.org/obo/BFO_0000051"/>
                <owl:someValuesFrom rdf:resource="http://openenergy-platform.org/ontology/oeo/OEO_00020008"/>
            </owl:Restriction>
        </rdfs:subClassOf>
        <obo:IAO_0000115 xml:lang="en">A heating grid is a supply grid that distributes thermal energy via circulating steam or liquids.</obo:IAO_0000115>
        <obo:IAO_0000233>issue: https://github.com/OpenEnergyPlatform/ontology/issues/36
pull request: https://github.com/OpenEnergyPlatform/ontology/385</obo:IAO_0000233>
        <rdfs:label xml:lang="en">heating grid</rdfs:label>
    </owl:Class>
    


    <!-- http://openenergy-platform.org/ontology/oeo/OEO_00020006 -->

    <owl:Class rdf:about="http://openenergy-platform.org/ontology/oeo/OEO_00020006">
        <rdfs:subClassOf rdf:resource="http://openenergy-platform.org/ontology/oeo/OEO_00000061"/>
        <rdfs:subClassOf>
            <owl:Restriction>
                <owl:onProperty rdf:resource="http://purl.obolibrary.org/obo/BFO_0000050"/>
                <owl:someValuesFrom rdf:resource="http://openenergy-platform.org/ontology/oeo/OEO_00000200"/>
            </owl:Restriction>
        </rdfs:subClassOf>
        <obo:IAO_0000115 xml:lang="en">A grid component is an artificial object that is a discrete part of a supply grid serving a specific purpose.</obo:IAO_0000115>
        <obo:IAO_0000233>issue: https://github.com/OpenEnergyPlatform/ontology/issues/36
pull request: https://github.com/OpenEnergyPlatform/ontology/pull/385</obo:IAO_0000233>
        <rdfs:label xml:lang="en">grid component</rdfs:label>
    </owl:Class>
    


    <!-- http://openenergy-platform.org/ontology/oeo/OEO_00020007 -->

    <owl:Class rdf:about="http://openenergy-platform.org/ontology/oeo/OEO_00020007">
        <owl:equivalentClass>
            <owl:Class>
                <owl:intersectionOf rdf:parseType="Collection">
                    <rdf:Description rdf:about="http://openenergy-platform.org/ontology/oeo/OEO_00020006"/>
                    <owl:Restriction>
                        <owl:onProperty rdf:resource="http://purl.obolibrary.org/obo/BFO_0000050"/>
                        <owl:someValuesFrom rdf:resource="http://openenergy-platform.org/ontology/oeo/OEO_00020004"/>
                    </owl:Restriction>
                </owl:intersectionOf>
            </owl:Class>
        </owl:equivalentClass>
        <rdfs:subClassOf rdf:resource="http://openenergy-platform.org/ontology/oeo/OEO_00020006"/>
        <obo:IAO_0000115 xml:lang="en">A gas grid component is a grid component that is part of a gas grid.</obo:IAO_0000115>
        <obo:IAO_0000233 xml:lang="en">issue: https://github.com/OpenEnergyPlatform/ontology/issues/36
issue: https://github.com/OpenEnergyPlatform/ontology/issues/231
pull request: https://github.com/OpenEnergyPlatform/ontology/pull/385</obo:IAO_0000233>
        <rdfs:label xml:lang="en">gas grid component</rdfs:label>
    </owl:Class>
    


    <!-- http://openenergy-platform.org/ontology/oeo/OEO_00020008 -->

    <owl:Class rdf:about="http://openenergy-platform.org/ontology/oeo/OEO_00020008">
        <owl:equivalentClass>
            <owl:Class>
                <owl:intersectionOf rdf:parseType="Collection">
                    <rdf:Description rdf:about="http://openenergy-platform.org/ontology/oeo/OEO_00020006"/>
                    <owl:Restriction>
                        <owl:onProperty rdf:resource="http://purl.obolibrary.org/obo/BFO_0000050"/>
                        <owl:someValuesFrom rdf:resource="http://openenergy-platform.org/ontology/oeo/OEO_00020005"/>
                    </owl:Restriction>
                </owl:intersectionOf>
            </owl:Class>
        </owl:equivalentClass>
        <rdfs:subClassOf rdf:resource="http://openenergy-platform.org/ontology/oeo/OEO_00020006"/>
        <obo:IAO_0000115 xml:lang="en">A heating grid component is a grid component that is part of a heating grid.</obo:IAO_0000115>
        <obo:IAO_0000233 xml:lang="en">issue: https://github.com/OpenEnergyPlatform/ontology/issues/36
issue: https://github.com/OpenEnergyPlatform/ontology/issues/231
pull request: https://github.com/OpenEnergyPlatform/ontology/pull/385</obo:IAO_0000233>
        <rdfs:label xml:lang="en">heating grid component</rdfs:label>
    </owl:Class>
    


    <!-- http://openenergy-platform.org/ontology/oeo/OEO_00020009 -->

    <owl:Class rdf:about="http://openenergy-platform.org/ontology/oeo/OEO_00020009">
        <rdfs:subClassOf rdf:resource="http://openenergy-platform.org/ontology/oeo/OEO_00020006"/>
        <rdfs:subClassOf>
            <owl:Restriction>
                <owl:onProperty rdf:resource="http://purl.obolibrary.org/obo/BFO_0000050"/>
                <owl:someValuesFrom rdf:resource="http://openenergy-platform.org/ontology/oeo/OEO_00000143"/>
            </owl:Restriction>
        </rdfs:subClassOf>
        <rdfs:subClassOf>
            <owl:Restriction>
                <owl:onProperty rdf:resource="http://purl.obolibrary.org/obo/BFO_0000051"/>
                <owl:someValuesFrom rdf:resource="http://openenergy-platform.org/ontology/oeo/OEO_00000420"/>
            </owl:Restriction>
        </rdfs:subClassOf>
        <obo:IAO_0000115 xml:lang="en">A switchyard is an electricity grid component that connects different levels of voltage</obo:IAO_0000115>
        <obo:IAO_0000233 xml:lang="en">issue: https://github.com/OpenEnergyPlatform/ontology/issues/231
pull request: https://github.com/OpenEnergyPlatform/ontology/pull/385</obo:IAO_0000233>
        <rdfs:label xml:lang="en">switchyard</rdfs:label>
    </owl:Class>
    


    <!-- http://openenergy-platform.org/ontology/oeo/OEO_00020037 -->

    <owl:Class rdf:about="http://openenergy-platform.org/ontology/oeo/OEO_00020037">
        <rdfs:subClassOf rdf:resource="http://purl.obolibrary.org/obo/BFO_0000015"/>
        <rdfs:subClassOf>
            <owl:Restriction>
                <owl:onProperty rdf:resource="http://purl.obolibrary.org/obo/RO_0000057"/>
                <owl:someValuesFrom rdf:resource="http://openenergy-platform.org/ontology/oeo/OEO_00230021"/>
            </owl:Restriction>
        </rdfs:subClassOf>
        <obo:IAO_0000115>Radiation is the process of emitting or transmitting energy in the form of waves or particles through a spatial region or a material entity.</obo:IAO_0000115>
        <obo:IAO_0000119>Adaptation of https://en.wikipedia.org/w/index.php?title=Radiation&amp;oldid=986678480</obo:IAO_0000119>
        <obo:IAO_0000233>issue: https://github.com/OpenEnergyPlatform/ontology/issues/362
pull request: https://github.com/OpenEnergyPlatform/ontology/pull/600</obo:IAO_0000233>
        <rdfs:label>radiation</rdfs:label>
    </owl:Class>
    


    <!-- http://openenergy-platform.org/ontology/oeo/OEO_00020038 -->

    <owl:Class rdf:about="http://openenergy-platform.org/ontology/oeo/OEO_00020038">
        <rdfs:subClassOf rdf:resource="http://openenergy-platform.org/ontology/oeo/OEO_00020037"/>
        <obo:IAO_0000115>Solar radiation is radiation that is emitted by the sun.</obo:IAO_0000115>
        <obo:IAO_0000233>issue: https://github.com/OpenEnergyPlatform/ontology/issues/362
pull request: https://github.com/OpenEnergyPlatform/ontology/pull/600</obo:IAO_0000233>
        <rdfs:label>solar radiation</rdfs:label>
    </owl:Class>
    


    <!-- http://openenergy-platform.org/ontology/oeo/OEO_00020039 -->

    <owl:Class rdf:about="http://openenergy-platform.org/ontology/oeo/OEO_00020039">
        <owl:equivalentClass>
            <owl:Class>
                <owl:intersectionOf rdf:parseType="Collection">
                    <rdf:Description rdf:about="http://purl.obolibrary.org/obo/BFO_0000040"/>
                    <owl:Restriction>
                        <owl:onProperty rdf:resource="http://purl.obolibrary.org/obo/RO_0000091"/>
                        <owl:someValuesFrom rdf:resource="http://openenergy-platform.org/ontology/oeo/OEO_00000151"/>
                    </owl:Restriction>
                </owl:intersectionOf>
            </owl:Class>
        </owl:equivalentClass>
        <rdfs:subClassOf rdf:resource="http://purl.obolibrary.org/obo/BFO_0000040"/>
        <obo:IAO_0000115>An energy carrier is a material entity that has the disposition energy carrier disposition.</obo:IAO_0000115>
        <obo:IAO_0000233>issue: https://github.com/OpenEnergyPlatform/ontology/issues/407
pull request: https://github.com/OpenEnergyPlatform/ontology/pull/627</obo:IAO_0000233>
        <rdfs:label>energy carrier</rdfs:label>
    </owl:Class>
    


    <!-- http://openenergy-platform.org/ontology/oeo/OEO_00020040 -->

    <owl:Class rdf:about="http://openenergy-platform.org/ontology/oeo/OEO_00020040">
        <rdfs:subClassOf rdf:resource="http://openenergy-platform.org/ontology/oeo/OEO_00000150"/>
        <obo:IAO_0000115>Radiative energy is energy that has been transmitted by a radiation process.</obo:IAO_0000115>
        <obo:IAO_0000233>issue: https://github.com/OpenEnergyPlatform/ontology/issues/660
pull request: https://github.com/OpenEnergyPlatform/ontology/pull/665</obo:IAO_0000233>
        <rdfs:label>radiative energy</rdfs:label>
    </owl:Class>
    


    <!-- http://openenergy-platform.org/ontology/oeo/OEO_00020043 -->

    <owl:Class rdf:about="http://openenergy-platform.org/ontology/oeo/OEO_00020043">
        <rdfs:subClassOf rdf:resource="http://openenergy-platform.org/ontology/oeo/OEO_00020003"/>
        <rdfs:subClassOf>
            <owl:Restriction>
                <owl:onProperty rdf:resource="http://openenergy-platform.org/ontology/oeo/OEO_00000532"/>
                <owl:someValuesFrom rdf:resource="http://openenergy-platform.org/ontology/oeo/OEO_00000446"/>
            </owl:Restriction>
        </rdfs:subClassOf>
        <rdfs:subClassOf>
            <owl:Restriction>
                <owl:onProperty rdf:resource="http://purl.obolibrary.org/obo/RO_0000057"/>
                <owl:someValuesFrom rdf:resource="http://openenergy-platform.org/ontology/oeo/OEO_00000044"/>
            </owl:Restriction>
        </rdfs:subClassOf>
        <rdfs:subClassOf>
            <owl:Restriction>
                <owl:onProperty rdf:resource="http://purl.obolibrary.org/obo/RO_0002234"/>
                <owl:someValuesFrom rdf:resource="http://openenergy-platform.org/ontology/oeo/OEO_00000139"/>
            </owl:Restriction>
        </rdfs:subClassOf>
        <obo:IAO_0000115>Wind energy transformation is an energy transformation that converts wind energy to electrical energy.</obo:IAO_0000115>
        <obo:IAO_0000233>issue: https://github.com/OpenEnergyPlatform/ontology/issues/662
pull request: https://github.com/OpenEnergyPlatform/ontology/pull/666
pull request: https://github.com/OpenEnergyPlatform/ontology/pull/702</obo:IAO_0000233>
        <rdfs:label>wind energy transformation</rdfs:label>
    </owl:Class>
    


    <!-- http://openenergy-platform.org/ontology/oeo/OEO_00020045 -->

    <owl:Class rdf:about="http://openenergy-platform.org/ontology/oeo/OEO_00020045">
        <rdfs:subClassOf rdf:resource="http://openenergy-platform.org/ontology/oeo/OEO_00000150"/>
        <obo:IAO_0000233>issue: https://github.com/OpenEnergyPlatform/ontology/issues/628
pull request: https://github.com/OpenEnergyPlatform/ontology/pull/670</obo:IAO_0000233>
        <rdfs:comment>Potential energy is the energy that a material entity contains due to its position relative to other material entities or to stresses within itself.</rdfs:comment>
        <rdfs:label>potential energy</rdfs:label>
    </owl:Class>
    


    <!-- http://openenergy-platform.org/ontology/oeo/OEO_00020046 -->

    <owl:Class rdf:about="http://openenergy-platform.org/ontology/oeo/OEO_00020046">
        <rdfs:subClassOf rdf:resource="http://openenergy-platform.org/ontology/oeo/OEO_00020003"/>
        <rdfs:subClassOf>
            <owl:Restriction>
                <owl:onProperty rdf:resource="http://openenergy-platform.org/ontology/oeo/OEO_00000532"/>
                <owl:someValuesFrom rdf:resource="http://openenergy-platform.org/ontology/oeo/OEO_00000384"/>
            </owl:Restriction>
        </rdfs:subClassOf>
        <obo:IAO_0000115>Solar energy transformation is an energy transformation that converts solar energy.</obo:IAO_0000115>
        <obo:IAO_0000233>class:
issue: https://github.com/OpenEnergyPlatform/ontology/issues/663
pull request: https://github.com/OpenEnergyPlatform/ontology/pull/672
has input relation:
issue: https://github.com/OpenEnergyPlatform/ontology/issues/668
pull request: https://github.com/OpenEnergyPlatform/ontology/pull/701</obo:IAO_0000233>
        <rdfs:label>solar energy transformation</rdfs:label>
    </owl:Class>
    


    <!-- http://openenergy-platform.org/ontology/oeo/OEO_00020047 -->

    <owl:Class rdf:about="http://openenergy-platform.org/ontology/oeo/OEO_00020047">
        <rdfs:subClassOf rdf:resource="http://openenergy-platform.org/ontology/oeo/OEO_00020046"/>
        <rdfs:subClassOf>
            <owl:Restriction>
                <owl:onProperty rdf:resource="http://purl.obolibrary.org/obo/RO_0000057"/>
                <owl:someValuesFrom rdf:resource="http://openenergy-platform.org/ontology/oeo/OEO_00000387"/>
            </owl:Restriction>
        </rdfs:subClassOf>
        <obo:IAO_0000115>Solar thermal energy transformation is a solar energy transformation that converts solar energy into thermal energy.</obo:IAO_0000115>
        <obo:IAO_0000233>issue: https://github.com/OpenEnergyPlatform/ontology/issues/663
pull request: https://github.com/OpenEnergyPlatform/ontology/pull/672</obo:IAO_0000233>
        <rdfs:label>solar thermal energy transformation</rdfs:label>
    </owl:Class>
    


    <!-- http://openenergy-platform.org/ontology/oeo/OEO_00020048 -->

    <owl:Class rdf:about="http://openenergy-platform.org/ontology/oeo/OEO_00020048">
        <rdfs:subClassOf rdf:resource="http://openenergy-platform.org/ontology/oeo/OEO_00020046"/>
        <rdfs:subClassOf>
            <owl:Restriction>
                <owl:onProperty rdf:resource="http://purl.obolibrary.org/obo/RO_0000057"/>
                <owl:someValuesFrom rdf:resource="http://openenergy-platform.org/ontology/oeo/OEO_00000032"/>
            </owl:Restriction>
        </rdfs:subClassOf>
        <obo:IAO_0000115>Photovoltaic energy transformation is a solar energy transformation that converts solar energy into electrical energy.</obo:IAO_0000115>
        <obo:IAO_0000233>issue: https://github.com/OpenEnergyPlatform/ontology/issues/663
pull request: https://github.com/OpenEnergyPlatform/ontology/pull/672</obo:IAO_0000233>
        <rdfs:label>photovoltaic energy transformation</rdfs:label>
    </owl:Class>
    


    <!-- http://openenergy-platform.org/ontology/oeo/OEO_00020050 -->

    <owl:Class rdf:about="http://openenergy-platform.org/ontology/oeo/OEO_00020050">
        <owl:equivalentClass>
            <owl:Class>
                <owl:intersectionOf rdf:parseType="Collection">
                    <owl:Restriction>
                        <owl:onProperty rdf:resource="http://openenergy-platform.org/ontology/oeo/OEO_00000530"/>
                        <owl:someValuesFrom rdf:resource="http://openenergy-platform.org/ontology/oeo/OEO_00030004"/>
                    </owl:Restriction>
                    <owl:Restriction>
                        <owl:onProperty rdf:resource="http://purl.obolibrary.org/obo/RO_0000091"/>
                        <owl:someValuesFrom rdf:resource="http://openenergy-platform.org/ontology/oeo/OEO_00000151"/>
                    </owl:Restriction>
                </owl:intersectionOf>
            </owl:Class>
        </owl:equivalentClass>
        <rdfs:subClassOf rdf:resource="http://openenergy-platform.org/ontology/oeo/OEO_00020039"/>
        <obo:IAO_0000115>A renewable energy carrier is an energy carrier that has a renewable origin.</obo:IAO_0000115>
        <obo:IAO_0000233>issue: https://github.com/OpenEnergyPlatform/ontology/issues/515
pull request: https://github.com/OpenEnergyPlatform/ontology/pull/684</obo:IAO_0000233>
        <rdfs:label>renewable energy carrier</rdfs:label>
    </owl:Class>
    


    <!-- http://openenergy-platform.org/ontology/oeo/OEO_00020053 -->

    <owl:Class rdf:about="http://openenergy-platform.org/ontology/oeo/OEO_00020053">
        <rdfs:subClassOf rdf:resource="http://purl.obolibrary.org/obo/BFO_0000015"/>
        <rdfs:subClassOf>
            <owl:Restriction>
                <owl:onProperty rdf:resource="http://purl.obolibrary.org/obo/RO_0000057"/>
                <owl:someValuesFrom rdf:resource="http://openenergy-platform.org/ontology/oeo/OEO_00000302"/>
            </owl:Restriction>
        </rdfs:subClassOf>
        <obo:IAO_0000115>Nuclear fission is a process of nuclear reaction or a radioactive decay in which the nucleus of an atom splits into two or more smaller, lighter nuclei.</obo:IAO_0000115>
        <obo:IAO_0000233>issue: https://github.com/OpenEnergyPlatform/ontology/issues/692
pull request: https://github.com/OpenEnergyPlatform/ontology/pull/698</obo:IAO_0000233>
        <rdfs:label>nuclear fission</rdfs:label>
    </owl:Class>
    


    <!-- http://openenergy-platform.org/ontology/oeo/OEO_00020054 -->

    <owl:Class rdf:about="http://openenergy-platform.org/ontology/oeo/OEO_00020054">
        <rdfs:subClassOf rdf:resource="http://openenergy-platform.org/ontology/oeo/OEO_00020003"/>
        <rdfs:subClassOf>
            <owl:Restriction>
                <owl:onProperty rdf:resource="http://openenergy-platform.org/ontology/oeo/OEO_00000532"/>
                <owl:someValuesFrom rdf:resource="http://openenergy-platform.org/ontology/oeo/OEO_00000300"/>
            </owl:Restriction>
        </rdfs:subClassOf>
        <rdfs:subClassOf>
            <owl:Restriction>
                <owl:onProperty rdf:resource="http://purl.obolibrary.org/obo/RO_0002234"/>
                <owl:someValuesFrom rdf:resource="http://openenergy-platform.org/ontology/oeo/OEO_00000207"/>
            </owl:Restriction>
        </rdfs:subClassOf>
        <obo:IAO_0000115>Nuclear energy transformation is an energy transformation that converts nuclear binding energy to thermal energy.</obo:IAO_0000115>
        <obo:IAO_0000233>issue: https://github.com/OpenEnergyPlatform/ontology/issues/692
pull request: https://github.com/OpenEnergyPlatform/ontology/pull/698
pull request: https://github.com/OpenEnergyPlatform/ontology/pull/702</obo:IAO_0000233>
        <rdfs:label>nuclear energy transformation</rdfs:label>
    </owl:Class>
    


    <!-- http://openenergy-platform.org/ontology/oeo/OEO_00020058 -->

    <owl:Class rdf:about="http://openenergy-platform.org/ontology/oeo/OEO_00020058">
        <rdfs:subClassOf rdf:resource="http://openenergy-platform.org/ontology/oeo/OEO_00000331"/>
        <rdfs:subClassOf>
            <owl:Restriction>
                <owl:onProperty rdf:resource="http://openenergy-platform.org/ontology/oeo/OEO_00000530"/>
                <owl:someValuesFrom rdf:resource="http://openenergy-platform.org/ontology/oeo/OEO_00030003"/>
            </owl:Restriction>
        </rdfs:subClassOf>
        <rdfs:subClassOf>
            <owl:Restriction>
                <owl:onProperty rdf:resource="http://openenergy-platform.org/ontology/oeo/OEO_00000530"/>
                <owl:someValuesFrom rdf:resource="http://openenergy-platform.org/ontology/oeo/OEO_00030004"/>
            </owl:Restriction>
        </rdfs:subClassOf>
        <rdfs:subClassOf>
            <owl:Restriction>
                <owl:onProperty rdf:resource="http://purl.obolibrary.org/obo/RO_0000091"/>
                <owl:someValuesFrom rdf:resource="http://openenergy-platform.org/ontology/oeo/OEO_00000151"/>
            </owl:Restriction>
        </rdfs:subClassOf>
        <rdfs:subClassOf>
            <owl:Restriction>
                <owl:onProperty rdf:resource="http://openenergy-platform.org/ontology/oeo/OEO_00000529"/>
                <owl:hasValue rdf:resource="http://openenergy-platform.org/ontology/oeo/OEO_00000390"/>
            </owl:Restriction>
        </rdfs:subClassOf>
        <obo:IAO_0000115>A rock is a portion of matter that is a naturally occurring solid aggregate of minerals or mineraloid matter that is part of the earth&apos;s crust.</obo:IAO_0000115>
        <obo:IAO_0000233>issue: https://github.com/OpenEnergyPlatform/ontology/issues/727
pull request: https://github.com/OpenEnergyPlatform/ontology/pull/739</obo:IAO_0000233>
        <rdfs:label>rock</rdfs:label>
    </owl:Class>
    


    <!-- http://openenergy-platform.org/ontology/oeo/OEO_00020059 -->

    <owl:Class rdf:about="http://openenergy-platform.org/ontology/oeo/OEO_00020059">
        <rdfs:subClassOf rdf:resource="http://openenergy-platform.org/ontology/oeo/OEO_00140101"/>
        <rdfs:subClassOf>
            <owl:Restriction>
                <owl:onProperty rdf:resource="http://openenergy-platform.org/ontology/oeo/OEO_00000532"/>
                <owl:allValuesFrom rdf:resource="http://openenergy-platform.org/ontology/oeo/OEO_00000191"/>
            </owl:Restriction>
        </rdfs:subClassOf>
        <obo:IAO_0000115>Geothermal heat transfer is a heat transfer from the earth crust to a transportable material entity. E.g. a liquid or gas.</obo:IAO_0000115>
        <obo:IAO_0000233>issue: https://github.com/OpenEnergyPlatform/ontology/issues/727
pull request: https://github.com/OpenEnergyPlatform/ontology/pull/739</obo:IAO_0000233>
        <rdfs:label>geothermal heat transfer</rdfs:label>
    </owl:Class>
    


    <!-- http://openenergy-platform.org/ontology/oeo/OEO_00030000 -->

    <owl:Class rdf:about="http://openenergy-platform.org/ontology/oeo/OEO_00030000">
        <rdfs:subClassOf rdf:resource="http://openenergy-platform.org/ontology/oeo/OEO_00000316"/>
        <obo:IAO_0000115>anthropogenic is an origin of portions of matter or energies created by human activity.</obo:IAO_0000115>
        <obo:IAO_0000233>include &quot;or energies&quot;
issue: https://github.com/OpenEnergyPlatform/ontology/issues/728
pull request: https://github.com/OpenEnergyPlatform/ontology/pull/742</obo:IAO_0000233>
        <obo:IAO_0000233>issue: https://github.com/OpenEnergyPlatform/ontology/issues/56
pull request: https://github.com/OpenEnergyPlatform/ontology/pull/234</obo:IAO_0000233>
        <rdfs:label>anthropogenic</rdfs:label>
    </owl:Class>
    


    <!-- http://openenergy-platform.org/ontology/oeo/OEO_00030001 -->

    <owl:Class rdf:about="http://openenergy-platform.org/ontology/oeo/OEO_00030001">
        <rdfs:subClassOf rdf:resource="http://openenergy-platform.org/ontology/oeo/OEO_00000316"/>
        <obo:IAO_0000115>biogenic is an origin of portions of matter made by or produced from life forms.</obo:IAO_0000115>
        <obo:IAO_0000233>issue: https://github.com/OpenEnergyPlatform/ontology/issues/108
pull request: https://github.com/OpenEnergyPlatform/ontology/pull/130</obo:IAO_0000233>
        <rdfs:label>biogenic</rdfs:label>
    </owl:Class>
    


    <!-- http://openenergy-platform.org/ontology/oeo/OEO_00030002 -->

    <owl:Class rdf:about="http://openenergy-platform.org/ontology/oeo/OEO_00030002">
        <rdfs:subClassOf rdf:resource="http://openenergy-platform.org/ontology/oeo/OEO_00030003"/>
        <obo:IAO_0000115>fossil is an origin of portions of matter created from organic material by geolocial processes lasting thousands or millions of years.

In real world, fossils are from biogenic origin some thousands or millions of years ago. However, this is irrelevant in the energy modelling domain.</obo:IAO_0000115>
        <obo:IAO_0000233>issue: https://github.com/OpenEnergyPlatform/ontology/issues/108
pull request: https://github.com/OpenEnergyPlatform/ontology/pull/130</obo:IAO_0000233>
        <rdfs:label>fossil</rdfs:label>
    </owl:Class>
    


    <!-- http://openenergy-platform.org/ontology/oeo/OEO_00030003 -->

    <owl:Class rdf:about="http://openenergy-platform.org/ontology/oeo/OEO_00030003">
        <rdfs:subClassOf rdf:resource="http://openenergy-platform.org/ontology/oeo/OEO_00000316"/>
        <obo:IAO_0000115>geogenic is an origin of portions of matter that are the result of geological processes.</obo:IAO_0000115>
        <obo:IAO_0000233>issue: https://github.com/OpenEnergyPlatform/ontology/issues/182
pull request: https://github.com/OpenEnergyPlatform/ontology/pull/237</obo:IAO_0000233>
        <rdfs:label>geogenic</rdfs:label>
    </owl:Class>
    


    <!-- http://openenergy-platform.org/ontology/oeo/OEO_00030004 -->

    <owl:Class rdf:about="http://openenergy-platform.org/ontology/oeo/OEO_00030004">
        <rdfs:subClassOf rdf:resource="http://openenergy-platform.org/ontology/oeo/OEO_00000316"/>
        <obo:IAO_0000115>Renewable is an origin of portions of matter or energies that replenish on a human time scale.</obo:IAO_0000115>
        <obo:IAO_0000233>include &quot;or energies&quot;
issue: https://github.com/OpenEnergyPlatform/ontology/issues/728
pull request: https://github.com/OpenEnergyPlatform/ontology/pull/742</obo:IAO_0000233>
        <obo:IAO_0000233>issue: https://github.com/OpenEnergyPlatform/ontology/issues/397
pull request: https://github.com/OpenEnergyPlatform/ontology/pull/398
issue: https://github.com/OpenEnergyPlatform/ontology/issues/108
pull request: https://github.com/OpenEnergyPlatform/ontology/pull/130</obo:IAO_0000233>
        <rdfs:label>renewable</rdfs:label>
    </owl:Class>
    


    <!-- http://openenergy-platform.org/ontology/oeo/OEO_00030005 -->

    <owl:Class rdf:about="http://openenergy-platform.org/ontology/oeo/OEO_00030005">
        <rdfs:subClassOf rdf:resource="http://openenergy-platform.org/ontology/oeo/OEO_00000316"/>
        <obo:IAO_0000115>synthetic is an origin of portions of matter created artifically by a chemical process.</obo:IAO_0000115>
        <obo:IAO_0000233>issue: https://github.com/OpenEnergyPlatform/ontology/issues/108
pull request: https://github.com/OpenEnergyPlatform/ontology/pull/130</obo:IAO_0000233>
        <rdfs:label>synthetic</rdfs:label>
    </owl:Class>
    


    <!-- http://openenergy-platform.org/ontology/oeo/OEO_00030019 -->

    <owl:Class rdf:about="http://openenergy-platform.org/ontology/oeo/OEO_00030019">
        <rdfs:subClassOf rdf:resource="http://purl.obolibrary.org/obo/BFO_0000003"/>
        <obo:IAO_0000115>A process attribute is a dependent occurrent that existentially depends on a process.</obo:IAO_0000115>
        <obo:IAO_0000233>issue: https://github.com/OpenEnergyPlatform/ontology/issues/205
pull request: https://github.com/OpenEnergyPlatform/ontology/pull/386</obo:IAO_0000233>
        <rdfs:label>process attribute</rdfs:label>
    </owl:Class>
    


    <!-- http://openenergy-platform.org/ontology/oeo/OEO_00030024 -->

    <owl:Class rdf:about="http://openenergy-platform.org/ontology/oeo/OEO_00030024">
        <rdfs:subClassOf rdf:resource="http://purl.obolibrary.org/obo/RO_0002577"/>
        <obo:IAO_0000115>An energy system is a system of spatially extended linked energy sources and sinks.</obo:IAO_0000115>
        <obo:IAO_0000233>issue: https://github.com/OpenEnergyPlatform/ontology/issues/432
pull request: https://github.com/OpenEnergyPlatform/ontology/pull/493</obo:IAO_0000233>
        <rdfs:label>energy system</rdfs:label>
    </owl:Class>
    


    <!-- http://openenergy-platform.org/ontology/oeo/OEO_00030025 -->

    <owl:Class rdf:about="http://openenergy-platform.org/ontology/oeo/OEO_00030025">
        <rdfs:subClassOf rdf:resource="http://purl.obolibrary.org/obo/RO_0002577"/>
        <obo:IAO_0000115>A supply system is a system that connects producers and consumers.</obo:IAO_0000115>
        <obo:IAO_0000233>issue: https://github.com/OpenEnergyPlatform/ontology/issues/432
pull request: https://github.com/OpenEnergyPlatform/ontology/pull/493</obo:IAO_0000233>
        <rdfs:label>supply system</rdfs:label>
    </owl:Class>
    


    <!-- http://openenergy-platform.org/ontology/oeo/OEO_00030026 -->

    <owl:Class rdf:about="http://openenergy-platform.org/ontology/oeo/OEO_00030026">
        <rdfs:subClassOf rdf:resource="http://purl.obolibrary.org/obo/BFO_0000015"/>
        <obo:IAO_0000115>Primary energy production is a process that prepares raw material for its use as primary energy carrier.</obo:IAO_0000115>
        <obo:IAO_0000233>issue: https://github.com/OpenEnergyPlatform/ontology/issues/77
pull request: https://github.com/OpenEnergyPlatform/ontology/pull/498</obo:IAO_0000233>
        <rdfs:label>primary energy production</rdfs:label>
    </owl:Class>
    


    <!-- http://openenergy-platform.org/ontology/oeo/OEO_00030027 -->

    <owl:Class rdf:about="http://openenergy-platform.org/ontology/oeo/OEO_00030027">
        <rdfs:subClassOf rdf:resource="http://openenergy-platform.org/ontology/oeo/OEO_00030026"/>
        <obo:IAO_0000115>Primary energy carrier mining is a primary energy production process that recovers non-renewable energy carriers from its natural site.</obo:IAO_0000115>
        <obo:IAO_0000233>issue: https://github.com/OpenEnergyPlatform/ontology/issues/77
pull request: https://github.com/OpenEnergyPlatform/ontology/pull/498</obo:IAO_0000233>
        <rdfs:label>primary energy carrier mining</rdfs:label>
    </owl:Class>
    


    <!-- http://openenergy-platform.org/ontology/oeo/OEO_00030028 -->

    <owl:Class rdf:about="http://openenergy-platform.org/ontology/oeo/OEO_00030028">
        <rdfs:subClassOf rdf:resource="http://openenergy-platform.org/ontology/oeo/OEO_00030026"/>
        <obo:IAO_0000115>Primary energy carrier harvest is a primary energy production process that collects solid biomass from its natural site.</obo:IAO_0000115>
        <obo:IAO_0000233>issue: https://github.com/OpenEnergyPlatform/ontology/issues/77
pull request: https://github.com/OpenEnergyPlatform/ontology/pull/498</obo:IAO_0000233>
        <rdfs:label>primary energy carrier harvest</rdfs:label>
    </owl:Class>
    


    <!-- http://openenergy-platform.org/ontology/oeo/OEO_00050000 -->

    <owl:Class rdf:about="http://openenergy-platform.org/ontology/oeo/OEO_00050000">
        <rdfs:subClassOf rdf:resource="http://purl.obolibrary.org/obo/BFO_0000015"/>
        <rdfs:subClassOf>
            <owl:Restriction>
                <owl:onProperty rdf:resource="http://purl.obolibrary.org/obo/RO_0002234"/>
                <owl:someValuesFrom>
                    <owl:Class>
                        <owl:unionOf rdf:parseType="Collection">
                            <rdf:Description rdf:about="http://purl.obolibrary.org/obo/BFO_0000027"/>
                            <rdf:Description rdf:about="http://purl.obolibrary.org/obo/BFO_0000030"/>
                        </owl:unionOf>
                    </owl:Class>
                </owl:someValuesFrom>
            </owl:Restriction>
        </rdfs:subClassOf>
        <obo:IAO_0000115>An industrial process is a process that has output object or object aggregates that are economic goods. An industrial process consists of several subprocesses. Examples of subprocesses that can be involved in an industrial process are energy transformations, mechanical operations and chemical reactions.</obo:IAO_0000115>
        <obo:IAO_0000233>issue: https://github.com/OpenEnergyPlatform/ontology/issues/534
pull request: https://github.com/OpenEnergyPlatform/ontology/pull/589</obo:IAO_0000233>
        <rdfs:label xml:lang="en">industrial process</rdfs:label>
    </owl:Class>
    


    <!-- http://openenergy-platform.org/ontology/oeo/OEO_00050001 -->

    <owl:Class rdf:about="http://openenergy-platform.org/ontology/oeo/OEO_00050001">
        <rdfs:subClassOf rdf:resource="http://openenergy-platform.org/ontology/oeo/OEO_00000419"/>
        <rdfs:subClassOf>
            <owl:Restriction>
                <owl:onProperty rdf:resource="http://openenergy-platform.org/ontology/oeo/OEO_00000500"/>
                <owl:someValuesFrom rdf:resource="http://openenergy-platform.org/ontology/oeo/OEO_00000148"/>
            </owl:Restriction>
        </rdfs:subClassOf>
        <rdfs:subClassOf>
            <owl:Restriction>
                <owl:onProperty rdf:resource="http://purl.obolibrary.org/obo/BFO_0000051"/>
                <owl:someValuesFrom rdf:resource="http://openenergy-platform.org/ontology/oeo/OEO_00000147"/>
            </owl:Restriction>
        </rdfs:subClassOf>
        <rdfs:subClassOf>
            <owl:Restriction>
                <owl:onProperty rdf:resource="http://purl.obolibrary.org/obo/BFO_0000051"/>
                <owl:someValuesFrom rdf:resource="http://openenergy-platform.org/ontology/oeo/OEO_00020003"/>
            </owl:Restriction>
        </rdfs:subClassOf>
        <rdfs:subClassOf>
            <owl:Restriction>
                <owl:onProperty rdf:resource="http://purl.obolibrary.org/obo/RO_0000057"/>
                <owl:someValuesFrom rdf:resource="http://openenergy-platform.org/ontology/oeo/OEO_00000174"/>
            </owl:Restriction>
        </rdfs:subClassOf>
        <rdfs:subClassOf>
            <owl:Restriction>
                <owl:onProperty rdf:resource="http://purl.obolibrary.org/obo/RO_0000057"/>
                <owl:someValuesFrom rdf:resource="http://openenergy-platform.org/ontology/oeo/OEO_00000175"/>
            </owl:Restriction>
        </rdfs:subClassOf>
        <obo:IAO_0000115>Fuel-powered electricity generation is a transformation that contains at least two sub process: An energy transformation of chemical energy from fuel into electrical energy and an emission process.</obo:IAO_0000115>
        <obo:IAO_0000233>issue: https://github.com/OpenEnergyPlatform/ontology/issues/582
pull request: https://github.com/OpenEnergyPlatform/ontology/pull/592</obo:IAO_0000233>
        <rdfs:label xml:lang="en">fuel-powered electricity generation</rdfs:label>
    </owl:Class>
    


    <!-- http://openenergy-platform.org/ontology/oeo/OEO_00050002 -->

    <owl:Class rdf:about="http://openenergy-platform.org/ontology/oeo/OEO_00050002">
        <rdfs:subClassOf rdf:resource="http://purl.obolibrary.org/obo/UO_0000111"/>
        <obo:IAO_0000115>An energy unit which is equal to 1,000 joules.</obo:IAO_0000115>
        <obo:IAO_0000233>issue: https://github.com/OpenEnergyPlatform/ontology/issues/606
pull request: https://github.com/OpenEnergyPlatform/ontology/pull/608</obo:IAO_0000233>
        <oboInOwl:hasExactSynonym>kJ</oboInOwl:hasExactSynonym>
        <rdfs:label xml:lang="en">kilojoule</rdfs:label>
    </owl:Class>
    


    <!-- http://openenergy-platform.org/ontology/oeo/OEO_00050003 -->

    <owl:Class rdf:about="http://openenergy-platform.org/ontology/oeo/OEO_00050003">
        <rdfs:subClassOf rdf:resource="http://purl.obolibrary.org/obo/UO_0000111"/>
        <obo:IAO_0000115>An energy unit which is equal to 1,000,000 joules.</obo:IAO_0000115>
        <obo:IAO_0000233>issue: https://github.com/OpenEnergyPlatform/ontology/issues/606
pull request: https://github.com/OpenEnergyPlatform/ontology/pull/608</obo:IAO_0000233>
        <oboInOwl:hasExactSynonym>MJ</oboInOwl:hasExactSynonym>
        <rdfs:label xml:lang="en">megajoule</rdfs:label>
    </owl:Class>
    


    <!-- http://openenergy-platform.org/ontology/oeo/OEO_00050004 -->

    <owl:Class rdf:about="http://openenergy-platform.org/ontology/oeo/OEO_00050004">
        <rdfs:subClassOf rdf:resource="http://purl.obolibrary.org/obo/UO_0000111"/>
        <obo:IAO_0000115>An energy unit which is equal to 10^9 joules.</obo:IAO_0000115>
        <obo:IAO_0000233>issue: https://github.com/OpenEnergyPlatform/ontology/issues/606
pull request: https://github.com/OpenEnergyPlatform/ontology/pull/608</obo:IAO_0000233>
        <oboInOwl:hasExactSynonym>GJ</oboInOwl:hasExactSynonym>
        <rdfs:label xml:lang="en">gigajoule</rdfs:label>
    </owl:Class>
    


    <!-- http://openenergy-platform.org/ontology/oeo/OEO_00050005 -->

    <owl:Class rdf:about="http://openenergy-platform.org/ontology/oeo/OEO_00050005">
        <rdfs:subClassOf rdf:resource="http://purl.obolibrary.org/obo/UO_0000111"/>
        <obo:IAO_0000115>An energy unit which is equal to 10^12 joules.</obo:IAO_0000115>
        <obo:IAO_0000233>issue: https://github.com/OpenEnergyPlatform/ontology/issues/606
pull request: https://github.com/OpenEnergyPlatform/ontology/pull/608</obo:IAO_0000233>
        <oboInOwl:hasExactSynonym>TJ</oboInOwl:hasExactSynonym>
        <rdfs:label xml:lang="en">terajoule</rdfs:label>
    </owl:Class>
    


    <!-- http://openenergy-platform.org/ontology/oeo/OEO_00050006 -->

    <owl:Class rdf:about="http://openenergy-platform.org/ontology/oeo/OEO_00050006">
        <rdfs:subClassOf rdf:resource="http://purl.obolibrary.org/obo/UO_0000111"/>
        <obo:IAO_0000115>An energy unit which is equal to 10^15 joules.</obo:IAO_0000115>
        <obo:IAO_0000233>issue: https://github.com/OpenEnergyPlatform/ontology/issues/606
pull request: https://github.com/OpenEnergyPlatform/ontology/pull/608</obo:IAO_0000233>
        <oboInOwl:hasExactSynonym>PJ</oboInOwl:hasExactSynonym>
        <rdfs:label xml:lang="en">petajoule</rdfs:label>
    </owl:Class>
    


    <!-- http://openenergy-platform.org/ontology/oeo/OEO_00050007 -->

    <owl:Class rdf:about="http://openenergy-platform.org/ontology/oeo/OEO_00050007">
        <rdfs:subClassOf rdf:resource="http://purl.obolibrary.org/obo/UO_0000111"/>
        <obo:IAO_0000115>An energy unit which is equal to 10^18 joules.</obo:IAO_0000115>
        <obo:IAO_0000233>issue: https://github.com/OpenEnergyPlatform/ontology/issues/606
pull request: https://github.com/OpenEnergyPlatform/ontology/pull/608</obo:IAO_0000233>
        <oboInOwl:hasExactSynonym>EJ</oboInOwl:hasExactSynonym>
        <rdfs:label xml:lang="en">exajoule</rdfs:label>
    </owl:Class>
    


    <!-- http://openenergy-platform.org/ontology/oeo/OEO_00050008 -->

    <owl:Class rdf:about="http://openenergy-platform.org/ontology/oeo/OEO_00050008">
        <rdfs:subClassOf rdf:resource="http://purl.obolibrary.org/obo/UO_0000111"/>
        <obo:IAO_0000115>An energy unit which is equal to 1,000,000 watt-hours.</obo:IAO_0000115>
        <obo:IAO_0000233>issue: https://github.com/OpenEnergyPlatform/ontology/issues/606
pull request: https://github.com/OpenEnergyPlatform/ontology/pull/608</obo:IAO_0000233>
        <oboInOwl:hasExactSynonym>MWh</oboInOwl:hasExactSynonym>
        <rdfs:label xml:lang="en">megawatt-hour</rdfs:label>
    </owl:Class>
    


    <!-- http://openenergy-platform.org/ontology/oeo/OEO_00050009 -->

    <owl:Class rdf:about="http://openenergy-platform.org/ontology/oeo/OEO_00050009">
        <rdfs:subClassOf rdf:resource="http://purl.obolibrary.org/obo/UO_0000111"/>
        <obo:IAO_0000115>An energy unit which is equal to 10^12 watt-hours.</obo:IAO_0000115>
        <obo:IAO_0000233>issue: https://github.com/OpenEnergyPlatform/ontology/issues/606
pull request: https://github.com/OpenEnergyPlatform/ontology/pull/608</obo:IAO_0000233>
        <oboInOwl:hasExactSynonym>TWh</oboInOwl:hasExactSynonym>
        <rdfs:label xml:lang="en">terawatt-hour</rdfs:label>
    </owl:Class>
    


    <!-- http://openenergy-platform.org/ontology/oeo/OEO_00050010 -->

    <owl:Class rdf:about="http://openenergy-platform.org/ontology/oeo/OEO_00050010">
        <rdfs:subClassOf rdf:resource="http://purl.obolibrary.org/obo/UO_0000111"/>
        <obo:IAO_0000115>An energy unit which is equal to 10^15 watt-hours.</obo:IAO_0000115>
        <obo:IAO_0000233>issue: https://github.com/OpenEnergyPlatform/ontology/issues/606
pull request: https://github.com/OpenEnergyPlatform/ontology/pull/608</obo:IAO_0000233>
        <oboInOwl:hasExactSynonym>PWh</oboInOwl:hasExactSynonym>
        <rdfs:label xml:lang="en">petawatt-hour</rdfs:label>
    </owl:Class>
    


    <!-- http://openenergy-platform.org/ontology/oeo/OEO_00050011 -->

    <owl:Class rdf:about="http://openenergy-platform.org/ontology/oeo/OEO_00050011">
        <rdfs:subClassOf rdf:resource="http://purl.obolibrary.org/obo/UO_0000111"/>
        <obo:IAO_0000115>An energy unit which is equal to 10^9 watt-hours.</obo:IAO_0000115>
        <obo:IAO_0000233>issue: https://github.com/OpenEnergyPlatform/ontology/issues/606
pull request: https://github.com/OpenEnergyPlatform/ontology/pull/608</obo:IAO_0000233>
        <oboInOwl:hasExactSynonym>GWh</oboInOwl:hasExactSynonym>
        <rdfs:label xml:lang="en">gigawatt-hour</rdfs:label>
    </owl:Class>
    


    <!-- http://openenergy-platform.org/ontology/oeo/OEO_00050016 -->

    <owl:Class rdf:about="http://openenergy-platform.org/ontology/oeo/OEO_00050016">
        <rdfs:subClassOf>
            <owl:Restriction>
                <owl:onProperty rdf:resource="http://openenergy-platform.org/ontology/oeo/OEO_00140002"/>
                <owl:someValuesFrom rdf:resource="http://openenergy-platform.org/ontology/oeo/OEO_00050019"/>
            </owl:Restriction>
        </rdfs:subClassOf>
    </owl:Class>
    


    <!-- http://openenergy-platform.org/ontology/oeo/OEO_00050017 -->

    <owl:Class rdf:about="http://openenergy-platform.org/ontology/oeo/OEO_00050017">
        <rdfs:subClassOf rdf:resource="http://openenergy-platform.org/ontology/oeo/OEO_00140039"/>
        <rdfs:subClassOf>
            <owl:Restriction>
                <owl:onProperty rdf:resource="http://openenergy-platform.org/ontology/oeo/OEO_00140002"/>
                <owl:someValuesFrom rdf:resource="http://openenergy-platform.org/ontology/oeo/OEO_00050019"/>
            </owl:Restriction>
        </rdfs:subClassOf>
        <obo:IAO_0000115 xml:lang="en">Gross inland energy consumption is the total consumption of energy in a spatial region (e.g. a country).</obo:IAO_0000115>
        <obo:IAO_0000116 xml:lang="en">Gross inland energy consumption represents the quantity of energy necessary to satisfy inland consumption of the spatial region (e.g. a country) under consideration.

Gross inland energy consumption covers:
  - consumption by the energy sector itself;
  - distribution and transformation losses;
  - final energy consumption by end users;
  - &apos;statistical differences&apos; (not already captured in the figures on primary energy consumption and final energy consumption).

Gross inland energy consumption does not include energy (fuel oil) provided to international maritime bunkers.</obo:IAO_0000116>
        <obo:IAO_0000118 xml:lang="en">Gross inland consumption</obo:IAO_0000118>
        <obo:IAO_0000118 xml:lang="en">Primary energy consumption including non-energy use of energy carriers.</obo:IAO_0000118>
        <obo:IAO_0000119 xml:lang="en">Eurostat Energy Glossary
https://ec.europa.eu/eurostat/statistics-explained/index.php/Glossary:Gross_inland_energy_consumption</obo:IAO_0000119>
        <obo:IAO_0000233 xml:lang="en">issue: https://github.com/OpenEnergyPlatform/ontology/issues/709
pull request: https://github.com/OpenEnergyPlatform/ontology/pull/719

issue: https://github.com/OpenEnergyPlatform/ontology/issues/576
pull request: https://github.com/OpenEnergyPlatform/ontology/pull/613</obo:IAO_0000233>
        <rdfs:label xml:lang="en">gross inland energy consumption</rdfs:label>
    </owl:Class>
    


    <!-- http://openenergy-platform.org/ontology/oeo/OEO_00050018 -->

    <owl:Class rdf:about="http://openenergy-platform.org/ontology/oeo/OEO_00050018">
        <rdfs:subClassOf rdf:resource="http://openenergy-platform.org/ontology/oeo/OEO_00140039"/>
        <rdfs:subClassOf>
            <owl:Restriction>
                <owl:onProperty rdf:resource="http://openenergy-platform.org/ontology/oeo/OEO_00140002"/>
                <owl:someValuesFrom rdf:resource="http://openenergy-platform.org/ontology/oeo/OEO_00050019"/>
            </owl:Restriction>
        </rdfs:subClassOf>
        <obo:IAO_0000115 xml:lang="en">Primary energy consumption is the total consumption of energy in a spatial region excluding the non-energetic use of fuels.</obo:IAO_0000115>
        <obo:IAO_0000116 xml:lang="en">Primary energy consumption covers consumption of the energy sector itself, losses during transformation (for example, from oil or gas into electricity) and distribution of energy, and the final consumption by end users. It excludes energy carriers used for non-energy purposes (such as petroleum not used not for combustion but for producing plastics).</obo:IAO_0000116>
        <obo:IAO_0000118 xml:lang="en">Primary energy consumption excluding non-energy use of energy carriers.</obo:IAO_0000118>
        <obo:IAO_0000119 xml:lang="en">Eurostat Energy Glossary
https://ec.europa.eu/eurostat/statistics-explained/index.php?title=Glossary:Primary_energy_consumption</obo:IAO_0000119>
        <obo:IAO_0000233 xml:lang="en">issue: https://github.com/OpenEnergyPlatform/ontology/issues/709
pull request: https://github.com/OpenEnergyPlatform/ontology/pull/719

issue: https://github.com/OpenEnergyPlatform/ontology/issues/576
pull request: https://github.com/OpenEnergyPlatform/ontology/pull/613</obo:IAO_0000233>
        <rdfs:label xml:lang="en">primary energy consumption</rdfs:label>
    </owl:Class>
    


    <!-- http://openenergy-platform.org/ontology/oeo/OEO_00050019 -->

    <owl:Class rdf:about="http://openenergy-platform.org/ontology/oeo/OEO_00050019">
        <rdfs:subClassOf rdf:resource="http://openenergy-platform.org/ontology/oeo/OEO_00000350"/>
        <rdfs:subClassOf>
            <owl:Restriction>
                <owl:onProperty rdf:resource="http://openenergy-platform.org/ontology/oeo/OEO_00040010"/>
                <owl:someValuesFrom rdf:resource="http://purl.obolibrary.org/obo/UO_0000111"/>
            </owl:Restriction>
        </rdfs:subClassOf>
        <obo:IAO_0000115 xml:lang="en">An energy amount value is a quantity value that has an energy unit as unit.</obo:IAO_0000115>
        <obo:IAO_0000233>issue: https://github.com/OpenEnergyPlatform/ontology/issues/576
pull request: https://github.com/OpenEnergyPlatform/ontology/pull/613</obo:IAO_0000233>
        <rdfs:label xml:lang="en">energy amount value</rdfs:label>
    </owl:Class>
    


    <!-- http://openenergy-platform.org/ontology/oeo/OEO_00050020 -->

    <owl:Class rdf:about="http://openenergy-platform.org/ontology/oeo/OEO_00050020">
        <rdfs:subClassOf rdf:resource="http://openenergy-platform.org/ontology/oeo/OEO_00020003"/>
        <rdfs:subClassOf>
            <owl:Restriction>
                <owl:onProperty rdf:resource="http://openenergy-platform.org/ontology/oeo/OEO_00000532"/>
                <owl:someValuesFrom rdf:resource="http://openenergy-platform.org/ontology/oeo/OEO_00000207"/>
            </owl:Restriction>
        </rdfs:subClassOf>
        <rdfs:subClassOf>
            <owl:Restriction>
                <owl:onProperty rdf:resource="http://purl.obolibrary.org/obo/RO_0000057"/>
                <owl:someValuesFrom rdf:resource="http://openenergy-platform.org/ontology/oeo/OEO_00000010"/>
            </owl:Restriction>
        </rdfs:subClassOf>
        <rdfs:subClassOf>
            <owl:Restriction>
                <owl:onProperty rdf:resource="http://purl.obolibrary.org/obo/RO_0000057"/>
                <owl:someValuesFrom rdf:resource="http://openenergy-platform.org/ontology/oeo/OEO_00000396"/>
            </owl:Restriction>
        </rdfs:subClassOf>
        <rdfs:subClassOf>
            <owl:Restriction>
                <owl:onProperty rdf:resource="http://purl.obolibrary.org/obo/RO_0002234"/>
                <owl:someValuesFrom rdf:resource="http://openenergy-platform.org/ontology/oeo/OEO_00000139"/>
            </owl:Restriction>
        </rdfs:subClassOf>
        <obo:IAO_0000115 xml:lang="en">A steam-electric process is an energy transformation that converts thermal energy to electrical energy. A steam turbine and an electro motive generator are participating in a steam-electric process.</obo:IAO_0000115>
        <obo:IAO_0000233 xml:lang="en">issue: https://github.com/OpenEnergyPlatform/ontology/issues/659
pull request: https://github.com/OpenEnergyPlatform/ontology/pull/691
pull request: https://github.com/OpenEnergyPlatform/ontology/pull/702</obo:IAO_0000233>
        <rdfs:label xml:lang="en">steam-electric process</rdfs:label>
    </owl:Class>
    


    <!-- http://openenergy-platform.org/ontology/oeo/OEO_00090000 -->

    <owl:Class rdf:about="http://openenergy-platform.org/ontology/oeo/OEO_00090000">
        <rdfs:subClassOf rdf:resource="http://openenergy-platform.org/ontology/oeo/OEO_00000350"/>
        <rdfs:subClassOf>
            <owl:Restriction>
                <owl:onProperty rdf:resource="http://openenergy-platform.org/ontology/oeo/OEO_00040010"/>
                <owl:someValuesFrom rdf:resource="http://purl.obolibrary.org/obo/UO_0000270"/>
            </owl:Restriction>
        </rdfs:subClassOf>
        <obo:IAO_0000115>A volumetric flow rate value is a quantity value that has a volumetric flow rate unit as unit.</obo:IAO_0000115>
        <obo:IAO_0000233>Issue: https://github.com/OpenEnergyPlatform/ontology/pull/693
Pull Request: https://github.com/OpenEnergyPlatform/ontology/pull/693</obo:IAO_0000233>
        <rdfs:label>volumetric flow rate value</rdfs:label>
    </owl:Class>
    


    <!-- http://openenergy-platform.org/ontology/oeo/OEO_00110000 -->

    <owl:Class rdf:about="http://openenergy-platform.org/ontology/oeo/OEO_00110000">
        <rdfs:subClassOf rdf:resource="http://openenergy-platform.org/ontology/oeo/OEO_00000441"/>
        <rdfs:subClassOf>
            <owl:Restriction>
                <owl:onProperty rdf:resource="http://purl.obolibrary.org/obo/RO_0000086"/>
                <owl:someValuesFrom rdf:resource="http://openenergy-platform.org/ontology/oeo/OEO_00000218"/>
            </owl:Restriction>
        </rdfs:subClassOf>
        <rdfs:subClassOf>
            <owl:Restriction>
                <owl:onProperty rdf:resource="http://openenergy-platform.org/ontology/oeo/OEO_00000531"/>
                <owl:hasValue rdf:resource="http://openenergy-platform.org/ontology/oeo/OEO_00000256"/>
            </owl:Restriction>
        </rdfs:subClassOf>
        <obo:IAO_0000115 xml:lang="en">Liquid water is water that has a liquid state of matter.</obo:IAO_0000115>
        <obo:IAO_0000233 xml:lang="en">issue: https://github.com/OpenEnergyPlatform/ontology/issues/679
pull request: https://github.com/OpenEnergyPlatform/ontology/pull/682</obo:IAO_0000233>
        <rdfs:label xml:lang="en">liquid water</rdfs:label>
    </owl:Class>
    


    <!-- http://openenergy-platform.org/ontology/oeo/OEO_00110001 -->

    <owl:Class rdf:about="http://openenergy-platform.org/ontology/oeo/OEO_00110001">
        <rdfs:subClassOf rdf:resource="http://openenergy-platform.org/ontology/oeo/OEO_00000441"/>
        <rdfs:subClassOf>
            <owl:Restriction>
                <owl:onProperty rdf:resource="http://openenergy-platform.org/ontology/oeo/OEO_00000531"/>
                <owl:hasValue rdf:resource="http://openenergy-platform.org/ontology/oeo/OEO_00000182"/>
            </owl:Restriction>
        </rdfs:subClassOf>
        <obo:IAO_0000115 xml:lang="en">Steam is water that has a gaseous state of matter.</obo:IAO_0000115>
        <obo:IAO_0000233 xml:lang="en">issue: https://github.com/OpenEnergyPlatform/ontology/issues/679
pull request: https://github.com/OpenEnergyPlatform/ontology/pull/682</obo:IAO_0000233>
        <rdfs:label xml:lang="en">steam</rdfs:label>
    </owl:Class>
    


    <!-- http://openenergy-platform.org/ontology/oeo/OEO_00110002 -->

    <owl:Class rdf:about="http://openenergy-platform.org/ontology/oeo/OEO_00110002">
        <rdfs:subClassOf rdf:resource="http://purl.obolibrary.org/obo/BFO_0000015"/>
        <rdfs:subClassOf>
            <owl:Restriction>
                <owl:onProperty rdf:resource="http://openenergy-platform.org/ontology/oeo/OEO_00000500"/>
                <owl:someValuesFrom rdf:resource="http://openenergy-platform.org/ontology/oeo/OEO_00110003"/>
            </owl:Restriction>
        </rdfs:subClassOf>
        <rdfs:subClassOf>
            <owl:Restriction>
                <owl:onProperty rdf:resource="http://purl.obolibrary.org/obo/RO_0000057"/>
                <owl:someValuesFrom rdf:resource="http://openenergy-platform.org/ontology/oeo/OEO_00110000"/>
            </owl:Restriction>
        </rdfs:subClassOf>
        <obo:IAO_0000115 xml:lang="en">Water flow is a process of liquid water moving.</obo:IAO_0000115>
        <obo:IAO_0000233 xml:lang="en">issue: https://github.com/OpenEnergyPlatform/ontology/issues/679
pull request: https://github.com/OpenEnergyPlatform/ontology/pull/682</obo:IAO_0000233>
        <rdfs:label xml:lang="en">water flow</rdfs:label>
    </owl:Class>
    


    <!-- http://openenergy-platform.org/ontology/oeo/OEO_00110003 -->

    <owl:Class rdf:about="http://openenergy-platform.org/ontology/oeo/OEO_00110003">
        <rdfs:subClassOf rdf:resource="http://openenergy-platform.org/ontology/oeo/OEO_00030019"/>
        <rdfs:subClassOf>
            <owl:Restriction>
                <owl:onProperty rdf:resource="http://openenergy-platform.org/ontology/oeo/OEO_00140002"/>
                <owl:someValuesFrom rdf:resource="http://openenergy-platform.org/ontology/oeo/OEO_00090000"/>
            </owl:Restriction>
        </rdfs:subClassOf>
        <obo:IAO_0000115 xml:lang="en">Water flow rate is the process attribute of water flow that quantifies the water volume per time unit.</obo:IAO_0000115>
        <obo:IAO_0000233 xml:lang="en">issue: https://github.com/OpenEnergyPlatform/ontology/issues/679
pull request: https://github.com/OpenEnergyPlatform/ontology/pull/682</obo:IAO_0000233>
        <rdfs:label xml:lang="en">water flow rate</rdfs:label>
    </owl:Class>
    


    <!-- http://openenergy-platform.org/ontology/oeo/OEO_00110004 -->

    <owl:Class rdf:about="http://openenergy-platform.org/ontology/oeo/OEO_00110004">
        <rdfs:subClassOf rdf:resource="http://openenergy-platform.org/ontology/oeo/OEO_00020003"/>
        <rdfs:subClassOf>
            <owl:Restriction>
                <owl:onProperty rdf:resource="http://openenergy-platform.org/ontology/oeo/OEO_00000532"/>
                <owl:someValuesFrom rdf:resource="http://openenergy-platform.org/ontology/oeo/OEO_00000218"/>
            </owl:Restriction>
        </rdfs:subClassOf>
        <obo:IAO_0000115 xml:lang="en">Hydro energy transformation is an energy transformation that converts hydro energy.</obo:IAO_0000115>
        <obo:IAO_0000233 xml:lang="en">issue: https://github.com/OpenEnergyPlatform/ontology/issues/679
pull request: https://github.com/OpenEnergyPlatform/ontology/pull/682
pull request: https://github.com/OpenEnergyPlatform/ontology/pull/702</obo:IAO_0000233>
        <rdfs:label xml:lang="en">hydro energy transformation</rdfs:label>
    </owl:Class>
    


    <!-- http://openenergy-platform.org/ontology/oeo/OEO_00110005 -->

    <owl:Class rdf:about="http://openenergy-platform.org/ontology/oeo/OEO_00110005">
        <rdfs:subClassOf rdf:resource="http://openenergy-platform.org/ontology/oeo/OEO_00110004"/>
        <rdfs:subClassOf>
            <owl:Restriction>
                <owl:onProperty rdf:resource="http://purl.obolibrary.org/obo/RO_0002234"/>
                <owl:someValuesFrom rdf:resource="http://openenergy-platform.org/ontology/oeo/OEO_00000139"/>
            </owl:Restriction>
        </rdfs:subClassOf>
        <obo:IAO_0000115 xml:lang="en">Hydroelectric energy transformation is an hydro energy transformation that converts hydro energy to electrical energy.</obo:IAO_0000115>
        <obo:IAO_0000233 xml:lang="en">issue: https://github.com/OpenEnergyPlatform/ontology/issues/679
pull request: https://github.com/OpenEnergyPlatform/ontology/pull/682</obo:IAO_0000233>
        <rdfs:label xml:lang="en">hydroelectric energy transformation</rdfs:label>
    </owl:Class>
    


    <!-- http://openenergy-platform.org/ontology/oeo/OEO_00110006 -->

    <owl:Class rdf:about="http://openenergy-platform.org/ontology/oeo/OEO_00110006">
        <rdfs:subClassOf rdf:resource="http://openenergy-platform.org/ontology/oeo/OEO_00110005"/>
        <obo:IAO_0000115 xml:lang="en">Run-off-river energy transformation is an hydroelectric energy transformation that converts hydro energy of a river to electrical energy.</obo:IAO_0000115>
        <obo:IAO_0000233 xml:lang="en">issue: https://github.com/OpenEnergyPlatform/ontology/issues/679
pull request: https://github.com/OpenEnergyPlatform/ontology/pull/682</obo:IAO_0000233>
        <rdfs:label xml:lang="en">run-off-river energy transformation</rdfs:label>
    </owl:Class>
    


    <!-- http://openenergy-platform.org/ontology/oeo/OEO_00110007 -->

    <owl:Class rdf:about="http://openenergy-platform.org/ontology/oeo/OEO_00110007">
        <rdfs:subClassOf rdf:resource="http://openenergy-platform.org/ontology/oeo/OEO_00110005"/>
        <obo:IAO_0000115 xml:lang="en">Hydroelectric dam energy transformation is an hydroelectric energy transformation that converts potential hydro energy of dammed water to electrical energy.</obo:IAO_0000115>
        <obo:IAO_0000233 xml:lang="en">issue: https://github.com/OpenEnergyPlatform/ontology/issues/679
pull request: https://github.com/OpenEnergyPlatform/ontology/pull/682</obo:IAO_0000233>
        <rdfs:label xml:lang="en">hydroelectric dam energy transformation</rdfs:label>
    </owl:Class>
    


    <!-- http://openenergy-platform.org/ontology/oeo/OEO_00140000 -->

    <owl:Class rdf:about="http://openenergy-platform.org/ontology/oeo/OEO_00140000">
        <rdfs:subClassOf rdf:resource="http://purl.obolibrary.org/obo/BFO_0000019"/>
        <rdfs:subClassOf>
            <owl:Restriction>
                <owl:onProperty rdf:resource="http://openenergy-platform.org/ontology/oeo/OEO_00140002"/>
                <owl:someValuesFrom rdf:resource="http://openenergy-platform.org/ontology/oeo/OEO_00140001"/>
            </owl:Restriction>
        </rdfs:subClassOf>
        <obo:IAO_0000115>Hub height is a quality of a wind energy converting unit that measures the distance between surface and center-line of the wind rotor.</obo:IAO_0000115>
        <obo:IAO_0000233>issue: https://github.com/OpenEnergyPlatform/ontology/issues/505
pull request: https://github.com/OpenEnergyPlatform/ontology/pull/509</obo:IAO_0000233>
        <rdfs:label xml:lang="en">hub height</rdfs:label>
    </owl:Class>
    


    <!-- http://openenergy-platform.org/ontology/oeo/OEO_00140001 -->

    <owl:Class rdf:about="http://openenergy-platform.org/ontology/oeo/OEO_00140001">
        <rdfs:subClassOf rdf:resource="http://openenergy-platform.org/ontology/oeo/OEO_00000350"/>
        <rdfs:subClassOf>
            <owl:Restriction>
                <owl:onProperty rdf:resource="http://purl.obolibrary.org/obo/BFO_0000051"/>
                <owl:someValuesFrom rdf:resource="http://purl.obolibrary.org/obo/UO_0000001"/>
            </owl:Restriction>
        </rdfs:subClassOf>
        <obo:IAO_0000115>Length value is a quantity value that has a length unit as unit.</obo:IAO_0000115>
        <obo:IAO_0000233>issue: https://github.com/OpenEnergyPlatform/ontology/issues/505
pull request: https://github.com/OpenEnergyPlatform/ontology/pull/509</obo:IAO_0000233>
        <rdfs:label xml:lang="en">length value</rdfs:label>
    </owl:Class>
    


    <!-- http://openenergy-platform.org/ontology/oeo/OEO_00140033 -->

    <owl:Class rdf:about="http://openenergy-platform.org/ontology/oeo/OEO_00140033">
        <rdfs:subClassOf rdf:resource="http://openenergy-platform.org/ontology/oeo/OEO_00000419"/>
        <obo:IAO_0000115>A chemical reaction is a transformation that involves the interconversion of chemical species.</obo:IAO_0000115>
        <obo:IAO_0000233>issue: https://github.com/OpenEnergyPlatform/ontology/issues/449
pull request: https://github.com/OpenEnergyPlatform/ontology/pull/568</obo:IAO_0000233>
        <rdfs:label xml:lang="en">chemical reaction</rdfs:label>
    </owl:Class>
    


    <!-- http://openenergy-platform.org/ontology/oeo/OEO_00140034 -->

    <owl:Class rdf:about="http://openenergy-platform.org/ontology/oeo/OEO_00140034">
        <rdfs:subClassOf rdf:resource="http://openenergy-platform.org/ontology/oeo/OEO_00140033"/>
        <obo:IAO_0000115>A redox reaction is a chemical reaction in which the oxidation of one reactant is coupled to the reduction of a second reactant.</obo:IAO_0000115>
        <obo:IAO_0000118>oxidation</obo:IAO_0000118>
        <obo:IAO_0000233>issue: https://github.com/OpenEnergyPlatform/ontology/issues/449
pull request: https://github.com/OpenEnergyPlatform/ontology/pull/568</obo:IAO_0000233>
        <rdfs:label xml:lang="en">redox reaction</rdfs:label>
    </owl:Class>
    


    <!-- http://openenergy-platform.org/ontology/oeo/OEO_00140035 -->

    <owl:Class rdf:about="http://openenergy-platform.org/ontology/oeo/OEO_00140035">
        <rdfs:subClassOf rdf:resource="http://openenergy-platform.org/ontology/oeo/OEO_00140033"/>
        <obo:IAO_0000115>Oxidation is a chemical reaction that describes the loss of electrons of an atom, an ion, or of certain atoms in a molecule and is a part of a redox reaction.</obo:IAO_0000115>
        <obo:IAO_0000233>issue: https://github.com/OpenEnergyPlatform/ontology/issues/449
pull request: https://github.com/OpenEnergyPlatform/ontology/pull/568</obo:IAO_0000233>
        <rdfs:label xml:lang="en">oxidation</rdfs:label>
    </owl:Class>
    


    <!-- http://openenergy-platform.org/ontology/oeo/OEO_00140036 -->

    <owl:Class rdf:about="http://openenergy-platform.org/ontology/oeo/OEO_00140036">
        <rdfs:subClassOf rdf:resource="http://openenergy-platform.org/ontology/oeo/OEO_00140033"/>
        <obo:IAO_0000115>Reduction is a chemical reaction that describes the gain of electrons of an atom, an ion, or of certain atoms in a molecule and is a part of a redox reaction.</obo:IAO_0000115>
        <obo:IAO_0000233>issue: https://github.com/OpenEnergyPlatform/ontology/issues/449
pull request: https://github.com/OpenEnergyPlatform/ontology/pull/568</obo:IAO_0000233>
        <rdfs:label xml:lang="en">reduction</rdfs:label>
    </owl:Class>
    


    <!-- http://openenergy-platform.org/ontology/oeo/OEO_00140037 -->

    <owl:Class rdf:about="http://openenergy-platform.org/ontology/oeo/OEO_00140037">
        <rdfs:subClassOf rdf:resource="http://openenergy-platform.org/ontology/oeo/OEO_00140033"/>
        <obo:IAO_0000115>An electrochemical reaction is a chemical reaction that describes the overall reactions of individual redox reactions being separated but connected by an external electric circuit and an intervening electrolyte.</obo:IAO_0000115>
        <obo:IAO_0000233>issue: https://github.com/OpenEnergyPlatform/ontology/issues/449
pull request: https://github.com/OpenEnergyPlatform/ontology/pull/568</obo:IAO_0000233>
        <rdfs:label xml:lang="en">electrochemical reaction</rdfs:label>
    </owl:Class>
    


    <!-- http://openenergy-platform.org/ontology/oeo/OEO_00140038 -->

    <owl:Class rdf:about="http://openenergy-platform.org/ontology/oeo/OEO_00140038">
        <rdfs:subClassOf rdf:resource="http://openenergy-platform.org/ontology/oeo/OEO_00140034"/>
        <obo:IAO_0000115>Combustion is an exothermic redox reaction between a fuel (the reductant) and an oxidant (usually atmospheric oxygen) which is initiated by a ignition source.</obo:IAO_0000115>
        <obo:IAO_0000233>issue: https://github.com/OpenEnergyPlatform/ontology/issues/449
pull request: https://github.com/OpenEnergyPlatform/ontology/pull/568</obo:IAO_0000233>
        <rdfs:label xml:lang="en">combustion</rdfs:label>
    </owl:Class>
    


    <!-- http://openenergy-platform.org/ontology/oeo/OEO_00140039 -->

    <owl:Class rdf:about="http://openenergy-platform.org/ontology/oeo/OEO_00140039"/>
    


    <!-- http://openenergy-platform.org/ontology/oeo/OEO_00140049 -->

    <owl:Class rdf:about="http://openenergy-platform.org/ontology/oeo/OEO_00140049">
        <rdfs:subClassOf rdf:resource="http://openenergy-platform.org/ontology/oeo/OEO_00030019"/>
        <rdfs:subClassOf>
            <owl:Restriction>
                <owl:onProperty rdf:resource="http://openenergy-platform.org/ontology/oeo/OEO_00000502"/>
                <owl:someValuesFrom rdf:resource="http://openenergy-platform.org/ontology/oeo/OEO_00020003"/>
            </owl:Restriction>
        </rdfs:subClassOf>
        <rdfs:subClassOf>
            <owl:Restriction>
                <owl:onProperty rdf:resource="http://openenergy-platform.org/ontology/oeo/OEO_00140002"/>
                <owl:someValuesFrom rdf:resource="http://openenergy-platform.org/ontology/oeo/OEO_00140050"/>
            </owl:Restriction>
        </rdfs:subClassOf>
        <obo:IAO_0000115>Energy conversion efficiency is a process attribute describing the ratio between the input of an energy transformation and the outputs that are used.</obo:IAO_0000115>
        <obo:IAO_0000233>issue: https://github.com/OpenEnergyPlatform/ontology/issues/434
pull request: https://github.com/OpenEnergyPlatform/ontology/pull/591</obo:IAO_0000233>
        <rdfs:label xml:lang="en">energy conversion efficiency</rdfs:label>
    </owl:Class>
    


    <!-- http://openenergy-platform.org/ontology/oeo/OEO_00140050 -->

    <owl:Class rdf:about="http://openenergy-platform.org/ontology/oeo/OEO_00140050">
        <rdfs:subClassOf rdf:resource="http://openenergy-platform.org/ontology/oeo/OEO_00000350"/>
        <rdfs:subClassOf>
            <owl:Restriction>
                <owl:onProperty rdf:resource="http://openenergy-platform.org/ontology/oeo/OEO_00040010"/>
                <owl:someValuesFrom rdf:resource="http://purl.obolibrary.org/obo/UO_0010006"/>
            </owl:Restriction>
        </rdfs:subClassOf>
        <obo:IAO_0000115>An efficiency value is a quantity value stating the ratio between a process&apos;s inputs and the outputs that are used.</obo:IAO_0000115>
        <obo:IAO_0000233>issue: https://github.com/OpenEnergyPlatform/ontology/issues/434
pull request: https://github.com/OpenEnergyPlatform/ontology/pull/591</obo:IAO_0000233>
        <rdfs:label xml:lang="en">efficiency value</rdfs:label>
    </owl:Class>
    


    <!-- http://openenergy-platform.org/ontology/oeo/OEO_00140051 -->

    <owl:Class rdf:about="http://openenergy-platform.org/ontology/oeo/OEO_00140051">
        <rdfs:subClassOf rdf:resource="http://openenergy-platform.org/ontology/oeo/OEO_00000350"/>
        <rdfs:subClassOf>
            <owl:Restriction>
                <owl:onProperty rdf:resource="http://openenergy-platform.org/ontology/oeo/OEO_00020056"/>
                <owl:someValuesFrom rdf:resource="http://openenergy-platform.org/ontology/oeo/OEO_00140052"/>
            </owl:Restriction>
        </rdfs:subClassOf>
        <rdfs:subClassOf>
            <owl:Restriction>
                <owl:onProperty rdf:resource="http://openenergy-platform.org/ontology/oeo/OEO_00040010"/>
                <owl:someValuesFrom rdf:resource="http://purl.obolibrary.org/obo/UO_0010006"/>
            </owl:Restriction>
        </rdfs:subClassOf>
        <obo:IAO_0000115>A coefficient of performance value is a quantity value stating the ratio between the work input and the total output of an energy conversion process.</obo:IAO_0000115>
        <obo:IAO_0000233>issue: https://github.com/OpenEnergyPlatform/ontology/issues/434
pull request: https://github.com/OpenEnergyPlatform/ontology/pull/591</obo:IAO_0000233>
        <rdfs:label xml:lang="en">coefficient of performance value</rdfs:label>
    </owl:Class>
    


    <!-- http://openenergy-platform.org/ontology/oeo/OEO_00140052 -->

    <owl:Class rdf:about="http://openenergy-platform.org/ontology/oeo/OEO_00140052">
        <rdfs:subClassOf rdf:resource="http://openenergy-platform.org/ontology/oeo/OEO_00030019"/>
        <rdfs:subClassOf>
            <owl:Restriction>
                <owl:onProperty rdf:resource="http://openenergy-platform.org/ontology/oeo/OEO_00000502"/>
                <owl:someValuesFrom rdf:resource="http://openenergy-platform.org/ontology/oeo/OEO_00020003"/>
            </owl:Restriction>
        </rdfs:subClassOf>
        <rdfs:subClassOf>
            <owl:Restriction>
                <owl:onProperty rdf:resource="http://openenergy-platform.org/ontology/oeo/OEO_00140002"/>
                <owl:someValuesFrom rdf:resource="http://openenergy-platform.org/ontology/oeo/OEO_00140051"/>
            </owl:Restriction>
        </rdfs:subClassOf>
        <obo:IAO_0000115>Energy conversion performance is a process attribute describing the ratio between the non-heat input of an energy transformation and the outputs that are used.</obo:IAO_0000115>
        <obo:IAO_0000233>issue: https://github.com/OpenEnergyPlatform/ontology/issues/434
pull request: https://github.com/OpenEnergyPlatform/ontology/pull/591</obo:IAO_0000233>
        <rdfs:label xml:lang="en">energy conversion performance</rdfs:label>
    </owl:Class>
    


    <!-- http://openenergy-platform.org/ontology/oeo/OEO_00140056 -->

    <owl:Class rdf:about="http://openenergy-platform.org/ontology/oeo/OEO_00140056">
        <rdfs:subClassOf rdf:resource="http://openenergy-platform.org/ontology/oeo/OEO_00000350"/>
        <obo:IAO_0000115>A flow potential is a quantity value that describes the upper limit of an input or output of a process in a spatial region of reference per unit time.</obo:IAO_0000115>
        <obo:IAO_0000233>issue: https://github.com/OpenEnergyPlatform/ontology/issues/481
pull request: https://github.com/OpenEnergyPlatform/ontology/pull/607</obo:IAO_0000233>
        <rdfs:label xml:lang="en">flow potential</rdfs:label>
    </owl:Class>
    


    <!-- http://openenergy-platform.org/ontology/oeo/OEO_00140057 -->

    <owl:Class rdf:about="http://openenergy-platform.org/ontology/oeo/OEO_00140057">
        <rdfs:subClassOf rdf:resource="http://openenergy-platform.org/ontology/oeo/OEO_00140056"/>
        <obo:IAO_0000115>A theoretical flow potential is a type of flow potential that identifies the physical upper limit of an input or output of a process in a spatial region of reference per unit time.</obo:IAO_0000115>
        <obo:IAO_0000233>issue: https://github.com/OpenEnergyPlatform/ontology/issues/481
pull request: https://github.com/OpenEnergyPlatform/ontology/pull/607</obo:IAO_0000233>
        <rdfs:label xml:lang="en">theoretical flow potential</rdfs:label>
    </owl:Class>
    


    <!-- http://openenergy-platform.org/ontology/oeo/OEO_00140058 -->

    <owl:Class rdf:about="http://openenergy-platform.org/ontology/oeo/OEO_00140058">
        <rdfs:subClassOf rdf:resource="http://openenergy-platform.org/ontology/oeo/OEO_00140056"/>
        <obo:IAO_0000115>A technological flow potential is a type of a flow potential derived from a theoretical flow potential, taking account of the annual efficiency of the respective conversion technology and the additional restrictions regarding the area that is realistically available for energy generation.</obo:IAO_0000115>
        <obo:IAO_0000233>issue: https://github.com/OpenEnergyPlatform/ontology/issues/481
pull request: https://github.com/OpenEnergyPlatform/ontology/pull/607</obo:IAO_0000233>
        <rdfs:label xml:lang="en">technological flow potential</rdfs:label>
    </owl:Class>
    


    <!-- http://openenergy-platform.org/ontology/oeo/OEO_00140059 -->

    <owl:Class rdf:about="http://openenergy-platform.org/ontology/oeo/OEO_00140059">
        <rdfs:subClassOf rdf:resource="http://openenergy-platform.org/ontology/oeo/OEO_00140056"/>
        <obo:IAO_0000115>An economic flow potential is a type of flow potential that identifies the proportion of the technological potential that can be utilized economically (based on economic boundary conditions).</obo:IAO_0000115>
        <obo:IAO_0000233>issue: https://github.com/OpenEnergyPlatform/ontology/issues/481
pull request: https://github.com/OpenEnergyPlatform/ontology/pull/607</obo:IAO_0000233>
        <rdfs:label xml:lang="en">economic flow potential</rdfs:label>
    </owl:Class>
    


    <!-- http://openenergy-platform.org/ontology/oeo/OEO_00140060 -->

    <owl:Class rdf:about="http://openenergy-platform.org/ontology/oeo/OEO_00140060">
        <rdfs:subClassOf rdf:resource="http://openenergy-platform.org/ontology/oeo/OEO_00140056"/>
        <obo:IAO_0000115>A developable flow potential is a type of flow potential that describes the fraction of the economic potential that can be developed under realistic conditions (regulations, environmental and social restrictions).</obo:IAO_0000115>
        <obo:IAO_0000233>issue: https://github.com/OpenEnergyPlatform/ontology/issues/481
pull request: https://github.com/OpenEnergyPlatform/ontology/pull/607</obo:IAO_0000233>
        <rdfs:label xml:lang="en">developable flow potential</rdfs:label>
    </owl:Class>
    


    <!-- http://openenergy-platform.org/ontology/oeo/OEO_00140061 -->

    <owl:Class rdf:about="http://openenergy-platform.org/ontology/oeo/OEO_00140061">
        <rdfs:subClassOf rdf:resource="http://openenergy-platform.org/ontology/oeo/OEO_00140056"/>
        <obo:IAO_0000115>A sustainable flow potential is a type of flow potential that takes into account all aspects of sustainability, which usually requires careful consideration and evaluation of different ecological and socio-economic aspects. The differentiation of the sustainable potential is blurred, since ecological aspects may already have been considered for the technological or economic potential, depending on the author.</obo:IAO_0000115>
        <obo:IAO_0000233>issue: https://github.com/OpenEnergyPlatform/ontology/issues/481
pull request: https://github.com/OpenEnergyPlatform/ontology/pull/607</obo:IAO_0000233>
        <rdfs:label xml:lang="en">sustainable flow potential</rdfs:label>
    </owl:Class>
    


    <!-- http://openenergy-platform.org/ontology/oeo/OEO_00140062 -->

    <owl:Class rdf:about="http://openenergy-platform.org/ontology/oeo/OEO_00140062">
        <rdfs:subClassOf rdf:resource="http://openenergy-platform.org/ontology/oeo/OEO_00000350"/>
        <obo:IAO_0000115>A stock potential is a quantity value that describes the upper limit of a stock of a source or sink in a spatial region of reference.</obo:IAO_0000115>
        <obo:IAO_0000233>issue: https://github.com/OpenEnergyPlatform/ontology/issues/481
pull request: https://github.com/OpenEnergyPlatform/ontology/pull/607</obo:IAO_0000233>
        <rdfs:label xml:lang="en">stock potential</rdfs:label>
    </owl:Class>
    


    <!-- http://openenergy-platform.org/ontology/oeo/OEO_00140063 -->

    <owl:Class rdf:about="http://openenergy-platform.org/ontology/oeo/OEO_00140063">
        <rdfs:subClassOf rdf:resource="http://openenergy-platform.org/ontology/oeo/OEO_00140062"/>
        <obo:IAO_0000115>A theoretical stock potential is a type of stock potential that identifies the physical upper limit of a stock of a source or sink in a spatial region of reference.</obo:IAO_0000115>
        <obo:IAO_0000233>issue: https://github.com/OpenEnergyPlatform/ontology/issues/481
pull request: https://github.com/OpenEnergyPlatform/ontology/pull/607</obo:IAO_0000233>
        <rdfs:label xml:lang="en">theoretical stock potential</rdfs:label>
    </owl:Class>
    


    <!-- http://openenergy-platform.org/ontology/oeo/OEO_00140064 -->

    <owl:Class rdf:about="http://openenergy-platform.org/ontology/oeo/OEO_00140064">
        <rdfs:subClassOf rdf:resource="http://openenergy-platform.org/ontology/oeo/OEO_00140062"/>
        <obo:IAO_0000115>A technological stock potential is a type of a stock potential derived from a theoretical stock potential, taking account of the annual efficiency of the respective conversion technology and the additional restrictions regarding the area that is realistically available for energy generation.</obo:IAO_0000115>
        <obo:IAO_0000233>issue: https://github.com/OpenEnergyPlatform/ontology/issues/481
pull request: https://github.com/OpenEnergyPlatform/ontology/pull/607</obo:IAO_0000233>
        <rdfs:label xml:lang="en">technological stock potential</rdfs:label>
    </owl:Class>
    


    <!-- http://openenergy-platform.org/ontology/oeo/OEO_00140065 -->

    <owl:Class rdf:about="http://openenergy-platform.org/ontology/oeo/OEO_00140065">
        <rdfs:subClassOf rdf:resource="http://openenergy-platform.org/ontology/oeo/OEO_00140062"/>
        <obo:IAO_0000115>An economic stock potential is a type of stock potential that identifies the proportion of the technological potential that can be utilized economically (based on economic boundary conditions).</obo:IAO_0000115>
        <obo:IAO_0000233>issue: https://github.com/OpenEnergyPlatform/ontology/issues/481
pull request: https://github.com/OpenEnergyPlatform/ontology/pull/607</obo:IAO_0000233>
        <rdfs:label xml:lang="en">economic stock potential</rdfs:label>
    </owl:Class>
    


    <!-- http://openenergy-platform.org/ontology/oeo/OEO_00140066 -->

    <owl:Class rdf:about="http://openenergy-platform.org/ontology/oeo/OEO_00140066">
        <rdfs:subClassOf rdf:resource="http://openenergy-platform.org/ontology/oeo/OEO_00140062"/>
        <obo:IAO_0000115>A developable stock potential is a type of stock potential that describes the fraction of the economic potential that can be developed under realistic conditions (regulations, environmental and social restrictions).</obo:IAO_0000115>
        <obo:IAO_0000233>issue: https://github.com/OpenEnergyPlatform/ontology/issues/481
pull request: https://github.com/OpenEnergyPlatform/ontology/pull/607</obo:IAO_0000233>
        <rdfs:label xml:lang="en">developable stock potential</rdfs:label>
    </owl:Class>
    


    <!-- http://openenergy-platform.org/ontology/oeo/OEO_00140067 -->

    <owl:Class rdf:about="http://openenergy-platform.org/ontology/oeo/OEO_00140067">
        <rdfs:subClassOf rdf:resource="http://openenergy-platform.org/ontology/oeo/OEO_00140062"/>
        <obo:IAO_0000115>A sustainable stock potential is a type of stock potential that takes into account all aspects of sustainability, which usually requires careful consideration and evaluation of different ecological and socio-economic aspects. The differentiation of the sustainable potential is blurred, since ecological aspects may already have been considered for the technological or economic potential, depending on the author.</obo:IAO_0000115>
        <obo:IAO_0000233>issue: https://github.com/OpenEnergyPlatform/ontology/issues/481
pull request: https://github.com/OpenEnergyPlatform/ontology/pull/607</obo:IAO_0000233>
        <rdfs:label xml:lang="en">sustainable stock potential</rdfs:label>
    </owl:Class>
    


    <!-- http://openenergy-platform.org/ontology/oeo/OEO_00140075 -->

    <owl:Class rdf:about="http://openenergy-platform.org/ontology/oeo/OEO_00140075">
        <rdfs:subClassOf rdf:resource="http://openenergy-platform.org/ontology/oeo/OEO_00000151"/>
        <obo:IAO_0000112>coals, cruide oil, natural gas, wood or moving air (wind) have the disposition of being primary energy carriers</obo:IAO_0000112>
        <obo:IAO_0000115>Primary energy carrier disposition is an energy carrier disposition of material entities that are extracted directly from natural resources or that are natural energy flows.</obo:IAO_0000115>
        <obo:IAO_0000233>issue: https://github.com/OpenEnergyPlatform/ontology/issues/575
pull request: https://github.com/OpenEnergyPlatform/ontology/pull/633</obo:IAO_0000233>
        <rdfs:label xml:lang="en">primary energy carrier disposition</rdfs:label>
    </owl:Class>
    


    <!-- http://openenergy-platform.org/ontology/oeo/OEO_00140076 -->

    <owl:Class rdf:about="http://openenergy-platform.org/ontology/oeo/OEO_00140076">
        <rdfs:subClassOf rdf:resource="http://openenergy-platform.org/ontology/oeo/OEO_00000151"/>
        <obo:IAO_0000112>blast furnace gas, coke oven gas, cokes, motor gasoline or electricity have the disposition to be a secondary energy carrier</obo:IAO_0000112>
        <obo:IAO_0000115>Secondary energy carrier disposition is an energy carrier disposition of material entities that are manufactured from primary energy carriers or from a different form of secondary energy carriers.</obo:IAO_0000115>
        <obo:IAO_0000233>issue: https://github.com/OpenEnergyPlatform/ontology/issues/575
pull request: https://github.com/OpenEnergyPlatform/ontology/pull/633</obo:IAO_0000233>
        <rdfs:label xml:lang="en">secondary energy carrier disposition</rdfs:label>
    </owl:Class>
    


    <!-- http://openenergy-platform.org/ontology/oeo/OEO_00140077 -->

    <owl:Class rdf:about="http://openenergy-platform.org/ontology/oeo/OEO_00140077">
        <rdfs:subClassOf rdf:resource="http://openenergy-platform.org/ontology/oeo/OEO_00000151"/>
        <obo:IAO_0000112>district heat or electricity have the disposition of being a final energy carrier</obo:IAO_0000112>
        <obo:IAO_0000115>Final energy carrier disposition is an energy carrier disposition of material entities that are delivered to energy consumers for their use.</obo:IAO_0000115>
        <obo:IAO_0000233>issue: https://github.com/OpenEnergyPlatform/ontology/issues/575
pull request: https://github.com/OpenEnergyPlatform/ontology/pull/633</obo:IAO_0000233>
        <rdfs:label xml:lang="en">final energy carrier disposition</rdfs:label>
    </owl:Class>
    


    <!-- http://openenergy-platform.org/ontology/oeo/OEO_00140078 -->

    <owl:Class rdf:about="http://openenergy-platform.org/ontology/oeo/OEO_00140078">
        <owl:equivalentClass>
            <owl:Class>
                <owl:intersectionOf rdf:parseType="Collection">
                    <rdf:Description rdf:about="http://purl.obolibrary.org/obo/BFO_0000040"/>
                    <owl:Restriction>
                        <owl:onProperty rdf:resource="http://purl.obolibrary.org/obo/RO_0000091"/>
                        <owl:someValuesFrom rdf:resource="http://openenergy-platform.org/ontology/oeo/OEO_00140075"/>
                    </owl:Restriction>
                </owl:intersectionOf>
            </owl:Class>
        </owl:equivalentClass>
        <rdfs:subClassOf rdf:resource="http://openenergy-platform.org/ontology/oeo/OEO_00020039"/>
        <obo:IAO_0000115>A primary energy carrier is an energy carrier that has the disposition primary energy carrier disposition.</obo:IAO_0000115>
        <obo:IAO_0000233>issue: https://github.com/OpenEnergyPlatform/ontology/issues/575
pull request: https://github.com/OpenEnergyPlatform/ontology/pull/633</obo:IAO_0000233>
        <rdfs:label xml:lang="en">primary energy carrier</rdfs:label>
    </owl:Class>
    


    <!-- http://openenergy-platform.org/ontology/oeo/OEO_00140079 -->

    <owl:Class rdf:about="http://openenergy-platform.org/ontology/oeo/OEO_00140079">
        <owl:equivalentClass>
            <owl:Class>
                <owl:intersectionOf rdf:parseType="Collection">
                    <rdf:Description rdf:about="http://purl.obolibrary.org/obo/BFO_0000040"/>
                    <owl:Restriction>
                        <owl:onProperty rdf:resource="http://purl.obolibrary.org/obo/RO_0000091"/>
                        <owl:someValuesFrom rdf:resource="http://openenergy-platform.org/ontology/oeo/OEO_00140076"/>
                    </owl:Restriction>
                </owl:intersectionOf>
            </owl:Class>
        </owl:equivalentClass>
        <rdfs:subClassOf rdf:resource="http://openenergy-platform.org/ontology/oeo/OEO_00020039"/>
        <obo:IAO_0000115>A secondary energy carrier is an energy carrier that has the disposition secondary energy carrier disposition.</obo:IAO_0000115>
        <obo:IAO_0000233>issue: https://github.com/OpenEnergyPlatform/ontology/issues/575
pull request: https://github.com/OpenEnergyPlatform/ontology/pull/633
fix error in definition
issue: https://github.com/OpenEnergyPlatform/ontology/issues/669
pull request: https://github.com/OpenEnergyPlatform/ontology/pull/678</obo:IAO_0000233>
        <rdfs:label xml:lang="en">secondary energy carrier</rdfs:label>
    </owl:Class>
    


    <!-- http://openenergy-platform.org/ontology/oeo/OEO_00140080 -->

    <owl:Class rdf:about="http://openenergy-platform.org/ontology/oeo/OEO_00140080">
        <owl:equivalentClass>
            <owl:Class>
                <owl:intersectionOf rdf:parseType="Collection">
                    <rdf:Description rdf:about="http://purl.obolibrary.org/obo/BFO_0000040"/>
                    <owl:Restriction>
                        <owl:onProperty rdf:resource="http://purl.obolibrary.org/obo/RO_0000091"/>
                        <owl:someValuesFrom rdf:resource="http://openenergy-platform.org/ontology/oeo/OEO_00140077"/>
                    </owl:Restriction>
                </owl:intersectionOf>
            </owl:Class>
        </owl:equivalentClass>
        <rdfs:subClassOf rdf:resource="http://openenergy-platform.org/ontology/oeo/OEO_00020039"/>
        <obo:IAO_0000115>A final energy carrier is an energy carrier that has the disposition final energy carrier disposition.</obo:IAO_0000115>
        <obo:IAO_0000233>issue: https://github.com/OpenEnergyPlatform/ontology/issues/575
pull request: https://github.com/OpenEnergyPlatform/ontology/pull/633</obo:IAO_0000233>
        <rdfs:label xml:lang="en">final energy carrier</rdfs:label>
    </owl:Class>
    


    <!-- http://openenergy-platform.org/ontology/oeo/OEO_00140081 -->

    <owl:Class rdf:about="http://openenergy-platform.org/ontology/oeo/OEO_00140081">
        <rdfs:subClassOf rdf:resource="http://openenergy-platform.org/ontology/oeo/OEO_00030019"/>
        <rdfs:subClassOf>
            <owl:Restriction>
                <owl:onProperty rdf:resource="http://openenergy-platform.org/ontology/oeo/OEO_00000502"/>
                <owl:someValuesFrom rdf:resource="http://openenergy-platform.org/ontology/oeo/OEO_00000147"/>
            </owl:Restriction>
        </rdfs:subClassOf>
        <rdfs:subClassOf>
            <owl:Restriction>
                <owl:onProperty rdf:resource="http://openenergy-platform.org/ontology/oeo/OEO_00140002"/>
                <owl:someValuesFrom rdf:resource="http://openenergy-platform.org/ontology/oeo/OEO_00010079"/>
            </owl:Restriction>
        </rdfs:subClassOf>
        <obo:IAO_0000115>An emission value is a process attribute that quantifies the output of an emission process. It can be calculated using the emission factor of that emission process.</obo:IAO_0000115>
        <obo:IAO_0000233>class:
issue: https://github.com/OpenEnergyPlatform/ontology/issues/420
pull request: https://github.com/OpenEnergyPlatform/ontology/pull/651
has quantity value axiom:
issue: https://github.com/OpenEnergyPlatform/ontology/issues/695
pull request: https://github.com/OpenEnergyPlatform/ontology/pull/697</obo:IAO_0000233>
        <rdfs:label xml:lang="en">emission value</rdfs:label>
    </owl:Class>
    


    <!-- http://openenergy-platform.org/ontology/oeo/OEO_00140082 -->

    <owl:Class rdf:about="http://openenergy-platform.org/ontology/oeo/OEO_00140082">
        <rdfs:subClassOf rdf:resource="http://openenergy-platform.org/ontology/oeo/OEO_00140081"/>
        <rdfs:subClassOf>
            <owl:Restriction>
                <owl:onProperty rdf:resource="http://openenergy-platform.org/ontology/oeo/OEO_00000502"/>
                <owl:someValuesFrom rdf:resource="http://openenergy-platform.org/ontology/oeo/OEO_00000199"/>
            </owl:Restriction>
        </rdfs:subClassOf>
        <obo:IAO_0000115>A greenhouse gas emission value is an emission value that quantifies the output of a greenhouse gas emission process.</obo:IAO_0000115>
        <obo:IAO_0000233>issue: https://github.com/OpenEnergyPlatform/ontology/issues/420
pull request: https://github.com/OpenEnergyPlatform/ontology/pull/651</obo:IAO_0000233>
        <rdfs:label xml:lang="en">greenhouse gas emission value</rdfs:label>
    </owl:Class>
    


    <!-- http://openenergy-platform.org/ontology/oeo/OEO_00140083 -->

    <owl:Class rdf:about="http://openenergy-platform.org/ontology/oeo/OEO_00140083">
        <rdfs:subClassOf rdf:resource="http://openenergy-platform.org/ontology/oeo/OEO_00140082"/>
        <obo:IAO_0000115>A carbon dioxide equivalent quantity is a greenhouse gas emission value that quantifies the combined effect of all emitted greenhouse gases by giving an equivalent amount of CO2 which would have the same effect on the climate.</obo:IAO_0000115>
        <obo:IAO_0000118>CO2 equivalent quantity</obo:IAO_0000118>
        <obo:IAO_0000233>issue: https://github.com/OpenEnergyPlatform/ontology/issues/420
pull request: https://github.com/OpenEnergyPlatform/ontology/pull/651</obo:IAO_0000233>
        <rdfs:label xml:lang="en">carbon dioxide equivalent quantity</rdfs:label>
    </owl:Class>
    


    <!-- http://openenergy-platform.org/ontology/oeo/OEO_00140091 -->

    <owl:Class rdf:about="http://openenergy-platform.org/ontology/oeo/OEO_00140091">
        <rdfs:subClassOf rdf:resource="http://openenergy-platform.org/ontology/oeo/OEO_00000331"/>
        <rdfs:subClassOf>
            <owl:Restriction>
                <owl:onProperty rdf:resource="http://purl.obolibrary.org/obo/RO_0000087"/>
                <owl:someValuesFrom rdf:resource="http://openenergy-platform.org/ontology/oeo/OEO_00000001"/>
            </owl:Restriction>
        </rdfs:subClassOf>
        <rdfs:subClassOf>
            <owl:Restriction>
                <owl:onProperty rdf:resource="http://purl.obolibrary.org/obo/RO_0000091"/>
                <owl:someValuesFrom rdf:resource="http://openenergy-platform.org/ontology/oeo/OEO_00000028"/>
            </owl:Restriction>
        </rdfs:subClassOf>
        <rdfs:subClassOf>
            <owl:Restriction>
                <owl:onProperty rdf:resource="http://openenergy-platform.org/ontology/oeo/OEO_00000529"/>
                <owl:hasValue rdf:resource="http://openenergy-platform.org/ontology/oeo/OEO_00000390"/>
            </owl:Restriction>
        </rdfs:subClassOf>
        <obo:IAO_0000115>Plutonium is a portion of matter with the chemical formula Pu. It has a solid normal state of matter.</obo:IAO_0000115>
        <obo:IAO_0000233>issue: https://github.com/OpenEnergyPlatform/ontology/issues/694
pull request: https://github.com/OpenEnergyPlatform/ontology/pull/708</obo:IAO_0000233>
        <rdfs:label xml:lang="en">plutonium</rdfs:label>
    </owl:Class>
    


    <!-- http://openenergy-platform.org/ontology/oeo/OEO_00140092 -->

    <owl:Class rdf:about="http://openenergy-platform.org/ontology/oeo/OEO_00140092">
        <rdfs:subClassOf rdf:resource="http://openenergy-platform.org/ontology/oeo/OEO_00000331"/>
        <rdfs:subClassOf>
            <owl:Restriction>
                <owl:onProperty rdf:resource="http://purl.obolibrary.org/obo/RO_0000087"/>
                <owl:someValuesFrom rdf:resource="http://openenergy-platform.org/ontology/oeo/OEO_00000001"/>
            </owl:Restriction>
        </rdfs:subClassOf>
        <rdfs:subClassOf>
            <owl:Restriction>
                <owl:onProperty rdf:resource="http://purl.obolibrary.org/obo/RO_0000091"/>
                <owl:someValuesFrom rdf:resource="http://openenergy-platform.org/ontology/oeo/OEO_00000028"/>
            </owl:Restriction>
        </rdfs:subClassOf>
        <rdfs:subClassOf>
            <owl:Restriction>
                <owl:onProperty rdf:resource="http://openenergy-platform.org/ontology/oeo/OEO_00000529"/>
                <owl:hasValue rdf:resource="http://openenergy-platform.org/ontology/oeo/OEO_00000390"/>
            </owl:Restriction>
        </rdfs:subClassOf>
        <obo:IAO_0000115>Thorium is a portion of matter with the chemical formula Th. It has a solid normal state of matter.</obo:IAO_0000115>
        <obo:IAO_0000233>issue: https://github.com/OpenEnergyPlatform/ontology/issues/694
pull request: https://github.com/OpenEnergyPlatform/ontology/pull/708</obo:IAO_0000233>
        <rdfs:label xml:lang="en">thorium</rdfs:label>
    </owl:Class>
    


    <!-- http://openenergy-platform.org/ontology/oeo/OEO_00140101 -->

    <owl:Class rdf:about="http://openenergy-platform.org/ontology/oeo/OEO_00140101">
        <rdfs:subClassOf rdf:resource="http://openenergy-platform.org/ontology/oeo/OEO_00020003"/>
        <rdfs:subClassOf>
            <owl:Restriction>
                <owl:onProperty rdf:resource="http://purl.obolibrary.org/obo/RO_0002233"/>
                <owl:allValuesFrom rdf:resource="http://openenergy-platform.org/ontology/oeo/OEO_00000207"/>
            </owl:Restriction>
        </rdfs:subClassOf>
        <rdfs:subClassOf>
            <owl:Restriction>
                <owl:onProperty rdf:resource="http://purl.obolibrary.org/obo/RO_0002234"/>
                <owl:allValuesFrom rdf:resource="http://openenergy-platform.org/ontology/oeo/OEO_00000207"/>
            </owl:Restriction>
        </rdfs:subClassOf>
        <obo:IAO_0000115>Heat transfer is an energy transformation with thermal energy as the only input and thermal energy as the only output.</obo:IAO_0000115>
        <obo:IAO_0000233>issue: https://github.com/OpenEnergyPlatform/ontology/issues/730
pull request: https://github.com/OpenEnergyPlatform/ontology/pull/733</obo:IAO_0000233>
        <rdfs:label xml:lang="en">heat transfer</rdfs:label>
    </owl:Class>
    


    <!-- http://openenergy-platform.org/ontology/oeo/OEO_00140102 -->

    <owl:Class rdf:about="http://openenergy-platform.org/ontology/oeo/OEO_00140102">
        <rdfs:subClassOf rdf:resource="http://openenergy-platform.org/ontology/oeo/OEO_00000011"/>
        <rdfs:subClassOf>
            <owl:Restriction>
                <owl:onProperty rdf:resource="http://purl.obolibrary.org/obo/RO_0000056"/>
                <owl:someValuesFrom rdf:resource="http://openenergy-platform.org/ontology/oeo/OEO_00140101"/>
            </owl:Restriction>
        </rdfs:subClassOf>
        <obo:IAO_0000115>A heat exchanger is an energy converting device that is used for a heat transfer process.</obo:IAO_0000115>
        <obo:IAO_0000233>issue: https://github.com/OpenEnergyPlatform/ontology/issues/713
pull request: https://github.com/OpenEnergyPlatform/ontology/pull/734</obo:IAO_0000233>
        <rdfs:label xml:lang="en">heat exchanger</rdfs:label>
    </owl:Class>
    


    <!-- http://openenergy-platform.org/ontology/oeo/OEO_00140104 -->

    <owl:Class rdf:about="http://openenergy-platform.org/ontology/oeo/OEO_00140104">
        <rdfs:subClassOf rdf:resource="http://openenergy-platform.org/ontology/oeo/OEO_00000056"/>
        <rdfs:subClassOf>
            <owl:Restriction>
                <owl:onProperty rdf:resource="http://openenergy-platform.org/ontology/oeo/OEO_00000530"/>
                <owl:someValuesFrom rdf:resource="http://openenergy-platform.org/ontology/oeo/OEO_00030004"/>
            </owl:Restriction>
        </rdfs:subClassOf>
        <obo:IAO_0000115>Natural ambient thermal energy is ambient thermal energy that has a renewable origin.</obo:IAO_0000115>
        <obo:IAO_0000233>issue: https://github.com/OpenEnergyPlatform/ontology/issues/728
pull request: https://github.com/OpenEnergyPlatform/ontology/pull/742</obo:IAO_0000233>
        <rdfs:label xml:lang="en">natural ambient thermal energy</rdfs:label>
    </owl:Class>
    


    <!-- http://openenergy-platform.org/ontology/oeo/OEO_00140105 -->

    <owl:Class rdf:about="http://openenergy-platform.org/ontology/oeo/OEO_00140105">
        <rdfs:subClassOf rdf:resource="http://openenergy-platform.org/ontology/oeo/OEO_00000056"/>
        <rdfs:subClassOf>
            <owl:Restriction>
                <owl:onProperty rdf:resource="http://openenergy-platform.org/ontology/oeo/OEO_00000530"/>
                <owl:someValuesFrom rdf:resource="http://openenergy-platform.org/ontology/oeo/OEO_00030000"/>
            </owl:Restriction>
        </rdfs:subClassOf>
        <obo:IAO_0000115>Artificial ambient thermal energy is ambient thermal energy that has an anthropogenic origin.</obo:IAO_0000115>
        <obo:IAO_0000233>issue: https://github.com/OpenEnergyPlatform/ontology/issues/728
pull request: https://github.com/OpenEnergyPlatform/ontology/pull/742</obo:IAO_0000233>
        <rdfs:label xml:lang="en">artificial ambient thermal energy</rdfs:label>
    </owl:Class>
    


    <!-- http://openenergy-platform.org/ontology/oeo/OEO_00140106 -->

    <owl:Class rdf:about="http://openenergy-platform.org/ontology/oeo/OEO_00140106">
        <rdfs:subClassOf rdf:resource="http://openenergy-platform.org/ontology/oeo/OEO_00140101"/>
        <rdfs:subClassOf>
            <owl:Restriction>
                <owl:onProperty rdf:resource="http://openenergy-platform.org/ontology/oeo/OEO_00000532"/>
                <owl:someValuesFrom rdf:resource="http://openenergy-platform.org/ontology/oeo/OEO_00000056"/>
            </owl:Restriction>
        </rdfs:subClassOf>
        <rdfs:subClassOf>
            <owl:Restriction>
                <owl:onProperty rdf:resource="http://purl.obolibrary.org/obo/RO_0000057"/>
                <owl:someValuesFrom rdf:resource="http://purl.obolibrary.org/obo/BFO_0000040"/>
            </owl:Restriction>
        </rdfs:subClassOf>
        <obo:IAO_0000115>Ambient thermal energy transfer is a heat transfer from the ambient air to a transportable material entity.</obo:IAO_0000115>
        <obo:IAO_0000233>issue: https://github.com/OpenEnergyPlatform/ontology/issues/728
pull request: https://github.com/OpenEnergyPlatform/ontology/pull/742</obo:IAO_0000233>
        <rdfs:label xml:lang="en">ambient thermal energy transfer</rdfs:label>
    </owl:Class>
    


    <!-- http://openenergy-platform.org/ontology/oeo/OEO_00230000 -->

    <owl:Class rdf:about="http://openenergy-platform.org/ontology/oeo/OEO_00230000">
        <rdfs:subClassOf rdf:resource="http://openenergy-platform.org/ontology/oeo/OEO_00000350"/>
        <rdfs:subClassOf>
            <owl:Restriction>
                <owl:onProperty rdf:resource="http://openenergy-platform.org/ontology/oeo/OEO_00020056"/>
                <owl:someValuesFrom rdf:resource="http://openenergy-platform.org/ontology/oeo/OEO_00000159"/>
            </owl:Restriction>
        </rdfs:subClassOf>
        <obo:IAO_0000115>Storage capacity is the quantity value stating the maximum energy an energy storage object can store.</obo:IAO_0000115>
        <obo:IAO_0000233>issue: https://github.com/OpenEnergyPlatform/ontology/issues/320
pull request: https://github.com/OpenEnergyPlatform/ontology/pull/391</obo:IAO_0000233>
        <rdfs:label>storage capacity</rdfs:label>
    </owl:Class>
    


    <!-- http://openenergy-platform.org/ontology/oeo/OEO_00230001 -->

    <owl:Class rdf:about="http://openenergy-platform.org/ontology/oeo/OEO_00230001">
        <rdfs:subClassOf rdf:resource="http://openenergy-platform.org/ontology/oeo/OEO_00000350"/>
        <rdfs:subClassOf>
            <owl:Restriction>
                <owl:onProperty rdf:resource="http://openenergy-platform.org/ontology/oeo/OEO_00020056"/>
                <owl:someValuesFrom rdf:resource="http://openenergy-platform.org/ontology/oeo/OEO_00000011"/>
            </owl:Restriction>
        </rdfs:subClassOf>
        <obo:IAO_0000115>Power rating is the quantity value stating the maximum power an energy converting device can convert.</obo:IAO_0000115>
        <obo:IAO_0000233>issue: https://github.com/OpenEnergyPlatform/ontology/issues/320
pull request: https://github.com/OpenEnergyPlatform/ontology/pull/391</obo:IAO_0000233>
        <rdfs:label xml:lang="en">power rating</rdfs:label>
    </owl:Class>
    


    <!-- http://openenergy-platform.org/ontology/oeo/OEO_00230002 -->

    <owl:Class rdf:about="http://openenergy-platform.org/ontology/oeo/OEO_00230002">
        <rdfs:subClassOf rdf:resource="http://openenergy-platform.org/ontology/oeo/OEO_00000350"/>
        <rdfs:subClassOf>
            <owl:Restriction>
                <owl:onProperty rdf:resource="http://openenergy-platform.org/ontology/oeo/OEO_00020056"/>
                <owl:someValuesFrom>
                    <owl:Class>
                        <owl:unionOf rdf:parseType="Collection">
                            <rdf:Description rdf:about="http://openenergy-platform.org/ontology/oeo/OEO_00000031"/>
                            <rdf:Description rdf:about="http://openenergy-platform.org/ontology/oeo/OEO_00000334"/>
                        </owl:unionOf>
                    </owl:Class>
                </owl:someValuesFrom>
            </owl:Restriction>
        </rdfs:subClassOf>
        <obo:IAO_0000115>Declared net capacity is the quantity value stating the maximum power a power generating unit or a power plant can deliver to the electrical grid. It equals the sum of the rated powers of all plant generators minus all power used internally within the plant.</obo:IAO_0000115>
        <obo:IAO_0000233>issue: https://github.com/OpenEnergyPlatform/ontology/issues/320
pull request: https://github.com/OpenEnergyPlatform/ontology/pull/391</obo:IAO_0000233>
        <rdfs:label xml:lang="en">declared net capacity</rdfs:label>
    </owl:Class>
    


    <!-- http://openenergy-platform.org/ontology/oeo/OEO_00230003 -->

    <owl:Class rdf:about="http://openenergy-platform.org/ontology/oeo/OEO_00230003">
        <rdfs:subClassOf rdf:resource="http://openenergy-platform.org/ontology/oeo/OEO_00000350"/>
        <rdfs:subClassOf>
            <owl:Restriction>
                <owl:onProperty rdf:resource="http://openenergy-platform.org/ontology/oeo/OEO_00020056"/>
                <owl:someValuesFrom>
                    <owl:Class>
                        <owl:unionOf rdf:parseType="Collection">
                            <rdf:Description rdf:about="http://openenergy-platform.org/ontology/oeo/OEO_00000031"/>
                            <rdf:Description rdf:about="http://openenergy-platform.org/ontology/oeo/OEO_00000334"/>
                        </owl:unionOf>
                    </owl:Class>
                </owl:someValuesFrom>
            </owl:Restriction>
        </rdfs:subClassOf>
        <obo:IAO_0000115>Nameplate capacity is the quantity value stating the maximum power a power generating unit or a power plant can generate, and the sum of the power ratings of all energy converting devices of that power plant.</obo:IAO_0000115>
        <obo:IAO_0000233>issue: https://github.com/OpenEnergyPlatform/ontology/issues/320
pull request: https://github.com/OpenEnergyPlatform/ontology/pull/391</obo:IAO_0000233>
        <rdfs:label xml:lang="en">nameplate capacity</rdfs:label>
    </owl:Class>
    


    <!-- http://openenergy-platform.org/ontology/oeo/OEO_00230020 -->

    <owl:Class rdf:about="http://openenergy-platform.org/ontology/oeo/OEO_00230020">
        <rdfs:subClassOf rdf:resource="http://openenergy-platform.org/ontology/oeo/OEO_00000150"/>
        <obo:IAO_0000115 xml:lang="en">Kinetic energy is the energy that a material entity possesses due to its motion. It is defined as the work needed to accelerate a body of a given mass from rest to a stated velocity.</obo:IAO_0000115>
        <obo:IAO_0000233 xml:lang="en">issue: https://github.com/OpenEnergyPlatform/ontology/issues/522
pull request: https://github.com/OpenEnergyPlatform/ontology/pull/609</obo:IAO_0000233>
        <rdfs:label xml:lang="en">kinetic energy</rdfs:label>
    </owl:Class>
    


    <!-- http://openenergy-platform.org/ontology/oeo/OEO_00230021 -->

    <owl:Class rdf:about="http://openenergy-platform.org/ontology/oeo/OEO_00230021">
        <rdfs:subClassOf rdf:resource="http://openenergy-platform.org/ontology/oeo/OEO_00000331"/>
        <rdfs:subClassOf>
            <owl:Restriction>
                <owl:onProperty rdf:resource="http://openenergy-platform.org/ontology/oeo/OEO_00000530"/>
                <owl:someValuesFrom rdf:resource="http://openenergy-platform.org/ontology/oeo/OEO_00030004"/>
            </owl:Restriction>
        </rdfs:subClassOf>
        <rdfs:subClassOf>
            <owl:Restriction>
                <owl:onProperty rdf:resource="http://purl.obolibrary.org/obo/RO_0000086"/>
                <owl:someValuesFrom rdf:resource="http://openenergy-platform.org/ontology/oeo/OEO_00020040"/>
            </owl:Restriction>
        </rdfs:subClassOf>
        <rdfs:subClassOf>
            <owl:Restriction>
                <owl:onProperty rdf:resource="http://purl.obolibrary.org/obo/RO_0000091"/>
                <owl:someValuesFrom rdf:resource="http://openenergy-platform.org/ontology/oeo/OEO_00000151"/>
            </owl:Restriction>
        </rdfs:subClassOf>
        <obo:IAO_0000115 xml:lang="en">A photon is a portion of matter that is a light particle.</obo:IAO_0000115>
        <obo:IAO_0000233 xml:lang="en">issue: https://github.com/OpenEnergyPlatform/ontology/issues/661
issue: https://github.com/OpenEnergyPlatform/ontology/issues/663
pull request: https://github.com/OpenEnergyPlatform/ontology/issues/674
add origin
issue: https://github.com/OpenEnergyPlatform/ontology/issues/515
pull request: https://github.com/OpenEnergyPlatform/ontology/pull/684</obo:IAO_0000233>
        <rdfs:label xml:lang="en">photon</rdfs:label>
    </owl:Class>
    <owl:Axiom>
        <owl:annotatedSource rdf:resource="http://openenergy-platform.org/ontology/oeo/OEO_00230021"/>
        <owl:annotatedProperty rdf:resource="http://www.w3.org/2000/01/rdf-schema#subClassOf"/>
        <owl:annotatedTarget>
            <owl:Restriction>
                <owl:onProperty rdf:resource="http://purl.obolibrary.org/obo/RO_0000091"/>
                <owl:someValuesFrom rdf:resource="http://openenergy-platform.org/ontology/oeo/OEO_00000151"/>
            </owl:Restriction>
        </owl:annotatedTarget>
        <obo:IAO_0000233>issue: https://github.com/OpenEnergyPlatform/ontology/issues/726
pull request: https://github.com/OpenEnergyPlatform/ontology/pull/732</obo:IAO_0000233>
    </owl:Axiom>
    


    <!-- http://purl.obolibrary.org/obo/BFO_0000002 -->

    <owl:Class rdf:about="http://purl.obolibrary.org/obo/BFO_0000002"/>
    


    <!-- http://purl.obolibrary.org/obo/BFO_0000003 -->

    <owl:Class rdf:about="http://purl.obolibrary.org/obo/BFO_0000003"/>
    


    <!-- http://purl.obolibrary.org/obo/BFO_0000006 -->

    <owl:Class rdf:about="http://purl.obolibrary.org/obo/BFO_0000006"/>
    


    <!-- http://purl.obolibrary.org/obo/BFO_0000009 -->

    <owl:Class rdf:about="http://purl.obolibrary.org/obo/BFO_0000009"/>
    


    <!-- http://purl.obolibrary.org/obo/BFO_0000015 -->

    <owl:Class rdf:about="http://purl.obolibrary.org/obo/BFO_0000015"/>
    


    <!-- http://purl.obolibrary.org/obo/BFO_0000016 -->

    <owl:Class rdf:about="http://purl.obolibrary.org/obo/BFO_0000016"/>
    


    <!-- http://purl.obolibrary.org/obo/BFO_0000019 -->

    <owl:Class rdf:about="http://purl.obolibrary.org/obo/BFO_0000019"/>
    


    <!-- http://purl.obolibrary.org/obo/BFO_0000023 -->

    <owl:Class rdf:about="http://purl.obolibrary.org/obo/BFO_0000023"/>
    


    <!-- http://purl.obolibrary.org/obo/BFO_0000024 -->

    <owl:Class rdf:about="http://purl.obolibrary.org/obo/BFO_0000024"/>
    


    <!-- http://purl.obolibrary.org/obo/BFO_0000027 -->

    <owl:Class rdf:about="http://purl.obolibrary.org/obo/BFO_0000027"/>
    


    <!-- http://purl.obolibrary.org/obo/BFO_0000029 -->

    <owl:Class rdf:about="http://purl.obolibrary.org/obo/BFO_0000029"/>
    


    <!-- http://purl.obolibrary.org/obo/BFO_0000030 -->

    <owl:Class rdf:about="http://purl.obolibrary.org/obo/BFO_0000030"/>
    


    <!-- http://purl.obolibrary.org/obo/BFO_0000031 -->

    <owl:Class rdf:about="http://purl.obolibrary.org/obo/BFO_0000031"/>
    


    <!-- http://purl.obolibrary.org/obo/BFO_0000034 -->

    <owl:Class rdf:about="http://purl.obolibrary.org/obo/BFO_0000034"/>
    


    <!-- http://purl.obolibrary.org/obo/BFO_0000038 -->

    <owl:Class rdf:about="http://purl.obolibrary.org/obo/BFO_0000038"/>
    


    <!-- http://purl.obolibrary.org/obo/BFO_0000040 -->

    <owl:Class rdf:about="http://purl.obolibrary.org/obo/BFO_0000040"/>
    


    <!-- http://purl.obolibrary.org/obo/BFO_0000141 -->

    <owl:Class rdf:about="http://purl.obolibrary.org/obo/BFO_0000141"/>
    


    <!-- http://purl.obolibrary.org/obo/BFO_0000144 -->

    <owl:Class rdf:about="http://purl.obolibrary.org/obo/BFO_0000144"/>
    


    <!-- http://purl.obolibrary.org/obo/IAO_0000030 -->

    <owl:Class rdf:about="http://purl.obolibrary.org/obo/IAO_0000030"/>
    


    <!-- http://purl.obolibrary.org/obo/RO_0002577 -->

    <owl:Class rdf:about="http://purl.obolibrary.org/obo/RO_0002577"/>
    


    <!-- http://purl.obolibrary.org/obo/UO_0000000 -->

    <owl:Class rdf:about="http://purl.obolibrary.org/obo/UO_0000000"/>
    


    <!-- http://purl.obolibrary.org/obo/UO_0000001 -->

    <owl:Class rdf:about="http://purl.obolibrary.org/obo/UO_0000001"/>
    


    <!-- http://purl.obolibrary.org/obo/UO_0000002 -->

    <owl:Class rdf:about="http://purl.obolibrary.org/obo/UO_0000002"/>
    


    <!-- http://purl.obolibrary.org/obo/UO_0000111 -->

    <owl:Class rdf:about="http://purl.obolibrary.org/obo/UO_0000111"/>
    


    <!-- http://purl.obolibrary.org/obo/UO_0000270 -->

    <owl:Class rdf:about="http://purl.obolibrary.org/obo/UO_0000270"/>
    


    <!-- http://purl.obolibrary.org/obo/UO_0010006 -->

    <owl:Class rdf:about="http://purl.obolibrary.org/obo/UO_0010006"/>
    


    <!-- 
    ///////////////////////////////////////////////////////////////////////////////////////
    //
    // Individuals
    //
    ///////////////////////////////////////////////////////////////////////////////////////
     -->

    


    <!-- http://openenergy-platform.org/ontology/oeo/OEO_00000182 -->

    <owl:NamedIndividual rdf:about="http://openenergy-platform.org/ontology/oeo/OEO_00000182">
        <rdf:type rdf:resource="http://openenergy-platform.org/ontology/oeo/OEO_00000395"/>
        <obo:IAO_0000115>The state of being a gas. A portion of matter is in gaseous state if and only if it has has no definite shape and no definite volume and is not electrically conductive.</obo:IAO_0000115>
        <rdfs:label>gaseous</rdfs:label>
    </owl:NamedIndividual>
    


    <!-- http://openenergy-platform.org/ontology/oeo/OEO_00000256 -->

    <owl:NamedIndividual rdf:about="http://openenergy-platform.org/ontology/oeo/OEO_00000256">
        <rdf:type rdf:resource="http://openenergy-platform.org/ontology/oeo/OEO_00000395"/>
        <obo:IAO_0000115>The state of being liquid. A portion of matter is liquid has has no definite shape but a definite volume (at a given temperature and pressure).</obo:IAO_0000115>
        <rdfs:label>liquid</rdfs:label>
    </owl:NamedIndividual>
    


    <!-- http://openenergy-platform.org/ontology/oeo/OEO_00000326 -->

    <owl:NamedIndividual rdf:about="http://openenergy-platform.org/ontology/oeo/OEO_00000326">
        <rdf:type rdf:resource="http://openenergy-platform.org/ontology/oeo/OEO_00000395"/>
        <obo:IAO_0000115>The state of being a plasma. A portion of matter is in plasmatic state if and only if it has has no definite shape and no definite volume and is electrically conductive.</obo:IAO_0000115>
        <rdfs:label>plasmatic</rdfs:label>
    </owl:NamedIndividual>
    


    <!-- http://openenergy-platform.org/ontology/oeo/OEO_00000390 -->

    <owl:NamedIndividual rdf:about="http://openenergy-platform.org/ontology/oeo/OEO_00000390">
        <rdf:type rdf:resource="http://openenergy-platform.org/ontology/oeo/OEO_00000395"/>
        <obo:IAO_0000115>The state being solid. A portion of matter is in solid state if and only if it has a definite shape and volume (at a given temperature and pressure).</obo:IAO_0000115>
        <rdfs:label>solid</rdfs:label>
    </owl:NamedIndividual>
    


    <!-- 
    ///////////////////////////////////////////////////////////////////////////////////////
    //
    // General axioms
    //
    ///////////////////////////////////////////////////////////////////////////////////////
     -->

    <rdf:Description>
        <rdf:type rdf:resource="http://www.w3.org/2002/07/owl#AllDisjointClasses"/>
        <owl:members rdf:parseType="Collection">
            <rdf:Description rdf:about="http://openenergy-platform.org/ontology/oeo/OEO_00000188"/>
            <rdf:Description rdf:about="http://openenergy-platform.org/ontology/oeo/OEO_00000210"/>
            <rdf:Description rdf:about="http://openenergy-platform.org/ontology/oeo/OEO_00000425"/>
        </owl:members>
    </rdf:Description>
</rdf:RDF>



<!-- Generated by the OWL API (version 4.5.6) https://github.com/owlcs/owlapi -->

